<?xml version="1.0"?>
<rdf:RDF xmlns="https://w3id.org/leo/onto/livestock-indicator/"
     xml:base="https://w3id.org/leo/onto/livestock-indicator/"
     xmlns:dc="http://purl.org/dc/elements/1.1/"
     xmlns:l0="https://w3id.org/italia/onto/l0/"
     xmlns:ns="http://www.w3.org/2006/vcard/ns#"
     xmlns:CLV="https://w3id.org/italia/onto/CLV/"
     xmlns:owl="http://www.w3.org/2002/07/owl#"
     xmlns:rdf="http://www.w3.org/1999/02/22-rdf-syntax-ns#"
     xmlns:xml="http://www.w3.org/XML/1998/namespace"
     xmlns:xsd="http://www.w3.org/2001/XMLSchema#"
     xmlns:ADMS="https://w3id.org/italia/onto/ADMS/"
     xmlns:dcat="http://www.w3.org/ns/dcat#"
     xmlns:foaf="http://xmlns.com/foaf/0.1/"
     xmlns:prov="http://www.w3.org/ns/prov#"
     xmlns:rdfs="http://www.w3.org/2000/01/rdf-schema#"
     xmlns:terms="http://purl.org/dc/terms/">
    <owl:Ontology rdf:about="https://w3id.org/leo/onto/livestock-indicator">
        <owl:versionIRI rdf:resource="https://w3id.org/leo/onto/livestock-indicator/0.4"/>
        <owl:imports rdf:resource="https://w3id.org/italia/onto/Indicator"/>
        <owl:imports rdf:resource="https://w3id.org/italia/onto/l0"/>
        <dc:description rdf:resource="https://www.dropbox.com/s/kb61f2wcx7sqz0q/livestock-indicator.png?raw=1"/>
        <terms:accrualPeriodicity rdf:resource="http://publications.europa.eu/resource/authority/frequency/IRREG"/>
        <terms:creator rdf:resource="https://w3id.org/leo/data/private-organization/00944701002"/>
        <terms:description xml:lang="it">Questa è l&apos;ontologia degli indicatori usati nel dominio zootecnico.</terms:description>
        <terms:description xml:lang="en">This is the ontology of indicators used in the livestock environment</terms:description>
        <terms:issued rdf:datatype="http://www.w3.org/2001/XMLSchema#date">2018-06-18</terms:issued>
        <terms:language rdf:resource="http://publications.europa.eu/resource/authority/language/ENG"/>
        <terms:language rdf:resource="http://publications.europa.eu/resource/authority/language/ITA"/>
        <terms:modified rdf:datatype="http://www.w3.org/2001/XMLSchema#date">2022-11-16</terms:modified>
        <terms:publisher rdf:resource="https://w3id.org/leo/data/private-organization/00944701002"/>
        <terms:rightsHolder rdf:resource="https://w3id.org/leo/data/private-organization/00944701002"/>
        <terms:subject rdf:resource="http://eurovoc.europa.eu/100254"/>
        <terms:title xml:lang="en">Livestock Indicator Ontology</terms:title>
        <terms:title xml:lang="it">Ontologia degli Indicatori del dominio Zootecnico</terms:title>
        <rdfs:comment xml:lang="it">Questa è l&apos;ontologia degli indicatori usati nel dominio zootecnico.</rdfs:comment>
        <rdfs:comment xml:lang="en">This is the ontology of indicators used in the livestock environment</rdfs:comment>
        <rdfs:isDefinedBy rdf:resource="https://w3id.org/leo/onto/livestock-indicator"/>
        <rdfs:label xml:lang="en">Livestock Indicator Ontology</rdfs:label>
        <rdfs:label xml:lang="it">Ontologia degli Indicatori del dominio Zootecnico</rdfs:label>
        <owl:versionInfo xml:lang="en">Version 0.4 - 2022 - Introduction of the concept of collection of livestock indicator collection, with related properties. Renamed some properties.</owl:versionInfo>
        <owl:versionInfo xml:lang="it">Versione 0.2 - 2022 - Introdotto il concetto di collezione di calcoli di indicatori zootecnici con relative proprietà. Rivisti i nomi di alcune proprietà.</owl:versionInfo>
        <dcat:contactPoint rdf:resource="https://w3id.org/leo/data/contact-point/onto-aia"/>
        <dcat:keyword xml:lang="it">Indicatore Genetico</dcat:keyword>
        <dcat:keyword xml:lang="it">Indicatore Zootecnico</dcat:keyword>
        <dcat:keyword xml:lang="it">Indicatore di Benessere</dcat:keyword>
        <dcat:theme rdf:resource="http://publications.europa.eu/resource/authority/data-theme/AGRI"/>
        <ADMS:acronym>LEO</ADMS:acronym>
        <ADMS:hasContributor rdf:resource="https://w3id.org/leo/data/private-organization/06695411006"/>
        <ADMS:hasFormalityLevel rdf:resource="https://w3id.org/italia/onto/ADMS/Formal"/>
        <ADMS:hasKeyClass rdf:resource="https://w3id.org/leo/onto/livestock-indicator/AnimalBasedIndicatorCalculation"/>
        <ADMS:hasKeyClass rdf:resource="https://w3id.org/leo/onto/livestock-indicator/CompanyBasedIndicatorCalculation"/>
        <ADMS:hasKeyClass rdf:resource="https://w3id.org/leo/onto/livestock-indicator/LivestockIndicator"/>
        <ADMS:hasKeyClass rdf:resource="https://w3id.org/leo/onto/livestock-indicator/LivestockIndicatorCalculation"/>
        <ADMS:hasOntologyLanguage rdf:resource="https://w3id.org/italia/onto/ADMS/OWL"/>
        <ADMS:hasSemanticAssetDistribution rdf:resource="https://w3id.org/leo/data/distribution/IND-JSON-LD"/>
        <ADMS:hasSemanticAssetDistribution rdf:resource="https://w3id.org/leo/data/distribution/IND-RDF-TURTLE"/>
        <ADMS:hasSemanticAssetDistribution rdf:resource="https://w3id.org/leo/data/distribution/IND-RDF-XML"/>
        <ADMS:hasTask rdf:resource="https://w3id.org/italia/onto/ADMS/AnnotationTask"/>
        <ADMS:hasTask rdf:resource="https://w3id.org/italia/onto/ADMS/QueryFormulationTask"/>
        <ADMS:hasTask rdf:resource="https://w3id.org/italia/onto/ADMS/SearchTask"/>
        <ADMS:officialURI rdf:datatype="http://www.w3.org/2001/XMLSchema#anyURI">https://w3id.org/leo/onto/livestock-indicator</ADMS:officialURI>
        <ADMS:prefix>li</ADMS:prefix>
        <ADMS:semanticAssetInUse rdf:resource="https://w3id.org/leo/data/project/LEO"/>
        <ADMS:status>catalogued</ADMS:status>
        <ADMS:target>Comunità open data</ADMS:target>
        <ADMS:target>Imprese</ADMS:target>
        <ADMS:target>Professionisti settore zootecnico</ADMS:target>
        <ADMS:target>Pubbliche Amministrazioni</ADMS:target>
        <ADMS:type rdf:resource="https://w3id.org/italia/onto/ADMS/DomainOntology"/>
    </owl:Ontology>
    


    <!-- 
    ///////////////////////////////////////////////////////////////////////////////////////
    //
    // Annotation properties
    //
    ///////////////////////////////////////////////////////////////////////////////////////
     -->

    


    <!-- http://purl.org/dc/elements/1.1/description -->

    <owl:AnnotationProperty rdf:about="http://purl.org/dc/elements/1.1/description"/>
    


    <!-- http://purl.org/dc/terms/accrualPeriodicity -->

    <owl:AnnotationProperty rdf:about="http://purl.org/dc/terms/accrualPeriodicity"/>
    


    <!-- http://purl.org/dc/terms/description -->

    <owl:AnnotationProperty rdf:about="http://purl.org/dc/terms/description"/>
    


    <!-- http://purl.org/dc/terms/format -->

    <owl:AnnotationProperty rdf:about="http://purl.org/dc/terms/format"/>
    


    <!-- http://purl.org/dc/terms/identifier -->

    <owl:AnnotationProperty rdf:about="http://purl.org/dc/terms/identifier"/>
    


    <!-- http://purl.org/dc/terms/language -->

    <owl:AnnotationProperty rdf:about="http://purl.org/dc/terms/language"/>
    


    <!-- http://purl.org/dc/terms/license -->

    <owl:AnnotationProperty rdf:about="http://purl.org/dc/terms/license"/>
    


    <!-- http://purl.org/dc/terms/publisher -->

    <owl:AnnotationProperty rdf:about="http://purl.org/dc/terms/publisher"/>
    


    <!-- http://purl.org/dc/terms/rightsHolder -->

    <owl:AnnotationProperty rdf:about="http://purl.org/dc/terms/rightsHolder"/>
    


    <!-- http://purl.org/dc/terms/subject -->

    <owl:AnnotationProperty rdf:about="http://purl.org/dc/terms/subject"/>
    


    <!-- http://purl.org/dc/terms/title -->

    <owl:AnnotationProperty rdf:about="http://purl.org/dc/terms/title"/>
    


    <!-- http://www.w3.org/2006/vcard/ns#fn -->

    <owl:AnnotationProperty rdf:about="http://www.w3.org/2006/vcard/ns#fn"/>
    


    <!-- http://www.w3.org/2006/vcard/ns#hasEmail -->

    <owl:AnnotationProperty rdf:about="http://www.w3.org/2006/vcard/ns#hasEmail"/>
    


    <!-- http://www.w3.org/ns/dcat#accessURL -->

    <owl:AnnotationProperty rdf:about="http://www.w3.org/ns/dcat#accessURL"/>
    


    <!-- http://www.w3.org/ns/dcat#contactPoint -->

    <owl:AnnotationProperty rdf:about="http://www.w3.org/ns/dcat#contactPoint"/>
    


    <!-- http://www.w3.org/ns/dcat#downloadURL -->

    <owl:AnnotationProperty rdf:about="http://www.w3.org/ns/dcat#downloadURL"/>
    


    <!-- http://www.w3.org/ns/dcat#keyword -->

    <owl:AnnotationProperty rdf:about="http://www.w3.org/ns/dcat#keyword"/>
    


    <!-- http://www.w3.org/ns/dcat#theme -->

    <owl:AnnotationProperty rdf:about="http://www.w3.org/ns/dcat#theme"/>
    


    <!-- http://www.w3.org/ns/prov#wasDerivedFrom -->

    <owl:AnnotationProperty rdf:about="http://www.w3.org/ns/prov#wasDerivedFrom"/>
    


    <!-- http://www.w3.org/ns/prov#wasInfluencedBy -->

    <owl:AnnotationProperty rdf:about="http://www.w3.org/ns/prov#wasInfluencedBy"/>
    


    <!-- http://xmlns.com/foaf/0.1/name -->

    <owl:AnnotationProperty rdf:about="http://xmlns.com/foaf/0.1/name"/>
    


    <!-- https://w3id.org/italia/onto/ADMS/acronym -->

    <owl:AnnotationProperty rdf:about="https://w3id.org/italia/onto/ADMS/acronym"/>
    


    <!-- https://w3id.org/italia/onto/ADMS/hasContributor -->

    <owl:AnnotationProperty rdf:about="https://w3id.org/italia/onto/ADMS/hasContributor"/>
    


    <!-- https://w3id.org/italia/onto/ADMS/hasFormalityLevel -->

    <owl:AnnotationProperty rdf:about="https://w3id.org/italia/onto/ADMS/hasFormalityLevel"/>
    


    <!-- https://w3id.org/italia/onto/ADMS/hasKeyClass -->

    <owl:AnnotationProperty rdf:about="https://w3id.org/italia/onto/ADMS/hasKeyClass"/>
    


    <!-- https://w3id.org/italia/onto/ADMS/hasOntologyLanguage -->

    <owl:AnnotationProperty rdf:about="https://w3id.org/italia/onto/ADMS/hasOntologyLanguage"/>
    


    <!-- https://w3id.org/italia/onto/ADMS/hasSemanticAssetDistribution -->

    <owl:AnnotationProperty rdf:about="https://w3id.org/italia/onto/ADMS/hasSemanticAssetDistribution"/>
    


    <!-- https://w3id.org/italia/onto/ADMS/hasTask -->

    <owl:AnnotationProperty rdf:about="https://w3id.org/italia/onto/ADMS/hasTask"/>
    


    <!-- https://w3id.org/italia/onto/ADMS/officialURI -->

    <owl:AnnotationProperty rdf:about="https://w3id.org/italia/onto/ADMS/officialURI"/>
    


    <!-- https://w3id.org/italia/onto/ADMS/prefix -->

    <owl:AnnotationProperty rdf:about="https://w3id.org/italia/onto/ADMS/prefix"/>
    


    <!-- https://w3id.org/italia/onto/ADMS/semanticAssetInUse -->

    <owl:AnnotationProperty rdf:about="https://w3id.org/italia/onto/ADMS/semanticAssetInUse"/>
    


    <!-- https://w3id.org/italia/onto/ADMS/status -->

    <owl:AnnotationProperty rdf:about="https://w3id.org/italia/onto/ADMS/status"/>
    


    <!-- https://w3id.org/italia/onto/ADMS/target -->

    <owl:AnnotationProperty rdf:about="https://w3id.org/italia/onto/ADMS/target"/>
    


    <!-- https://w3id.org/italia/onto/ADMS/type -->

    <owl:AnnotationProperty rdf:about="https://w3id.org/italia/onto/ADMS/type"/>
    


    <!-- https://w3id.org/italia/onto/l0/controlledVocabulary -->

    <owl:AnnotationProperty rdf:about="https://w3id.org/italia/onto/l0/controlledVocabulary"/>
    


    <!-- https://w3id.org/italia/onto/l0/name -->

    <owl:AnnotationProperty rdf:about="https://w3id.org/italia/onto/l0/name"/>
    


    <!-- 
    ///////////////////////////////////////////////////////////////////////////////////////
    //
    // Object Properties
    //
    ///////////////////////////////////////////////////////////////////////////////////////
     -->

    


    <!-- https://w3id.org/leo/onto/animal/doneForIndicatorType -->

    <owl:ObjectProperty rdf:about="https://w3id.org/leo/onto/animal/doneForIndicatorType">
        <rdfs:domain rdf:resource="https://w3id.org/leo/onto/livestock-indicator/LivestockIndicatorCalculation"/>
        <rdfs:range rdf:resource="https://w3id.org/italia/onto/Indicator/IndicatorType"/>
        <rdfs:comment xml:lang="en">Property used to associate the speciifc calculation of a livestock indicator to the indicator type</rdfs:comment>
        <rdfs:comment xml:lang="it">Proprietà utilizzata per associare uno specifico calcolo dell&apos;indicatore zootecnico al tipo di indicatore (e.g., genetico, genomico, pedigree)</rdfs:comment>
        <rdfs:isDefinedBy rdf:resource="https://w3id.org/leo/onto/livestock-indicator"/>
        <rdfs:label xml:lang="it">(calcolo) fatto per tipo indicatore</rdfs:label>
        <rdfs:label xml:lang="en">done for indicator type</rdfs:label>
        <owl:versionInfo xml:lang="it">stabile</owl:versionInfo>
        <owl:versionInfo xml:lang="en">stable</owl:versionInfo>
    </owl:ObjectProperty>
    


    <!-- https://w3id.org/leo/onto/livestock-indicator/associatedWithBreed -->

    <owl:ObjectProperty rdf:about="https://w3id.org/leo/onto/livestock-indicator/associatedWithBreed">
        <rdfs:domain rdf:resource="https://w3id.org/leo/onto/livestock-indicator/CompanyBasedIndicatorCalculation"/>
        <rdfs:range rdf:resource="https://w3id.org/leo/onto/animal/Breed"/>
        <rdfs:comment xml:lang="en">Property used to link indicators calculated at farm level with the breed. In particular, this property is valorised in the presence of indicators such as Indicator Age 1 Parturition</rdfs:comment>
        <rdfs:comment xml:lang="it">Proprietà utilizzata per collegare indicatori calcolati a livello aziendale con la razza. In particolare, questa proprietà è valorizzata in presenza di indicatori quali Indicatore Età 1 Parto</rdfs:comment>
        <rdfs:isDefinedBy rdf:resource="https://w3id.org/leo/onto/livestock-indicator"/>
        <rdfs:label xml:lang="en">associated with breed</rdfs:label>
        <rdfs:label xml:lang="it">associato con razza</rdfs:label>
        <owl:versionInfo xml:lang="it">stabile</owl:versionInfo>
        <owl:versionInfo xml:lang="en">stable</owl:versionInfo>
    </owl:ObjectProperty>
    


    <!-- https://w3id.org/leo/onto/livestock-indicator/associatedWithCompany -->

    <owl:ObjectProperty rdf:about="https://w3id.org/leo/onto/livestock-indicator/associatedWithCompany">
        <rdfs:domain>
            <owl:Class>
                <owl:unionOf rdf:parseType="Collection">
                    <rdf:Description rdf:about="https://w3id.org/leo/onto/livestock-indicator/CompanyBasedIndicatorCalculation"/>
                    <rdf:Description rdf:about="https://w3id.org/leo/onto/livestock-indicator/LivestockIndicatorCalcCollection"/>
                </owl:unionOf>
            </owl:Class>
        </rdfs:domain>
        <rdfs:range rdf:resource="https://w3id.org/leo/onto/co/LivestockFarm"/>
        <rdfs:comment xml:lang="en">Property that links the company-based livestock indicator calculation and its possible collection to the company.</rdfs:comment>
        <rdfs:comment xml:lang="it">Proprietà che collega il calcolo dell&apos;indicatore zootecnico aziendale e le possibili collezioni di questi all&apos;azienda.</rdfs:comment>
        <rdfs:isDefinedBy rdf:resource="https://w3id.org/leo/onto/livestock-indicator"/>
        <rdfs:label xml:lang="en">associated with company</rdfs:label>
        <rdfs:label xml:lang="it">associato con azienda</rdfs:label>
        <owl:versionInfo xml:lang="it">stabile</owl:versionInfo>
        <owl:versionInfo xml:lang="en">stable</owl:versionInfo>
    </owl:ObjectProperty>
    


    <!-- https://w3id.org/leo/onto/livestock-indicator/associatedWithIndicator -->

    <owl:ObjectProperty rdf:about="https://w3id.org/leo/onto/livestock-indicator/associatedWithIndicator">
        <rdfs:domain rdf:resource="http://www.w3.org/2002/07/owl#Thing"/>
        <rdfs:range rdf:resource="https://w3id.org/leo/onto/livestock-indicator/LivestockIndicator"/>
        <rdfs:comment xml:lang="en">A general property that links an entity to an indicator.</rdfs:comment>
        <rdfs:comment xml:lang="it">Proprietà generica che collega una generica entitò a un indicatore.</rdfs:comment>
        <rdfs:isDefinedBy rdf:resource="https://w3id.org/leo/onto/livestock-indicator"/>
        <rdfs:label xml:lang="en">associated with indicator</rdfs:label>
        <rdfs:label xml:lang="it">associato con indicatore</rdfs:label>
        <owl:versionInfo xml:lang="it">stabile</owl:versionInfo>
        <owl:versionInfo xml:lang="en">stable</owl:versionInfo>
    </owl:ObjectProperty>
    


    <!-- https://w3id.org/leo/onto/livestock-indicator/associatedWithProductionTarget -->

    <owl:ObjectProperty rdf:about="https://w3id.org/leo/onto/livestock-indicator/associatedWithProductionTarget">
        <rdfs:domain>
            <owl:Class>
                <owl:unionOf rdf:parseType="Collection">
                    <rdf:Description rdf:about="https://w3id.org/leo/onto/livestock-indicator/CompanyBasedIndicatorCalculation"/>
                    <rdf:Description rdf:about="https://w3id.org/leo/onto/livestock-indicator/LivestockIndicatorCalcCollection"/>
                </owl:unionOf>
            </owl:Class>
        </rdfs:domain>
        <rdfs:range rdf:resource="https://w3id.org/leo/onto/animal/ProductionType"/>
        <rdfs:comment xml:lang="en">Property that links the livestock indicator calculation (and in particular the company-based livestock indicator calculation) or its collection with the production target/type of the livestock species</rdfs:comment>
        <rdfs:comment xml:lang="it">Proprietà che collega il calcolo dell&apos;indicatore zootecnico (e in particolare il calcolo dell&apos;indicatore zootecnico aziendale) o la collezione di questi indicatori con l&apos;indirizzo produttivo della specie animale</rdfs:comment>
        <rdfs:isDefinedBy rdf:resource="https://w3id.org/leo/onto/livestock-indicator"/>
        <rdfs:label xml:lang="en">associated with production target</rdfs:label>
        <rdfs:label xml:lang="it">associato con indirizzo produttivo</rdfs:label>
        <owl:versionInfo xml:lang="it">stabile</owl:versionInfo>
        <owl:versionInfo xml:lang="en">stable</owl:versionInfo>
    </owl:ObjectProperty>
    


    <!-- https://w3id.org/leo/onto/livestock-indicator/associatedWithSpecies -->

    <owl:ObjectProperty rdf:about="https://w3id.org/leo/onto/livestock-indicator/associatedWithSpecies">
        <rdfs:domain>
            <owl:Class>
                <owl:unionOf rdf:parseType="Collection">
                    <rdf:Description rdf:about="https://w3id.org/leo/onto/livestock-indicator/LivestockIndicatorCalcCollection"/>
                    <rdf:Description rdf:about="https://w3id.org/leo/onto/livestock-indicator/LivestockIndicatorCalculation"/>
                </owl:unionOf>
            </owl:Class>
        </rdfs:domain>
        <rdfs:range rdf:resource="https://w3id.org/leo/onto/animal/LivestockSpecies"/>
        <rdfs:comment xml:lang="en">Property that links the livestock indicator calculation or a collection of livestock indicator calculations to the livestock species they refer.</rdfs:comment>
        <rdfs:comment xml:lang="it">Proprietà che collega il calcolo dell&apos;indicatore zootecnico o la collezione di calcoli delll&apos;indicatore zootecnico alla specie a cui si riferiscono.</rdfs:comment>
        <rdfs:isDefinedBy rdf:resource="https://w3id.org/leo/onto/livestock-indicator"/>
        <rdfs:label xml:lang="en">associato con specie</rdfs:label>
        <rdfs:label xml:lang="it">è associato con specie</rdfs:label>
        <owl:versionInfo xml:lang="it">stabile</owl:versionInfo>
        <owl:versionInfo xml:lang="en">stable</owl:versionInfo>
    </owl:ObjectProperty>
    


    <!-- https://w3id.org/leo/onto/livestock-indicator/basedOnCalculation -->

    <owl:ObjectProperty rdf:about="https://w3id.org/leo/onto/livestock-indicator/basedOnCalculation">
        <rdfs:domain rdf:resource="https://w3id.org/leo/onto/livestock-indicator/LivestockIndicatorCalculation"/>
        <rdfs:range rdf:resource="https://w3id.org/leo/onto/livestock-indicator/LivestockIndicatorCalculation"/>
        <rdfs:comment xml:lang="en">Property that enables the modelling of hierarchies in calculations of livestock indicators.</rdfs:comment>
        <rdfs:comment xml:lang="it">Proprietà che consente di modellare gerarchie nei calcoli degli indicatori zootecnici.</rdfs:comment>
        <rdfs:isDefinedBy rdf:resource="https://w3id.org/leo/onto/livestock-indicator"/>
        <rdfs:label xml:lang="it">basato su calcolo</rdfs:label>
        <rdfs:label xml:lang="en">based on calculation</rdfs:label>
        <owl:versionInfo xml:lang="it">stabile</owl:versionInfo>
        <owl:versionInfo xml:lang="en">stable</owl:versionInfo>
    </owl:ObjectProperty>
    


    <!-- https://w3id.org/leo/onto/livestock-indicator/computedForFarmAnimal -->

    <owl:ObjectProperty rdf:about="https://w3id.org/leo/onto/livestock-indicator/computedForFarmAnimal">
        <rdfs:subPropertyOf rdf:resource="https://w3id.org/italia/onto/Indicator/isIndicatorCalculationOf"/>
        <rdfs:domain rdf:resource="https://w3id.org/leo/onto/livestock-indicator/AnimalBasedIndicatorCalculation"/>
        <rdfs:range rdf:resource="https://w3id.org/leo/onto/animal/FarmAnimal"/>
        <rdfs:comment xml:lang="en">Property that links the animal-based livestock indicator calculation (in particular the genetic indicators/indexes) to the farm animal.</rdfs:comment>
        <rdfs:comment xml:lang="it">Proprietà che collega il calcolo degli indicatori zootecnici basati sull&apos;animale (in particolare gli indicatori/indici genetici) all&apos;animale da allevamento.</rdfs:comment>
        <rdfs:isDefinedBy rdf:resource="https://w3id.org/leo/onto/livestock-indicator"/>
        <rdfs:label xml:lang="it">calcolato per animale d&apos;allevamento</rdfs:label>
        <rdfs:label xml:lang="en">computed for farm animal</rdfs:label>
        <owl:versionInfo xml:lang="it">stabile</owl:versionInfo>
        <owl:versionInfo xml:lang="en">stable</owl:versionInfo>
    </owl:ObjectProperty>
    


    <!-- https://w3id.org/leo/onto/livestock-indicator/forLivestockIndicator -->

    <owl:ObjectProperty rdf:about="https://w3id.org/leo/onto/livestock-indicator/forLivestockIndicator">
        <rdfs:subPropertyOf rdf:resource="https://w3id.org/italia/onto/Indicator/forIndicator"/>
        <rdfs:domain rdf:resource="https://w3id.org/leo/onto/livestock-indicator/LivestockIndicatorCalculation"/>
        <rdfs:range rdf:resource="https://w3id.org/leo/onto/livestock-indicator/LivestockIndicator"/>
        <rdfs:comment xml:lang="en">Property that links the livestock indicator calculcation with the related livestock indicator</rdfs:comment>
        <rdfs:comment xml:lang="it">Proprietà che collega il calcolo dell&apos;indicatore zootecnico all&apos;indicatore relativo.</rdfs:comment>
        <rdfs:isDefinedBy rdf:resource="https://w3id.org/leo/onto/livestock-indicator"/>
        <rdfs:label xml:lang="en">for livestock indicator</rdfs:label>
        <rdfs:label xml:lang="it">per indicatore zootecnico</rdfs:label>
        <owl:versionInfo xml:lang="it">stabile</owl:versionInfo>
        <owl:versionInfo xml:lang="en">stable</owl:versionInfo>
    </owl:ObjectProperty>
    


    <!-- https://w3id.org/leo/onto/livestock-indicator/hasCalculationAccuracy -->

    <owl:ObjectProperty rdf:about="https://w3id.org/leo/onto/livestock-indicator/hasCalculationAccuracy">
        <rdfs:domain rdf:resource="https://w3id.org/leo/onto/livestock-indicator/LivestockIndicatorCalculation"/>
        <rdfs:range rdf:resource="https://w3id.org/italia/onto/MU/Value"/>
        <rdfs:comment xml:lang="en">Property that allows one to specify the accuracy in percentage of the livestock indicator calculation.</rdfs:comment>
        <rdfs:comment xml:lang="it">Proprietà che consente di specificare l&apos;accuratezza, in percentuale, del calcolo dell&apos;indicatore zootecnico.</rdfs:comment>
        <rdfs:isDefinedBy rdf:resource="https://w3id.org/leo/onto/livestock-indicator"/>
        <rdfs:label xml:lang="it">ha accuratezza del calcolo</rdfs:label>
        <rdfs:label xml:lang="en">has calculation accuracy</rdfs:label>
        <owl:versionInfo xml:lang="it">stabile</owl:versionInfo>
        <owl:versionInfo xml:lang="en">stable</owl:versionInfo>
    </owl:ObjectProperty>
    


    <!-- https://w3id.org/leo/onto/livestock-indicator/hasComplementaryInfo -->

    <owl:ObjectProperty rdf:about="https://w3id.org/leo/onto/livestock-indicator/hasComplementaryInfo">
        <rdfs:domain>
            <owl:Class>
                <owl:unionOf rdf:parseType="Collection">
                    <rdf:Description rdf:about="https://w3id.org/leo/onto/livestock-indicator/ComplementaryInfoDescription"/>
                    <rdf:Description rdf:about="https://w3id.org/leo/onto/livestock-indicator/LivestockIndicator"/>
                </owl:unionOf>
            </owl:Class>
        </rdfs:domain>
        <rdfs:range rdf:resource="https://w3id.org/leo/onto/livestock-indicator/ComplementaryInfo"/>
        <rdfs:comment xml:lang="en">Property that links the description of the complementary information or the livestock indicator with the type of complementary information used in the livestock indicator calculation.</rdfs:comment>
        <rdfs:comment xml:lang="it">Proprietà che collega la descrizione delle informazioni complementari o l&apos;indicatore zootecnico stesso con il tipo di informazioni complementari utilizzate nel calcolo dell&apos;indicatore zootecnico.</rdfs:comment>
        <rdfs:isDefinedBy rdf:resource="https://w3id.org/leo/onto/livestock-indicator"/>
        <rdfs:label xml:lang="it">ha informazione complementare</rdfs:label>
        <rdfs:label xml:lang="en">has complementary information</rdfs:label>
        <owl:versionInfo xml:lang="it">stabile</owl:versionInfo>
        <owl:versionInfo xml:lang="en">stable</owl:versionInfo>
    </owl:ObjectProperty>
    


    <!-- https://w3id.org/leo/onto/livestock-indicator/hasComplementaryInformationDesc -->

    <owl:ObjectProperty rdf:about="https://w3id.org/leo/onto/livestock-indicator/hasComplementaryInformationDesc">
        <rdfs:domain>
            <owl:Class>
                <owl:unionOf rdf:parseType="Collection">
                    <rdf:Description rdf:about="https://w3id.org/leo/onto/livestock-indicator/LivestockIndicatorCalcCollection"/>
                    <rdf:Description rdf:about="https://w3id.org/leo/onto/livestock-indicator/LivestockIndicatorCalculation"/>
                </owl:unionOf>
            </owl:Class>
        </rdfs:domain>
        <rdfs:range rdf:resource="https://w3id.org/leo/onto/livestock-indicator/ComplementaryInfoDescription"/>
        <rdfs:comment xml:lang="it">Proprietà che consente di collegare il calcolo dell&apos;indicatore zootecnico o le collezioni di calcoli alle descrizioni (informazione complementare e valore) di ciascuna informazione complementare usata nel calcolo.

ex:myIndicatorCalculation1 a li:LivestockIndicatorCalculation ;
li:hasComplementaryInformationDesc ex:myComplementaryInfoDescND-3 .

ex:myComplementaryInfoDescND-3 a li:ComplementaryInfoDescription ;
mu:hasValue ex:myValue3-0 ;
li:hasComplementaryInfo ex:myComplementaryInfoND .

ex:myValue3-0 a mu:Value ;
mu:value 3;
mu:hasMeasurementUnit &lt;https://w3id.org/leo/controlled-vocabulary/measurement-unit/0&gt; .

ex:myComplementaryInfoND a li:ComplementaryInfo ;
rdfs:label &quot;Number of daughters&quot;@en , &quot;Numero figlie&quot;@it ;
l0:name &quot;Number of daughters&quot;@en , &quot;Numero figlie&quot;@it.</rdfs:comment>
        <rdfs:comment xml:lang="en">ex:myIndicatorCalculation1 a li:LivestockIndicatorCalculation ;
li:hasComplementaryInformationDesc ex:myComplementaryInfoDescND-3 .

ex:myComplementaryInfoDescND-3 a li:ComplementaryInfoDescription ;
mu:hasValue ex:myValue3-0 ;
li:hasComplementaryInfo ex:myComplementaryInfoND .

ex:myValue3-0 a mu:Value ;
mu:value 3;
mu:hasMeasurementUnit &lt;https://w3id.org/leo/controlled-vocabulary/measurement-unit/0&gt; .

ex:myComplementaryInfoND a li:ComplementaryInfo ;
rdfs:label &quot;Number of daughters&quot;@en , &quot;Numero figlie&quot;@it ;
l0:name &quot;Number of daughters&quot;@en , &quot;Numero figlie&quot;@it.</rdfs:comment>
        <rdfs:isDefinedBy rdf:resource="https://w3id.org/leo/onto/livestock-indicator"/>
        <rdfs:label xml:lang="it">ha descrizione informazioni complementari</rdfs:label>
        <rdfs:label xml:lang="en">has complementary information description</rdfs:label>
        <owl:versionInfo xml:lang="it">stabile</owl:versionInfo>
        <owl:versionInfo xml:lang="en">stable</owl:versionInfo>
    </owl:ObjectProperty>
    


    <!-- https://w3id.org/leo/onto/livestock-indicator/hasCountryOfInfluence -->

    <owl:ObjectProperty rdf:about="https://w3id.org/leo/onto/livestock-indicator/hasCountryOfInfluence">
        <rdfs:domain rdf:resource="https://w3id.org/leo/onto/livestock-indicator/LivestockIndicatorCalculation"/>
        <rdfs:range rdf:resource="http://www.w3.org/2004/02/skos/core#Concept"/>
        <rdfs:comment xml:lang="it">La proprietà che lega il calcolo dell&apos;indicatore zootecnico con i paesi (esteri) che influenzano sul calcolo stesso.</rdfs:comment>
        <rdfs:comment xml:lang="en">The property that links the calculation of the livestock indicator with the (foreign) countries that influence the calculation.</rdfs:comment>
        <rdfs:isDefinedBy rdf:resource="https://w3id.org/leo/onto/livestock-indicator"/>
        <rdfs:label xml:lang="it">ha area geografica (estera) di influenza sul calcolo</rdfs:label>
        <rdfs:label xml:lang="en">has country of influence</rdfs:label>
        <owl:versionInfo xml:lang="it">stabile</owl:versionInfo>
        <owl:versionInfo xml:lang="en">stable</owl:versionInfo>
    </owl:ObjectProperty>
    


    <!-- https://w3id.org/leo/onto/livestock-indicator/hasOriginType -->

    <owl:ObjectProperty rdf:about="https://w3id.org/leo/onto/livestock-indicator/hasOriginType">
        <rdfs:domain rdf:resource="https://w3id.org/leo/onto/livestock-indicator/LivestockIndicatorCalculation"/>
        <rdfs:range rdf:resource="https://w3id.org/leo/onto/livestock-indicator/LivestockIndicatorOriginType"/>
        <rdfs:comment xml:lang="en">Property used to specify all the sources fot the livestock indicator calculation that are not the foreign countries of influence on the calculation.</rdfs:comment>
        <rdfs:comment xml:lang="it">Proprietà utilizzata per specificare tutte le fonti per il calcolo dell&apos;indicatore zootecnico che non sono i Paesi stranieri di influenza sul calcolo.</rdfs:comment>
        <rdfs:isDefinedBy rdf:resource="https://w3id.org/leo/onto/livestock-indicator"/>
        <rdfs:label xml:lang="it">ha tipologia origine (diversa dal paese straniero d&apos;influenza)</rdfs:label>
        <rdfs:label xml:lang="en">has origin type (different from foreign country of influence)</rdfs:label>
        <owl:versionInfo xml:lang="it">stabile</owl:versionInfo>
        <owl:versionInfo xml:lang="en">stable</owl:versionInfo>
    </owl:ObjectProperty>
    


    <!-- https://w3id.org/leo/onto/livestock-indicator/hasYearOfReference -->

    <owl:ObjectProperty rdf:about="https://w3id.org/leo/onto/livestock-indicator/hasYearOfReference">
        <rdfs:subPropertyOf rdf:resource="https://w3id.org/italia/onto/TI/hasYear"/>
        <rdfs:domain>
            <owl:Class>
                <owl:unionOf rdf:parseType="Collection">
                    <rdf:Description rdf:about="https://w3id.org/leo/onto/livestock-indicator/LivestockIndicatorCalcCollection"/>
                    <rdf:Description rdf:about="https://w3id.org/leo/onto/livestock-indicator/LivestockIndicatorCalculation"/>
                </owl:unionOf>
            </owl:Class>
        </rdfs:domain>
        <rdfs:range rdf:resource="https://w3id.org/italia/onto/TI/Year"/>
        <rdfs:comment xml:lang="en">Property allowing one to specify the reference year of the livestock indicator calculation.</rdfs:comment>
        <rdfs:comment xml:lang="it">Proprietà che consente di specificare l&apos;anno di riferimento del calcolo dell&apos;indicatore zootecnico.</rdfs:comment>
        <rdfs:isDefinedBy rdf:resource="https://w3id.org/leo/onto/livestock-indicator"/>
        <rdfs:label xml:lang="it">ha anno di riferimento</rdfs:label>
        <rdfs:label xml:lang="en">has year of reference</rdfs:label>
        <owl:versionInfo xml:lang="it">stabile</owl:versionInfo>
        <owl:versionInfo xml:lang="en">stable</owl:versionInfo>
    </owl:ObjectProperty>
    


    <!-- 
    ///////////////////////////////////////////////////////////////////////////////////////
    //
    // Data properties
    //
    ///////////////////////////////////////////////////////////////////////////////////////
     -->

    


    <!-- https://w3id.org/leo/onto/livestock-indicator/computationDate -->

    <owl:DatatypeProperty rdf:about="https://w3id.org/leo/onto/livestock-indicator/computationDate">
        <rdfs:subPropertyOf rdf:resource="https://w3id.org/italia/onto/TI/date"/>
        <rdfs:domain rdf:resource="https://w3id.org/leo/onto/livestock-indicator/LivestockIndicator"/>
        <rdfs:range>
            <rdfs:Datatype>
                <owl:unionOf rdf:parseType="Collection">
                    <rdf:Description rdf:about="http://www.w3.org/2001/XMLSchema#date"/>
                    <rdf:Description rdf:about="http://www.w3.org/2001/XMLSchema#dateTime"/>
                </owl:unionOf>
            </rdfs:Datatype>
        </rdfs:range>
        <rdfs:comment xml:lang="it">La data di calcolo dell&apos;indicatore.</rdfs:comment>
        <rdfs:comment xml:lang="en">The computation date of the indicator.</rdfs:comment>
        <rdfs:isDefinedBy rdf:resource="https://w3id.org/leo/onto/livestock-indicator"/>
        <rdfs:label xml:lang="en">computation date</rdfs:label>
        <rdfs:label xml:lang="it">data di calcolo</rdfs:label>
        <owl:versionInfo xml:lang="it">stabile</owl:versionInfo>
        <owl:versionInfo xml:lang="en">stable</owl:versionInfo>
    </owl:DatatypeProperty>
    


    <!-- 
    ///////////////////////////////////////////////////////////////////////////////////////
    //
    // Classes
    //
    ///////////////////////////////////////////////////////////////////////////////////////
     -->

    


    <!-- http://www.w3.org/2004/02/skos/core#Concept -->

    <owl:Class rdf:about="http://www.w3.org/2004/02/skos/core#Concept"/>
    


    <!-- https://w3id.org/leo/onto/animal/Breed -->

    <owl:Class rdf:about="https://w3id.org/leo/onto/animal/Breed"/>
    


    <!-- https://w3id.org/leo/onto/animal/FarmAnimal -->

    <owl:Class rdf:about="https://w3id.org/leo/onto/animal/FarmAnimal"/>
    


    <!-- https://w3id.org/leo/onto/animal/LivestockSpecies -->

    <owl:Class rdf:about="https://w3id.org/leo/onto/animal/LivestockSpecies"/>
    


    <!-- https://w3id.org/leo/onto/animal/ProductionType -->

    <owl:Class rdf:about="https://w3id.org/leo/onto/animal/ProductionType"/>
    


    <!-- https://w3id.org/leo/onto/co/LivestockFarm -->

    <owl:Class rdf:about="https://w3id.org/leo/onto/co/LivestockFarm"/>
    


    <!-- https://w3id.org/leo/onto/livestock-indicator/AnimalBasedIndicatorCalculation -->

    <owl:Class rdf:about="https://w3id.org/leo/onto/livestock-indicator/AnimalBasedIndicatorCalculation">
        <rdfs:subClassOf rdf:resource="https://w3id.org/leo/onto/livestock-indicator/LivestockIndicatorCalculation"/>
        <rdfs:subClassOf>
            <owl:Restriction>
                <owl:onProperty rdf:resource="https://w3id.org/leo/onto/livestock-indicator/computedForFarmAnimal"/>
                <owl:someValuesFrom rdf:resource="https://w3id.org/leo/onto/animal/FarmAnimal"/>
            </owl:Restriction>
        </rdfs:subClassOf>
        <rdfs:subClassOf>
            <owl:Restriction>
                <owl:onProperty rdf:resource="https://w3id.org/leo/onto/livestock-indicator/computedForFarmAnimal"/>
                <owl:allValuesFrom rdf:resource="https://w3id.org/leo/onto/animal/FarmAnimal"/>
            </owl:Restriction>
        </rdfs:subClassOf>
        <rdfs:comment xml:lang="it">La classe del calcolo di tutti gli indicatori che si basano sul singolo animale d&apos;allevamento. Rientrano in questa categoria il calcolo degli indici genetici.</rdfs:comment>
        <rdfs:comment xml:lang="en">The class of calculating all indicators that are based on the individual farm animal. This category includes the calculation of genetic indexes.</rdfs:comment>
        <rdfs:isDefinedBy rdf:resource="https://w3id.org/leo/onto/livestock-indicator"/>
        <rdfs:label xml:lang="en">Animal-based Indicator Calculation</rdfs:label>
        <rdfs:label xml:lang="it">Calcolo Indicatore Zootecnico su Animale</rdfs:label>
        <owl:versionInfo xml:lang="it">stabile</owl:versionInfo>
        <owl:versionInfo xml:lang="en">stable</owl:versionInfo>
    </owl:Class>
    


    <!-- https://w3id.org/leo/onto/livestock-indicator/CompanyBasedIndicatorCalculation -->

    <owl:Class rdf:about="https://w3id.org/leo/onto/livestock-indicator/CompanyBasedIndicatorCalculation">
        <rdfs:subClassOf rdf:resource="https://w3id.org/leo/onto/livestock-indicator/LivestockIndicatorCalculation"/>
        <rdfs:subClassOf>
            <owl:Restriction>
                <owl:onProperty rdf:resource="https://w3id.org/leo/onto/livestock-indicator/associatedWithCompany"/>
                <owl:someValuesFrom rdf:resource="https://w3id.org/leo/onto/co/LivestockFarm"/>
            </owl:Restriction>
        </rdfs:subClassOf>
        <rdfs:subClassOf>
            <owl:Restriction>
                <owl:onProperty rdf:resource="https://w3id.org/leo/onto/livestock-indicator/associatedWithProductionTarget"/>
                <owl:someValuesFrom rdf:resource="https://w3id.org/leo/onto/animal/ProductionType"/>
            </owl:Restriction>
        </rdfs:subClassOf>
        <rdfs:subClassOf>
            <owl:Restriction>
                <owl:onProperty rdf:resource="https://w3id.org/leo/onto/livestock-indicator/associatedWithCompany"/>
                <owl:allValuesFrom rdf:resource="https://w3id.org/leo/onto/co/LivestockFarm"/>
            </owl:Restriction>
        </rdfs:subClassOf>
        <rdfs:subClassOf>
            <owl:Restriction>
                <owl:onProperty rdf:resource="https://w3id.org/leo/onto/livestock-indicator/associatedWithBreed"/>
                <owl:maxQualifiedCardinality rdf:datatype="http://www.w3.org/2001/XMLSchema#nonNegativeInteger">1</owl:maxQualifiedCardinality>
                <owl:onClass rdf:resource="https://w3id.org/leo/onto/animal/Breed"/>
            </owl:Restriction>
        </rdfs:subClassOf>
        <rdfs:comment xml:lang="en">The class of calculating all indicators that are based on the individual farm company. This category includes the calculation of the wellbeing farm animal indicator.</rdfs:comment>
        <rdfs:isDefinedBy rdf:resource="https://w3id.org/leo/onto/livestock-indicator"/>
        <rdfs:label xml:lang="it">Calcolo Indicatore Zootecnico su Azienda</rdfs:label>
        <rdfs:label xml:lang="en">Company-based Indicator Calculation</rdfs:label>
        <rdfs:label xml:lang="it">La classe di calcolo di tutti gli indicatori che si basano sull&apos;azienda da allevamento. Questa categoria comprende il calcolo dell&apos;indicatore di benessere degli animali da allevamento.</rdfs:label>
        <owl:versionInfo xml:lang="it">stabile</owl:versionInfo>
        <owl:versionInfo xml:lang="en">stable</owl:versionInfo>
    </owl:Class>
    


    <!-- https://w3id.org/leo/onto/livestock-indicator/ComplementaryInfo -->

    <owl:Class rdf:about="https://w3id.org/leo/onto/livestock-indicator/ComplementaryInfo">
        <rdfs:subClassOf rdf:resource="https://w3id.org/italia/onto/l0/Concept"/>
        <rdfs:subClassOf>
            <owl:Restriction>
                <owl:onProperty rdf:resource="https://w3id.org/italia/onto/l0/name"/>
                <owl:someValuesFrom rdf:resource="http://www.w3.org/2000/01/rdf-schema#Literal"/>
            </owl:Restriction>
        </rdfs:subClassOf>
        <rdfs:subClassOf>
            <owl:Restriction>
                <owl:onProperty rdf:resource="https://w3id.org/italia/onto/l0/name"/>
                <owl:allValuesFrom rdf:resource="http://www.w3.org/2000/01/rdf-schema#Literal"/>
            </owl:Restriction>
        </rdfs:subClassOf>
        <rdfs:comment xml:lang="it">La classe del tipo di informazioni complementari per il calcolo dell&apos;indicatore  zootecnico.</rdfs:comment>
        <rdfs:comment xml:lang="en">The class of the type of complementary information for the calculation of the livestock indicator.</rdfs:comment>
        <rdfs:isDefinedBy rdf:resource="https://w3id.org/leo/onto/livestock-indicator"/>
        <rdfs:label xml:lang="en">Complementary Information</rdfs:label>
        <rdfs:label xml:lang="it">Informazione Complementare</rdfs:label>
        <owl:versionInfo xml:lang="it">stabile</owl:versionInfo>
        <owl:versionInfo xml:lang="en">stable</owl:versionInfo>
    </owl:Class>
    


    <!-- https://w3id.org/leo/onto/livestock-indicator/ComplementaryInfoDescription -->

    <owl:Class rdf:about="https://w3id.org/leo/onto/livestock-indicator/ComplementaryInfoDescription">
        <rdfs:subClassOf rdf:resource="https://w3id.org/italia/onto/l0/Description"/>
        <rdfs:subClassOf>
            <owl:Restriction>
                <owl:onProperty rdf:resource="https://w3id.org/italia/onto/MU/hasValue"/>
                <owl:someValuesFrom rdf:resource="https://w3id.org/italia/onto/MU/Value"/>
            </owl:Restriction>
        </rdfs:subClassOf>
        <rdfs:subClassOf>
            <owl:Restriction>
                <owl:onProperty rdf:resource="https://w3id.org/leo/onto/livestock-indicator/hasComplementaryInfo"/>
                <owl:qualifiedCardinality rdf:datatype="http://www.w3.org/2001/XMLSchema#nonNegativeInteger">1</owl:qualifiedCardinality>
                <owl:onClass rdf:resource="https://w3id.org/leo/onto/livestock-indicator/ComplementaryInfo"/>
            </owl:Restriction>
        </rdfs:subClassOf>
        <rdfs:comment xml:lang="it">La classe rappresenta la descrizione complessiva delle informazioni complementari (quali informazioni e il loro valore) utilizzate nel calcolo dell&apos;indicatore zootecnico. Esempi includono, numero di figlie = 3, numero di aziende = 1, ecc.</rdfs:comment>
        <rdfs:comment xml:lang="en">The class represents the overall description of the complementary information (what information and its value) used in the calculation of the livestock indicator. Example are: number of daughters = 3, number of companies = 1, etc.</rdfs:comment>
        <rdfs:isDefinedBy rdf:resource="https://w3id.org/leo/onto/livestock-indicator"/>
        <rdfs:label xml:lang="en">Complementary Information Description</rdfs:label>
        <rdfs:label xml:lang="it">Descrizione Informazioni Complementari</rdfs:label>
        <owl:versionInfo xml:lang="it">stabile</owl:versionInfo>
        <owl:versionInfo xml:lang="en">stable</owl:versionInfo>
    </owl:Class>
    


    <!-- https://w3id.org/leo/onto/livestock-indicator/LivestockIndicator -->

    <owl:Class rdf:about="https://w3id.org/leo/onto/livestock-indicator/LivestockIndicator">
        <rdfs:subClassOf rdf:resource="https://w3id.org/italia/onto/Indicator/Indicator"/>
        <rdfs:comment xml:lang="en">It represents an indicator used in the livestock context. The Livestock Indicator is defined through  a name and a description. Example: the farm animal wellbeing indicator, the genetic feed conversion ratio, etc.</rdfs:comment>
        <rdfs:comment xml:lang="it">Rappresenta un indicatore usato nell&apos;ambito zootecnico. L&apos;indicatore è definito sulla base di un nome e una descrizione. Peer esempio l&apos;indice benessere animale, l&apos;indice genetico di conversione alimentare (ICA), ecc.</rdfs:comment>
        <rdfs:isDefinedBy rdf:resource="https://w3id.org/leo/onto/livestock-indicator"/>
        <rdfs:label xml:lang="it">Indicatore Zootecnico</rdfs:label>
        <rdfs:label xml:lang="en">Livestock Indicator</rdfs:label>
        <owl:versionInfo xml:lang="it">stabile</owl:versionInfo>
        <owl:versionInfo xml:lang="en">stable</owl:versionInfo>
    </owl:Class>
    


    <!-- https://w3id.org/leo/onto/livestock-indicator/LivestockIndicatorCalcCollection -->

    <owl:Class rdf:about="https://w3id.org/leo/onto/livestock-indicator/LivestockIndicatorCalcCollection">
        <rdfs:subClassOf rdf:resource="https://w3id.org/italia/onto/l0/Collection"/>
        <rdfs:subClassOf>
            <owl:Restriction>
                <owl:onProperty rdf:resource="https://w3id.org/italia/onto/l0/hasMember"/>
                <owl:someValuesFrom rdf:resource="https://w3id.org/leo/onto/livestock-indicator/LivestockIndicatorCalculation"/>
            </owl:Restriction>
        </rdfs:subClassOf>
        <rdfs:subClassOf>
            <owl:Restriction>
                <owl:onProperty rdf:resource="https://w3id.org/leo/onto/livestock-indicator/associatedWithCompany"/>
                <owl:someValuesFrom rdf:resource="https://w3id.org/leo/onto/co/LivestockFarm"/>
            </owl:Restriction>
        </rdfs:subClassOf>
        <rdfs:subClassOf>
            <owl:Restriction>
                <owl:onProperty rdf:resource="https://w3id.org/leo/onto/livestock-indicator/hasComplementaryInformationDesc"/>
                <owl:allValuesFrom rdf:resource="https://w3id.org/leo/onto/livestock-indicator/ComplementaryInfoDescription"/>
            </owl:Restriction>
        </rdfs:subClassOf>
        <rdfs:subClassOf>
            <owl:Restriction>
                <owl:onProperty rdf:resource="https://w3id.org/leo/onto/livestock-indicator/associatedWithProductionTarget"/>
                <owl:maxQualifiedCardinality rdf:datatype="http://www.w3.org/2001/XMLSchema#nonNegativeInteger">1</owl:maxQualifiedCardinality>
                <owl:onClass rdf:resource="https://w3id.org/leo/onto/animal/ProductionType"/>
            </owl:Restriction>
        </rdfs:subClassOf>
        <rdfs:subClassOf>
            <owl:Restriction>
                <owl:onProperty rdf:resource="https://w3id.org/leo/onto/livestock-indicator/associatedWithSpecies"/>
                <owl:maxQualifiedCardinality rdf:datatype="http://www.w3.org/2001/XMLSchema#nonNegativeInteger">1</owl:maxQualifiedCardinality>
                <owl:onClass rdf:resource="https://w3id.org/leo/onto/animal/LivestockSpecies"/>
            </owl:Restriction>
        </rdfs:subClassOf>
        <rdfs:subClassOf>
            <owl:Restriction>
                <owl:onProperty rdf:resource="https://w3id.org/leo/onto/livestock-indicator/hasYearOfReference"/>
                <owl:maxQualifiedCardinality rdf:datatype="http://www.w3.org/2001/XMLSchema#nonNegativeInteger">1</owl:maxQualifiedCardinality>
                <owl:onClass rdf:resource="https://w3id.org/italia/onto/TI/Year"/>
            </owl:Restriction>
        </rdfs:subClassOf>
        <rdfs:comment xml:lang="it">La classe che consente di raggruppare in una collezione calcoli di indicatori zootecnici. Utilizzata per l&apos;indicatore estate-inverno.</rdfs:comment>
        <rdfs:comment xml:lang="en">The class for grouping calculations of livestock indicators in a collection. Used for the summer-winter indicator.</rdfs:comment>
        <rdfs:isDefinedBy rdf:resource="https://w3id.org/leo/onto/livestock-indicator"/>
        <rdfs:label xml:lang="it">Collezione di Indicatori Zootecnici</rdfs:label>
        <rdfs:label xml:lang="en">Livestock Indicator Calculation Collection</rdfs:label>
        <owl:versionInfo xml:lang="it">stabile</owl:versionInfo>
        <owl:versionInfo xml:lang="en">stable</owl:versionInfo>
    </owl:Class>
    


    <!-- https://w3id.org/leo/onto/livestock-indicator/LivestockIndicatorCalculation -->

    <owl:Class rdf:about="https://w3id.org/leo/onto/livestock-indicator/LivestockIndicatorCalculation">
        <rdfs:subClassOf rdf:resource="https://w3id.org/italia/onto/Indicator/IndicatorCalculation"/>
        <rdfs:subClassOf>
            <owl:Restriction>
                <owl:onProperty rdf:resource="https://w3id.org/leo/onto/livestock-indicator/associatedWithSpecies"/>
                <owl:allValuesFrom rdf:resource="https://w3id.org/leo/onto/animal/LivestockSpecies"/>
            </owl:Restriction>
        </rdfs:subClassOf>
        <rdfs:subClassOf>
            <owl:Restriction>
                <owl:onProperty rdf:resource="https://w3id.org/leo/onto/livestock-indicator/basedOnCalculation"/>
                <owl:allValuesFrom rdf:resource="https://w3id.org/leo/onto/livestock-indicator/LivestockIndicatorCalculation"/>
            </owl:Restriction>
        </rdfs:subClassOf>
        <rdfs:subClassOf>
            <owl:Restriction>
                <owl:onProperty rdf:resource="https://w3id.org/leo/onto/livestock-indicator/hasCalculationAccuracy"/>
                <owl:allValuesFrom rdf:resource="https://w3id.org/italia/onto/MU/Value"/>
            </owl:Restriction>
        </rdfs:subClassOf>
        <rdfs:subClassOf>
            <owl:Restriction>
                <owl:onProperty rdf:resource="https://w3id.org/leo/onto/livestock-indicator/hasComplementaryInformationDesc"/>
                <owl:allValuesFrom rdf:resource="https://w3id.org/leo/onto/livestock-indicator/ComplementaryInfoDescription"/>
            </owl:Restriction>
        </rdfs:subClassOf>
        <rdfs:subClassOf>
            <owl:Restriction>
                <owl:onProperty rdf:resource="https://w3id.org/leo/onto/livestock-indicator/hasCountryOfInfluence"/>
                <owl:allValuesFrom rdf:resource="http://www.w3.org/2004/02/skos/core#Concept"/>
            </owl:Restriction>
        </rdfs:subClassOf>
        <rdfs:subClassOf>
            <owl:Restriction>
                <owl:onProperty rdf:resource="https://w3id.org/leo/onto/livestock-indicator/hasOriginType"/>
                <owl:allValuesFrom rdf:resource="https://w3id.org/leo/onto/livestock-indicator/LivestockIndicatorOriginType"/>
            </owl:Restriction>
        </rdfs:subClassOf>
        <rdfs:subClassOf>
            <owl:Restriction>
                <owl:onProperty rdf:resource="https://w3id.org/leo/onto/livestock-indicator/hasYearOfReference"/>
                <owl:allValuesFrom rdf:resource="https://w3id.org/italia/onto/TI/Year"/>
            </owl:Restriction>
        </rdfs:subClassOf>
        <rdfs:subClassOf>
            <owl:Restriction>
                <owl:onProperty rdf:resource="https://w3id.org/leo/onto/livestock-indicator/computationDate"/>
                <owl:maxQualifiedCardinality rdf:datatype="http://www.w3.org/2001/XMLSchema#nonNegativeInteger">1</owl:maxQualifiedCardinality>
                <owl:onDataRange rdf:resource="http://www.w3.org/2001/XMLSchema#date"/>
            </owl:Restriction>
        </rdfs:subClassOf>
        <rdfs:comment xml:lang="it">La classe del calcolo di uno specifico indicatore zootecnico eseguito seguendo un certo metodo di calcolo. La classe consente di separare il calcolo dell&apos;indicatore zootecnico con i valori e le metriche che contribuiscono al calcolo, con l&apos;indicatore zootecnico stesso.</rdfs:comment>
        <rdfs:comment xml:lang="en">The class of calculation of a specific livestock indicator performed following a certain calculation method and using one or more complementary information. The class allows one to separate the calculation of the livestock indicator with the values and metrics that contribute to the calculation, with the livestock indicator itself.</rdfs:comment>
        <rdfs:isDefinedBy rdf:resource="https://w3id.org/leo/onto/livestock-indicator"/>
        <rdfs:label xml:lang="it">Calcolo Indicatore Zootecnico</rdfs:label>
        <rdfs:label xml:lang="en">Livestock Indicator Calculation</rdfs:label>
        <owl:versionInfo xml:lang="it">stabile</owl:versionInfo>
        <owl:versionInfo xml:lang="en">stable</owl:versionInfo>
    </owl:Class>
    


    <!-- https://w3id.org/leo/onto/livestock-indicator/LivestockIndicatorOriginType -->

    <owl:Class rdf:about="https://w3id.org/leo/onto/livestock-indicator/LivestockIndicatorOriginType">
        <rdfs:subClassOf rdf:resource="https://w3id.org/italia/onto/l0/Characteristic"/>
        <rdfs:subClassOf>
            <owl:Restriction>
                <owl:onProperty rdf:resource="https://w3id.org/italia/onto/l0/name"/>
                <owl:someValuesFrom rdf:resource="http://www.w3.org/2000/01/rdf-schema#Literal"/>
            </owl:Restriction>
        </rdfs:subClassOf>
        <rdfs:subClassOf>
            <owl:Restriction>
                <owl:onProperty rdf:resource="https://w3id.org/italia/onto/l0/name"/>
                <owl:allValuesFrom rdf:resource="http://www.w3.org/2000/01/rdf-schema#Literal"/>
            </owl:Restriction>
        </rdfs:subClassOf>
        <rdfs:comment xml:lang="it">La classe di tutti i tipi di origini, utilizzate nel calcolo degli indicatori zootecnici,diverse dal Paese estero di influenza del calcolo. Esempi includono: sistemi specifici di conversione.</rdfs:comment>
        <rdfs:comment xml:lang="en">The class of all types of sources, used in the calculation of the livestock indicators, that are different from the foreign country of influence of the calculation. Examples include specific conversion systems.</rdfs:comment>
        <rdfs:isDefinedBy rdf:resource="https://w3id.org/leo/onto/livestock-indicator"/>
        <rdfs:label xml:lang="en">Livestock Indicator Origin Type</rdfs:label>
        <rdfs:label xml:lang="it">Tipo Origine Indicatore Zootecnico</rdfs:label>
        <owl:versionInfo xml:lang="it">stabile</owl:versionInfo>
        <owl:versionInfo xml:lang="en">stable</owl:versionInfo>
    </owl:Class>
    


    <!-- 
    ///////////////////////////////////////////////////////////////////////////////////////
    //
    // Individuals
    //
    ///////////////////////////////////////////////////////////////////////////////////////
     -->

    


    <!-- https://w3id.org/leo/data/contact-point/onto-aia -->

    <owl:NamedIndividual rdf:about="https://w3id.org/leo/data/contact-point/onto-aia">
        <rdf:type rdf:resource="http://dati.gov.it/onto/dcatapit#Organization"/>
        <rdf:type rdf:resource="http://www.w3.org/2006/vcard/ns#Kind"/>
        <rdf:type rdf:resource="http://www.w3.org/2006/vcard/ns#Organization"/>
        <rdfs:label xml:lang="it">Sistemi informativi</rdfs:label>
        <ns:fn xml:lang="it">Sistemi informativi</ns:fn>
        <ns:hasEmail rdf:resource="mailto:affarigenerali@pec.aia.it"/>
    </owl:NamedIndividual>
    


    <!-- https://w3id.org/leo/data/distribution/IND-JSON-LD -->

    <owl:NamedIndividual rdf:about="https://w3id.org/leo/data/distribution/IND-JSON-LD">
        <rdf:type rdf:resource="https://w3id.org/italia/onto/ADMS/SemanticAssetDistribution"/>
        <terms:description xml:lang="it">Questa è la distribuzione JSON-LD dell&apos;ontologia sugli indicatori del dominio zootecnico</terms:description>
        <terms:description xml:lang="en">This is the distribution in JSON-LD of Livestock Indicator ontology</terms:description>
        <terms:format rdf:resource="http://publications.europa.eu/resource/authority/file-type/JSON_LD"/>
        <terms:license rdf:resource="https://w3id.org/italia/controlled-vocabulary/licences/A21_CCBY40"/>
        <terms:title xml:lang="it">Distribuzione JSON-LD ontologia Indicatori</terms:title>
        <terms:title xml:lang="en">JSON-LD distribution of Indicator Ontology</terms:title>
        <rdfs:comment xml:lang="it">Questa è la distribuzione JSON-LD dell&apos;ontologia sugli indicatori del dominio zootecnico</rdfs:comment>
        <rdfs:comment xml:lang="en">This is the distribution in JSON-LD of Livestock Indicator ontology</rdfs:comment>
        <rdfs:label xml:lang="it">Distribuzione JSON-LD ontologia Indicatori</rdfs:label>
        <rdfs:label xml:lang="en">JSON-LD distribution of Indicator Ontology</rdfs:label>
        <dcat:accessURL rdf:resource="https://www.leo-project.it/Ontologie/indicator/latest"/>
        <dcat:downloadURL rdf:resource="https://www.leo-project.it/Ontologie/indicator/latest/indicator.jsonld"/>
    </owl:NamedIndividual>
    


    <!-- https://w3id.org/leo/data/distribution/IND-RDF-TURTLE -->

    <owl:NamedIndividual rdf:about="https://w3id.org/leo/data/distribution/IND-RDF-TURTLE">
        <rdf:type rdf:resource="https://w3id.org/italia/onto/ADMS/SemanticAssetDistribution"/>
        <terms:description xml:lang="it">Questa è la distribuzione RDF/Turtle dell&apos;ontologia sugli indicatori del dominio zootecnico</terms:description>
        <terms:description xml:lang="en">This is the distribution in RDF/Turtle of Livestock Indicator ontology</terms:description>
        <terms:format rdf:resource="http://publications.europa.eu/resource/authority/file-type/RDF_TURTLE"/>
        <terms:license rdf:resource="https://w3id.org/italia/controlled-vocabulary/licences/A21_CCBY40"/>
        <terms:title xml:lang="it">Distribuzione RDF/Turtle ontologia Indicatori</terms:title>
        <terms:title xml:lang="en">RDF/Turtle distribution of Indicator Ontology</terms:title>
        <rdfs:comment xml:lang="it">Questa è la distribuzione RDF/Turtle dell&apos;ontologia sugli indicatori del dominio zootecnico</rdfs:comment>
        <rdfs:comment xml:lang="en">This is the distribution in RDF/Turtle of Livestock Indicator ontology</rdfs:comment>
        <rdfs:label xml:lang="it">Distribuzione RDF/Turtle ontologia Indicatori</rdfs:label>
        <rdfs:label xml:lang="en">RDF/Turtle distribution of Indicator Ontology</rdfs:label>
        <dcat:accessURL rdf:resource="https://www.leo-project.it/Ontologie/indicator/latest"/>
        <dcat:downloadURL rdf:resource="https://www.leo-project.it/Ontologie/indicator/latest/indicator.ttl"/>
    </owl:NamedIndividual>
    


    <!-- https://w3id.org/leo/data/distribution/IND-RDF-XML -->

    <owl:NamedIndividual rdf:about="https://w3id.org/leo/data/distribution/IND-RDF-XML">
        <rdf:type rdf:resource="https://w3id.org/italia/onto/ADMS/SemanticAssetDistribution"/>
        <terms:description xml:lang="it">Questa è la distribuzione RDF/XML dell&apos;ontologia sugli indicatori del dominio zootecnico</terms:description>
        <terms:description xml:lang="en">This is the distribution in RDF/XML of Livestock Indicator ontology</terms:description>
        <terms:format rdf:resource="http://publications.europa.eu/resource/authority/file-type/RDF_XML"/>
        <terms:license rdf:resource="https://w3id.org/italia/controlled-vocabulary/licences/A21_CCBY40"/>
        <terms:title xml:lang="it">Distribuzione RDF/XML ontologia Indicatori</terms:title>
        <terms:title xml:lang="en">RDF/XML distribution of Indicator Ontology</terms:title>
        <rdfs:comment xml:lang="it">Questa è la distribuzione RDF/XML dell&apos;ontologia sugli indicatori del dominio zootecnico</rdfs:comment>
        <rdfs:comment xml:lang="en">This is the distribution in RDF/XML of Livestock Indicator ontology</rdfs:comment>
        <rdfs:label xml:lang="it">Distribuzione RDF/XML ontologia Indicatori</rdfs:label>
        <rdfs:label xml:lang="en">RDF/XML distribution of Indicator Ontology</rdfs:label>
        <dcat:accessURL rdf:resource="https://www.leo-project.it/Ontologie/indicator/latest"/>
        <dcat:downloadURL rdf:resource="https://www.leo-project.it/Ontologie/indicator/latest/indicator.rdf"/>
    </owl:NamedIndividual>
    


    <!-- https://w3id.org/leo/data/private-organization/00944701002 -->

    <owl:NamedIndividual rdf:about="https://w3id.org/leo/data/private-organization/00944701002">
        <rdf:type rdf:resource="http://dati.gov.it/onto/dcatapit#Agent"/>
        <rdf:type rdf:resource="http://xmlns.com/foaf/0.1/Agent"/>
        <terms:identifier>00944701002</terms:identifier>
        <foaf:name xml:lang="it">Associazione Italiana Allevatori</foaf:name>
        <foaf:name xml:lang="en">Italian Breeders&apos; Association</foaf:name>
    </owl:NamedIndividual>
    


    <!-- https://w3id.org/leo/data/private-organization/06695411006 -->

    <owl:NamedIndividual rdf:about="https://w3id.org/leo/data/private-organization/06695411006">
        <rdf:type rdf:resource="http://dati.gov.it/onto/dcatapit#Agent"/>
        <rdf:type rdf:resource="http://xmlns.com/foaf/0.1/Agent"/>
        <terms:identifier>06695411006</terms:identifier>
        <foaf:name xml:lang="en">Bluarancio</foaf:name>
        <foaf:name xml:lang="it">Bluarancio</foaf:name>
    </owl:NamedIndividual>
    


    <!-- https://w3id.org/leo/data/project/LEO -->

    <owl:NamedIndividual rdf:about="https://w3id.org/leo/data/project/LEO">
        <rdf:type rdf:resource="https://w3id.org/italia/onto/ADMS/Project"/>
        <rdfs:label xml:lang="it">LEO - Livestok Environment Open Data</rdfs:label>
        <l0:name xml:lang="it">LEO - Livestok Environment Open Data</l0:name>
    </owl:NamedIndividual>
    


    <!-- https://w3id.org/leo/onto/indicator -->

    <owl:NamedIndividual rdf:about="https://w3id.org/leo/onto/indicator">
        <rdf:type rdf:resource="https://w3id.org/italia/onto/ADMS/SemanticAsset"/>
    </owl:NamedIndividual>
</rdf:RDF>



<!-- Generated by the OWL API (version 4.5.9.2019-02-01T07:24:44Z) https://github.com/owlcs/owlapi -->

