<?xml version="1.0"?>
<rdf:RDF xmlns="https://w3id.org/leo/onto/weather/"
     xml:base="https://w3id.org/leo/onto/weather/"
     xmlns:dc="http://purl.org/dc/elements/1.1/"
     xmlns:l0="https://w3id.org/italia/onto/l0/"
     xmlns:ns="http://www.w3.org/2006/vcard/ns#"
     xmlns:CLV="https://w3id.org/italia/onto/CLV/"
     xmlns:owl="http://www.w3.org/2002/07/owl#"
     xmlns:rdf="http://www.w3.org/1999/02/22-rdf-syntax-ns#"
     xmlns:xml="http://www.w3.org/XML/1998/namespace"
     xmlns:xsd="http://www.w3.org/2001/XMLSchema#"
     xmlns:ADMS="https://w3id.org/italia/onto/ADMS/"
     xmlns:dcat="http://www.w3.org/ns/dcat#"
     xmlns:foaf="http://xmlns.com/foaf/0.1/"
     xmlns:prov="http://www.w3.org/ns/prov#"
     xmlns:rdfs="http://www.w3.org/2000/01/rdf-schema#"
     xmlns:terms="http://purl.org/dc/terms/">
    <owl:Ontology rdf:about="https://w3id.org/leo/onto/weather">
        <owl:versionIRI rdf:resource="https://w3id.org/leo/onto/weather/0.3"/>
        <owl:imports rdf:resource="https://w3id.org/italia/onto/IoT"/>
        <owl:imports rdf:resource="https://w3id.org/italia/onto/l0"/>
        <dc:description rdf:resource="https://raw.githubusercontent.com/Bluarancio/Leo-OpenData/master/RappresentazioneGraficaOntologie/PNG/WeatherModule.png"/>
        <terms:accrualPeriodicity rdf:resource="http://publications.europa.eu/resource/authority/frequency/IRREG"/>
        <terms:creator rdf:resource="https://w3id.org/leo/data/private-organization/00944701002"/>
        <terms:description xml:lang="it">Questa è l&apos;ontologia per modellare i dati detti ClimData nel progetto LEO ovvero i dati raccolti di tipo climatico, intesi come osservazioni catturate da stazioni meteo. L&apos;ontologia include anche i concetti che consentono di rappresentare l&apos;installazione delle centraline meteo all&apos;interno di insediamenti dell&apos;allevamento.</terms:description>
        <terms:description xml:lang="en">This is the ontology for modelling the data known as ClimData in the LEO project, i.e. climate data collected as observations captured by weather stations. The ontology also includes the concepts for representing the installation of weather stations within livestock companies&apos; settlements.</terms:description>
        <terms:identifier>onto-BA-5</terms:identifier>
        <terms:issued rdf:datatype="http://www.w3.org/2001/XMLSchema#date">2019-11-20</terms:issued>
        <terms:language rdf:resource="http://publications.europa.eu/resource/authority/language/ENG"/>
        <terms:language rdf:resource="http://publications.europa.eu/resource/authority/language/ITA"/>
        <terms:modified xml:lang="en">2023-06-22</terms:modified>
        <terms:publisher rdf:resource="https://w3id.org/leo/data/private-organization/00944701002"/>
        <terms:rightsHolder rdf:resource="https://w3id.org/leo/data/private-organization/00944701002"/>
        <terms:subject rdf:resource="http://eurovoc.europa.eu/1892"/>
        <terms:title xml:lang="it">Ontologia dei dati meteo del progetto LEO (Livestock Environment Open Data) - ClimData</terms:title>
        <terms:title xml:lang="en">Weather Ontology of the LEO Project (Livestock Environment Open Data)</terms:title>
        <rdfs:comment xml:lang="it">Questa è l&apos;ontologia per modellare i dati detti ClimData nel progetto LEO ovvero i dati raccolti di tipo climatico, intesi come osservazioni catturate da stazioni meteo.</rdfs:comment>
        <rdfs:comment xml:lang="en">This is the ontology used to model the data called ClimData in the LEO project, i.e. the collected climate data intended to be observations captured by weather stations.</rdfs:comment>
        <rdfs:isDefinedBy rdf:resource="https://w3id.org/leo/onto/weather"/>
        <rdfs:label xml:lang="it">Ontologia dei dati meteo del progetto LEO (Livestock Environment Open Data) - ClimData</rdfs:label>
        <rdfs:label xml:lang="en">Weather Ontology of the LEO Project (Livestock Environment Open Data)</rdfs:label>
        <owl:versionInfo xml:lang="en">Version 0.3 - June 2023 - Introduction of the installation concept for weather stations located within buildings of the livestock farm company site</owl:versionInfo>
        <owl:versionInfo xml:lang="it">Versione 0.3 - Giugno 2023 - Introduzione del concetto di installazione di centraline meteo localizzate all&apos;interno di insediamenti zootecnici.</owl:versionInfo>
        <dcat:contactPoint rdf:resource="https://w3id.org/leo/data/contact-point/onto-aia"/>
        <dcat:keyword xml:lang="it">Centraline Meteo</dcat:keyword>
        <dcat:keyword xml:lang="it">Meteo</dcat:keyword>
        <dcat:keyword xml:lang="it">Precipitazioni</dcat:keyword>
        <dcat:keyword xml:lang="it">Temperatura</dcat:keyword>
        <dcat:keyword xml:lang="it">Umidità</dcat:keyword>
        <dcat:keyword xml:lang="it">Ventosìtà</dcat:keyword>
        <dcat:theme rdf:resource="http://publications.europa.eu/resource/authority/data-theme/ENVI"/>
        <ADMS:acronym>WT</ADMS:acronym>
        <ADMS:hasContributor rdf:resource="https://w3id.org/leo/data/private-organization/06695411006"/>
        <ADMS:hasFormalityLevel rdf:resource="https://w3id.org/italia/onto/ADMS/Formal"/>
        <ADMS:hasKeyClass rdf:resource="https://w3id.org/leo/onto/weather/WeatherObservation"/>
        <ADMS:hasKeyClass rdf:resource="https://w3id.org/leo/onto/weather/WeatherStation"/>
        <ADMS:hasOntologyLanguage rdf:resource="https://w3id.org/italia/onto/ADMS/OWL"/>
        <ADMS:hasSemanticAssetDistribution rdf:resource="https://w3id.org/leo/data/distribution/WT-JSON-LD"/>
        <ADMS:hasSemanticAssetDistribution rdf:resource="https://w3id.org/leo/data/distribution/WT-RDF-TURTLE"/>
        <ADMS:hasSemanticAssetDistribution rdf:resource="https://w3id.org/leo/data/distribution/WT-RDF-XML"/>
        <ADMS:hasTask rdf:resource="https://w3id.org/italia/onto/ADMS/AnnotationTask"/>
        <ADMS:hasTask rdf:resource="https://w3id.org/italia/onto/ADMS/QueryFormulationTask"/>
        <ADMS:hasTask rdf:resource="https://w3id.org/italia/onto/ADMS/SearchTask"/>
        <ADMS:officialURI rdf:datatype="http://www.w3.org/2001/XMLSchema#anyURI">https://w3id.org/leo/onto/weather</ADMS:officialURI>
        <ADMS:prefix>wt</ADMS:prefix>
        <ADMS:semanticAssetInUse rdf:resource="https://w3id.org/leo/data/project/LEO"/>
        <ADMS:status>catalogued</ADMS:status>
        <ADMS:target xml:lang="it">Comunità open data</ADMS:target>
        <ADMS:target>Imprese</ADMS:target>
        <ADMS:target xml:lang="it">Professionisti del settore zootecnico</ADMS:target>
        <ADMS:target>Pubbliche Amministrazioni</ADMS:target>
        <ADMS:type rdf:resource="https://w3id.org/italia/onto/ADMS/DomainOntology"/>
    </owl:Ontology>



    <!--
    ///////////////////////////////////////////////////////////////////////////////////////
    //
    // Annotation properties
    //
    ///////////////////////////////////////////////////////////////////////////////////////
     -->




    <!-- http://purl.org/dc/elements/1.1/description -->

    <owl:AnnotationProperty rdf:about="http://purl.org/dc/elements/1.1/description"/>



    <!-- http://purl.org/dc/terms/description -->

    <owl:AnnotationProperty rdf:about="http://purl.org/dc/terms/description"/>



    <!-- http://purl.org/dc/terms/format -->

    <owl:AnnotationProperty rdf:about="http://purl.org/dc/terms/format"/>



    <!-- http://purl.org/dc/terms/identifier -->

    <owl:AnnotationProperty rdf:about="http://purl.org/dc/terms/identifier"/>



    <!-- http://purl.org/dc/terms/label -->

    <owl:AnnotationProperty rdf:about="http://purl.org/dc/terms/label"/>



    <!-- http://purl.org/dc/terms/license -->

    <owl:AnnotationProperty rdf:about="http://purl.org/dc/terms/license"/>



    <!-- http://purl.org/dc/terms/subject -->

    <owl:AnnotationProperty rdf:about="http://purl.org/dc/terms/subject"/>



    <!-- http://purl.org/dc/terms/title -->

    <owl:AnnotationProperty rdf:about="http://purl.org/dc/terms/title"/>



    <!-- http://www.w3.org/2006/vcard/ns#fn -->

    <owl:AnnotationProperty rdf:about="http://www.w3.org/2006/vcard/ns#fn"/>



    <!-- http://www.w3.org/2006/vcard/ns#hasEmail -->

    <owl:AnnotationProperty rdf:about="http://www.w3.org/2006/vcard/ns#hasEmail"/>



    <!-- http://www.w3.org/ns/dcat#accessURL -->

    <owl:AnnotationProperty rdf:about="http://www.w3.org/ns/dcat#accessURL"/>



    <!-- http://www.w3.org/ns/dcat#downloadURL -->

    <owl:AnnotationProperty rdf:about="http://www.w3.org/ns/dcat#downloadURL"/>



    <!-- http://www.w3.org/ns/prov#wasDerivedFrom -->

    <owl:AnnotationProperty rdf:about="http://www.w3.org/ns/prov#wasDerivedFrom"/>



    <!-- http://www.w3.org/ns/prov#wasInfluencedBy -->

    <owl:AnnotationProperty rdf:about="http://www.w3.org/ns/prov#wasInfluencedBy"/>



    <!-- http://xmlns.com/foaf/0.1/name -->

    <owl:AnnotationProperty rdf:about="http://xmlns.com/foaf/0.1/name"/>



    <!-- https://w3id.org/italia/onto/ADMS/acronym -->

    <owl:AnnotationProperty rdf:about="https://w3id.org/italia/onto/ADMS/acronym"/>



    <!-- https://w3id.org/italia/onto/ADMS/hasContributor -->

    <owl:AnnotationProperty rdf:about="https://w3id.org/italia/onto/ADMS/hasContributor"/>



    <!-- https://w3id.org/italia/onto/ADMS/hasFormalityLevel -->

    <owl:AnnotationProperty rdf:about="https://w3id.org/italia/onto/ADMS/hasFormalityLevel"/>



    <!-- https://w3id.org/italia/onto/ADMS/hasKeyClass -->

    <owl:AnnotationProperty rdf:about="https://w3id.org/italia/onto/ADMS/hasKeyClass"/>



    <!-- https://w3id.org/italia/onto/ADMS/hasOntologyLanguage -->

    <owl:AnnotationProperty rdf:about="https://w3id.org/italia/onto/ADMS/hasOntologyLanguage"/>



    <!-- https://w3id.org/italia/onto/ADMS/hasSemanticAssetDistribution -->

    <owl:AnnotationProperty rdf:about="https://w3id.org/italia/onto/ADMS/hasSemanticAssetDistribution"/>



    <!-- https://w3id.org/italia/onto/ADMS/hasTask -->

    <owl:AnnotationProperty rdf:about="https://w3id.org/italia/onto/ADMS/hasTask"/>



    <!-- https://w3id.org/italia/onto/ADMS/officialURI -->

    <owl:AnnotationProperty rdf:about="https://w3id.org/italia/onto/ADMS/officialURI"/>



    <!-- https://w3id.org/italia/onto/ADMS/prefix -->

    <owl:AnnotationProperty rdf:about="https://w3id.org/italia/onto/ADMS/prefix"/>



    <!-- https://w3id.org/italia/onto/ADMS/semanticAssetInUse -->

    <owl:AnnotationProperty rdf:about="https://w3id.org/italia/onto/ADMS/semanticAssetInUse"/>



    <!-- https://w3id.org/italia/onto/ADMS/status -->

    <owl:AnnotationProperty rdf:about="https://w3id.org/italia/onto/ADMS/status"/>



    <!-- https://w3id.org/italia/onto/ADMS/target -->

    <owl:AnnotationProperty rdf:about="https://w3id.org/italia/onto/ADMS/target"/>



    <!-- https://w3id.org/italia/onto/ADMS/type -->

    <owl:AnnotationProperty rdf:about="https://w3id.org/italia/onto/ADMS/type"/>



    <!-- https://w3id.org/italia/onto/l0/controlledVocabulary -->

    <owl:AnnotationProperty rdf:about="https://w3id.org/italia/onto/l0/controlledVocabulary"/>



    <!-- https://w3id.org/italia/onto/l0/name -->

    <owl:AnnotationProperty rdf:about="https://w3id.org/italia/onto/l0/name"/>



    <!--
    ///////////////////////////////////////////////////////////////////////////////////////
    //
    // Object Properties
    //
    ///////////////////////////////////////////////////////////////////////////////////////
     -->




    <!-- https://w3id.org/leo/onto/weather/consistsOfWO -->

    <owl:ObjectProperty rdf:about="https://w3id.org/leo/onto/weather/consistsOfWO">
        <rdfs:subPropertyOf rdf:resource="https://w3id.org/italia/onto/IoT/consistsOf"/>
        <rdfs:domain rdf:resource="https://w3id.org/leo/onto/weather/WeatherObservationCollection"/>
        <rdfs:range rdf:resource="https://w3id.org/leo/onto/weather/WeatherObservation"/>
        <rdfs:comment xml:lang="en">Property that links the collection of weather observations to each single observations.</rdfs:comment>
        <rdfs:comment xml:lang="it">Proprietà che collega la collezione di osservazioni meteorologiche a ogni singola osservazione.</rdfs:comment>
        <rdfs:isDefinedBy rdf:resource="https://w3id.org/leo/onto/weather"/>
        <rdfs:label xml:lang="it">consiste di osservazioni meteo</rdfs:label>
        <rdfs:label xml:lang="en">consists of weather observation</rdfs:label>
        <owl:versionInfo xml:lang="it">stabile</owl:versionInfo>
        <owl:versionInfo xml:lang="en">stable</owl:versionInfo>
    </owl:ObjectProperty>



    <!-- https://w3id.org/leo/onto/weather/isInstallationOf -->

    <owl:ObjectProperty rdf:about="https://w3id.org/leo/onto/weather/isInstallationOf">
        <rdfs:domain rdf:resource="https://w3id.org/leo/onto/weather/WeatherStationInstallation"/>
        <rdfs:range rdf:resource="https://w3id.org/leo/onto/weather/WeatherStation"/>
        <rdfs:comment xml:lang="en">Property that allows one to link the situation concerning the installation of a weather station (within a farm zone) to the weather station itself.</rdfs:comment>
        <rdfs:comment xml:lang="it">Proprietà che consente di collegare la situazione relativa all&apos;installazione di una centralina meteo (all&apos;interno di una zona dell&apos;allevamento) alla centralina stessa.</rdfs:comment>
        <rdfs:isDefinedBy rdf:resource="https://w3id.org/leo/onto/weather"/>
        <rdfs:label xml:lang="en">is installation of</rdfs:label>
        <rdfs:label xml:lang="it">è installazione di</rdfs:label>
        <owl:versionInfo xml:lang="it">stabile</owl:versionInfo>
        <owl:versionInfo xml:lang="en">stable</owl:versionInfo>
    </owl:ObjectProperty>



    <!-- https://w3id.org/leo/onto/weather/isInstalledInArea -->

    <owl:ObjectProperty rdf:about="https://w3id.org/leo/onto/weather/isInstalledInArea">
        <rdfs:domain rdf:resource="https://w3id.org/leo/onto/weather/WeatherStationInstallation"/>
        <rdfs:range rdf:resource="https://w3id.org/leo/onto/livestockfarm-building-description/BuildingStructure"/>
        <rdfs:comment xml:lang="en">Property allowing one to link the situation regarding the installation of a weather station (typically within a farm) to the area of the farm where the weather station is installed. The area could be: heifer house, feeding area, etc.</rdfs:comment>
        <rdfs:comment xml:lang="it">Proprietà che consente di collegare la situazione relativa all&apos;installazione di una centralina meteo (tipicamente all&apos;interno di un allevamento) con l&apos;area dell&apos;allevamento dove si installa. L&apos;area potrebbe essere: vitellaia, zona di alimentazione, ecc.</rdfs:comment>
        <rdfs:isDefinedBy rdf:resource="https://w3id.org/leo/onto/weather"/>
        <rdfs:label xml:lang="en">is installed in area</rdfs:label>
        <rdfs:label xml:lang="it">è installata in area</rdfs:label>
        <owl:versionInfo xml:lang="it">stabile</owl:versionInfo>
        <owl:versionInfo xml:lang="en">stable</owl:versionInfo>
    </owl:ObjectProperty>



    <!-- https://w3id.org/leo/onto/weather/managedBy -->

    <owl:ObjectProperty rdf:about="https://w3id.org/leo/onto/weather/managedBy">
        <owl:inverseOf rdf:resource="https://w3id.org/leo/onto/weather/managesWeatherStation"/>
        <rdfs:domain rdf:resource="https://w3id.org/leo/onto/weather/WeatherStation"/>
        <rdfs:range rdf:resource="https://w3id.org/italia/onto/COV/Organization"/>
        <rdfs:comment xml:lang="en">Property that links the weather station to the organization it manages it</rdfs:comment>
        <rdfs:comment xml:lang="it">Proprietà che collega la stazione meteo all&apos;organizzazione che la gestisce.</rdfs:comment>
        <rdfs:isDefinedBy rdf:resource="https://w3id.org/leo/onto/weather"/>
        <rdfs:label xml:lang="it">gestita da</rdfs:label>
        <rdfs:label xml:lang="en">managed by</rdfs:label>
        <owl:versionInfo xml:lang="it">stabile</owl:versionInfo>
        <owl:versionInfo xml:lang="en">stable</owl:versionInfo>
    </owl:ObjectProperty>



    <!-- https://w3id.org/leo/onto/weather/managesWeatherStation -->

    <owl:ObjectProperty rdf:about="https://w3id.org/leo/onto/weather/managesWeatherStation">
        <rdfs:domain rdf:resource="https://w3id.org/italia/onto/COV/Organization"/>
        <rdfs:range rdf:resource="https://w3id.org/leo/onto/weather/WeatherStation"/>
        <rdfs:comment xml:lang="en">Inverse property of &quot;managed by&quot; that links an organization to the weather station it manages.</rdfs:comment>
        <rdfs:comment xml:lang="it">Proprietà inversa di &quot;gestita da&quot; che collega l&apos;organizzazione alla stazione meteo che essa gestisce.</rdfs:comment>
        <rdfs:isDefinedBy rdf:resource="https://w3id.org/leo/onto/weather"/>
        <rdfs:label xml:lang="it">gestisce stazione meteo</rdfs:label>
        <rdfs:label xml:lang="en">manages weather station</rdfs:label>
        <owl:versionInfo xml:lang="it">stabile</owl:versionInfo>
        <owl:versionInfo xml:lang="en">stable</owl:versionInfo>
    </owl:ObjectProperty>



    <!--
    ///////////////////////////////////////////////////////////////////////////////////////
    //
    // Data properties
    //
    ///////////////////////////////////////////////////////////////////////////////////////
     -->




    <!-- https://w3id.org/leo/onto/livestockfarm-building-description/buildingCode -->

    <owl:DatatypeProperty rdf:about="https://w3id.org/leo/onto/livestockfarm-building-description/buildingCode"/>



    <!-- https://w3id.org/leo/onto/weather/IMEICode -->

    <owl:DatatypeProperty rdf:about="https://w3id.org/leo/onto/weather/IMEICode">
        <rdfs:subPropertyOf rdf:resource="https://w3id.org/italia/onto/l0/identifier"/>
        <rdfs:domain rdf:resource="https://w3id.org/leo/onto/weather/WeatherStation"/>
        <rdfs:range rdf:resource="http://www.w3.org/2000/01/rdf-schema#Literal"/>
        <rdfs:comment xml:lang="en">Identification number of installed weather station</rdfs:comment>
        <rdfs:comment xml:lang="it">Numero identificativo della centralina meteo installata</rdfs:comment>
        <rdfs:isDefinedBy rdf:resource="https://w3id.org/leo/onto/weather"/>
        <rdfs:label xml:lang="en">IMEI (International Mobile Equipment Identity) code</rdfs:label>
        <rdfs:label xml:lang="it">codice IMEI</rdfs:label>
        <owl:versionInfo xml:lang="it">stabile</owl:versionInfo>
        <owl:versionInfo xml:lang="en">stable</owl:versionInfo>
    </owl:DatatypeProperty>



    <!-- https://w3id.org/leo/onto/weather/isValid -->

    <owl:DatatypeProperty rdf:about="https://w3id.org/leo/onto/weather/isValid">
        <rdf:type rdf:resource="http://www.w3.org/2002/07/owl#FunctionalProperty"/>
        <rdfs:domain rdf:resource="https://w3id.org/leo/onto/weather/WeatherObservationCollection"/>
        <rdfs:range rdf:resource="http://www.w3.org/2001/XMLSchema#boolean"/>
        <rdfs:comment xml:lang="en">Property used to specify whether the collection of weather observations that have been done are valid. It is a boolean, true (yes) or false (no).</rdfs:comment>
        <rdfs:comment xml:lang="it">Proprietà utilizzata per specificare se la collezione di rilevazioni meteo che è stata fatta è valida o meno. È un booleano: vero (sì), falso (no).</rdfs:comment>
        <rdfs:isDefinedBy rdf:resource="https://w3id.org/leo/onto/weather"/>
        <rdfs:label xml:lang="en">is valid</rdfs:label>
        <rdfs:label xml:lang="it">rilevazione valida</rdfs:label>
        <owl:versionInfo xml:lang="it">stabile</owl:versionInfo>
        <owl:versionInfo xml:lang="en">stable</owl:versionInfo>
    </owl:DatatypeProperty>



    <!-- https://w3id.org/leo/onto/weather/weatherStationInstallationDate -->

    <owl:DatatypeProperty rdf:about="https://w3id.org/leo/onto/weather/weatherStationInstallationDate">
        <rdfs:subPropertyOf rdf:resource="https://w3id.org/italia/onto/TI/date"/>
        <rdfs:domain rdf:resource="https://w3id.org/leo/onto/weather/WeatherStationInstallation"/>
        <rdfs:range>
            <rdfs:Datatype>
                <owl:unionOf rdf:parseType="Collection">
                    <rdf:Description rdf:about="http://www.w3.org/2001/XMLSchema#date"/>
                    <rdf:Description rdf:about="http://www.w3.org/2001/XMLSchema#dateTime"/>
                </owl:unionOf>
            </rdfs:Datatype>
        </rdfs:range>
        <rdfs:comment xml:lang="it">La proprietà indica la data e l&apos;ora di installazone della centralina meteo (in un allevamento).</rdfs:comment>
        <rdfs:comment xml:lang="en">The property indicates the date and time of installation of the weather station (within a farm).</rdfs:comment>
        <rdfs:isDefinedBy rdf:resource="https://w3id.org/leo/onto/weather"/>
        <rdfs:label xml:lang="it">data e ora installazione centralina meteo</rdfs:label>
        <rdfs:label xml:lang="en">weather station installation date</rdfs:label>
        <owl:versionInfo xml:lang="it">stabile</owl:versionInfo>
        <owl:versionInfo xml:lang="en">stable</owl:versionInfo>
    </owl:DatatypeProperty>



    <!-- https://w3id.org/leo/onto/weather/wocGenerationTime -->

    <owl:DatatypeProperty rdf:about="https://w3id.org/leo/onto/weather/wocGenerationTime">
        <rdfs:subPropertyOf rdf:resource="https://w3id.org/italia/onto/TI/date"/>
        <rdfs:domain rdf:resource="https://w3id.org/leo/onto/weather/WeatherObservationCollection"/>
        <rdfs:range>
            <rdfs:Datatype>
                <owl:unionOf rdf:parseType="Collection">
                    <rdf:Description rdf:about="http://www.w3.org/2001/XMLSchema#date"/>
                    <rdf:Description rdf:about="http://www.w3.org/2001/XMLSchema#dateTime"/>
                </owl:unionOf>
            </rdfs:Datatype>
        </rdfs:range>
        <rdfs:comment xml:lang="it">La proprietà consente di specificare la data e l&apos;ora di rilevamento delle osservazioni meteo che possono essere fatte nella zona di installazione della centralina (nell&apos;allevamento).</rdfs:comment>
        <rdfs:comment xml:lang="en">This property allows one to specify the date and time of a collection of weather observations that can be made in the area where the weather station is installed (within the farm).</rdfs:comment>
        <rdfs:isDefinedBy rdf:resource="https://w3id.org/leo/onto/weather"/>
        <rdfs:label xml:lang="it">tempo di generazione collezione osservazioni meteo</rdfs:label>
        <rdfs:label xml:lang="en">weather observation collection generation time</rdfs:label>
        <owl:versionInfo xml:lang="it">stabile</owl:versionInfo>
        <owl:versionInfo xml:lang="en">stable</owl:versionInfo>
    </owl:DatatypeProperty>



    <!-- https://w3id.org/leo/onto/weather/wocTransmissionTime -->

    <owl:DatatypeProperty rdf:about="https://w3id.org/leo/onto/weather/wocTransmissionTime">
        <rdfs:subPropertyOf rdf:resource="https://w3id.org/italia/onto/TI/date"/>
        <rdfs:domain rdf:resource="https://w3id.org/leo/onto/weather/WeatherObservationCollection"/>
        <rdfs:range>
            <rdfs:Datatype>
                <owl:unionOf rdf:parseType="Collection">
                    <rdf:Description rdf:about="http://www.w3.org/2001/XMLSchema#date"/>
                    <rdf:Description rdf:about="http://www.w3.org/2001/XMLSchema#dateTime"/>
                </owl:unionOf>
            </rdfs:Datatype>
        </rdfs:range>
        <rdfs:comment xml:lang="it">La proprietà consente di specificare la data e l&apos;ora in cui una serie di osservazioni meteo rilevati dalle centraline (presenti in allevamento) sono trasmessi.</rdfs:comment>
        <rdfs:comment xml:lang="en">The property allows one to specify the date and time when a series of weather observations from the weather stations (present within the farm) are transmitted.</rdfs:comment>
        <rdfs:isDefinedBy rdf:resource="https://w3id.org/leo/onto/weather"/>
        <rdfs:label xml:lang="it">tempo di trasmissione della collezione osservazioni meteo</rdfs:label>
        <rdfs:label xml:lang="en">weather observation collection transmission time</rdfs:label>
        <owl:versionInfo xml:lang="it">stabile</owl:versionInfo>
        <owl:versionInfo xml:lang="en">stable</owl:versionInfo>
    </owl:DatatypeProperty>



    <!--
    ///////////////////////////////////////////////////////////////////////////////////////
    //
    // Classes
    //
    ///////////////////////////////////////////////////////////////////////////////////////
     -->




    <!-- https://w3id.org/leo/onto/livestockfarm-building-description/BuildingStructure -->

    <owl:Class rdf:about="https://w3id.org/leo/onto/livestockfarm-building-description/BuildingStructure"/>



    <!-- https://w3id.org/leo/onto/weather/BioClimaticIndex -->

    <owl:Class rdf:about="https://w3id.org/leo/onto/weather/BioClimaticIndex">
        <rdfs:subClassOf rdf:resource="https://w3id.org/italia/onto/IoT/ObservationParameter"/>
        <owl:disjointWith rdf:resource="https://w3id.org/leo/onto/weather/WeatherObservableProperty"/>
        <rdfs:comment xml:lang="it">La classe degli indici bioclimatici. Le istanze di questa classe possono essere l&apos;indice temperatura umidità (THI), l&apos;indice temperatura umidità (THI) load, ecc.</rdfs:comment>
        <rdfs:comment xml:lang="en">The class of the bioclimatic indexes. Instances of this class can be the Temperature Humidity Index (THI), the Temperature Humidity Index (THI) load, etc.</rdfs:comment>
        <rdfs:isDefinedBy rdf:resource="https://w3id.org/leo/onto/weather"/>
        <rdfs:label xml:lang="en">Bioclimatic Index</rdfs:label>
        <rdfs:label xml:lang="it">Indice Bioclimatico</rdfs:label>
        <owl:versionInfo xml:lang="it">stabile</owl:versionInfo>
        <owl:versionInfo xml:lang="en">stable</owl:versionInfo>
    </owl:Class>



    <!-- https://w3id.org/leo/onto/weather/WeatherFeatureOfInterest -->

    <owl:Class rdf:about="https://w3id.org/leo/onto/weather/WeatherFeatureOfInterest">
        <rdfs:subClassOf rdf:resource="https://w3id.org/italia/onto/IoT/FeatureOfInterest"/>
        <rdfs:comment xml:lang="en">It represents the feature of interest in weather whose attribute is observed by a sensor to obtain a value. Examples of features of interest in weather are: air, rainfall, wind, etc.</rdfs:comment>
        <rdfs:comment xml:lang="it">Rappresenta la caratteristica di interesse meteo il cui attributo osservato è osservato da un sensore per ottenere un valore. Esempi di caratteristiche di interesse nell&apos;ambito meteo sono: l&apos;aria, la pioggia, il vento, ecc.</rdfs:comment>
        <rdfs:isDefinedBy rdf:resource="https://w3id.org/leo/onto/weather"/>
        <rdfs:label xml:lang="it">Caratteristica di interesse meteo</rdfs:label>
        <rdfs:label xml:lang="en">Weather Feature of Interest</rdfs:label>
        <owl:versionInfo xml:lang="it">stabile</owl:versionInfo>
        <owl:versionInfo xml:lang="en">stable</owl:versionInfo>
    </owl:Class>



    <!-- https://w3id.org/leo/onto/weather/WeatherObservableProperty -->

    <owl:Class rdf:about="https://w3id.org/leo/onto/weather/WeatherObservableProperty">
        <rdfs:subClassOf rdf:resource="https://w3id.org/italia/onto/IoT/ObservationParameter"/>
        <rdfs:comment xml:lang="it">La classe di tutte le proprietà di un&apos;osservazione che possono essere osservate nel contesto meteorologico.  Esempi includono: temperatura, umidità, pressione, precipitazione, ecc.</rdfs:comment>
        <rdfs:comment xml:lang="en">The class of all the properties of an observation that can be observed in the weather context. Examples include: temperature, humidity, pressure, precipitation, etc.</rdfs:comment>
        <rdfs:isDefinedBy rdf:resource="https://w3id.org/leo/onto/weather"/>
        <rdfs:label xml:lang="it">Proprietà Meteo Osservabile</rdfs:label>
        <rdfs:label xml:lang="en">Weather Observable Property</rdfs:label>
        <owl:versionInfo xml:lang="it">stabile</owl:versionInfo>
        <owl:versionInfo xml:lang="en">stable</owl:versionInfo>
    </owl:Class>



    <!-- https://w3id.org/leo/onto/weather/WeatherObservation -->

    <owl:Class rdf:about="https://w3id.org/leo/onto/weather/WeatherObservation">
        <rdfs:subClassOf rdf:resource="https://w3id.org/italia/onto/IoT/Observation"/>
        <rdfs:comment xml:lang="it">Questa classe rappresenta un&apos;osservazione di tipo meteo.</rdfs:comment>
        <rdfs:comment xml:lang="en">This class represents a specific observation of Meteo type</rdfs:comment>
        <rdfs:label rdf:resource="https://w3id.org/leo/onto/weather"/>
        <rdfs:label xml:lang="it">Osservazione Meteo</rdfs:label>
        <rdfs:label xml:lang="en">Weather Observation</rdfs:label>
        <owl:versionInfo xml:lang="it">stabile</owl:versionInfo>
        <owl:versionInfo xml:lang="en">stable</owl:versionInfo>
    </owl:Class>



    <!-- https://w3id.org/leo/onto/weather/WeatherObservationCollection -->

    <owl:Class rdf:about="https://w3id.org/leo/onto/weather/WeatherObservationCollection">
        <rdfs:subClassOf rdf:resource="https://w3id.org/italia/onto/IoT/ObservationCollection"/>
        <rdfs:subClassOf>
            <owl:Restriction>
                <owl:onProperty rdf:resource="https://w3id.org/leo/onto/weather/consistsOfWO"/>
                <owl:someValuesFrom rdf:resource="https://w3id.org/leo/onto/weather/WeatherObservation"/>
            </owl:Restriction>
        </rdfs:subClassOf>
        <rdfs:subClassOf>
            <owl:Restriction>
                <owl:onProperty rdf:resource="https://w3id.org/leo/onto/weather/consistsOfWO"/>
                <owl:allValuesFrom rdf:resource="https://w3id.org/leo/onto/weather/WeatherObservation"/>
            </owl:Restriction>
        </rdfs:subClassOf>
        <rdfs:subClassOf>
            <owl:Restriction>
                <owl:onProperty rdf:resource="https://w3id.org/leo/onto/weather/wocGenerationTime"/>
                <owl:qualifiedCardinality rdf:datatype="http://www.w3.org/2001/XMLSchema#nonNegativeInteger">1</owl:qualifiedCardinality>
                <owl:onDataRange>
                    <rdfs:Datatype>
                        <owl:unionOf rdf:parseType="Collection">
                            <rdf:Description rdf:about="http://www.w3.org/2001/XMLSchema#date"/>
                            <rdf:Description rdf:about="http://www.w3.org/2001/XMLSchema#dateTime"/>
                        </owl:unionOf>
                    </rdfs:Datatype>
                </owl:onDataRange>
            </owl:Restriction>
        </rdfs:subClassOf>
        <rdfs:subClassOf>
            <owl:Restriction>
                <owl:onProperty rdf:resource="https://w3id.org/leo/onto/weather/isValid"/>
                <owl:maxQualifiedCardinality rdf:datatype="http://www.w3.org/2001/XMLSchema#nonNegativeInteger">1</owl:maxQualifiedCardinality>
                <owl:onDataRange rdf:resource="http://www.w3.org/2001/XMLSchema#boolean"/>
            </owl:Restriction>
        </rdfs:subClassOf>
        <rdfs:subClassOf>
            <owl:Restriction>
                <owl:onProperty rdf:resource="https://w3id.org/leo/onto/weather/wocTransmissionTime"/>
                <owl:maxQualifiedCardinality rdf:datatype="http://www.w3.org/2001/XMLSchema#nonNegativeInteger">1</owl:maxQualifiedCardinality>
                <owl:onDataRange>
                    <rdfs:Datatype>
                        <owl:unionOf rdf:parseType="Collection">
                            <rdf:Description rdf:about="http://www.w3.org/2001/XMLSchema#date"/>
                            <rdf:Description rdf:about="http://www.w3.org/2001/XMLSchema#dateTime"/>
                        </owl:unionOf>
                    </rdfs:Datatype>
                </owl:onDataRange>
            </owl:Restriction>
        </rdfs:subClassOf>
        <rdfs:comment xml:lang="it">La classe rappresenta una collezione di singole osservazioni meteo rilevate dalle centraline meteo (tipicamente installate all&apos;interno dell&apos;insediamento dell&apos;azienda di allevamento).</rdfs:comment>
        <rdfs:comment xml:lang="en">This class that represents a set of weather observation that come from a weather station (usually installed within livestock farm sites).</rdfs:comment>
        <rdfs:isDefinedBy rdf:resource="https://w3id.org/leo/onto/weather"/>
        <rdfs:label xml:lang="it">Collezione di Osservazioni Meteo</rdfs:label>
        <rdfs:label xml:lang="en">Weather Observation Collection</rdfs:label>
        <owl:versionInfo xml:lang="it">stabile</owl:versionInfo>
        <owl:versionInfo xml:lang="en">stable</owl:versionInfo>
    </owl:Class>



    <!-- https://w3id.org/leo/onto/weather/WeatherStation -->

    <owl:Class rdf:about="https://w3id.org/leo/onto/weather/WeatherStation">
        <rdfs:subClassOf rdf:resource="https://w3id.org/italia/onto/IoT/Platform"/>
        <rdfs:subClassOf>
            <owl:Restriction>
                <owl:onProperty rdf:resource="https://w3id.org/italia/onto/CLV/hasSpatialCoverage"/>
                <owl:someValuesFrom rdf:resource="https://w3id.org/italia/onto/CLV/Feature"/>
            </owl:Restriction>
        </rdfs:subClassOf>
        <rdfs:subClassOf>
            <owl:Restriction>
                <owl:onProperty rdf:resource="https://w3id.org/italia/onto/CLV/hasGeometry"/>
                <owl:qualifiedCardinality rdf:datatype="http://www.w3.org/2001/XMLSchema#nonNegativeInteger">1</owl:qualifiedCardinality>
                <owl:onClass rdf:resource="https://w3id.org/italia/onto/CLV/Geometry"/>
            </owl:Restriction>
        </rdfs:subClassOf>
        <rdfs:subClassOf>
            <owl:Restriction>
                <owl:onProperty rdf:resource="https://w3id.org/leo/onto/weather/managedBy"/>
                <owl:maxQualifiedCardinality rdf:datatype="http://www.w3.org/2001/XMLSchema#nonNegativeInteger">1</owl:maxQualifiedCardinality>
                <owl:onClass rdf:resource="https://w3id.org/italia/onto/COV/Organization"/>
            </owl:Restriction>
        </rdfs:subClassOf>
        <rdfs:subClassOf>
            <owl:Restriction>
                <owl:onProperty rdf:resource="https://w3id.org/italia/onto/l0/name"/>
                <owl:someValuesFrom rdf:resource="http://www.w3.org/2000/01/rdf-schema#Literal"/>
            </owl:Restriction>
        </rdfs:subClassOf>
        <rdfs:subClassOf>
            <owl:Restriction>
                <owl:onProperty rdf:resource="https://w3id.org/italia/onto/l0/identifier"/>
                <owl:cardinality rdf:datatype="http://www.w3.org/2001/XMLSchema#nonNegativeInteger">1</owl:cardinality>
            </owl:Restriction>
        </rdfs:subClassOf>
        <rdfs:subClassOf>
            <owl:Restriction>
                <owl:onProperty rdf:resource="https://w3id.org/leo/onto/weather/IMEICode"/>
                <owl:maxCardinality rdf:datatype="http://www.w3.org/2001/XMLSchema#nonNegativeInteger">1</owl:maxCardinality>
            </owl:Restriction>
        </rdfs:subClassOf>
        <rdfs:comment xml:lang="it">Questa classe rappresenta la stazione meteo. La stazione è identificata univocamente da un identificativo, è gestita da un&apos;organizzazione ed ha una geometria (tipicamente un punto) associata.</rdfs:comment>
        <rdfs:comment xml:lang="en">This class represents the weather station. The station is uniquely identified by an identifier, is managed by an organization and has a geometry (usually a point) associated with it.</rdfs:comment>
        <rdfs:isDefinedBy rdf:resource="https://w3id.org/leo/onto/weather"/>
        <rdfs:label xml:lang="it">Stazione Meteo</rdfs:label>
        <rdfs:label xml:lang="en">Weather Station</rdfs:label>
        <owl:versionInfo xml:lang="it">stabile</owl:versionInfo>
        <owl:versionInfo xml:lang="en">stable</owl:versionInfo>
    </owl:Class>



    <!-- https://w3id.org/leo/onto/weather/WeatherStationInstallation -->

    <owl:Class rdf:about="https://w3id.org/leo/onto/weather/WeatherStationInstallation">
        <rdfs:subClassOf rdf:resource="https://w3id.org/italia/onto/l0/EventOrSituation"/>
        <rdfs:subClassOf>
            <owl:Restriction>
                <owl:onProperty rdf:resource="https://w3id.org/leo/onto/weather/isInstallationOf"/>
                <owl:qualifiedCardinality rdf:datatype="http://www.w3.org/2001/XMLSchema#nonNegativeInteger">1</owl:qualifiedCardinality>
                <owl:onClass rdf:resource="https://w3id.org/leo/onto/weather/WeatherStation"/>
            </owl:Restriction>
        </rdfs:subClassOf>
        <rdfs:subClassOf>
            <owl:Restriction>
                <owl:onProperty rdf:resource="https://w3id.org/leo/onto/weather/isInstalledInArea"/>
                <owl:maxQualifiedCardinality rdf:datatype="http://www.w3.org/2001/XMLSchema#nonNegativeInteger">1</owl:maxQualifiedCardinality>
                <owl:onClass rdf:resource="https://w3id.org/leo/onto/livestockfarm-building-description/BuildingStructure"/>
            </owl:Restriction>
        </rdfs:subClassOf>
        <rdfs:subClassOf>
            <owl:Restriction>
                <owl:onProperty rdf:resource="https://w3id.org/leo/onto/weather/weatherStationInstallationDate"/>
                <owl:qualifiedCardinality rdf:datatype="http://www.w3.org/2001/XMLSchema#nonNegativeInteger">1</owl:qualifiedCardinality>
                <owl:onDataRange>
                    <rdfs:Datatype>
                        <owl:unionOf rdf:parseType="Collection">
                            <rdf:Description rdf:about="http://www.w3.org/2001/XMLSchema#date"/>
                            <rdf:Description rdf:about="http://www.w3.org/2001/XMLSchema#dateTime"/>
                        </owl:unionOf>
                    </rdfs:Datatype>
                </owl:onDataRange>
            </owl:Restriction>
        </rdfs:subClassOf>
        <rdfs:subClassOf>
            <owl:Restriction>
                <owl:onProperty rdf:resource="https://w3id.org/leo/onto/livestockfarm-building-description/buildingCode"/>
                <owl:maxCardinality rdf:datatype="http://www.w3.org/2001/XMLSchema#nonNegativeInteger">1</owl:maxCardinality>
            </owl:Restriction>
        </rdfs:subClassOf>
        <rdfs:comment xml:lang="it">La classe che rappresenta la situazione relativa all&apos;installazione di una centralina meteo (tipicamente all&apos;interno di zone specifiche di un allevamento).</rdfs:comment>
        <rdfs:comment xml:lang="en">The class representing the situation regarding the installation of a weather station (typically within specific areas of a livestock company site).</rdfs:comment>
        <rdfs:isDefinedBy rdf:resource="https://w3id.org/leo/onto/weather"/>
        <rdfs:label xml:lang="it">Installazione Centralina Meteo</rdfs:label>
        <rdfs:label xml:lang="en">Weather Station Installation</rdfs:label>
        <owl:versionInfo xml:lang="it">stabile</owl:versionInfo>
        <owl:versionInfo xml:lang="en">stable</owl:versionInfo>
    </owl:Class>



    <!--
    ///////////////////////////////////////////////////////////////////////////////////////
    //
    // Individuals
    //
    ///////////////////////////////////////////////////////////////////////////////////////
     -->




    <!-- https://w3id.org/leo/data/contact-point/onto-aia -->

    <owl:NamedIndividual rdf:about="https://w3id.org/leo/data/contact-point/onto-aia">
        <rdf:type rdf:resource="http://dati.gov.it/onto/dcatapit#Organization"/>
        <rdf:type rdf:resource="http://www.w3.org/2006/vcard/ns#Kind"/>
        <rdf:type rdf:resource="http://www.w3.org/2006/vcard/ns#Organization"/>
        <rdfs:label xml:lang="it">Sistemi informativi</rdfs:label>
        <ns:fn xml:lang="it">Sistemi informativi</ns:fn>
        <ns:hasEmail rdf:resource="mailto:affarigenerali@pec.aia.it"/>
    </owl:NamedIndividual>



    <!-- https://w3id.org/leo/data/distribution/WT-JSON-LD -->

    <owl:NamedIndividual rdf:about="https://w3id.org/leo/data/distribution/WT-JSON-LD">
        <rdf:type rdf:resource="https://w3id.org/italia/onto/ADMS/SemanticAssetDistribution"/>
        <terms:description xml:lang="it">Questa è la distribuzione JSON-LD dell&apos;ontologia sul meteo</terms:description>
        <terms:description xml:lang="en">This is the distribution in JSON-LD of weather ontology</terms:description>
        <terms:format rdf:resource="http://publications.europa.eu/resource/authority/file-type/JSON_LD"/>
        <terms:label xml:lang="it">Distribuzione JSON-LD ontologia Weather</terms:label>
        <terms:label xml:lang="en">JSON-LD distribution of Weather Ontology</terms:label>
        <terms:license rdf:resource="https://w3id.org/italia/controlled-vocabulary/licences/A21_CCBY40"/>
        <terms:title xml:lang="it">Distribuzione JSON-LD ontologia Weather</terms:title>
        <terms:title xml:lang="en">JSON-LD distribution of Weather Ontology</terms:title>
        <rdfs:comment xml:lang="it">Questa è la distribuzione JSON-LD dell&apos;ontologia sul meteo</rdfs:comment>
        <rdfs:comment xml:lang="en">This is the distribution in JSON-LD of weather ontology</rdfs:comment>
        <dcat:accessURL rdf:resource="https://www.leo-project.it/Ontologie/weather/latest"/>
        <dcat:downloadURL rdf:resource="https://www.leo-project.it/Ontologie/weathr/latest/weather.jsonld"/>
    </owl:NamedIndividual>



    <!-- https://w3id.org/leo/data/distribution/WT-RDF-TURTLE -->

    <owl:NamedIndividual rdf:about="https://w3id.org/leo/data/distribution/WT-RDF-TURTLE">
        <rdf:type rdf:resource="https://w3id.org/italia/onto/ADMS/SemanticAssetDistribution"/>
        <terms:description xml:lang="it">Questa è la distribuzione RDF/Turtle dell&apos;ontologia sul meteo</terms:description>
        <terms:description xml:lang="en">This is the distribution in RDF/Turtle of Weather ontology</terms:description>
        <terms:format rdf:resource="http://publications.europa.eu/resource/authority/file-type/RDF_TURTLE"/>
        <terms:license rdf:resource="https://w3id.org/italia/controlled-vocabulary/licences/A21_CCBY40"/>
        <terms:title xml:lang="it">Distribuzione RDF/Turtle ontologia Weather</terms:title>
        <terms:title xml:lang="en">RDF/Turtle distribution of Weather Ontology</terms:title>
        <rdfs:comment xml:lang="it">Questa è la distribuzione RDF/Turtle dell&apos;ontologia sul meteo</rdfs:comment>
        <rdfs:comment xml:lang="en">This is the distribution in RDF/Turtle of Weather ontology</rdfs:comment>
        <rdfs:label xml:lang="it">Distribuzione RDF/Turtle ontologia Weather</rdfs:label>
        <rdfs:label xml:lang="en">RDF/Turtle distribution of Weather Ontology</rdfs:label>
        <dcat:accessURL rdf:resource="https://www.leo-project.it/Ontologie/weather/latest"/>
        <dcat:downloadURL rdf:resource="https://www.leo-project.it/Ontologie/weather/latest/weather.ttl"/>
    </owl:NamedIndividual>



    <!-- https://w3id.org/leo/data/distribution/WT-RDF-XML -->

    <owl:NamedIndividual rdf:about="https://w3id.org/leo/data/distribution/WT-RDF-XML">
        <rdf:type rdf:resource="https://w3id.org/italia/onto/ADMS/SemanticAssetDistribution"/>
        <terms:description xml:lang="it">Questa è la distribuzione RDF/XML dell&apos;ontologia sul meteo</terms:description>
        <terms:description xml:lang="en">This is the distribution in RDF/XML of Weather ontology</terms:description>
        <terms:format rdf:resource="http://publications.europa.eu/resource/authority/file-type/RDF_XML"/>
        <terms:license rdf:resource="https://w3id.org/italia/controlled-vocabulary/licences/A21_CCBY40"/>
        <terms:title xml:lang="it">Distribuzione RDF/XML ontologia Weather</terms:title>
        <terms:title xml:lang="en">RDF/XML distribution of Weather Ontology</terms:title>
        <rdfs:comment xml:lang="it">Questa è la distribuzione RDF/XML dell&apos;ontologia sul meteo</rdfs:comment>
        <rdfs:comment xml:lang="en">This is the distribution in RDF/XML of Weather ontology</rdfs:comment>
        <rdfs:label xml:lang="it">Distribuzione RDF/XML ontologia Weather</rdfs:label>
        <rdfs:label xml:lang="en">RDF/XML distribution of Weather Ontology</rdfs:label>
        <dcat:accessURL rdf:resource="https://www.leo-project.it/Ontologie/weather/latest"/>
        <dcat:downloadURL rdf:resource="https://www.leo-project.it/Ontologie/weather/latest/weather.rdf"/>
    </owl:NamedIndividual>



    <!-- https://w3id.org/leo/data/private-organization/00944701002 -->

    <owl:NamedIndividual rdf:about="https://w3id.org/leo/data/private-organization/00944701002">
        <rdf:type rdf:resource="http://dati.gov.it/onto/dcatapit#Agent"/>
        <rdf:type rdf:resource="http://xmlns.com/foaf/0.1/Agent"/>
        <terms:identifier>00944701002</terms:identifier>
        <foaf:name xml:lang="it">Associazione Italiana Allevatori</foaf:name>
        <foaf:name xml:lang="en">Italian Breeders&apos; Association</foaf:name>
    </owl:NamedIndividual>



    <!-- https://w3id.org/leo/data/private-organization/06695411006 -->

    <owl:NamedIndividual rdf:about="https://w3id.org/leo/data/private-organization/06695411006">
        <rdf:type rdf:resource="http://dati.gov.it/onto/dcatapit#Agent"/>
        <rdf:type rdf:resource="http://xmlns.com/foaf/0.1/Agent"/>
        <terms:identifier>06695411006</terms:identifier>
        <foaf:name xml:lang="en">Bluarancio</foaf:name>
        <foaf:name xml:lang="it">Bluarancio</foaf:name>
    </owl:NamedIndividual>



    <!-- https://w3id.org/leo/data/project/LEO -->

    <owl:NamedIndividual rdf:about="https://w3id.org/leo/data/project/LEO">
        <rdf:type rdf:resource="https://w3id.org/italia/onto/ADMS/Project"/>
        <rdfs:label xml:lang="it">LEO - Livestok Environment Open Data</rdfs:label>
        <l0:name xml:lang="it">LEO - Livestok Environment Open Data</l0:name>
    </owl:NamedIndividual>



    <!-- https://w3id.org/leo/onto/weather -->

    <owl:NamedIndividual rdf:about="https://w3id.org/leo/onto/weather">
        <rdf:type rdf:resource="https://w3id.org/italia/onto/ADMS/SemanticAsset"/>
    </owl:NamedIndividual>



    <!-- https://w3id.org/leo/onto/weather/Air -->

    <owl:NamedIndividual rdf:about="https://w3id.org/leo/onto/weather/Air">
        <rdf:type rdf:resource="https://w3id.org/leo/onto/weather/WeatherFeatureOfInterest"/>
        <rdfs:isDefinedBy rdf:resource="https://w3id.org/leo/onto/weather"/>
        <rdfs:label xml:lang="en">Air</rdfs:label>
        <rdfs:label xml:lang="it">Aria</rdfs:label>
        <owl:versionInfo xml:lang="it">stabile</owl:versionInfo>
        <owl:versionInfo xml:lang="en">stable</owl:versionInfo>
    </owl:NamedIndividual>



    <!-- https://w3id.org/leo/onto/weather/GroundLevelSoil -->

    <owl:NamedIndividual rdf:about="https://w3id.org/leo/onto/weather/GroundLevelSoil">
        <rdf:type rdf:resource="https://w3id.org/leo/onto/weather/WeatherFeatureOfInterest"/>
        <rdfs:isDefinedBy rdf:resource="https://w3id.org/leo/onto/weather"/>
        <rdfs:label xml:lang="en">Ground Level Soil</rdfs:label>
        <rdfs:label xml:lang="it">Livello del Suolo</rdfs:label>
        <owl:versionInfo xml:lang="it">stabile</owl:versionInfo>
        <owl:versionInfo xml:lang="en">stable</owl:versionInfo>
    </owl:NamedIndividual>



    <!-- https://w3id.org/leo/onto/weather/Rainfall -->

    <owl:NamedIndividual rdf:about="https://w3id.org/leo/onto/weather/Rainfall">
        <rdf:type rdf:resource="https://w3id.org/leo/onto/weather/WeatherFeatureOfInterest"/>
        <rdfs:isDefinedBy rdf:resource="https://w3id.org/leo/onto/weather"/>
        <rdfs:label xml:lang="it">Pioggia</rdfs:label>
        <rdfs:label xml:lang="en">Rainfall</rdfs:label>
        <owl:versionInfo xml:lang="it">stabile</owl:versionInfo>
        <owl:versionInfo xml:lang="en">stable</owl:versionInfo>
    </owl:NamedIndividual>



    <!-- https://w3id.org/leo/onto/weather/Wind -->

    <owl:NamedIndividual rdf:about="https://w3id.org/leo/onto/weather/Wind">
        <rdf:type rdf:resource="https://w3id.org/leo/onto/weather/WeatherFeatureOfInterest"/>
        <rdfs:isDefinedBy rdf:resource="https://w3id.org/leo/onto/weather"/>
        <rdfs:label xml:lang="it">Vento</rdfs:label>
        <rdfs:label xml:lang="en">Wind</rdfs:label>
        <owl:versionInfo xml:lang="it">stabile</owl:versionInfo>
        <owl:versionInfo xml:lang="en">stable</owl:versionInfo>
    </owl:NamedIndividual>
</rdf:RDF>



<!-- Generated by the OWL API (version 4.5.9.2019-02-01T07:24:44Z) https://github.com/owlcs/owlapi -->
