<?xml version="1.0"?>
<rdf:RDF xmlns="https://w3id.org/leo/onto/livestock-assessment/"
     xml:base="https://w3id.org/leo/onto/livestock-assessment/"
     xmlns:ns="http://www.w3.org/2006/vcard/ns#"
     xmlns:owl="http://www.w3.org/2002/07/owl#"
     xmlns:rdf="http://www.w3.org/1999/02/22-rdf-syntax-ns#"
     xmlns:xml="http://www.w3.org/XML/1998/namespace"
     xmlns:xsd="http://www.w3.org/2001/XMLSchema#"
     xmlns:ADMS="https://w3id.org/italia/onto/ADMS/"
     xmlns:dcat="http://www.w3.org/ns/dcat#"
     xmlns:foaf="http://xmlns.com/foaf/0.1/"
     xmlns:prov="http://www.w3.org/ns/prov#"
     xmlns:rdfs="http://www.w3.org/2000/01/rdf-schema#"
     xmlns:terms="http://purl.org/dc/terms/">
    <owl:Ontology rdf:about="https://w3id.org/leo/onto/livestock-assessment">
        <owl:versionIRI rdf:resource="https://w3id.org/leo/onto/livestock-assessment/0.1"/>
        <owl:imports rdf:resource="https://w3id.org/italia/onto/MU"/>
        <owl:imports rdf:resource="https://w3id.org/italia/onto/TI"/>
        <owl:imports rdf:resource="https://w3id.org/italia/onto/l0"/>
        <terms:accrualPeriodicity rdf:resource="http://publications.europa.eu/resource/authority/frequency/IRREG"/>
        <terms:creator rdf:resource="https://w3id.org/leo/data/private-organization/00944701002"/>
        <terms:description rdf:resource="https://www.dropbox.com/s/1a7atu5ic1drplo/livestock-assessment.png??raw=1"/>
        <terms:description xml:lang="it">Questa ontologia implementa un pattern generale per modellare controlli in ambito zootecnico. Questa sarà specializzata in diversi tipi di controlli: gli accertamenti zootecnici, i controlli funzionali sul latte, i controlli sull&apos;efficienza della mungitura.</terms:description>
        <terms:description xml:lang="en">This ontology implements a general pattern for modelling zootechnical controls. It will specialise in different types of controls: livestock checks, functional milk controls, milking efficiency controls.</terms:description>
        <terms:identifier xml:lang="it">onto-BA-11</terms:identifier>
        <terms:issued rdf:datatype="http://www.w3.org/2001/XMLSchema#date">2023-02-15</terms:issued>
        <terms:language rdf:resource="http://publications.europa.eu/resource/authority/language/ENG"/>
        <terms:language rdf:resource="http://publications.europa.eu/resource/authority/language/ITA"/>
        <terms:modified rdf:datatype="http://www.w3.org/2001/XMLSchema#date">2023-02-15</terms:modified>
        <terms:publisher rdf:resource="https://w3id.org/leo/data/private-organization/00944701002"/>
        <terms:rightsHolder rdf:resource="https://w3id.org/leo/data/private-organization/00944701002"/>
        <terms:subject rdf:resource="http://eurovoc.europa.eu/6271"/>
        <terms:subject rdf:resource="http://eurovoc.europa.eu/6272"/>
        <terms:title xml:lang="en">Livestock Assessment Ontology</terms:title>
        <terms:title xml:lang="it">Ontologia degli Accertamenti in ambito Zootecnia</terms:title>
        <rdfs:comment xml:lang="it">Questa ontologia implementa un pattern generale per modellare controlli in ambito zootecnico. Questa sarà specializzata in diversi tipi di controlli: gli accertamenti zootecnici, i controlli funzionali sul latte, i controlli sull&apos;efficienza della mungitura.</rdfs:comment>
        <rdfs:comment xml:lang="en">This ontology implements a general pattern for modelling zootechnical controls. It will specialise in different types of controls: livestock checks, functional milk controls, milking efficiency controls.</rdfs:comment>
        <rdfs:isDefinedBy rdf:resource="https://w3id.org/leo/onto/livestock-assessment"/>
        <rdfs:label xml:lang="en">Livestock Assessment Ontology</rdfs:label>
        <rdfs:label xml:lang="it">Ontologia degli Accertamenti in ambito Zootecnia</rdfs:label>
        <owl:versionInfo xml:lang="en">Version 0.1 - 2023 - First version of the ontology - ontology creation</owl:versionInfo>
        <owl:versionInfo xml:lang="it">Versione 0.1 - 2023 - Prima versione dell&apos;ontologia - creazione dell&apos;ontologia</owl:versionInfo>
        <dcat:contactPoint rdf:resource="https://w3id.org/leo/data/contact-point/onto-aia"/>
        <dcat:keyword xml:lang="it">Accertamenti zootecnici</dcat:keyword>
        <dcat:keyword xml:lang="it">Controlli</dcat:keyword>
        <dcat:keyword xml:lang="it">Controlli zootecnici</dcat:keyword>
        <dcat:theme rdf:resource="http://publications.europa.eu/resource/authority/data-theme/AGRI"/>
        <ADMS:acronym>LA</ADMS:acronym>
        <ADMS:hasContributor rdf:resource="https://w3id.org/leo/data/private-organization/06695411006"/>
        <ADMS:hasFormalityLevel rdf:resource="https://w3id.org/italia/onto/ADMS/Formal"/>
        <ADMS:hasKeyClass rdf:resource="https://w3id.org/leo/onto/livestock-assessment/AssessmentResult"/>
        <ADMS:hasKeyClass rdf:resource="https://w3id.org/leo/onto/livestock-assessment/LivestockAssessment"/>
        <ADMS:hasOntologyLanguage rdf:resource="https://w3id.org/italia/onto/ADMS/OWL"/>
        <ADMS:hasSemanticAssetDistribution rdf:resource="https://w3id.org/leo/data/distribution/LA-JSON-LD"/>
        <ADMS:hasSemanticAssetDistribution rdf:resource="https://w3id.org/leo/data/distribution/LA-RDF-TURTLE"/>
        <ADMS:hasSemanticAssetDistribution rdf:resource="https://w3id.org/leo/data/distribution/LA-RDF-XML"/>
        <ADMS:hasTask rdf:resource="https://w3id.org/italia/onto/ADMS/AnnotationTask"/>
        <ADMS:hasTask rdf:resource="https://w3id.org/italia/onto/ADMS/QueryFormulationTask"/>
        <ADMS:hasTask rdf:resource="https://w3id.org/italia/onto/ADMS/SearchTask"/>
        <ADMS:officialURI rdf:datatype="http://www.w3.org/2001/XMLSchema#anyURI">https://w3id.org/leo/onto/livestock-assessment</ADMS:officialURI>
        <ADMS:prefix>la</ADMS:prefix>
        <ADMS:semanticAssetInUse rdf:resource="https://w3id.org/leo/data/project/LEO"/>
        <ADMS:status>published</ADMS:status>
        <ADMS:target xml:lang="it">Comunità Open Data</ADMS:target>
        <ADMS:target>Imprese</ADMS:target>
        <ADMS:target>Pubbliche Amministrazioni</ADMS:target>
        <ADMS:target xml:lang="it">Specialisti del settore zootecnico</ADMS:target>
        <ADMS:type rdf:resource="https://w3id.org/italia/onto/ADMS/DomainOntology"/>
    </owl:Ontology>
    


    <!-- 
    ///////////////////////////////////////////////////////////////////////////////////////
    //
    // Annotation properties
    //
    ///////////////////////////////////////////////////////////////////////////////////////
     -->

    


    <!-- http://purl.org/dc/terms/accrualPeriodicity -->

    <owl:AnnotationProperty rdf:about="http://purl.org/dc/terms/accrualPeriodicity"/>
    


    <!-- http://purl.org/dc/terms/creator -->

    <owl:AnnotationProperty rdf:about="http://purl.org/dc/terms/creator"/>
    


    <!-- http://purl.org/dc/terms/description -->

    <owl:AnnotationProperty rdf:about="http://purl.org/dc/terms/description"/>
    


    <!-- http://purl.org/dc/terms/format -->

    <owl:AnnotationProperty rdf:about="http://purl.org/dc/terms/format"/>
    


    <!-- http://purl.org/dc/terms/identifier -->

    <owl:AnnotationProperty rdf:about="http://purl.org/dc/terms/identifier"/>
    


    <!-- http://purl.org/dc/terms/issued -->

    <owl:AnnotationProperty rdf:about="http://purl.org/dc/terms/issued"/>
    


    <!-- http://purl.org/dc/terms/language -->

    <owl:AnnotationProperty rdf:about="http://purl.org/dc/terms/language"/>
    


    <!-- http://purl.org/dc/terms/license -->

    <owl:AnnotationProperty rdf:about="http://purl.org/dc/terms/license"/>
    


    <!-- http://purl.org/dc/terms/modified -->

    <owl:AnnotationProperty rdf:about="http://purl.org/dc/terms/modified"/>
    


    <!-- http://purl.org/dc/terms/publisher -->

    <owl:AnnotationProperty rdf:about="http://purl.org/dc/terms/publisher"/>
    


    <!-- http://purl.org/dc/terms/rightsHolder -->

    <owl:AnnotationProperty rdf:about="http://purl.org/dc/terms/rightsHolder"/>
    


    <!-- http://purl.org/dc/terms/subject -->

    <owl:AnnotationProperty rdf:about="http://purl.org/dc/terms/subject"/>
    


    <!-- http://purl.org/dc/terms/title -->

    <owl:AnnotationProperty rdf:about="http://purl.org/dc/terms/title"/>
    


    <!-- http://www.w3.org/ns/dcat#accessURL -->

    <owl:AnnotationProperty rdf:about="http://www.w3.org/ns/dcat#accessURL"/>
    


    <!-- http://www.w3.org/ns/dcat#contactPoint -->

    <owl:AnnotationProperty rdf:about="http://www.w3.org/ns/dcat#contactPoint"/>
    


    <!-- http://www.w3.org/ns/dcat#downloadURL -->

    <owl:AnnotationProperty rdf:about="http://www.w3.org/ns/dcat#downloadURL"/>
    


    <!-- http://www.w3.org/ns/dcat#keyword -->

    <owl:AnnotationProperty rdf:about="http://www.w3.org/ns/dcat#keyword"/>
    


    <!-- http://www.w3.org/ns/dcat#theme -->

    <owl:AnnotationProperty rdf:about="http://www.w3.org/ns/dcat#theme"/>
    


    <!-- https://w3id.org/italia/onto/ADMS/acronym -->

    <owl:AnnotationProperty rdf:about="https://w3id.org/italia/onto/ADMS/acronym"/>
    


    <!-- https://w3id.org/italia/onto/ADMS/hasContributor -->

    <owl:AnnotationProperty rdf:about="https://w3id.org/italia/onto/ADMS/hasContributor"/>
    


    <!-- https://w3id.org/italia/onto/ADMS/hasFormalityLevel -->

    <owl:AnnotationProperty rdf:about="https://w3id.org/italia/onto/ADMS/hasFormalityLevel"/>
    


    <!-- https://w3id.org/italia/onto/ADMS/hasKeyClass -->

    <owl:AnnotationProperty rdf:about="https://w3id.org/italia/onto/ADMS/hasKeyClass"/>
    


    <!-- https://w3id.org/italia/onto/ADMS/hasOntologyLanguage -->

    <owl:AnnotationProperty rdf:about="https://w3id.org/italia/onto/ADMS/hasOntologyLanguage"/>
    


    <!-- https://w3id.org/italia/onto/ADMS/hasSemanticAssetDistribution -->

    <owl:AnnotationProperty rdf:about="https://w3id.org/italia/onto/ADMS/hasSemanticAssetDistribution"/>
    


    <!-- https://w3id.org/italia/onto/ADMS/hasTask -->

    <owl:AnnotationProperty rdf:about="https://w3id.org/italia/onto/ADMS/hasTask"/>
    


    <!-- https://w3id.org/italia/onto/ADMS/officialURI -->

    <owl:AnnotationProperty rdf:about="https://w3id.org/italia/onto/ADMS/officialURI"/>
    


    <!-- https://w3id.org/italia/onto/ADMS/prefix -->

    <owl:AnnotationProperty rdf:about="https://w3id.org/italia/onto/ADMS/prefix"/>
    


    <!-- https://w3id.org/italia/onto/ADMS/semanticAssetInUse -->

    <owl:AnnotationProperty rdf:about="https://w3id.org/italia/onto/ADMS/semanticAssetInUse"/>
    


    <!-- https://w3id.org/italia/onto/ADMS/status -->

    <owl:AnnotationProperty rdf:about="https://w3id.org/italia/onto/ADMS/status"/>
    


    <!-- https://w3id.org/italia/onto/ADMS/target -->

    <owl:AnnotationProperty rdf:about="https://w3id.org/italia/onto/ADMS/target"/>
    


    <!-- https://w3id.org/italia/onto/ADMS/type -->

    <owl:AnnotationProperty rdf:about="https://w3id.org/italia/onto/ADMS/type"/>
    


    <!-- 
    ///////////////////////////////////////////////////////////////////////////////////////
    //
    // Datatypes
    //
    ///////////////////////////////////////////////////////////////////////////////////////
     -->

    


    <!-- http://www.w3.org/2001/XMLSchema#date -->

    <rdfs:Datatype rdf:about="http://www.w3.org/2001/XMLSchema#date"/>
    


    <!-- 
    ///////////////////////////////////////////////////////////////////////////////////////
    //
    // Object Properties
    //
    ///////////////////////////////////////////////////////////////////////////////////////
     -->

    


    <!-- https://w3id.org/leo/onto/analysis/hasUnitOfMeasure -->

    <owl:ObjectProperty rdf:about="https://w3id.org/leo/onto/analysis/hasUnitOfMeasure"/>
    


    <!-- https://w3id.org/leo/onto/livestock-assessment/applies -->

    <owl:ObjectProperty rdf:about="https://w3id.org/leo/onto/livestock-assessment/applies">
        <rdfs:domain rdf:resource="https://w3id.org/leo/onto/livestock-assessment/LivestockAssessment"/>
        <rdfs:range rdf:resource="https://w3id.org/leo/onto/livestock-assessment/Method"/>
        <rdfs:comment xml:lang="en">Property used to indicate the method that the livestock assessmnet applies.</rdfs:comment>
        <rdfs:comment xml:lang="it">Proprietà utilizzata per indicare il metodo che l&apos;accertamento applica</rdfs:comment>
        <rdfs:isDefinedBy rdf:resource="https://w3id.org/leo/onto/livestock-assessment"/>
        <rdfs:label xml:lang="it">applica</rdfs:label>
        <rdfs:label xml:lang="en">applies</rdfs:label>
        <owl:versionInfo xml:lang="it">stabile</owl:versionInfo>
        <owl:versionInfo xml:lang="en">stable</owl:versionInfo>
    </owl:ObjectProperty>
    


    <!-- https://w3id.org/leo/onto/livestock-assessment/hasAssessedSinglePropertyValue -->

    <owl:ObjectProperty rdf:about="https://w3id.org/leo/onto/livestock-assessment/hasAssessedSinglePropertyValue">
        <rdfs:domain rdf:resource="https://w3id.org/leo/onto/livestock-assessment/LivestockAssessment"/>
        <rdfs:range rdf:resource="https://w3id.org/leo/onto/livestock-assessment/AssessedSinglePropertyValue"/>
        <rdfs:comment xml:lang="en">Property used to specify all the measured properties with their values in a livestock assessment</rdfs:comment>
        <rdfs:comment xml:lang="it">Proprietà utilizzata per specificare tutte le proprietà misurate con i relativi valori in un accertamento svolto in ambito zootecnico</rdfs:comment>
        <rdfs:isDefinedBy rdf:resource="https://w3id.org/leo/onto/livestock-assessment"/>
        <rdfs:label xml:lang="it">ha valore della singola proprietà misurata</rdfs:label>
        <rdfs:label xml:lang="en">has assessed single property value</rdfs:label>
        <owl:versionInfo xml:lang="it">stabile</owl:versionInfo>
        <owl:versionInfo xml:lang="en">stable</owl:versionInfo>
    </owl:ObjectProperty>
    


    <!-- https://w3id.org/leo/onto/livestock-assessment/hasAssessmentResult -->

    <owl:ObjectProperty rdf:about="https://w3id.org/leo/onto/livestock-assessment/hasAssessmentResult">
        <rdfs:domain rdf:resource="https://w3id.org/leo/onto/livestock-assessment/LivestockAssessment"/>
        <rdfs:range rdf:resource="https://w3id.org/leo/onto/livestock-assessment/AssessmentResult"/>
        <rdfs:comment xml:lang="en">Property used to specify the result of a livestock assessment</rdfs:comment>
        <rdfs:comment xml:lang="it">Proprietà utilizzata per specificare un risultato dell&apos;accertamento fatto in ambito zootecnico</rdfs:comment>
        <rdfs:isDefinedBy rdf:resource="https://w3id.org/leo/onto/livestock-assessment"/>
        <rdfs:label xml:lang="it">ha risultato dell&apos;accertamento</rdfs:label>
        <rdfs:label xml:lang="en">has assessment result</rdfs:label>
        <owl:versionInfo xml:lang="it">stabile</owl:versionInfo>
        <owl:versionInfo xml:lang="en">stable</owl:versionInfo>
    </owl:ObjectProperty>
    


    <!-- https://w3id.org/leo/onto/livestock-assessment/hasMeasureProperty -->

    <owl:ObjectProperty rdf:about="https://w3id.org/leo/onto/livestock-assessment/hasMeasureProperty">
        <rdfs:domain rdf:resource="https://w3id.org/leo/onto/livestock-assessment/AssessedSinglePropertyValue"/>
        <rdfs:range rdf:resource="https://w3id.org/leo/onto/livestock-assessment/MeasureProperty"/>
        <rdfs:comment xml:lang="en">Property used to link the technical class of the assessed single property value with the specific property being measured.</rdfs:comment>
        <rdfs:comment xml:lang="it">Proprietà utilizzata per collegare la classe tecnica del valore della singola proprietà valutata con la proprietà specifica misurata</rdfs:comment>
        <rdfs:isDefinedBy rdf:resource="https://w3id.org/leo/onto/livestock-assessment"/>
        <rdfs:label xml:lang="it">ha proprietà misurata/accertata</rdfs:label>
        <rdfs:label xml:lang="en">has measure property</rdfs:label>
        <owl:versionInfo xml:lang="it">stabile</owl:versionInfo>
        <owl:versionInfo xml:lang="en">stable</owl:versionInfo>
    </owl:ObjectProperty>
    


    <!-- https://w3id.org/leo/onto/livestock-assessment/hasPerformer -->

    <owl:ObjectProperty rdf:about="https://w3id.org/leo/onto/livestock-assessment/hasPerformer">
        <rdfs:domain rdf:resource="https://w3id.org/leo/onto/livestock-assessment/LivestockAssessment"/>
        <rdfs:range rdf:resource="https://w3id.org/italia/onto/l0/Agent"/>
        <rdfs:comment xml:lang="en">Property used to specify the entity that performs the livestock assessment</rdfs:comment>
        <rdfs:comment xml:lang="it">Proprietà utilizzata per specificare l&apos;entità che esegue la valutazione in ambito zootecnico</rdfs:comment>
        <rdfs:isDefinedBy rdf:resource="https://w3id.org/leo/onto/livestock-assessment"/>
        <rdfs:label xml:lang="it">ha esecutore di accertamento</rdfs:label>
        <rdfs:label xml:lang="en">has performer</rdfs:label>
        <owl:versionInfo xml:lang="it">stabile</owl:versionInfo>
        <owl:versionInfo xml:lang="en">stable</owl:versionInfo>
    </owl:ObjectProperty>
    


    <!-- https://w3id.org/leo/onto/livestock-assessment/hasSubject -->

    <owl:ObjectProperty rdf:about="https://w3id.org/leo/onto/livestock-assessment/hasSubject">
        <rdfs:domain rdf:resource="https://w3id.org/leo/onto/livestock-assessment/LivestockAssessment"/>
        <rdfs:range rdf:resource="https://w3id.org/italia/onto/l0/Entity"/>
        <rdfs:comment xml:lang="en">Property used to specify the subject/entity subjected to assessmnet in the livestock context</rdfs:comment>
        <rdfs:comment xml:lang="it">Proprietà utilizzata per specificare il soggetto/entità sottoposto/a ad accertamento in ambito zootecnico</rdfs:comment>
        <rdfs:isDefinedBy rdf:resource="https://w3id.org/leo/onto/livestock-assessment"/>
        <rdfs:label xml:lang="it">ha soggetto accertamento</rdfs:label>
        <rdfs:label xml:lang="en">has subject</rdfs:label>
        <owl:versionInfo xml:lang="it">stabile</owl:versionInfo>
        <owl:versionInfo xml:lang="en">stable</owl:versionInfo>
    </owl:ObjectProperty>
    


    <!-- https://w3id.org/leo/onto/livestock-assessment/isAssessmentOf -->

    <owl:ObjectProperty rdf:about="https://w3id.org/leo/onto/livestock-assessment/isAssessmentOf">
        <rdfs:domain rdf:resource="https://w3id.org/leo/onto/livestock-assessment/LivestockAssessment"/>
        <rdfs:range rdf:resource="https://w3id.org/italia/onto/l0/Entity"/>
        <rdfs:comment xml:lang="en">Property used to attribute the entity to which the livestock assessment refers. An example can be to use this property to specify the farm company to which the assessment refers.</rdfs:comment>
        <rdfs:comment xml:lang="it">Proprietà utilizzata per attribuire l&apos;entità a cui si riferisce la valutazione fatta in ambito zootecnico. Un esempio può essere quello di utilizzare questa proprietà per specificare l&apos;azienda agricola a cui si riferisce l&apos;accertamento.</rdfs:comment>
        <rdfs:isDefinedBy rdf:resource="https://w3id.org/leo/onto/livestock-assessment"/>
        <rdfs:label xml:lang="en">is assessment of</rdfs:label>
        <rdfs:label xml:lang="it">è accertamento di</rdfs:label>
        <owl:versionInfo xml:lang="it">stabile</owl:versionInfo>
        <owl:versionInfo xml:lang="en">stable</owl:versionInfo>
    </owl:ObjectProperty>
    


    <!-- https://w3id.org/leo/onto/livestock-assessment/uses -->

    <owl:ObjectProperty rdf:about="https://w3id.org/leo/onto/livestock-assessment/uses">
        <rdfs:domain rdf:resource="https://w3id.org/leo/onto/livestock-assessment/LivestockAssessment"/>
        <rdfs:range rdf:resource="https://w3id.org/leo/onto/livestock-assessment/Device"/>
        <rdfs:comment xml:lang="en">Property used to indicate the device used in the livestock assessment</rdfs:comment>
        <rdfs:comment xml:lang="it">Proprietà utilizzata per indicare lo strumento usato nell&apos;accertamento</rdfs:comment>
        <rdfs:isDefinedBy rdf:resource="https://w3id.org/leo/onto/livestock-assessment"/>
        <rdfs:label xml:lang="it">usa</rdfs:label>
        <rdfs:label xml:lang="en">uses</rdfs:label>
        <owl:versionInfo xml:lang="it">stabile</owl:versionInfo>
        <owl:versionInfo xml:lang="en">stable</owl:versionInfo>
    </owl:ObjectProperty>
    


    <!-- 
    ///////////////////////////////////////////////////////////////////////////////////////
    //
    // Data properties
    //
    ///////////////////////////////////////////////////////////////////////////////////////
     -->

    


    <!-- https://w3id.org/italia/onto/MU/value -->

    <owl:DatatypeProperty rdf:about="https://w3id.org/italia/onto/MU/value"/>
    


    <!-- https://w3id.org/italia/onto/TI/date -->

    <owl:DatatypeProperty rdf:about="https://w3id.org/italia/onto/TI/date"/>
    


    <!-- https://w3id.org/leo/onto/livestock-assessment/assessmentId -->

    <owl:DatatypeProperty rdf:about="https://w3id.org/leo/onto/livestock-assessment/assessmentId">
        <rdfs:subPropertyOf rdf:resource="https://w3id.org/italia/onto/l0/identifier"/>
        <rdfs:domain rdf:resource="https://w3id.org/leo/onto/livestock-assessment/LivestockAssessment"/>
        <rdfs:range rdf:resource="http://www.w3.org/2000/01/rdf-schema#Literal"/>
        <rdfs:comment xml:lang="en">A unique identifier of the assessment</rdfs:comment>
        <rdfs:comment xml:lang="it">Un codice identificativo univoco dell&apos;accertamento</rdfs:comment>
        <rdfs:isDefinedBy rdf:resource="https://w3id.org/leo/onto/livestock-assessment"/>
        <rdfs:label xml:lang="en">assessment identifier</rdfs:label>
        <rdfs:label xml:lang="it">codice accertamento</rdfs:label>
        <owl:versionInfo xml:lang="it">stabile</owl:versionInfo>
        <owl:versionInfo xml:lang="en">stable</owl:versionInfo>
    </owl:DatatypeProperty>
    


    <!-- 
    ///////////////////////////////////////////////////////////////////////////////////////
    //
    // Classes
    //
    ///////////////////////////////////////////////////////////////////////////////////////
     -->

    


    <!-- https://w3id.org/italia/onto/ADMS/SemanticAsset -->

    <owl:Class rdf:about="https://w3id.org/italia/onto/ADMS/SemanticAsset"/>
    


    <!-- https://w3id.org/italia/onto/ADMS/SemanticAssetDistribution -->

    <owl:Class rdf:about="https://w3id.org/italia/onto/ADMS/SemanticAssetDistribution"/>
    


    <!-- https://w3id.org/italia/onto/l0/Agent -->

    <owl:Class rdf:about="https://w3id.org/italia/onto/l0/Agent"/>
    


    <!-- https://w3id.org/italia/onto/l0/Characteristic -->

    <owl:Class rdf:about="https://w3id.org/italia/onto/l0/Characteristic"/>
    


    <!-- https://w3id.org/italia/onto/l0/Entity -->

    <owl:Class rdf:about="https://w3id.org/italia/onto/l0/Entity"/>
    


    <!-- https://w3id.org/italia/onto/l0/EventOrSituation -->

    <owl:Class rdf:about="https://w3id.org/italia/onto/l0/EventOrSituation"/>
    


    <!-- https://w3id.org/leo/onto/analysis/UnitOfMeasure -->

    <owl:Class rdf:about="https://w3id.org/leo/onto/analysis/UnitOfMeasure"/>
    


    <!-- https://w3id.org/leo/onto/livestock-assessment/AssessedSinglePropertyValue -->

    <owl:Class rdf:about="https://w3id.org/leo/onto/livestock-assessment/AssessedSinglePropertyValue">
        <rdfs:subClassOf rdf:resource="https://w3id.org/italia/onto/l0/EventOrSituation"/>
        <rdfs:subClassOf>
            <owl:Restriction>
                <owl:onProperty rdf:resource="https://w3id.org/italia/onto/MU/hasValue"/>
                <owl:someValuesFrom rdf:resource="https://w3id.org/italia/onto/MU/Value"/>
            </owl:Restriction>
        </rdfs:subClassOf>
        <rdfs:subClassOf>
            <owl:Restriction>
                <owl:onProperty rdf:resource="https://w3id.org/italia/onto/MU/hasValue"/>
                <owl:allValuesFrom rdf:resource="https://w3id.org/italia/onto/MU/Value"/>
            </owl:Restriction>
        </rdfs:subClassOf>
        <rdfs:subClassOf>
            <owl:Restriction>
                <owl:onProperty rdf:resource="https://w3id.org/leo/onto/livestock-assessment/hasMeasureProperty"/>
                <owl:qualifiedCardinality rdf:datatype="http://www.w3.org/2001/XMLSchema#nonNegativeInteger">1</owl:qualifiedCardinality>
                <owl:onClass rdf:resource="https://w3id.org/leo/onto/livestock-assessment/MeasureProperty"/>
            </owl:Restriction>
        </rdfs:subClassOf>
        <rdfs:comment xml:lang="it">Questa è una classe tecnica utilizzata per collegare le single proprietà misurate in fase di accertamento con i relativi valori delle proprietà misurate.</rdfs:comment>
        <rdfs:comment xml:lang="en">This is a technical class used to connect the single properties that are being assessed during the livestock assessment with the related values</rdfs:comment>
        <rdfs:isDefinedBy rdf:resource="https://w3id.org/leo/onto/livestock-assessment"/>
        <rdfs:label xml:lang="en">Assessed Single Property Value</rdfs:label>
        <rdfs:label xml:lang="it">Valore della Singola Proprietà Valutata</rdfs:label>
        <owl:versionInfo xml:lang="it">stabile</owl:versionInfo>
        <owl:versionInfo xml:lang="en">stable</owl:versionInfo>
    </owl:Class>
    


    <!-- https://w3id.org/leo/onto/livestock-assessment/AssessmentResult -->

    <owl:Class rdf:about="https://w3id.org/leo/onto/livestock-assessment/AssessmentResult">
        <rdfs:subClassOf rdf:resource="https://w3id.org/italia/onto/l0/Characteristic"/>
        <rdfs:comment xml:lang="it">La classe dei risultati degli accertamenti zootecnici. Un risultato può essere qualitativo (e.g., positivo, negativo, ecc.) o quantitativa (un valore numerico).</rdfs:comment>
        <rdfs:comment xml:lang="en">The class of the results of  assessments. A result can be qualitative (e.g. positive, negative, etc.) or quantitative (a numerical value).</rdfs:comment>
        <rdfs:isDefinedBy rdf:resource="https://w3id.org/leo/onto/livestock-assessment"/>
        <rdfs:label xml:lang="en">Assessment Result</rdfs:label>
        <rdfs:label xml:lang="it">Esito dell&apos;Accertamento</rdfs:label>
        <owl:versionInfo xml:lang="it">stabile</owl:versionInfo>
        <owl:versionInfo xml:lang="en">stable</owl:versionInfo>
    </owl:Class>
    


    <!-- https://w3id.org/leo/onto/livestock-assessment/Device -->

    <owl:Class rdf:about="https://w3id.org/leo/onto/livestock-assessment/Device">
        <rdfs:subClassOf rdf:resource="https://w3id.org/italia/onto/l0/Object"/>
        <rdfs:comment xml:lang="it">La classe rappresenta lo strumento utilizzato per effettuare l&apos;accertamento in ambito zootecnico. Può essere un tipo di palmare, o altro strumento specifico.</rdfs:comment>
        <rdfs:comment xml:lang="en">The class represents the device/instrument used to carry out the assessment in the livestock context. It can be a type of palmtop, or another specific device.</rdfs:comment>
        <rdfs:isDefinedBy rdf:resource="https://w3id.org/leo/onto/livestock-assessment"/>
        <rdfs:label xml:lang="en">Device</rdfs:label>
        <rdfs:label xml:lang="it">Strumento</rdfs:label>
        <owl:versionInfo xml:lang="it">stabile</owl:versionInfo>
        <owl:versionInfo xml:lang="en">stable</owl:versionInfo>
    </owl:Class>
    


    <!-- https://w3id.org/leo/onto/livestock-assessment/LivestockAssessment -->

    <owl:Class rdf:about="https://w3id.org/leo/onto/livestock-assessment/LivestockAssessment">
        <rdfs:subClassOf rdf:resource="https://w3id.org/italia/onto/l0/EventOrSituation"/>
        <rdfs:subClassOf>
            <owl:Restriction>
                <owl:onProperty rdf:resource="https://w3id.org/leo/onto/livestock-assessment/hasAssessmentResult"/>
                <owl:someValuesFrom rdf:resource="https://w3id.org/leo/onto/livestock-assessment/AssessmentResult"/>
            </owl:Restriction>
        </rdfs:subClassOf>
        <rdfs:subClassOf>
            <owl:Restriction>
                <owl:onProperty rdf:resource="https://w3id.org/leo/onto/livestock-assessment/hasSubject"/>
                <owl:someValuesFrom rdf:resource="https://w3id.org/italia/onto/l0/Entity"/>
            </owl:Restriction>
        </rdfs:subClassOf>
        <rdfs:subClassOf>
            <owl:Restriction>
                <owl:onProperty rdf:resource="https://w3id.org/leo/onto/livestock-assessment/applies"/>
                <owl:allValuesFrom rdf:resource="https://w3id.org/leo/onto/livestock-assessment/Method"/>
            </owl:Restriction>
        </rdfs:subClassOf>
        <rdfs:subClassOf>
            <owl:Restriction>
                <owl:onProperty rdf:resource="https://w3id.org/leo/onto/livestock-assessment/hasAssessedSinglePropertyValue"/>
                <owl:allValuesFrom rdf:resource="https://w3id.org/leo/onto/livestock-assessment/MeasureProperty"/>
            </owl:Restriction>
        </rdfs:subClassOf>
        <rdfs:subClassOf>
            <owl:Restriction>
                <owl:onProperty rdf:resource="https://w3id.org/leo/onto/livestock-assessment/hasAssessmentResult"/>
                <owl:allValuesFrom rdf:resource="https://w3id.org/leo/onto/livestock-assessment/AssessmentResult"/>
            </owl:Restriction>
        </rdfs:subClassOf>
        <rdfs:subClassOf>
            <owl:Restriction>
                <owl:onProperty rdf:resource="https://w3id.org/leo/onto/livestock-assessment/hasSubject"/>
                <owl:allValuesFrom rdf:resource="https://w3id.org/italia/onto/l0/Entity"/>
            </owl:Restriction>
        </rdfs:subClassOf>
        <rdfs:subClassOf>
            <owl:Restriction>
                <owl:onProperty rdf:resource="https://w3id.org/leo/onto/livestock-assessment/isAssessmentOf"/>
                <owl:allValuesFrom rdf:resource="https://w3id.org/italia/onto/l0/Entity"/>
            </owl:Restriction>
        </rdfs:subClassOf>
        <rdfs:subClassOf>
            <owl:Restriction>
                <owl:onProperty rdf:resource="https://w3id.org/italia/onto/TI/atTime"/>
                <owl:maxQualifiedCardinality rdf:datatype="http://www.w3.org/2001/XMLSchema#nonNegativeInteger">1</owl:maxQualifiedCardinality>
                <owl:onClass rdf:resource="https://w3id.org/italia/onto/TI/TimeInterval"/>
            </owl:Restriction>
        </rdfs:subClassOf>
        <rdfs:subClassOf>
            <owl:Restriction>
                <owl:onProperty rdf:resource="https://w3id.org/leo/onto/livestock-assessment/hasPerformer"/>
                <owl:maxQualifiedCardinality rdf:datatype="http://www.w3.org/2001/XMLSchema#nonNegativeInteger">1</owl:maxQualifiedCardinality>
                <owl:onClass rdf:resource="https://w3id.org/italia/onto/l0/Agent"/>
            </owl:Restriction>
        </rdfs:subClassOf>
        <rdfs:subClassOf>
            <owl:Restriction>
                <owl:onProperty rdf:resource="https://w3id.org/leo/onto/livestock-assessment/uses"/>
                <owl:maxQualifiedCardinality rdf:datatype="http://www.w3.org/2001/XMLSchema#nonNegativeInteger">1</owl:maxQualifiedCardinality>
                <owl:onClass rdf:resource="https://w3id.org/leo/onto/livestock-assessment/Device"/>
            </owl:Restriction>
        </rdfs:subClassOf>
        <rdfs:subClassOf>
            <owl:Restriction>
                <owl:onProperty rdf:resource="https://w3id.org/italia/onto/TI/date"/>
                <owl:maxQualifiedCardinality rdf:datatype="http://www.w3.org/2001/XMLSchema#nonNegativeInteger">1</owl:maxQualifiedCardinality>
                <owl:onDataRange>
                    <rdfs:Datatype>
                        <owl:unionOf rdf:parseType="Collection">
                            <rdf:Description rdf:about="http://www.w3.org/2001/XMLSchema#date"/>
                            <rdf:Description rdf:about="http://www.w3.org/2001/XMLSchema#dateTime"/>
                        </owl:unionOf>
                    </rdfs:Datatype>
                </owl:onDataRange>
            </owl:Restriction>
        </rdfs:subClassOf>
        <rdfs:subClassOf>
            <owl:Restriction>
                <owl:onProperty rdf:resource="https://w3id.org/leo/onto/livestock-assessment/assessmentId"/>
                <owl:maxCardinality rdf:datatype="http://www.w3.org/2001/XMLSchema#nonNegativeInteger">1</owl:maxCardinality>
            </owl:Restriction>
        </rdfs:subClassOf>
        <rdfs:comment xml:lang="it">La classe include tutti i tipi di accertamenti e controlli che possono essere di interesse per il settore zootecnico (e.g., accertamenti zootecnici, controlli funzionali, ecc.)</rdfs:comment>
        <rdfs:comment xml:lang="en">The class includes all the types of  assessments that are of interest for the livestock sector (e.g., livestock assessments, milk functional assessment, etc.)</rdfs:comment>
        <rdfs:isDefinedBy rdf:resource="https://w3id.org/leo/onto/livestock-assessment"/>
        <rdfs:label xml:lang="it">Accertamento Zootecnico</rdfs:label>
        <rdfs:label xml:lang="en">Livestock Assessment</rdfs:label>
        <owl:versionInfo xml:lang="it">stabile</owl:versionInfo>
        <owl:versionInfo xml:lang="en">stable</owl:versionInfo>
    </owl:Class>
    


    <!-- https://w3id.org/leo/onto/livestock-assessment/MeasureProperty -->

    <owl:Class rdf:about="https://w3id.org/leo/onto/livestock-assessment/MeasureProperty">
        <rdfs:subClassOf rdf:resource="https://w3id.org/italia/onto/l0/Characteristic"/>
        <rdfs:subClassOf>
            <owl:Restriction>
                <owl:onProperty rdf:resource="https://w3id.org/italia/onto/l0/name"/>
                <owl:someValuesFrom rdf:resource="http://www.w3.org/1999/02/22-rdf-syntax-ns#PlainLiteral"/>
            </owl:Restriction>
        </rdfs:subClassOf>
        <rdfs:subClassOf>
            <owl:Restriction>
                <owl:onProperty rdf:resource="https://w3id.org/italia/onto/l0/description"/>
                <owl:allValuesFrom rdf:resource="http://www.w3.org/2000/01/rdf-schema#Literal"/>
            </owl:Restriction>
        </rdfs:subClassOf>
        <rdfs:subClassOf>
            <owl:Restriction>
                <owl:onProperty rdf:resource="https://w3id.org/italia/onto/l0/identifier"/>
                <owl:maxCardinality rdf:datatype="http://www.w3.org/2001/XMLSchema#nonNegativeInteger">1</owl:maxCardinality>
            </owl:Restriction>
        </rdfs:subClassOf>
        <rdfs:isDefinedBy rdf:resource="https://w3id.org/leo/onto/livestock-assessment"/>
        <rdfs:isDefinedBy xml:lang="it">La classe di tutte le misure che vengono rilevate in fase di accertamento. Esempi includono la quantità di latte (deviazione standard), l&apos;ora del flusso massimo di latte (media), ecc.</rdfs:isDefinedBy>
        <rdfs:isDefinedBy xml:lang="en">The class of all the measure properties detected during the livestock assessment. Examples include the quantity of milk (standard deviation), the hour of the maximum flow of milk (average), etc.</rdfs:isDefinedBy>
        <rdfs:label xml:lang="en">Measure Property</rdfs:label>
        <rdfs:label xml:lang="it">Proprietà misurata</rdfs:label>
        <owl:versionInfo xml:lang="it">stabile</owl:versionInfo>
        <owl:versionInfo xml:lang="en">stable</owl:versionInfo>
    </owl:Class>
    


    <!-- https://w3id.org/leo/onto/livestock-assessment/Method -->

    <owl:Class rdf:about="https://w3id.org/leo/onto/livestock-assessment/Method">
        <rdfs:subClassOf rdf:resource="https://w3id.org/italia/onto/l0/Description"/>
        <rdfs:comment xml:lang="it">La classe delle tecniche analitiche utilizzate per l&apos;accertamento zootecnicio. La tecnica usata è identificata da un codice (Codici EFSA)</rdfs:comment>
        <rdfs:comment xml:lang="en">The class of analytical techniques used for livestock assessments. The technique used is identified by a code (EFSA Codes)</rdfs:comment>
        <rdfs:isDefinedBy rdf:resource="https://w3id.org/leo/onto/livestock-assessment"/>
        <rdfs:label xml:lang="en">Method</rdfs:label>
        <rdfs:label xml:lang="it">Metodo</rdfs:label>
        <owl:versionInfo xml:lang="it">stabile</owl:versionInfo>
        <owl:versionInfo xml:lang="en">stable</owl:versionInfo>
    </owl:Class>
    


    <!-- 
    ///////////////////////////////////////////////////////////////////////////////////////
    //
    // Individuals
    //
    ///////////////////////////////////////////////////////////////////////////////////////
     -->

    


    <!-- https://w3id.org/leo/data/distribution/LA-JSON-LD -->

    <owl:NamedIndividual rdf:about="https://w3id.org/leo/data/distribution/LA-JSON-LD">
        <rdf:type rdf:resource="https://w3id.org/italia/onto/ADMS/SemanticAssetDistribution"/>
        <terms:description xml:lang="it">Questa è la distribuzione JSON-LD dell&apos;ontologia sugli accertamenti zootecnici</terms:description>
        <terms:description xml:lang="en">This is the distribution in JSON-LD of livestock assessments ontology</terms:description>
        <terms:format rdf:resource="http://publications.europa.eu/resource/authority/file-type/JSON_LD"/>
        <terms:license rdf:resource="https://w3id.org/italia/controlled-vocabulary/licences/A21_CCBY40"/>
        <terms:title xml:lang="it">Distribuzione JSON-LD ontologia Accertamenti Zootecnici</terms:title>
        <terms:title xml:lang="en">JSON-LD distribution of Livestock Assessment Ontology</terms:title>
        <rdfs:comment xml:lang="it">Questa è la distribuzione JSON-LD dell&apos;ontologia sugli accertamenti zootecnici</rdfs:comment>
        <rdfs:comment xml:lang="en">This is the distribution in JSON-LD of livestock assessments ontology</rdfs:comment>
        <rdfs:label xml:lang="it">Distribuzione JSON-LD ontologia Accertamenti Zootecnici</rdfs:label>
        <rdfs:label xml:lang="en">JSON-LD distribution of Livestock Assessment Ontology</rdfs:label>
        <dcat:accessURL rdf:resource="https://www.leo-project.it/Ontologie/livestock-assessment/latest"/>
        <dcat:downloadURL rdf:resource="https://raw.githubusercontent.com/Bluarancio/Leo-OpenData/master/Ontologie/livestock-assessment/latest/livestock-assessment.jsonld"/>
    </owl:NamedIndividual>
    


    <!-- https://w3id.org/leo/data/distribution/LA-RDF-TURTLE -->

    <owl:NamedIndividual rdf:about="https://w3id.org/leo/data/distribution/LA-RDF-TURTLE">
        <rdf:type rdf:resource="https://w3id.org/italia/onto/ADMS/SemanticAssetDistribution"/>
        <terms:description xml:lang="it">Questa è la distribuzione RDF/Turtle dell&apos;ontologia sugli accertamenti zootecnici</terms:description>
        <terms:description xml:lang="en">This is the distribution in RDF/Turtle of livestock assessments ontology</terms:description>
        <terms:format rdf:resource="http://publications.europa.eu/resource/authority/file-type/RDF_TURTLE"/>
        <terms:license rdf:resource="https://w3id.org/italia/controlled-vocabulary/licences/A21_CCBY40"/>
        <terms:title xml:lang="it">Distribuzione RDF/Turtle ontologia Accertamenti Zootecnici</terms:title>
        <terms:title xml:lang="en">RDF/Turtle distribution of Livestock Assessment Ontology</terms:title>
        <rdfs:comment xml:lang="it">Questa è la distribuzione RDF/Turtle dell&apos;ontologia sugli accertamenti zootecnici</rdfs:comment>
        <rdfs:comment xml:lang="en">This is the distribution in RDF/Turtle of livestock assessments ontology</rdfs:comment>
        <rdfs:label xml:lang="it">Distribuzione RDF/Turtle ontologia Accertamenti Zootecnici</rdfs:label>
        <rdfs:label xml:lang="en">RDF/Turtle distribution of Livestock Assessment Ontology</rdfs:label>
        <dcat:accessURL rdf:resource="https://www.leo-project.it/Ontologie/livestock-assessment/latest"/>
        <dcat:downloadURL rdf:resource="https://raw.githubusercontent.com/Bluarancio/Leo-OpenData/master/Ontologie/livestock-assessment/latest/livestock-assessment.ttl"/>
    </owl:NamedIndividual>
    


    <!-- https://w3id.org/leo/data/distribution/LA-RDF-XML -->

    <owl:NamedIndividual rdf:about="https://w3id.org/leo/data/distribution/LA-RDF-XML">
        <rdf:type rdf:resource="https://w3id.org/italia/onto/ADMS/SemanticAssetDistribution"/>
        <terms:description xml:lang="it">Questa è la distribuzione RDF/XML dell&apos;ontologia sugli accertamenti zootecnici</terms:description>
        <terms:description xml:lang="en">This is the distribution in RDF/XML of livestock assessments ontology</terms:description>
        <terms:format rdf:resource="http://publications.europa.eu/resource/authority/file-type/RDF_XML"/>
        <terms:license rdf:resource="https://w3id.org/italia/controlled-vocabulary/licences/A21_CCBY40"/>
        <terms:title xml:lang="it">Distribuzione RDF/XML ontologia Accertamenti Zootecnici</terms:title>
        <terms:title xml:lang="en">RDF/XML distribution of Livestock Assessment Ontology</terms:title>
        <rdfs:comment xml:lang="it">Questa è la distribuzione RDF/XML dell&apos;ontologia sugli accertamenti zootecnici</rdfs:comment>
        <rdfs:comment xml:lang="en">This is the distribution in RDF/XML of livestock assessments ontology</rdfs:comment>
        <rdfs:label xml:lang="it">Distribuzione RDF/XML ontologia Accertamenti Zootecnici</rdfs:label>
        <rdfs:label xml:lang="en">RDF/XML distribution of Livestock Assessment Ontology</rdfs:label>
        <dcat:accessURL rdf:resource="https://www.leo-project.it/Ontologie/livestock-assessment/latest"/>
        <dcat:downloadURL rdf:resource="https://raw.githubusercontent.com/Bluarancio/Leo-OpenData/master/Ontologie/livestock-assessment/latest/livestock-assessment.rdf"/>
    </owl:NamedIndividual>
    


    <!-- https://w3id.org/leo/onto/livestock-assessment -->

    <owl:NamedIndividual rdf:about="https://w3id.org/leo/onto/livestock-assessment">
        <rdf:type rdf:resource="https://w3id.org/italia/onto/ADMS/SemanticAsset"/>
    </owl:NamedIndividual>
</rdf:RDF>



<!-- Generated by the OWL API (version 4.5.9.2019-02-01T07:24:44Z) https://github.com/owlcs/owlapi -->

