<?xml version="1.0"?>
<rdf:RDF xmlns="https://w3id.org/leo/onto/health-assessment/"
     xml:base="https://w3id.org/leo/onto/health-assessment/"
     xmlns:dc="http://purl.org/dc/elements/1.1/"
     xmlns:ns="http://www.w3.org/2006/vcard/ns#"
     xmlns:owl="http://www.w3.org/2002/07/owl#"
     xmlns:rdf="http://www.w3.org/1999/02/22-rdf-syntax-ns#"
     xmlns:xml="http://www.w3.org/XML/1998/namespace"
     xmlns:xsd="http://www.w3.org/2001/XMLSchema#"
     xmlns:ADMS="https://w3id.org/italia/onto/ADMS/"
     xmlns:dcat="http://www.w3.org/ns/dcat#"
     xmlns:foaf="http://xmlns.com/foaf/0.1/"
     xmlns:prov="http://www.w3.org/ns/prov#"
     xmlns:rdfs="http://www.w3.org/2000/01/rdf-schema#"
     xmlns:terms="http://purl.org/dc/terms/">
    <owl:Ontology rdf:about="https://w3id.org/leo/onto/health-assessment">
        <owl:versionIRI rdf:resource="https://w3id.org/leo/onto/health-assessment/0.2"/>
        <owl:imports rdf:resource="https://w3id.org/leo/onto/livestock-assessment"/>
        <dc:description rdf:resource="https://www.dropbox.com/s/v7d9md0op4v9o9y/HealthAssessment.png?raw=1"/>
        <terms:accrualPeriodicity rdf:resource="http://publications.europa.eu/resource/authority/frequency/IRREG"/>
        <terms:creator rdf:resource="https://w3id.org/leo/data/private-organization/00944701002"/>
        <terms:creator rdf:resource="https://w3id.org/leo/data/private-organization/06695411006"/>
        <terms:description xml:lang="it">Questa è l&apos;ontologia usata per modellare i dati di tipo HealthData nel progetto LEO ovvero dati relativi ad accertamenti sanitari che riguardano sia singoli animali che cosiddetti screening aziendali. I dati sono acquisiti in cooperazione applicativa direttamente dall’Istituto Zooprofilattico Umbria-Marche.</terms:description>
        <terms:description xml:lang="en">This is the ontology used to model data of HealthData type in the LEO project. Specifically, the ontology represents the data on health assessments concerning both individual animals and so-called farm screenings. The data is acquired through machine-to-machine mechanisms directly from the &apos;Istituto Zooprofilattico Umbria-Marche&apos;.</terms:description>
        <terms:identifier xml:lang="it">onto-BA-10</terms:identifier>
        <terms:issued rdf:datatype="http://www.w3.org/2001/XMLSchema#date">2022-11-22</terms:issued>
        <terms:language rdf:resource="http://publications.europa.eu/resource/authority/language/ENG"/>
        <terms:language rdf:resource="http://publications.europa.eu/resource/authority/language/ITA"/>
        <terms:modified rdf:datatype="http://www.w3.org/2001/XMLSchema#date">2023-03-09</terms:modified>
        <terms:publisher rdf:resource="https://w3id.org/leo/data/private-organization/06695411006"/>
        <terms:rightsHolder rdf:resource="https://w3id.org/leo/data/private-organization/00944701002"/>
        <terms:subject rdf:resource="http://eurovoc.europa.eu/6271"/>
        <terms:subject rdf:resource="http://eurovoc.europa.eu/6272"/>
        <terms:title xml:lang="en">Health Assessment Ontology - HeathData</terms:title>
        <terms:title xml:lang="it">Ontologia degli Accertamenti Sanitari (inclusi Screening Aziendali)- HealthData</terms:title>
        <rdfs:comment xml:lang="it">Questa è l&apos;ontologia usata per modellare i dati di tipo HealthData nel progetto LEO ovvero dati relativi ad accertamenti sanitari che riguardano sia singoli animali che cosiddetti screening aziendali. I dati sono acquisiti in cooperazione applicativa direttamente dall’Istituto Zooprofilattico Umbria-Marche.</rdfs:comment>
        <rdfs:comment xml:lang="en">This is the ontology used to model data of HealthData type in the LEO project. Specifically, the ontology represents the data on health assessments concerning both individual animals and so-called farm screenings. The data is acquired through machine-to-machine mechanisms directly from the &apos;Istituto Zooprofilattico Umbria-Marche&apos;.</rdfs:comment>
        <rdfs:isDefinedBy rdf:resource="https://w3id.org/leo/onto/health-assessment"/>
        <rdfs:label xml:lang="en">Health Assessment Ontology - HeathData</rdfs:label>
        <rdfs:label xml:lang="it">Ontologia degli Accertamenti Sanitari (inclusi Screening Aziendali)- HealthData</rdfs:label>
        <owl:versionInfo xml:lang="en">Version 0.2 - 2023 - Revision of the ontology based on the availability of livestock assessment general ontology</owl:versionInfo>
        <owl:versionInfo xml:lang="it">Versione 0.1 - 2023 - Revisione dell&apos;ontologia sulla base della disponibilità dell&apos;ontologia generale sugli accertamenti in ambito zootecnico</owl:versionInfo>
        <dcat:contactPoint rdf:resource="https://w3id.org/leo/data/contact-point/onto-aia"/>
        <dcat:keyword xml:lang="it">Accertamento Sanitario</dcat:keyword>
        <dcat:keyword xml:lang="it">Malattia</dcat:keyword>
        <dcat:keyword xml:lang="it">Prelievo</dcat:keyword>
        <dcat:keyword xml:lang="it">Screening Aziendale</dcat:keyword>
        <dcat:theme rdf:resource="http://publications.europa.eu/resource/authority/data-theme/HEAL"/>
        <ADMS:acronym>HA</ADMS:acronym>
        <ADMS:hasFormalityLevel rdf:resource="https://w3id.org/italia/onto/ADMS/Formal"/>
        <ADMS:hasKeyClass rdf:resource="https://w3id.org/leo/onto/health-assessment/CompanyScreening"/>
        <ADMS:hasKeyClass rdf:resource="https://w3id.org/leo/onto/health-assessment/DiagnosticHealthAssessment"/>
        <ADMS:hasKeyClass rdf:resource="https://w3id.org/leo/onto/health-assessment/Disease"/>
        <ADMS:hasKeyClass rdf:resource="https://w3id.org/leo/onto/health-assessment/SingleAnimalHealthAssessment"/>
        <ADMS:hasOntologyLanguage rdf:resource="https://w3id.org/italia/onto/ADMS/OWL"/>
        <ADMS:hasSemanticAssetDistribution rdf:resource="https://w3id.org/leo/data/distribution/HA-JSON-LD"/>
        <ADMS:hasSemanticAssetDistribution rdf:resource="https://w3id.org/leo/data/distribution/HA-RDF-TURTLE"/>
        <ADMS:hasSemanticAssetDistribution rdf:resource="https://w3id.org/leo/data/distribution/HA-RDF-XML"/>
        <ADMS:hasTask rdf:resource="https://w3id.org/italia/onto/ADMS/AnnotationTask"/>
        <ADMS:hasTask rdf:resource="https://w3id.org/italia/onto/ADMS/QueryFormulationTask"/>
        <ADMS:hasTask rdf:resource="https://w3id.org/italia/onto/ADMS/SearchTask"/>
        <ADMS:officialURI rdf:datatype="http://www.w3.org/2001/XMLSchema#anyURI">https://w3id.org/leo/onto/health-assessment</ADMS:officialURI>
        <ADMS:prefix>ha</ADMS:prefix>
        <ADMS:semanticAssetInUse rdf:resource="https://w3id.org/leo/data/project/LEO"/>
        <ADMS:status>published</ADMS:status>
        <ADMS:target xml:lang="it">Comunità Open Data</ADMS:target>
        <ADMS:target>Imprese</ADMS:target>
        <ADMS:target>Pubbliche Amministrazioni</ADMS:target>
        <ADMS:target xml:lang="it">Specialisti del settore zootecnico</ADMS:target>
        <ADMS:type rdf:resource="https://w3id.org/italia/onto/ADMS/DomainOntology"/>
    </owl:Ontology>



    <!--
    ///////////////////////////////////////////////////////////////////////////////////////
    //
    // Annotation properties
    //
    ///////////////////////////////////////////////////////////////////////////////////////
     -->




    <!-- http://purl.org/dc/terms/accrualPeriodicity -->

    <owl:AnnotationProperty rdf:about="http://purl.org/dc/terms/accrualPeriodicity"/>



    <!-- http://purl.org/dc/terms/creator -->

    <owl:AnnotationProperty rdf:about="http://purl.org/dc/terms/creator"/>



    <!-- http://purl.org/dc/terms/description -->

    <owl:AnnotationProperty rdf:about="http://purl.org/dc/terms/description"/>



    <!-- http://purl.org/dc/terms/format -->

    <owl:AnnotationProperty rdf:about="http://purl.org/dc/terms/format"/>



    <!-- http://purl.org/dc/terms/identifier -->

    <owl:AnnotationProperty rdf:about="http://purl.org/dc/terms/identifier"/>



    <!-- http://purl.org/dc/terms/issued -->

    <owl:AnnotationProperty rdf:about="http://purl.org/dc/terms/issued"/>



    <!-- http://purl.org/dc/terms/language -->

    <owl:AnnotationProperty rdf:about="http://purl.org/dc/terms/language"/>



    <!-- http://purl.org/dc/terms/license -->

    <owl:AnnotationProperty rdf:about="http://purl.org/dc/terms/license"/>



    <!-- http://purl.org/dc/terms/modified -->

    <owl:AnnotationProperty rdf:about="http://purl.org/dc/terms/modified"/>



    <!-- http://purl.org/dc/terms/publisher -->

    <owl:AnnotationProperty rdf:about="http://purl.org/dc/terms/publisher"/>



    <!-- http://purl.org/dc/terms/rightsHolder -->

    <owl:AnnotationProperty rdf:about="http://purl.org/dc/terms/rightsHolder"/>



    <!-- http://purl.org/dc/terms/subject -->

    <owl:AnnotationProperty rdf:about="http://purl.org/dc/terms/subject"/>



    <!-- http://purl.org/dc/terms/title -->

    <owl:AnnotationProperty rdf:about="http://purl.org/dc/terms/title"/>



    <!-- http://www.w3.org/ns/dcat#accessURL -->

    <owl:AnnotationProperty rdf:about="http://www.w3.org/ns/dcat#accessURL"/>



    <!-- http://www.w3.org/ns/dcat#contactPoint -->

    <owl:AnnotationProperty rdf:about="http://www.w3.org/ns/dcat#contactPoint"/>



    <!-- http://www.w3.org/ns/dcat#downloadURL -->

    <owl:AnnotationProperty rdf:about="http://www.w3.org/ns/dcat#downloadURL"/>



    <!-- http://www.w3.org/ns/dcat#keyword -->

    <owl:AnnotationProperty rdf:about="http://www.w3.org/ns/dcat#keyword"/>



    <!-- http://www.w3.org/ns/dcat#theme -->

    <owl:AnnotationProperty rdf:about="http://www.w3.org/ns/dcat#theme"/>



    <!-- https://w3id.org/italia/onto/ADMS/acronym -->

    <owl:AnnotationProperty rdf:about="https://w3id.org/italia/onto/ADMS/acronym"/>



    <!-- https://w3id.org/italia/onto/ADMS/hasFormalityLevel -->

    <owl:AnnotationProperty rdf:about="https://w3id.org/italia/onto/ADMS/hasFormalityLevel"/>



    <!-- https://w3id.org/italia/onto/ADMS/hasKeyClass -->

    <owl:AnnotationProperty rdf:about="https://w3id.org/italia/onto/ADMS/hasKeyClass"/>



    <!-- https://w3id.org/italia/onto/ADMS/hasOntologyLanguage -->

    <owl:AnnotationProperty rdf:about="https://w3id.org/italia/onto/ADMS/hasOntologyLanguage"/>



    <!-- https://w3id.org/italia/onto/ADMS/hasSemanticAssetDistribution -->

    <owl:AnnotationProperty rdf:about="https://w3id.org/italia/onto/ADMS/hasSemanticAssetDistribution"/>



    <!-- https://w3id.org/italia/onto/ADMS/hasTask -->

    <owl:AnnotationProperty rdf:about="https://w3id.org/italia/onto/ADMS/hasTask"/>



    <!-- https://w3id.org/italia/onto/ADMS/officialURI -->

    <owl:AnnotationProperty rdf:about="https://w3id.org/italia/onto/ADMS/officialURI"/>



    <!-- https://w3id.org/italia/onto/ADMS/prefix -->

    <owl:AnnotationProperty rdf:about="https://w3id.org/italia/onto/ADMS/prefix"/>



    <!-- https://w3id.org/italia/onto/ADMS/semanticAssetInUse -->

    <owl:AnnotationProperty rdf:about="https://w3id.org/italia/onto/ADMS/semanticAssetInUse"/>



    <!-- https://w3id.org/italia/onto/ADMS/status -->

    <owl:AnnotationProperty rdf:about="https://w3id.org/italia/onto/ADMS/status"/>



    <!-- https://w3id.org/italia/onto/ADMS/target -->

    <owl:AnnotationProperty rdf:about="https://w3id.org/italia/onto/ADMS/target"/>



    <!-- https://w3id.org/italia/onto/ADMS/type -->

    <owl:AnnotationProperty rdf:about="https://w3id.org/italia/onto/ADMS/type"/>



    <!--
    ///////////////////////////////////////////////////////////////////////////////////////
    //
    // Object Properties
    //
    ///////////////////////////////////////////////////////////////////////////////////////
     -->




    <!-- https://w3id.org/leo/onto/analysis/hasUnitOfMeasure -->

    <owl:ObjectProperty rdf:about="https://w3id.org/leo/onto/analysis/hasUnitOfMeasure"/>



    <!-- https://w3id.org/leo/onto/health-assessment/doneForSample -->

    <owl:ObjectProperty rdf:about="https://w3id.org/leo/onto/health-assessment/doneForSample">
        <rdfs:domain rdf:resource="https://w3id.org/leo/onto/health-assessment/DiagnosticHealthAssessment"/>
        <rdfs:range rdf:resource="https://w3id.org/leo/onto/analysis/Sample"/>
        <rdfs:comment xml:lang="en">Property used to specify for which sample the health assessment was done.</rdfs:comment>
        <rdfs:comment xml:lang="it">Proprietà usata per indicare per quale campione è stato fatto l&apos;accertamento sanitario.</rdfs:comment>
        <rdfs:isDefinedBy rdf:resource="https://w3id.org/leo/onto/health-assessment"/>
        <rdfs:label xml:lang="en">done for sample</rdfs:label>
        <rdfs:label xml:lang="it">fatto per campione</rdfs:label>
        <owl:versionInfo xml:lang="it">stabile</owl:versionInfo>
        <owl:versionInfo xml:lang="en">stable</owl:versionInfo>
    </owl:ObjectProperty>



    <!-- https://w3id.org/leo/onto/health-assessment/hasAnalysedDisease -->

    <owl:ObjectProperty rdf:about="https://w3id.org/leo/onto/health-assessment/hasAnalysedDisease">
        <rdfs:domain rdf:resource="https://w3id.org/leo/onto/health-assessment/DiagnosticHealthAssessment"/>
        <rdfs:range rdf:resource="https://w3id.org/leo/onto/health-assessment/Disease"/>
        <rdfs:comment xml:lang="en">Property used to indicate the analysed disease in the health assessment.</rdfs:comment>
        <rdfs:comment xml:lang="it">Proprietà utilizzata per specificare quale malattia è stata analizzata nell&apos;accertamento sanitario.</rdfs:comment>
        <rdfs:isDefinedBy rdf:resource="https://w3id.org/leo/onto/health-assessment"/>
        <rdfs:label xml:lang="it">ha malattia analizzata</rdfs:label>
        <rdfs:label xml:lang="en">has analysed disease</rdfs:label>
        <owl:versionInfo xml:lang="it">stabile</owl:versionInfo>
        <owl:versionInfo xml:lang="en">stable</owl:versionInfo>
    </owl:ObjectProperty>



    <!-- https://w3id.org/leo/onto/health-assessment/hasExaminedMaterial -->

    <owl:ObjectProperty rdf:about="https://w3id.org/leo/onto/health-assessment/hasExaminedMaterial">
        <rdfs:domain rdf:resource="https://w3id.org/leo/onto/health-assessment/DiagnosticHealthAssessment"/>
        <rdfs:range rdf:resource="https://w3id.org/leo/onto/analysis/BiologicalMaterial"/>
        <rdfs:comment xml:lang="en">Property used to represent the biological material that is being analysed in the health assessment.</rdfs:comment>
        <rdfs:comment xml:lang="it">Proprietà usata per rappresentare il materiale esaminato nell&apos;accertamento sanitario.</rdfs:comment>
        <rdfs:isDefinedBy rdf:resource="https://w3id.org/leo/onto/health-assessment"/>
        <rdfs:label xml:lang="it">ha materiale esaminato</rdfs:label>
        <rdfs:label xml:lang="en">has examined material</rdfs:label>
        <owl:versionInfo xml:lang="it">stabile</owl:versionInfo>
        <owl:versionInfo xml:lang="en">stable</owl:versionInfo>
    </owl:ObjectProperty>



    <!-- https://w3id.org/leo/onto/health-assessment/hasReason -->

    <owl:ObjectProperty rdf:about="https://w3id.org/leo/onto/health-assessment/hasReason">
        <rdfs:domain rdf:resource="https://w3id.org/leo/onto/health-assessment/Sampling"/>
        <rdfs:range rdf:resource="https://w3id.org/leo/onto/health-assessment/Reason"/>
        <rdfs:comment xml:lang="en">Property used to specify the reason for the sampling activity.</rdfs:comment>
        <rdfs:comment xml:lang="it">Proprietà utilizzata per specificare il motivo per effettuare il prelievo.</rdfs:comment>
        <rdfs:isDefinedBy rdf:resource="https://w3id.org/leo/onto/health-assessment"/>
        <rdfs:label xml:lang="it">ha motivo prelievo</rdfs:label>
        <rdfs:label xml:lang="en">has reason for sampling</rdfs:label>
        <owl:versionInfo xml:lang="it">stabile</owl:versionInfo>
        <owl:versionInfo xml:lang="en">stable</owl:versionInfo>
    </owl:ObjectProperty>



    <!-- https://w3id.org/leo/onto/health-assessment/hasReplacedTestReport -->

    <owl:ObjectProperty rdf:about="https://w3id.org/leo/onto/health-assessment/hasReplacedTestReport">
        <rdfs:domain rdf:resource="https://w3id.org/leo/onto/health-assessment/DiagnosticHealthAssessment"/>
        <rdfs:range rdf:resource="https://w3id.org/leo/onto/health-assessment/TestReport"/>
        <rdfs:comment xml:lang="en">Property used to indicate the replaced test report in a health assessment</rdfs:comment>
        <rdfs:comment xml:lang="it">Proprietà per indicare il rapporto di prova sostituito in un accertamento sanitario</rdfs:comment>
        <rdfs:isDefinedBy rdf:resource="https://w3id.org/leo/onto/health-assessment"/>
        <rdfs:label xml:lang="it">ha rapporto di prova sostituito</rdfs:label>
        <rdfs:label xml:lang="en">has replaced test report</rdfs:label>
        <owl:versionInfo xml:lang="it">stabile</owl:versionInfo>
        <owl:versionInfo xml:lang="en">stable</owl:versionInfo>
    </owl:ObjectProperty>



    <!-- https://w3id.org/leo/onto/health-assessment/hasSampleAcceptor -->

    <owl:ObjectProperty rdf:about="https://w3id.org/leo/onto/health-assessment/hasSampleAcceptor">
        <rdfs:domain rdf:resource="https://w3id.org/leo/onto/health-assessment/DiagnosticHealthAssessment"/>
        <rdfs:range rdf:resource="https://w3id.org/leo/onto/health-assessment/ZooprophylacticLab"/>
        <rdfs:comment xml:lang="en">Property used to represent the laboratory that accepted the sample on which the health assessment is done.</rdfs:comment>
        <rdfs:comment xml:lang="it">Proprietà usata per indicare il laboratorio che accetta il campione oggetto di accertamento sanitario.</rdfs:comment>
        <rdfs:isDefinedBy rdf:resource="https://w3id.org/leo/onto/health-assessment"/>
        <rdfs:label xml:lang="it">ha laboratorio che accetta campione</rdfs:label>
        <rdfs:label xml:lang="en">has sample acceptor</rdfs:label>
        <owl:versionInfo xml:lang="it">stabile</owl:versionInfo>
        <owl:versionInfo xml:lang="en">stable</owl:versionInfo>
    </owl:ObjectProperty>



    <!-- https://w3id.org/leo/onto/health-assessment/hasSampleJudgement -->

    <owl:ObjectProperty rdf:about="https://w3id.org/leo/onto/health-assessment/hasSampleJudgement">
        <rdfs:domain rdf:resource="https://w3id.org/leo/onto/health-assessment/DiagnosticHealthAssessment"/>
        <rdfs:range rdf:resource="https://w3id.org/leo/onto/health-assessment/SampleJudgement"/>
        <rdfs:comment xml:lang="en">Property representing jthe udgement done in the context of the health assessment on the sample</rdfs:comment>
        <rdfs:comment xml:lang="it">Proprietà che rappresenta il giudizio nel contesto dell&apos;accertamento sanitario in merito al campione</rdfs:comment>
        <rdfs:isDefinedBy rdf:resource="https://w3id.org/leo/onto/health-assessment"/>
        <rdfs:label xml:lang="it">ha giudizio sul campione</rdfs:label>
        <rdfs:label xml:lang="en">has sample judgement</rdfs:label>
        <owl:versionInfo xml:lang="it">stabile</owl:versionInfo>
        <owl:versionInfo xml:lang="en">stable</owl:versionInfo>
    </owl:ObjectProperty>



    <!-- https://w3id.org/leo/onto/health-assessment/hasTestReport -->

    <owl:ObjectProperty rdf:about="https://w3id.org/leo/onto/health-assessment/hasTestReport">
        <rdfs:domain rdf:resource="https://w3id.org/leo/onto/health-assessment/DiagnosticHealthAssessment"/>
        <rdfs:range rdf:resource="https://w3id.org/leo/onto/health-assessment/TestReport"/>
        <rdfs:comment xml:lang="it">Proprietà usata per specificare il rapporto di prova associato all&apos;accertamento sanitario.</rdfs:comment>
        <rdfs:comment xml:lang="en">The property used to specify the test report for the health assessment</rdfs:comment>
        <rdfs:isDefinedBy rdf:resource="https://w3id.org/leo/onto/health-assessment"/>
        <rdfs:label xml:lang="it">ha rapporto di prova</rdfs:label>
        <rdfs:label xml:lang="en">has test report</rdfs:label>
        <owl:versionInfo xml:lang="it">stabile</owl:versionInfo>
        <owl:versionInfo xml:lang="en">stable</owl:versionInfo>
    </owl:ObjectProperty>



    <!-- https://w3id.org/leo/onto/health-assessment/hasUsedAnalyticalTechnique -->

    <owl:ObjectProperty rdf:about="https://w3id.org/leo/onto/health-assessment/hasUsedAnalyticalTechnique">
        <rdfs:subPropertyOf rdf:resource="https://w3id.org/leo/onto/livestock-assessment/applies"/>
        <owl:inverseOf rdf:resource="https://w3id.org/leo/onto/health-assessment/isAnalyticalTechniqueOf"/>
        <rdfs:domain rdf:resource="https://w3id.org/leo/onto/health-assessment/DiagnosticHealthAssessment"/>
        <rdfs:range rdf:resource="https://w3id.org/leo/onto/health-assessment/Technique"/>
        <rdfs:comment xml:lang="en">Property used to specify the analytical method/technique used in the health assessment</rdfs:comment>
        <rdfs:comment xml:lang="it">Proprietà utilizzata per specificare la/il tecnica/metodo analitica/o usata/o nell&apos;accertamento sanitario.</rdfs:comment>
        <rdfs:isDefinedBy rdf:resource="https://w3id.org/leo/onto/health-assessment"/>
        <rdfs:label xml:lang="it">ha tecnica analitica usata</rdfs:label>
        <rdfs:label xml:lang="en">has used analytical technique</rdfs:label>
        <owl:versionInfo xml:lang="it">stabile</owl:versionInfo>
        <owl:versionInfo xml:lang="en">stable</owl:versionInfo>
    </owl:ObjectProperty>



    <!-- https://w3id.org/leo/onto/health-assessment/isAnalyticalTechniqueOf -->

    <owl:ObjectProperty rdf:about="https://w3id.org/leo/onto/health-assessment/isAnalyticalTechniqueOf">
        <rdfs:domain rdf:resource="https://w3id.org/leo/onto/health-assessment/Technique"/>
        <rdfs:range rdf:resource="https://w3id.org/leo/onto/health-assessment/DiagnosticHealthAssessment"/>
        <rdfs:comment xml:lang="en">Inverse property of &apos;has used analytical technique&apos; which links the technique or method to the health assessment.</rdfs:comment>
        <rdfs:comment xml:lang="it">Proprietà inversa di &apos;ha tecnica analitica utilizzata&apos; che collega la tecnica o metodo all&apos;accertamento sanitario.</rdfs:comment>
        <rdfs:isDefinedBy rdf:resource="https://w3id.org/leo/onto/health-assessment"/>
        <rdfs:label xml:lang="en">is analytical technique of</rdfs:label>
        <rdfs:label xml:lang="it">è tecnica analitica di</rdfs:label>
        <owl:versionInfo xml:lang="it">stabile</owl:versionInfo>
        <owl:versionInfo xml:lang="en">stable</owl:versionInfo>
    </owl:ObjectProperty>



    <!-- https://w3id.org/leo/onto/health-assessment/isReferredToSampling -->

    <owl:ObjectProperty rdf:about="https://w3id.org/leo/onto/health-assessment/isReferredToSampling">
        <rdfs:domain rdf:resource="https://w3id.org/leo/onto/health-assessment/DiagnosticHealthAssessment"/>
        <rdfs:range rdf:resource="https://w3id.org/leo/onto/health-assessment/Sampling"/>
        <rdfs:comment xml:lang="en">Property used to link the health assessmnet to sampling activity.</rdfs:comment>
        <rdfs:comment xml:lang="it">Proprietà usata per collegare l&apos;accertamento sanitario all&apos;attività di prelievo del campione.</rdfs:comment>
        <rdfs:isDefinedBy rdf:resource="https://w3id.org/leo/onto/health-assessment"/>
        <rdfs:label xml:lang="en">is referred to sampling</rdfs:label>
        <rdfs:label xml:lang="it">è riferito a prelievo</rdfs:label>
        <owl:versionInfo xml:lang="it">stabile</owl:versionInfo>
        <owl:versionInfo xml:lang="en">stable</owl:versionInfo>
    </owl:ObjectProperty>



    <!-- https://w3id.org/leo/onto/health-assessment/replaced -->

    <owl:ObjectProperty rdf:about="https://w3id.org/leo/onto/health-assessment/replaced">
        <rdfs:domain rdf:resource="https://w3id.org/leo/onto/health-assessment/TestReport"/>
        <rdfs:range rdf:resource="https://w3id.org/leo/onto/health-assessment/TestReport"/>
        <rdfs:comment xml:lang="en">Property used to indicate that a trial report has replaced another  report</rdfs:comment>
        <rdfs:comment xml:lang="it">Proprietà usata per indicare che un rapporto di prova ha sostituito un altro rapporto di prova</rdfs:comment>
        <rdfs:isDefinedBy rdf:resource="https://w3id.org/leo/onto/health-assessment"/>
        <rdfs:label xml:lang="en">replaced</rdfs:label>
        <rdfs:label xml:lang="it">sostituito</rdfs:label>
        <owl:versionInfo xml:lang="it">stabile</owl:versionInfo>
        <owl:versionInfo xml:lang="en">stable</owl:versionInfo>
    </owl:ObjectProperty>



    <!-- https://w3id.org/leo/onto/health-assessment/resultingInSample -->

    <owl:ObjectProperty rdf:about="https://w3id.org/leo/onto/health-assessment/resultingInSample">
        <rdfs:domain rdf:resource="https://w3id.org/leo/onto/health-assessment/Sampling"/>
        <rdfs:range rdf:resource="https://w3id.org/leo/onto/analysis/Sample"/>
        <rdfs:comment xml:lang="en">Property used to represent the sample resulting from a sampling activity</rdfs:comment>
        <rdfs:comment xml:lang="it">Proprietà utilizzata per rappresentare il campione risultante da un&apos;attività di campionamento.</rdfs:comment>
        <rdfs:isDefinedBy rdf:resource="https://w3id.org/leo/onto/health-assessment"/>
        <rdfs:label xml:lang="en">resulting in sample</rdfs:label>
        <rdfs:label xml:lang="it">risultante in campione</rdfs:label>
        <owl:versionInfo xml:lang="it">stabile</owl:versionInfo>
        <owl:versionInfo xml:lang="en">stable</owl:versionInfo>
    </owl:ObjectProperty>



    <!--
    ///////////////////////////////////////////////////////////////////////////////////////
    //
    // Data properties
    //
    ///////////////////////////////////////////////////////////////////////////////////////
     -->




    <!-- https://w3id.org/leo/onto/health-assessment/efsaCode -->

    <owl:DatatypeProperty rdf:about="https://w3id.org/leo/onto/health-assessment/efsaCode">
        <rdfs:subPropertyOf rdf:resource="https://w3id.org/italia/onto/l0/identifier"/>
        <rdfs:domain rdf:resource="http://www.w3.org/2002/07/owl#Thing"/>
        <rdfs:range rdf:resource="http://www.w3.org/2000/01/rdf-schema#Literal"/>
        <rdfs:comment xml:lang="en">It represents the EFSA - European Food Safety Authority codes used in health inspections to identify various elements including the zooprophylactic institutes, the analytical technique used.</rdfs:comment>
        <rdfs:comment xml:lang="it">Rappresenta i codici EFSA - European Food Safety Authority usati negli accertamenti sanitari per identificare diversi elementi tra cui gli istituti zooprofilattici, la tecnica analitica utilizzata.</rdfs:comment>
        <rdfs:isDefinedBy rdf:resource="https://w3id.org/leo/onto/health-assessment"/>
        <rdfs:label xml:lang="en">EFSA code</rdfs:label>
        <rdfs:label xml:lang="it">codice EFSA</rdfs:label>
        <owl:versionInfo xml:lang="it">stabile</owl:versionInfo>
        <owl:versionInfo xml:lang="en">stable</owl:versionInfo>
    </owl:DatatypeProperty>



    <!-- https://w3id.org/leo/onto/health-assessment/note -->

    <owl:DatatypeProperty rdf:about="https://w3id.org/leo/onto/health-assessment/note">
        <rdfs:subPropertyOf rdf:resource="https://w3id.org/italia/onto/l0/description"/>
        <rdfs:domain rdf:resource="https://w3id.org/leo/onto/health-assessment/DiagnosticHealthAssessment"/>
        <rdfs:range rdf:resource="http://www.w3.org/1999/02/22-rdf-syntax-ns#PlainLiteral"/>
        <rdfs:comment xml:lang="it">Eventuali note sull&apos;accertamento sanitario</rdfs:comment>
        <rdfs:comment xml:lang="en">Some descriptive note on the health assessment</rdfs:comment>
        <rdfs:isDefinedBy rdf:resource="https://w3id.org/leo/onto/health-assessment"/>
        <rdfs:label xml:lang="it">nota</rdfs:label>
        <rdfs:label xml:lang="en">note</rdfs:label>
        <owl:versionInfo xml:lang="it">stabile</owl:versionInfo>
        <owl:versionInfo xml:lang="en">stable</owl:versionInfo>
    </owl:DatatypeProperty>



    <!-- https://w3id.org/leo/onto/health-assessment/numNegativeSamples -->

    <owl:DatatypeProperty rdf:about="https://w3id.org/leo/onto/health-assessment/numNegativeSamples">
        <rdfs:subPropertyOf rdf:resource="https://w3id.org/italia/onto/MU/value"/>
        <rdfs:domain rdf:resource="https://w3id.org/leo/onto/health-assessment/CompanyScreening"/>
        <rdfs:range rdf:resource="http://www.w3.org/2001/XMLSchema#integer"/>
        <rdfs:comment xml:lang="en">Property used to specify the number of negative samples in company screenings</rdfs:comment>
        <rdfs:comment xml:lang="it">Proprietà usata per specificare il numero di campioni negativi negli screening aziendali</rdfs:comment>
        <rdfs:isDefinedBy rdf:resource="https://w3id.org/leo/onto/health-assessment"/>
        <rdfs:label xml:lang="en">number negative samples</rdfs:label>
        <rdfs:label xml:lang="it">numero campioni negativi</rdfs:label>
        <owl:versionInfo xml:lang="it">stabile</owl:versionInfo>
        <owl:versionInfo xml:lang="en">stable</owl:versionInfo>
    </owl:DatatypeProperty>



    <!-- https://w3id.org/leo/onto/health-assessment/numNotExaminedUnsuitableSamples -->

    <owl:DatatypeProperty rdf:about="https://w3id.org/leo/onto/health-assessment/numNotExaminedUnsuitableSamples">
        <rdfs:subPropertyOf rdf:resource="https://w3id.org/italia/onto/MU/value"/>
        <rdfs:domain rdf:resource="https://w3id.org/leo/onto/health-assessment/CompanyScreening"/>
        <rdfs:range rdf:resource="http://www.w3.org/2001/XMLSchema#integer"/>
        <rdfs:comment xml:lang="it">Il numero di campioni non esaminati o non idonei negli screening aziendali</rdfs:comment>
        <rdfs:comment xml:lang="en">The number of samples that are not examined in company screenings</rdfs:comment>
        <rdfs:isDefinedBy rdf:resource="https://w3id.org/leo/onto/health-assessment"/>
        <rdfs:label xml:lang="en">number not examined/unsuitable samples</rdfs:label>
        <rdfs:label xml:lang="it">numero campioni non esaminati/idonei</rdfs:label>
        <owl:versionInfo xml:lang="it">stabile</owl:versionInfo>
        <owl:versionInfo xml:lang="en">stable</owl:versionInfo>
    </owl:DatatypeProperty>



    <!-- https://w3id.org/leo/onto/health-assessment/numPositiveSamples -->

    <owl:DatatypeProperty rdf:about="https://w3id.org/leo/onto/health-assessment/numPositiveSamples">
        <rdfs:subPropertyOf rdf:resource="https://w3id.org/italia/onto/MU/value"/>
        <rdfs:domain rdf:resource="https://w3id.org/leo/onto/health-assessment/CompanyScreening"/>
        <rdfs:range rdf:resource="http://www.w3.org/2001/XMLSchema#integer"/>
        <rdfs:comment xml:lang="it">Il numero di campioni positivi negli screening aziendali</rdfs:comment>
        <rdfs:comment xml:lang="en">The number of positive samples in the compnay screenings.</rdfs:comment>
        <rdfs:isDefinedBy rdf:resource="https://w3id.org/leo/onto/health-assessment"/>
        <rdfs:label xml:lang="en">number positive samples</rdfs:label>
        <rdfs:label xml:lang="it">numero campioni positivi</rdfs:label>
        <owl:versionInfo xml:lang="it">stabile</owl:versionInfo>
        <owl:versionInfo xml:lang="en">stable</owl:versionInfo>
    </owl:DatatypeProperty>



    <!-- https://w3id.org/leo/onto/health-assessment/samplingAcceptingDate -->

    <owl:DatatypeProperty rdf:about="https://w3id.org/leo/onto/health-assessment/samplingAcceptingDate">
        <rdfs:subPropertyOf rdf:resource="https://w3id.org/italia/onto/TI/date"/>
        <rdfs:domain rdf:resource="https://w3id.org/leo/onto/health-assessment/DiagnosticHealthAssessment"/>
        <rdfs:range>
            <rdfs:Datatype>
                <owl:unionOf rdf:parseType="Collection">
                    <rdf:Description rdf:about="http://www.w3.org/2001/XMLSchema#date"/>
                    <rdf:Description rdf:about="http://www.w3.org/2001/XMLSchema#dateTime"/>
                </owl:unionOf>
            </rdfs:Datatype>
        </rdfs:range>
        <rdfs:comment xml:lang="it">La data di accettazione del campione in accertamento sanitario</rdfs:comment>
        <rdfs:comment xml:lang="en">The date of acceptance of the sample in a health assessment</rdfs:comment>
        <rdfs:isDefinedBy rdf:resource="https://w3id.org/leo/onto/health-assessment"/>
        <rdfs:label xml:lang="it">data accettazione campione</rdfs:label>
        <rdfs:label xml:lang="en">sampling accepting date</rdfs:label>
        <owl:versionInfo xml:lang="it">stabile</owl:versionInfo>
        <owl:versionInfo xml:lang="en">stable</owl:versionInfo>
    </owl:DatatypeProperty>



    <!-- https://w3id.org/leo/onto/health-assessment/samplingDate -->

    <owl:DatatypeProperty rdf:about="https://w3id.org/leo/onto/health-assessment/samplingDate">
        <rdfs:subPropertyOf rdf:resource="https://w3id.org/italia/onto/TI/date"/>
        <rdfs:domain rdf:resource="https://w3id.org/leo/onto/health-assessment/Sampling"/>
        <rdfs:range>
            <rdfs:Datatype>
                <owl:unionOf rdf:parseType="Collection">
                    <rdf:Description rdf:about="http://www.w3.org/2001/XMLSchema#date"/>
                    <rdf:Description rdf:about="http://www.w3.org/2001/XMLSchema#dateTime"/>
                </owl:unionOf>
            </rdfs:Datatype>
        </rdfs:range>
        <rdfs:comment xml:lang="it">La data in cui il campione è stato prelevato</rdfs:comment>
        <rdfs:comment xml:lang="en">The date on which the sample was taken</rdfs:comment>
        <rdfs:isDefinedBy rdf:resource="https://w3id.org/leo/onto/health-assessment"/>
        <rdfs:label xml:lang="it">data prelievo</rdfs:label>
        <rdfs:label xml:lang="en">sampling date</rdfs:label>
        <owl:versionInfo xml:lang="it">stabile</owl:versionInfo>
        <owl:versionInfo xml:lang="en">stable</owl:versionInfo>
    </owl:DatatypeProperty>



    <!-- https://w3id.org/leo/onto/health-assessment/testReportDate -->

    <owl:DatatypeProperty rdf:about="https://w3id.org/leo/onto/health-assessment/testReportDate">
        <rdfs:subPropertyOf rdf:resource="https://w3id.org/italia/onto/TI/date"/>
        <rdfs:domain rdf:resource="https://w3id.org/leo/onto/health-assessment/TestReport"/>
        <rdfs:range>
            <rdfs:Datatype>
                <owl:unionOf rdf:parseType="Collection">
                    <rdf:Description rdf:about="http://www.w3.org/2001/XMLSchema#date"/>
                    <rdf:Description rdf:about="http://www.w3.org/2001/XMLSchema#dateTime"/>
                </owl:unionOf>
            </rdfs:Datatype>
        </rdfs:range>
        <rdfs:comment xml:lang="it">La data associata al rapporto di prova</rdfs:comment>
        <rdfs:comment xml:lang="en">The date associated to the test report</rdfs:comment>
        <rdfs:isDefinedBy rdf:resource="https://w3id.org/leo/onto/health-assessment"/>
        <rdfs:label xml:lang="it">data rapporto di prova</rdfs:label>
        <rdfs:label xml:lang="en">test report date</rdfs:label>
        <owl:versionInfo xml:lang="it">stabile</owl:versionInfo>
        <owl:versionInfo xml:lang="en">stable</owl:versionInfo>
    </owl:DatatypeProperty>



    <!-- https://w3id.org/leo/onto/health-assessment/testReportNumber -->

    <owl:DatatypeProperty rdf:about="https://w3id.org/leo/onto/health-assessment/testReportNumber">
        <rdfs:subPropertyOf rdf:resource="https://w3id.org/italia/onto/l0/identifier"/>
        <rdfs:domain rdf:resource="https://w3id.org/leo/onto/health-assessment/TestReport"/>
        <rdfs:range rdf:resource="http://www.w3.org/2000/01/rdf-schema#Literal"/>
        <rdfs:comment xml:lang="it">L&apos;identificativo univoco, espresso come numbero, del rapporto di prova in un accertamento sanitario</rdfs:comment>
        <rdfs:comment xml:lang="en">The unique identifier of the test report</rdfs:comment>
        <rdfs:isDefinedBy rdf:resource="https://w3id.org/leo/onto/health-assessment"/>
        <rdfs:label xml:lang="it">numero rapporto di prova</rdfs:label>
        <rdfs:label xml:lang="en">test report number</rdfs:label>
        <owl:versionInfo xml:lang="it">stabile</owl:versionInfo>
        <owl:versionInfo xml:lang="en">stable</owl:versionInfo>
    </owl:DatatypeProperty>



    <!--
    ///////////////////////////////////////////////////////////////////////////////////////
    //
    // Classes
    //
    ///////////////////////////////////////////////////////////////////////////////////////
     -->




    <!-- https://w3id.org/italia/onto/ADMS/SemanticAsset -->

    <owl:Class rdf:about="https://w3id.org/italia/onto/ADMS/SemanticAsset"/>



    <!-- https://w3id.org/italia/onto/ADMS/SemanticAssetDistribution -->

    <owl:Class rdf:about="https://w3id.org/italia/onto/ADMS/SemanticAssetDistribution"/>



    <!-- https://w3id.org/italia/onto/COV/Organization -->

    <owl:Class rdf:about="https://w3id.org/italia/onto/COV/Organization"/>



    <!-- https://w3id.org/italia/onto/l0/EventOrSituation -->

    <owl:Class rdf:about="https://w3id.org/italia/onto/l0/EventOrSituation"/>



    <!-- https://w3id.org/leo/onto/analysis/BiologicalMaterial -->

    <owl:Class rdf:about="https://w3id.org/leo/onto/analysis/BiologicalMaterial"/>



    <!-- https://w3id.org/leo/onto/analysis/Sample -->

    <owl:Class rdf:about="https://w3id.org/leo/onto/analysis/Sample"/>



    <!-- https://w3id.org/leo/onto/analysis/UnitOfMeasure -->

    <owl:Class rdf:about="https://w3id.org/leo/onto/analysis/UnitOfMeasure"/>



    <!-- https://w3id.org/leo/onto/animal/FarmAnimal -->

    <owl:Class rdf:about="https://w3id.org/leo/onto/animal/FarmAnimal"/>



    <!-- https://w3id.org/leo/onto/animal/LivestockSpecies -->

    <owl:Class rdf:about="https://w3id.org/leo/onto/animal/LivestockSpecies"/>



    <!-- https://w3id.org/leo/onto/co/LivestockCompany -->

    <owl:Class rdf:about="https://w3id.org/leo/onto/co/LivestockCompany"/>



    <!-- https://w3id.org/leo/onto/health-assessment/CompanyScreening -->

    <owl:Class rdf:about="https://w3id.org/leo/onto/health-assessment/CompanyScreening">
        <rdfs:subClassOf rdf:resource="https://w3id.org/leo/onto/health-assessment/DiagnosticHealthAssessment"/>
        <rdfs:subClassOf>
            <owl:Restriction>
                <owl:onProperty rdf:resource="https://w3id.org/leo/onto/livestock-assessment/hasSubject"/>
                <owl:someValuesFrom rdf:resource="https://w3id.org/leo/onto/animal/LivestockSpecies"/>
            </owl:Restriction>
        </rdfs:subClassOf>
        <rdfs:subClassOf>
            <owl:Restriction>
                <owl:onProperty rdf:resource="https://w3id.org/leo/onto/health-assessment/numNegativeSamples"/>
                <owl:maxQualifiedCardinality rdf:datatype="http://www.w3.org/2001/XMLSchema#nonNegativeInteger">1</owl:maxQualifiedCardinality>
                <owl:onDataRange rdf:resource="http://www.w3.org/2001/XMLSchema#integer"/>
            </owl:Restriction>
        </rdfs:subClassOf>
        <rdfs:subClassOf>
            <owl:Restriction>
                <owl:onProperty rdf:resource="https://w3id.org/leo/onto/health-assessment/numNotExaminedUnsuitableSamples"/>
                <owl:maxQualifiedCardinality rdf:datatype="http://www.w3.org/2001/XMLSchema#nonNegativeInteger">1</owl:maxQualifiedCardinality>
                <owl:onDataRange rdf:resource="http://www.w3.org/2001/XMLSchema#integer"/>
            </owl:Restriction>
        </rdfs:subClassOf>
        <rdfs:subClassOf>
            <owl:Restriction>
                <owl:onProperty rdf:resource="https://w3id.org/leo/onto/health-assessment/numPositiveSamples"/>
                <owl:maxQualifiedCardinality rdf:datatype="http://www.w3.org/2001/XMLSchema#nonNegativeInteger">1</owl:maxQualifiedCardinality>
                <owl:onDataRange rdf:resource="http://www.w3.org/2001/XMLSchema#integer"/>
            </owl:Restriction>
        </rdfs:subClassOf>
        <owl:disjointWith rdf:resource="https://w3id.org/leo/onto/health-assessment/SingleAnimalHealthAssessment"/>
        <rdfs:comment xml:lang="en">Company Screenings are diagnostic health checks that refer to a set of animals and therefore offer the summary result.</rdfs:comment>
        <rdfs:comment xml:lang="it">Gli Screening Aziendali sono degli accertamenti sanitari diagnostici che fanno riferimento ad un insieme di animali e pertanto offrono il risultato di sintesi.</rdfs:comment>
        <rdfs:isDefinedBy rdf:resource="https://w3id.org/leo/onto/health-assessment"/>
        <rdfs:label xml:lang="en">Company Screening</rdfs:label>
        <rdfs:label xml:lang="it">Screening Aziendale</rdfs:label>
        <owl:versionInfo xml:lang="it">stabile</owl:versionInfo>
        <owl:versionInfo xml:lang="en">stable</owl:versionInfo>
    </owl:Class>



    <!-- https://w3id.org/leo/onto/health-assessment/DiagnosticHealthAssessment -->

    <owl:Class rdf:about="https://w3id.org/leo/onto/health-assessment/DiagnosticHealthAssessment">
        <rdfs:subClassOf rdf:resource="https://w3id.org/leo/onto/livestock-assessment/LivestockAssessment"/>
        <rdfs:subClassOf>
            <owl:Restriction>
                <owl:onProperty rdf:resource="https://w3id.org/leo/onto/livestock-assessment/hasPerformer"/>
                <owl:someValuesFrom rdf:resource="https://w3id.org/leo/onto/health-assessment/ZooprophylacticLab"/>
            </owl:Restriction>
        </rdfs:subClassOf>
        <rdfs:subClassOf>
            <owl:Restriction>
                <owl:onProperty rdf:resource="https://w3id.org/leo/onto/livestock-assessment/isAssessmentOf"/>
                <owl:someValuesFrom rdf:resource="https://w3id.org/leo/onto/co/LivestockCompany"/>
            </owl:Restriction>
        </rdfs:subClassOf>
        <rdfs:subClassOf>
            <owl:Restriction>
                <owl:onProperty rdf:resource="https://w3id.org/leo/onto/health-assessment/hasAnalysedDisease"/>
                <owl:allValuesFrom rdf:resource="https://w3id.org/leo/onto/health-assessment/Disease"/>
            </owl:Restriction>
        </rdfs:subClassOf>
        <rdfs:subClassOf>
            <owl:Restriction>
                <owl:onProperty rdf:resource="https://w3id.org/leo/onto/health-assessment/hasExaminedMaterial"/>
                <owl:allValuesFrom rdf:resource="https://w3id.org/leo/onto/analysis/BiologicalMaterial"/>
            </owl:Restriction>
        </rdfs:subClassOf>
        <rdfs:subClassOf>
            <owl:Restriction>
                <owl:onProperty rdf:resource="https://w3id.org/leo/onto/health-assessment/hasSampleJudgement"/>
                <owl:allValuesFrom rdf:resource="https://w3id.org/leo/onto/health-assessment/SampleJudgement"/>
            </owl:Restriction>
        </rdfs:subClassOf>
        <rdfs:subClassOf>
            <owl:Restriction>
                <owl:onProperty rdf:resource="https://w3id.org/leo/onto/health-assessment/hasUsedAnalyticalTechnique"/>
                <owl:allValuesFrom rdf:resource="https://w3id.org/leo/onto/health-assessment/Technique"/>
            </owl:Restriction>
        </rdfs:subClassOf>
        <rdfs:subClassOf>
            <owl:Restriction>
                <owl:onProperty rdf:resource="https://w3id.org/leo/onto/health-assessment/isReferredToSampling"/>
                <owl:allValuesFrom rdf:resource="https://w3id.org/leo/onto/health-assessment/Sampling"/>
            </owl:Restriction>
        </rdfs:subClassOf>
        <rdfs:subClassOf>
            <owl:Restriction>
                <owl:onProperty rdf:resource="https://w3id.org/leo/onto/health-assessment/doneForSample"/>
                <owl:maxQualifiedCardinality rdf:datatype="http://www.w3.org/2001/XMLSchema#nonNegativeInteger">1</owl:maxQualifiedCardinality>
                <owl:onClass rdf:resource="https://w3id.org/leo/onto/analysis/Sample"/>
            </owl:Restriction>
        </rdfs:subClassOf>
        <rdfs:subClassOf>
            <owl:Restriction>
                <owl:onProperty rdf:resource="https://w3id.org/leo/onto/health-assessment/hasReplacedTestReport"/>
                <owl:maxQualifiedCardinality rdf:datatype="http://www.w3.org/2001/XMLSchema#nonNegativeInteger">1</owl:maxQualifiedCardinality>
                <owl:onClass rdf:resource="https://w3id.org/leo/onto/health-assessment/TestReport"/>
            </owl:Restriction>
        </rdfs:subClassOf>
        <rdfs:subClassOf>
            <owl:Restriction>
                <owl:onProperty rdf:resource="https://w3id.org/leo/onto/health-assessment/hasSampleAcceptor"/>
                <owl:maxQualifiedCardinality rdf:datatype="http://www.w3.org/2001/XMLSchema#nonNegativeInteger">1</owl:maxQualifiedCardinality>
                <owl:onClass rdf:resource="https://w3id.org/leo/onto/health-assessment/ZooprophylacticLab"/>
            </owl:Restriction>
        </rdfs:subClassOf>
        <rdfs:subClassOf>
            <owl:Restriction>
                <owl:onProperty rdf:resource="https://w3id.org/leo/onto/health-assessment/hasTestReport"/>
                <owl:maxQualifiedCardinality rdf:datatype="http://www.w3.org/2001/XMLSchema#nonNegativeInteger">1</owl:maxQualifiedCardinality>
                <owl:onClass rdf:resource="https://w3id.org/leo/onto/health-assessment/TestReport"/>
            </owl:Restriction>
        </rdfs:subClassOf>
        <rdfs:subClassOf>
            <owl:Restriction>
                <owl:onProperty rdf:resource="https://w3id.org/leo/onto/health-assessment/note"/>
                <owl:allValuesFrom rdf:resource="http://www.w3.org/1999/02/22-rdf-syntax-ns#PlainLiteral"/>
            </owl:Restriction>
        </rdfs:subClassOf>
        <rdfs:subClassOf>
            <owl:Restriction>
                <owl:onProperty rdf:resource="https://w3id.org/leo/onto/health-assessment/samplingAcceptingDate"/>
                <owl:maxQualifiedCardinality rdf:datatype="http://www.w3.org/2001/XMLSchema#nonNegativeInteger">1</owl:maxQualifiedCardinality>
                <owl:onDataRange>
                    <rdfs:Datatype>
                        <owl:unionOf rdf:parseType="Collection">
                            <rdf:Description rdf:about="http://www.w3.org/2001/XMLSchema#date"/>
                            <rdf:Description rdf:about="http://www.w3.org/2001/XMLSchema#dateTime"/>
                        </owl:unionOf>
                    </rdfs:Datatype>
                </owl:onDataRange>
            </owl:Restriction>
        </rdfs:subClassOf>
        <rdfs:comment xml:lang="it">La classe degli accertamenti diagnostici di patologie di interesse zootecnico</rdfs:comment>
        <rdfs:comment xml:lang="en">The class of diagnostic assessments for diseases of zootechnical interest</rdfs:comment>
        <rdfs:isDefinedBy rdf:resource="https://w3id.org/leo/onto/health-assessment"/>
        <rdfs:label xml:lang="it">Accertamento Sanitario Diagnostico</rdfs:label>
        <rdfs:label xml:lang="en">Diagnostic Health Assessment</rdfs:label>
        <owl:versionInfo xml:lang="it">stabile</owl:versionInfo>
        <owl:versionInfo xml:lang="en">stable</owl:versionInfo>
    </owl:Class>



    <!-- https://w3id.org/leo/onto/health-assessment/Disease -->

    <owl:Class rdf:about="https://w3id.org/leo/onto/health-assessment/Disease">
        <rdfs:subClassOf rdf:resource="https://w3id.org/italia/onto/l0/Concept"/>
        <rdfs:subClassOf>
            <owl:Restriction>
                <owl:onProperty rdf:resource="https://w3id.org/italia/onto/l0/name"/>
                <owl:someValuesFrom rdf:resource="http://www.w3.org/2000/01/rdf-schema#Literal"/>
            </owl:Restriction>
        </rdfs:subClassOf>
        <rdfs:subClassOf>
            <owl:Restriction>
                <owl:onProperty rdf:resource="https://w3id.org/italia/onto/l0/identifier"/>
                <owl:cardinality rdf:datatype="http://www.w3.org/2001/XMLSchema#nonNegativeInteger">1</owl:cardinality>
            </owl:Restriction>
        </rdfs:subClassOf>
        <rdfs:comment xml:lang="it">La classe delle malattie analizzate nell&apos;accertamento sanitario. Le malattie sono identificate da un codice (codice SIMAN).</rdfs:comment>
        <rdfs:comment xml:lang="en">The class of diseases analysed in the health assessment. Diseases are identified by a code (SIMAN code).</rdfs:comment>
        <rdfs:isDefinedBy rdf:resource="https://w3id.org/leo/onto/health-assessment"/>
        <rdfs:label xml:lang="en">Disease</rdfs:label>
        <rdfs:label xml:lang="it">Malattia</rdfs:label>
        <owl:versionInfo xml:lang="it">stabile</owl:versionInfo>
        <owl:versionInfo xml:lang="en">stable</owl:versionInfo>
    </owl:Class>



    <!-- https://w3id.org/leo/onto/health-assessment/QualitativeResult -->

    <owl:Class rdf:about="https://w3id.org/leo/onto/health-assessment/QualitativeResult">
        <rdfs:subClassOf rdf:resource="https://w3id.org/leo/onto/livestock-assessment/AssessmentResult"/>
        <rdfs:subClassOf>
            <owl:Restriction>
                <owl:onProperty rdf:resource="https://w3id.org/italia/onto/MU/value"/>
                <owl:cardinality rdf:datatype="http://www.w3.org/2001/XMLSchema#nonNegativeInteger">1</owl:cardinality>
            </owl:Restriction>
        </rdfs:subClassOf>
        <owl:disjointWith rdf:resource="https://w3id.org/leo/onto/health-assessment/QuantitativeResult"/>
        <rdfs:comment xml:lang="it">La classe degli esiti degli accertamenti di tipo qualitativo (e.g., positivo, negativo).</rdfs:comment>
        <rdfs:comment xml:lang="en">The class of qualitative results of the health assessments (e.g. positive, negative).</rdfs:comment>
        <rdfs:isDefinedBy rdf:resource="https://w3id.org/leo/onto/health-assessment"/>
        <rdfs:label xml:lang="en">Qualitative Result</rdfs:label>
        <rdfs:label xml:lang="it">Risultato Qualitativo</rdfs:label>
        <owl:versionInfo xml:lang="it">stabile</owl:versionInfo>
        <owl:versionInfo xml:lang="en">stable</owl:versionInfo>
    </owl:Class>



    <!-- https://w3id.org/leo/onto/health-assessment/QuantitativeResult -->

    <owl:Class rdf:about="https://w3id.org/leo/onto/health-assessment/QuantitativeResult">
        <rdfs:subClassOf rdf:resource="https://w3id.org/italia/onto/MU/Value"/>
        <rdfs:subClassOf rdf:resource="https://w3id.org/leo/onto/livestock-assessment/AssessmentResult"/>
        <rdfs:subClassOf>
            <owl:Restriction>
                <owl:onProperty rdf:resource="https://w3id.org/leo/onto/analysis/hasUnitOfMeasure"/>
                <owl:qualifiedCardinality rdf:datatype="http://www.w3.org/2001/XMLSchema#nonNegativeInteger">1</owl:qualifiedCardinality>
                <owl:onClass rdf:resource="https://w3id.org/leo/onto/analysis/UnitOfMeasure"/>
            </owl:Restriction>
        </rdfs:subClassOf>
        <rdfs:comment xml:lang="it">La classe degli esiti quantitativi, ossia risultati di tipo numerico, associati a un&apos;unità di misura</rdfs:comment>
        <rdfs:comment xml:lang="en">The class of quantitative outcomes, i.e. results of a numerical type, associated with a unit of measurement</rdfs:comment>
        <rdfs:isDefinedBy rdf:resource="https://w3id.org/leo/onto/health-assessment"/>
        <rdfs:label xml:lang="it">Esito Quantitativo</rdfs:label>
        <rdfs:label xml:lang="en">Quantitative Result</rdfs:label>
        <owl:versionInfo xml:lang="it">stabile</owl:versionInfo>
        <owl:versionInfo xml:lang="en">stable</owl:versionInfo>
    </owl:Class>



    <!-- https://w3id.org/leo/onto/health-assessment/Reason -->

    <owl:Class rdf:about="https://w3id.org/leo/onto/health-assessment/Reason">
        <rdfs:subClassOf rdf:resource="https://w3id.org/italia/onto/l0/Characteristic"/>
        <rdfs:subClassOf rdf:resource="https://w3id.org/italia/onto/l0/Concept"/>
        <rdfs:subClassOf>
            <owl:Restriction>
                <owl:onProperty rdf:resource="https://w3id.org/italia/onto/l0/name"/>
                <owl:someValuesFrom rdf:resource="http://www.w3.org/2000/01/rdf-schema#Literal"/>
            </owl:Restriction>
        </rdfs:subClassOf>
        <rdfs:subClassOf>
            <owl:Restriction>
                <owl:onProperty rdf:resource="https://w3id.org/italia/onto/l0/identifier"/>
                <owl:cardinality rdf:datatype="http://www.w3.org/2001/XMLSchema#nonNegativeInteger">1</owl:cardinality>
            </owl:Restriction>
        </rdfs:subClassOf>
        <rdfs:comment xml:lang="it">La classe di tutte le motivazioni per l&apos;esecuzione di un prelievo riferito agli accertamenti sanitari.</rdfs:comment>
        <rdfs:comment xml:lang="en">The class of all the motivations for carrying out a sampling referred in health assessments.</rdfs:comment>
        <rdfs:isDefinedBy rdf:resource="https://w3id.org/leo/onto/health-assessment"/>
        <rdfs:label xml:lang="it">Motivo del Prelievo</rdfs:label>
        <rdfs:label xml:lang="en">Reason (of the Sampling)</rdfs:label>
        <owl:versionInfo xml:lang="it">stabile</owl:versionInfo>
        <owl:versionInfo xml:lang="en">stable</owl:versionInfo>
    </owl:Class>



    <!-- https://w3id.org/leo/onto/health-assessment/SampleJudgement -->

    <owl:Class rdf:about="https://w3id.org/leo/onto/health-assessment/SampleJudgement">
        <rdfs:subClassOf rdf:resource="https://w3id.org/italia/onto/l0/Description"/>
        <rdfs:comment xml:lang="it">Indica il giudizio relativo al campione. i valori possibili sono negativo, positivo, non esaminato, non idoneo, dubbio</rdfs:comment>
        <rdfs:comment xml:lang="en">Indicates the rating for the sample. possible values are negative, positive, not examined, unsuitable, doubtful</rdfs:comment>
        <rdfs:isDefinedBy rdf:resource="https://w3id.org/leo/onto/health-assessment"/>
        <rdfs:label xml:lang="it">Giudizio Campione</rdfs:label>
        <rdfs:label xml:lang="en">Sample Judgement</rdfs:label>
        <owl:versionInfo xml:lang="it">stabile</owl:versionInfo>
        <owl:versionInfo xml:lang="en">stable</owl:versionInfo>
    </owl:Class>



    <!-- https://w3id.org/leo/onto/health-assessment/Sampling -->

    <owl:Class rdf:about="https://w3id.org/leo/onto/health-assessment/Sampling">
        <rdfs:subClassOf rdf:resource="https://w3id.org/italia/onto/l0/Activity"/>
        <rdfs:subClassOf>
            <owl:Restriction>
                <owl:onProperty rdf:resource="https://w3id.org/leo/onto/health-assessment/hasReason"/>
                <owl:allValuesFrom rdf:resource="https://w3id.org/leo/onto/health-assessment/Reason"/>
            </owl:Restriction>
        </rdfs:subClassOf>
        <rdfs:subClassOf>
            <owl:Restriction>
                <owl:onProperty rdf:resource="https://w3id.org/leo/onto/health-assessment/resultingInSample"/>
                <owl:maxQualifiedCardinality rdf:datatype="http://www.w3.org/2001/XMLSchema#nonNegativeInteger">1</owl:maxQualifiedCardinality>
                <owl:onClass rdf:resource="https://w3id.org/leo/onto/analysis/Sample"/>
            </owl:Restriction>
        </rdfs:subClassOf>
        <rdfs:subClassOf>
            <owl:Restriction>
                <owl:onProperty rdf:resource="https://w3id.org/leo/onto/health-assessment/samplingDate"/>
                <owl:maxQualifiedCardinality rdf:datatype="http://www.w3.org/2001/XMLSchema#nonNegativeInteger">1</owl:maxQualifiedCardinality>
                <owl:onDataRange>
                    <rdfs:Datatype>
                        <owl:unionOf rdf:parseType="Collection">
                            <rdf:Description rdf:about="http://www.w3.org/2001/XMLSchema#date"/>
                            <rdf:Description rdf:about="http://www.w3.org/2001/XMLSchema#dateTime"/>
                        </owl:unionOf>
                    </rdfs:Datatype>
                </owl:onDataRange>
            </owl:Restriction>
        </rdfs:subClassOf>
        <rdfs:comment xml:lang="it">L&apos;attività di prelievo necessaria per lo svolgimento di accertamenti sanitari</rdfs:comment>
        <rdfs:comment xml:lang="en">The activity of sampling referred to some health assessment</rdfs:comment>
        <rdfs:isDefinedBy rdf:resource="https://w3id.org/leo/onto/health-assessment"/>
        <rdfs:label xml:lang="it">Prelievo</rdfs:label>
        <rdfs:label xml:lang="en">Sampling</rdfs:label>
        <owl:versionInfo xml:lang="it">stabile</owl:versionInfo>
        <owl:versionInfo xml:lang="en">stable</owl:versionInfo>
        <prov:wasDerivedFrom rdf:resource="http://www.w3.org/ns/sosa/Sampling"/>
    </owl:Class>



    <!-- https://w3id.org/leo/onto/health-assessment/SingleAnimalHealthAssessment -->

    <owl:Class rdf:about="https://w3id.org/leo/onto/health-assessment/SingleAnimalHealthAssessment">
        <rdfs:subClassOf rdf:resource="https://w3id.org/leo/onto/health-assessment/DiagnosticHealthAssessment"/>
        <rdfs:subClassOf>
            <owl:Restriction>
                <owl:onProperty rdf:resource="https://w3id.org/leo/onto/livestock-assessment/hasSubject"/>
                <owl:someValuesFrom rdf:resource="https://w3id.org/leo/onto/animal/FarmAnimal"/>
            </owl:Restriction>
        </rdfs:subClassOf>
        <rdfs:comment xml:lang="it">La classe degli accertamenti sanitari diagnostici effettuati su singoli animali.</rdfs:comment>
        <rdfs:comment xml:lang="en">The class of all the diagnostic health assessments done on single farm animals</rdfs:comment>
        <rdfs:isDefinedBy rdf:resource="https://w3id.org/leo/onto/health-assessment"/>
        <rdfs:label xml:lang="it">Accertamento Sanitario su Singolo Animale</rdfs:label>
        <rdfs:label xml:lang="en">Single Animal Health Assessment</rdfs:label>
        <owl:versionInfo xml:lang="it">stabile</owl:versionInfo>
        <owl:versionInfo xml:lang="en">stable</owl:versionInfo>
    </owl:Class>



    <!-- https://w3id.org/leo/onto/health-assessment/Technique -->

    <owl:Class rdf:about="https://w3id.org/leo/onto/health-assessment/Technique">
        <rdfs:subClassOf rdf:resource="https://w3id.org/leo/onto/livestock-assessment/Method"/>
        <rdfs:subClassOf>
            <owl:Restriction>
                <owl:onProperty rdf:resource="https://w3id.org/italia/onto/l0/name"/>
                <owl:someValuesFrom rdf:resource="http://www.w3.org/2000/01/rdf-schema#Literal"/>
            </owl:Restriction>
        </rdfs:subClassOf>
        <rdfs:subClassOf>
            <owl:Restriction>
                <owl:onProperty rdf:resource="https://w3id.org/leo/onto/health-assessment/efsaCode"/>
                <owl:cardinality rdf:datatype="http://www.w3.org/2001/XMLSchema#nonNegativeInteger">1</owl:cardinality>
            </owl:Restriction>
        </rdfs:subClassOf>
        <rdfs:comment xml:lang="it">La classe delle tecniche analitiche utilizzate per l&apos;accertamento sanitario. La tecnica usata è identificata da un codice (Codici EFSA)</rdfs:comment>
        <rdfs:comment xml:lang="en">The class of analytical techniques used for health assessments. The technique used is identified by a code (EFSA Codes)</rdfs:comment>
        <rdfs:isDefinedBy rdf:resource="https://w3id.org/leo/onto/health-assessment"/>
        <rdfs:label xml:lang="en">Technique</rdfs:label>
        <rdfs:label xml:lang="it">Tecnica</rdfs:label>
        <owl:versionInfo xml:lang="it">stabile</owl:versionInfo>
        <owl:versionInfo xml:lang="en">stable</owl:versionInfo>
    </owl:Class>



    <!-- https://w3id.org/leo/onto/health-assessment/TestReport -->

    <owl:Class rdf:about="https://w3id.org/leo/onto/health-assessment/TestReport">
        <rdfs:subClassOf rdf:resource="https://w3id.org/italia/onto/l0/Object"/>
        <rdfs:subClassOf>
            <owl:Restriction>
                <owl:onProperty rdf:resource="https://w3id.org/leo/onto/health-assessment/replaced"/>
                <owl:allValuesFrom rdf:resource="https://w3id.org/leo/onto/health-assessment/TestReport"/>
            </owl:Restriction>
        </rdfs:subClassOf>
        <rdfs:subClassOf>
            <owl:Restriction>
                <owl:onProperty rdf:resource="https://w3id.org/leo/onto/health-assessment/testReportNumber"/>
                <owl:cardinality rdf:datatype="http://www.w3.org/2001/XMLSchema#nonNegativeInteger">1</owl:cardinality>
            </owl:Restriction>
        </rdfs:subClassOf>
        <rdfs:subClassOf>
            <owl:Restriction>
                <owl:onProperty rdf:resource="https://w3id.org/leo/onto/health-assessment/testReportDate"/>
                <owl:maxQualifiedCardinality rdf:datatype="http://www.w3.org/2001/XMLSchema#nonNegativeInteger">1</owl:maxQualifiedCardinality>
                <owl:onDataRange>
                    <rdfs:Datatype>
                        <owl:unionOf rdf:parseType="Collection">
                            <rdf:Description rdf:about="http://www.w3.org/2001/XMLSchema#date"/>
                            <rdf:Description rdf:about="http://www.w3.org/2001/XMLSchema#dateTime"/>
                        </owl:unionOf>
                    </rdfs:Datatype>
                </owl:onDataRange>
            </owl:Restriction>
        </rdfs:subClassOf>
        <rdfs:comment xml:lang="it">La classe di tutti i rapporti di prova che sono documenti, in formato digitale o cartaceo, che sono redatti dagli istituti zooprofilattici a conclusione del percorso diagnostico. Questi rapporti di prova possono essere poi mandati a destinatari quali il Ministero della Salute e il Servizio Veterinario Regionale.</rdfs:comment>
        <rdfs:comment xml:lang="en">The class of all test reports, which are documents, in digital or paper format, that are drawn up by zooprophylactic institutes at the end of the diagnostic process. These test reports can then be sent to recipients such as the Ministry of Health and the Regional Veterinary Service.</rdfs:comment>
        <rdfs:isDefinedBy rdf:resource="https://w3id.org/leo/onto/health-assessment"/>
        <rdfs:label xml:lang="it">Rapporto di Prova</rdfs:label>
        <rdfs:label xml:lang="en">Test Report</rdfs:label>
        <owl:versionInfo xml:lang="it">stabile</owl:versionInfo>
        <owl:versionInfo xml:lang="en">stable</owl:versionInfo>
    </owl:Class>



    <!-- https://w3id.org/leo/onto/health-assessment/ZooprophylacticLab -->

    <owl:Class rdf:about="https://w3id.org/leo/onto/health-assessment/ZooprophylacticLab">
        <rdfs:subClassOf rdf:resource="https://w3id.org/italia/onto/COV/Organization"/>
        <rdfs:subClassOf>
            <owl:Restriction>
                <owl:onProperty rdf:resource="https://w3id.org/italia/onto/l0/name"/>
                <owl:someValuesFrom rdf:resource="http://www.w3.org/2000/01/rdf-schema#Literal"/>
            </owl:Restriction>
        </rdfs:subClassOf>
        <rdfs:subClassOf>
            <owl:Restriction>
                <owl:onProperty rdf:resource="https://w3id.org/leo/onto/health-assessment/efsaCode"/>
                <owl:cardinality rdf:datatype="http://www.w3.org/2001/XMLSchema#nonNegativeInteger">1</owl:cardinality>
            </owl:Restriction>
        </rdfs:subClassOf>
        <rdfs:comment xml:lang="en">A public law health body with management and administrative autonomy, forming part of the Italian National Health Service, as a technical and operational tool for animal health.</rdfs:comment>
        <rdfs:comment xml:lang="it">Un ente sanitario di diritto pubblico con autonomia gestionale ed amministrativa, facente parte del Servizio sanitario nazionale,  quale strumento tecnico ed operativo per la sanità animale.</rdfs:comment>
        <rdfs:isDefinedBy rdf:resource="https://w3id.org/leo/onto/health-assessment"/>
        <rdfs:label xml:lang="it">Laboratorio Zooprofilattico</rdfs:label>
        <rdfs:label xml:lang="en">Zooprophylactics Laboratory</rdfs:label>
        <owl:versionInfo xml:lang="it">stabile</owl:versionInfo>
        <owl:versionInfo xml:lang="en">stable</owl:versionInfo>
    </owl:Class>



    <!--
    ///////////////////////////////////////////////////////////////////////////////////////
    //
    // Individuals
    //
    ///////////////////////////////////////////////////////////////////////////////////////
     -->




    <!-- https://w3id.org/leo/data/distribution/HA-JSON-LD -->

    <owl:NamedIndividual rdf:about="https://w3id.org/leo/data/distribution/HA-JSON-LD">
        <rdf:type rdf:resource="https://w3id.org/italia/onto/ADMS/SemanticAssetDistribution"/>
        <terms:description xml:lang="it">Questa è la distribuzione JSON-LD dell&apos;ontologia sugli accertamenti sanitari</terms:description>
        <terms:description xml:lang="en">This is the distribution in JSON-LD of health assessments ontology</terms:description>
        <terms:format rdf:resource="http://publications.europa.eu/resource/authority/file-type/JSON_LD"/>
        <terms:license rdf:resource="https://w3id.org/italia/controlled-vocabulary/licences/A21_CCBY40"/>
        <terms:title xml:lang="it">Distribuzione JSON-LD ontologia Accertamenti Sanitari</terms:title>
        <terms:title xml:lang="en">JSON-LD distribution of Health Assessment Ontology</terms:title>
        <rdfs:comment xml:lang="it">Questa è la distribuzione JSON-LD dell&apos;ontologia sugli accertamenti sanitarli</rdfs:comment>
        <rdfs:comment xml:lang="en">This is the distribution in JSON-LD of health assessments ontology</rdfs:comment>
        <rdfs:label xml:lang="it">Distribuzione JSON-LD ontologia Accertamenti Sanitari</rdfs:label>
        <rdfs:label xml:lang="en">JSON-LD distribution of Health Assessment Ontology</rdfs:label>
        <dcat:accessURL rdf:resource="https://github.com/Bluarancio/Leo-OpenData/tree/master/Ontologie/health-assessment/latest"/>
        <dcat:downloadURL rdf:resource="https://raw.githubusercontent.com/Bluarancio/Leo-OpenData/master/Ontologie/health-assessment/latest/health-assessment.jsonld"/>
    </owl:NamedIndividual>



    <!-- https://w3id.org/leo/data/distribution/HA-RDF-TURTLE -->

    <owl:NamedIndividual rdf:about="https://w3id.org/leo/data/distribution/HA-RDF-TURTLE">
        <rdf:type rdf:resource="https://w3id.org/italia/onto/ADMS/SemanticAssetDistribution"/>
        <terms:description xml:lang="it">Questa è la distribuzione RDF/Turtle dell&apos;ontologia sugli accertamenti sanitari</terms:description>
        <terms:description xml:lang="en">This is the distribution in RDF/Turtle of health assessments ontology</terms:description>
        <terms:format rdf:resource="http://publications.europa.eu/resource/authority/file-type/RDF_TURTLE"/>
        <terms:license rdf:resource="https://w3id.org/italia/controlled-vocabulary/licences/A21_CCBY40"/>
        <terms:title xml:lang="it">Distribuzione RDF/Turtle ontologia Accertamenti Sanitari</terms:title>
        <terms:title xml:lang="en">RDF/Turtle distribution of Health Assessment Ontology</terms:title>
        <rdfs:comment xml:lang="it">Questa è la distribuzione RDF/Turtle dell&apos;ontologia sugli accertamenti sanitari</rdfs:comment>
        <rdfs:comment xml:lang="en">This is the distribution in RDF/Turtle of health assessments ontology</rdfs:comment>
        <rdfs:label xml:lang="it">Distribuzione RDF/Turtle ontologia Accertamenti Sanitari</rdfs:label>
        <rdfs:label xml:lang="en">RDF/Turtle distribution of Health Assessment Ontology</rdfs:label>
        <dcat:accessURL rdf:resource="https://github.com/Bluarancio/Leo-OpenData/tree/master/Ontologie/health-assessment/latest"/>
        <dcat:downloadURL rdf:resource="https://raw.githubusercontent.com/Bluarancio/Leo-OpenData/master/Ontologie/health-assessment/latest/health-assessment.ttl"/>
    </owl:NamedIndividual>



    <!-- https://w3id.org/leo/data/distribution/HA-RDF-XML -->

    <owl:NamedIndividual rdf:about="https://w3id.org/leo/data/distribution/HA-RDF-XML">
        <rdf:type rdf:resource="https://w3id.org/italia/onto/ADMS/SemanticAssetDistribution"/>
        <terms:description xml:lang="it">Questa è la distribuzione RDF/XML dell&apos;ontologia sugli accertamenti sanitari</terms:description>
        <terms:description xml:lang="en">This is the distribution in RDF/XML of health assessments ontology</terms:description>
        <terms:format rdf:resource="http://publications.europa.eu/resource/authority/file-type/RDF_XML"/>
        <terms:license rdf:resource="https://w3id.org/italia/controlled-vocabulary/licences/A21_CCBY40"/>
        <terms:title xml:lang="it">Distribuzione RDF/XML ontologia Accertamenti Sanitari</terms:title>
        <terms:title xml:lang="en">RDF/XML distribution of Health Assessment Ontology</terms:title>
        <rdfs:comment xml:lang="it">Questa è la distribuzione RDF/XML dell&apos;ontologia sugli accertamenti sanitari</rdfs:comment>
        <rdfs:comment xml:lang="en">This is the distribution in RDF/XML of health assessments ontology</rdfs:comment>
        <rdfs:label xml:lang="it">Distribuzione RDF/XML ontologia Accertamenti Sanitari</rdfs:label>
        <rdfs:label xml:lang="en">RDF/XML distribution of Health Assessment Ontology</rdfs:label>
        <dcat:accessURL rdf:resource="https://github.com/Bluarancio/Leo-OpenData/tree/master/Ontologie/health-assessment/latest"/>
        <dcat:downloadURL rdf:resource="https://raw.githubusercontent.com/Bluarancio/Leo-OpenData/master/Ontologie/health-assessment/latest/health-assessment.rdf"/>
    </owl:NamedIndividual>


      <!-- https://w3id.org/leo/data/private-organization/00944701002 -->

      <owl:NamedIndividual rdf:about="https://w3id.org/leo/data/private-organization/00944701002">
          <rdf:type rdf:resource="http://dati.gov.it/onto/dcatapit#Agent"/>
          <rdf:type rdf:resource="http://xmlns.com/foaf/0.1/Agent"/>
          <terms:identifier>00944701002</terms:identifier>
          <foaf:name xml:lang="it">Associazione Italiana Allevatori</foaf:name>
          <foaf:name xml:lang="en">Italian Breeders&apos; Association</foaf:name>
      </owl:NamedIndividual>



      <!-- https://w3id.org/leo/data/private-organization/06695411006 -->

      <owl:NamedIndividual rdf:about="https://w3id.org/leo/data/private-organization/06695411006">
          <rdf:type rdf:resource="http://dati.gov.it/onto/dcatapit#Agent"/>
          <rdf:type rdf:resource="http://xmlns.com/foaf/0.1/Agent"/>
          <terms:identifier>06695411006</terms:identifier>
          <foaf:name xml:lang="en">Bluarancio</foaf:name>
          <foaf:name xml:lang="it">Bluarancio</foaf:name>
      </owl:NamedIndividual>



      <!-- https://w3id.org/leo/data/project/LEO -->

      <owl:NamedIndividual rdf:about="https://w3id.org/leo/data/project/LEO">
          <rdf:type rdf:resource="https://w3id.org/italia/onto/ADMS/Project"/>
          <rdfs:comment xml:lang="it">Il progetto LEO dove viene usata l&apos;ontologia</rdfs:comment>
          <rdfs:comment xml:lang="en">LEO project where the ontology is used</rdfs:comment>
          <rdfs:label xml:lang="en">LEO - Livestok Environment Open Data</rdfs:label>
          <rdfs:label xml:lang="it">LEO - Livestok Environment Open Data</rdfs:label>
          <l0:name xml:lang="it">LEO - Livestok Environment Open Data</l0:name>
      </owl:NamedIndividual>



    <!-- https://w3id.org/leo/onto/health-assessment -->

    <owl:NamedIndividual rdf:about="https://w3id.org/leo/onto/health-assessment">
        <rdf:type rdf:resource="https://w3id.org/italia/onto/ADMS/SemanticAsset"/>
    </owl:NamedIndividual>



    <!-- https://w3id.org/leo/onto/health-assessment/Doubtful -->

    <owl:NamedIndividual rdf:about="https://w3id.org/leo/onto/health-assessment/Doubtful">
        <rdf:type rdf:resource="https://w3id.org/leo/onto/health-assessment/SampleJudgement"/>
        <rdfs:isDefinedBy rdf:resource="https://w3id.org/leo/onto/health-assessment"/>
        <rdfs:label xml:lang="en">Doubtful</rdfs:label>
        <rdfs:label xml:lang="it">Dubbio</rdfs:label>
        <owl:versionInfo xml:lang="it">stabile</owl:versionInfo>
        <owl:versionInfo xml:lang="en">stable</owl:versionInfo>
    </owl:NamedIndividual>



    <!-- https://w3id.org/leo/onto/health-assessment/Negative -->

    <owl:NamedIndividual rdf:about="https://w3id.org/leo/onto/health-assessment/Negative">
        <rdf:type rdf:resource="https://w3id.org/leo/onto/health-assessment/SampleJudgement"/>
        <rdfs:isDefinedBy rdf:resource="https://w3id.org/leo/onto/health-assessment"/>
        <rdfs:label xml:lang="en">Negative</rdfs:label>
        <rdfs:label xml:lang="it">Negativo</rdfs:label>
        <owl:versionInfo xml:lang="it">stabile</owl:versionInfo>
        <owl:versionInfo xml:lang="en">stable</owl:versionInfo>
    </owl:NamedIndividual>



    <!-- https://w3id.org/leo/onto/health-assessment/NotExamined -->

    <owl:NamedIndividual rdf:about="https://w3id.org/leo/onto/health-assessment/NotExamined">
        <rdf:type rdf:resource="https://w3id.org/leo/onto/health-assessment/SampleJudgement"/>
        <rdfs:isDefinedBy rdf:resource="https://w3id.org/leo/onto/health-assessment"/>
        <rdfs:label xml:lang="it">Non Esaminato</rdfs:label>
        <rdfs:label xml:lang="en">Not Examined</rdfs:label>
        <owl:versionInfo xml:lang="it">stabile</owl:versionInfo>
        <owl:versionInfo xml:lang="en">stable</owl:versionInfo>
    </owl:NamedIndividual>



    <!-- https://w3id.org/leo/onto/health-assessment/Positive -->

    <owl:NamedIndividual rdf:about="https://w3id.org/leo/onto/health-assessment/Positive">
        <rdf:type rdf:resource="https://w3id.org/leo/onto/health-assessment/SampleJudgement"/>
        <rdfs:isDefinedBy rdf:resource="https://w3id.org/leo/onto/health-assessment"/>
        <rdfs:label xml:lang="en">Positive</rdfs:label>
        <rdfs:label xml:lang="it">Positivo</rdfs:label>
        <owl:versionInfo xml:lang="it">stabile</owl:versionInfo>
        <owl:versionInfo xml:lang="en">stable</owl:versionInfo>
    </owl:NamedIndividual>



    <!-- https://w3id.org/leo/onto/health-assessment/Unsuitable -->

    <owl:NamedIndividual rdf:about="https://w3id.org/leo/onto/health-assessment/Unsuitable">
        <rdf:type rdf:resource="https://w3id.org/leo/onto/health-assessment/SampleJudgement"/>
        <rdfs:isDefinedBy rdf:resource="https://w3id.org/leo/onto/health-assessment"/>
        <rdfs:label xml:lang="it">Non Idoneo</rdfs:label>
        <rdfs:label xml:lang="en">Unsuitable</rdfs:label>
        <owl:versionInfo xml:lang="it">stabile</owl:versionInfo>
        <owl:versionInfo xml:lang="en">stable</owl:versionInfo>
    </owl:NamedIndividual>
</rdf:RDF>



<!-- Generated by the OWL API (version 4.5.9.2019-02-01T07:24:44Z) https://github.com/owlcs/owlapi -->
