<?xml version="1.0"?>
<rdf:RDF xmlns="https://w3id.org/leo/onto/weather/"
     xml:base="https://w3id.org/leo/onto/weather/"
     xmlns:dc="http://purl.org/dc/elements/1.1/"
     xmlns:l0="https://w3id.org/italia/onto/l0/"
     xmlns:CLV="https://w3id.org/italia/onto/CLV/"
     xmlns:cov="https://w3id.org/italia/onto/COV/"
     xmlns:dct="http://purl.org/dc/terms/"
     xmlns:iot="https://w3id.org/italia/onto/IoT/"
     xmlns:owl="http://www.w3.org/2002/07/owl#"
     xmlns:rdf="http://www.w3.org/1999/02/22-rdf-syntax-ns#"
     xmlns:xml="http://www.w3.org/XML/1998/namespace"
     xmlns:xsd="http://www.w3.org/2001/XMLSchema#"
     xmlns:dcat="http://www.w3.org/ns/dcat#"
     xmlns:foaf="http://xmlns.com/foaf/0.1/"
     xmlns:prov="http://www.w3.org/ns/prov#"
     xmlns:rdfs="http://www.w3.org/2000/01/rdf-schema#"
     xmlns:vcard="http://www.w3.org/2006/vcard/ns#"
     xmlns:admsapit="https://w3id.org/italia/onto/ADMS/">
    <owl:Ontology rdf:about="https://w3id.org/leo/onto/weather">
        <owl:versionIRI rdf:resource="https://w3id.org/leo/onto/weather/0.2"/>
        <owl:imports rdf:resource="https://w3id.org/italia/onto/IoT"/>
        <owl:imports rdf:resource="https://w3id.org/italia/onto/l0"/>
        <dc:description rdf:resource="https://www.dropbox.com/s/6ecruj6h3joi6ua/WeatherModule.png?raw=1"/>
        <dct:accrualPeriodicity rdf:resource="http://publications.europa.eu/resource/authority/frequency/IRREG"/>
        <dct:creator rdf:resource="https://w3id.org/leo/data/private-organization/00944701002"/>
        <dct:description xml:lang="it">Questa è l&apos;ontologia per modellare i dati detti ClimData nel progetto LEO ovvero i dati raccolti di tipo climatico, intesi come osservazioni catturate da stazioni meteo.</dct:description>
        <dct:description xml:lang="en">This is the ontology used to model the data called ClimData in the LEO project, i.e. the collected climate data intended to be observations captured by weather stations.</dct:description>
        <dct:identifier>onto-BA-5</dct:identifier>
        <dct:issued rdf:datatype="http://www.w3.org/2001/XMLSchema#date">2019-11-20</dct:issued>
        <dct:language rdf:resource="http://publications.europa.eu/resource/authority/language/ENG"/>
        <dct:language rdf:resource="http://publications.europa.eu/resource/authority/language/ITA"/>
        <dct:modified xml:lang="en">2022-04-24</dct:modified>
        <dct:publisher rdf:resource="https://w3id.org/leo/data/private-organization/00944701002"/>
        <dct:rightsHolder rdf:resource="https://w3id.org/leo/data/private-organization/00944701002"/>
        <dct:subject rdf:resource="http://eurovoc.europa.eu/1892"/>
        <dct:title xml:lang="it">Ontologia dei dati meteo - ClimData</dct:title>
        <dct:title xml:lang="en">Weather Ontology</dct:title>
        <rdfs:comment xml:lang="it">Questa è l&apos;ontologia per modellare i dati detti ClimData nel progetto LEO ovvero i dati raccolti di tipo climatico, intesi come osservazioni catturate da stazioni meteo.</rdfs:comment>
        <rdfs:comment xml:lang="en">This is the ontology used to model the data called ClimData in the LEO project, i.e. the collected climate data intended to be observations captured by weather stations.</rdfs:comment>
        <rdfs:isDefinedBy rdf:resource="https://w3id.org/leo/onto/weather"/>
        <rdfs:label xml:lang="it">Ontologia dei dati meteo - ClimData</rdfs:label>
        <rdfs:label xml:lang="en">Weather Ontology</rdfs:label>
        <owl:versionInfo xml:lang="en">Version 0.2 - April 2022 - Revision of the ontology: renamed the class Weather in WeatherObservation. Revised the FeatureOfInterest not as class but as individuals of a new introduced class named WeatherFeatureOfInterest; introduced the classes WeatherObservableProperty and BioclimaticIndex as subclasses of ObservationParameter.</owl:versionInfo>
        <owl:versionInfo xml:lang="it">Versione 0.2 - Aprile 2022 - Revisione dell&apos;ontologia: rinominata la classe Weather in WeatherObservation. Riviste tutte le classe di FeatureOfInterest che sono diventati individui di una nuova classe introdotta chiamata WeatherFeatureOfInterest; introdotte le classi WeatherObservableProperty e BioclimaticIndex intese come sottoclassi di ObservationParameter.</owl:versionInfo>
        <dcat:contactPoint rdf:resource="https://w3id.org/leo/data/contact-point/onto-aia"/>
        <dcat:keyword xml:lang="it">Meteo</dcat:keyword>
        <dcat:keyword xml:lang="it">precipitazioni</dcat:keyword>
        <dcat:keyword xml:lang="en">ventosìtà</dcat:keyword>
        <dcat:theme rdf:resource="http://publications.europa.eu/resource/authority/data-theme/ENVI"/>
        <admsapit:acronym>WT</admsapit:acronym>
        <admsapit:hasContributor rdf:resource="https://w3id.org/leo/data/private-organization/06695411006"/>
        <admsapit:hasFormalityLevel rdf:resource="https://w3id.org/italia/onto/ADMS/Formal"/>
        <admsapit:hasKeyClass rdf:resource="https://w3id.org/leo/onto/weather/WeatherObservation"/>
        <admsapit:hasKeyClass rdf:resource="https://w3id.org/leo/onto/weather/WeatherStation"/>
        <admsapit:hasOntologyLanguage rdf:resource="https://w3id.org/italia/onto/ADMS/OWL"/>
        <admsapit:hasSemanticAssetDistribution rdf:resource="https://w3id.org/leo/data/distribution/WT-JSON-LD"/>
        <admsapit:hasSemanticAssetDistribution rdf:resource="https://w3id.org/leo/data/distribution/WT-RDF-TURTLE"/>
        <admsapit:hasSemanticAssetDistribution rdf:resource="https://w3id.org/leo/data/distribution/WT-RDF-XML"/>
        <admsapit:hasTask rdf:resource="https://w3id.org/italia/onto/ADMS/AnnotationTask"/>
        <admsapit:hasTask rdf:resource="https://w3id.org/italia/onto/ADMS/QueryFormulationTask"/>
        <admsapit:hasTask rdf:resource="https://w3id.org/italia/onto/ADMS/SearchTask"/>
        <admsapit:officialURI rdf:datatype="http://www.w3.org/2001/XMLSchema#anyURI">https://w3id.org/leo/onto/weather</admsapit:officialURI>
        <admsapit:prefix>wt</admsapit:prefix>
        <admsapit:semanticAssetInUse rdf:resource="https://w3id.org/leo/data/project/LEO"/>
        <admsapit:status>catalogued</admsapit:status>
        <admsapit:target xml:lang="it">Comunità open data</admsapit:target>
        <admsapit:target>Imprese</admsapit:target>
        <admsapit:target xml:lang="it">Professionisti del settore zootecnico</admsapit:target>
        <admsapit:target>Pubbliche Amministrazioni</admsapit:target>
        <admsapit:type rdf:resource="https://w3id.org/italia/onto/ADMS/DomainOntology"/>
    </owl:Ontology>
    


    <!-- 
    ///////////////////////////////////////////////////////////////////////////////////////
    //
    // Annotation properties
    //
    ///////////////////////////////////////////////////////////////////////////////////////
     -->

    


    <!-- http://purl.org/dc/elements/1.1/description -->

    <owl:AnnotationProperty rdf:about="http://purl.org/dc/elements/1.1/description"/>
    


    <!-- http://purl.org/dc/terms/description -->

    <owl:AnnotationProperty rdf:about="http://purl.org/dc/terms/description"/>
    


    <!-- http://purl.org/dc/terms/format -->

    <owl:AnnotationProperty rdf:about="http://purl.org/dc/terms/format"/>
    


    <!-- http://purl.org/dc/terms/identifier -->

    <owl:AnnotationProperty rdf:about="http://purl.org/dc/terms/identifier"/>
    


    <!-- http://purl.org/dc/terms/label -->

    <owl:AnnotationProperty rdf:about="http://purl.org/dc/terms/label"/>
    


    <!-- http://purl.org/dc/terms/license -->

    <owl:AnnotationProperty rdf:about="http://purl.org/dc/terms/license"/>
    


    <!-- http://purl.org/dc/terms/subject -->

    <owl:AnnotationProperty rdf:about="http://purl.org/dc/terms/subject"/>
    


    <!-- http://purl.org/dc/terms/title -->

    <owl:AnnotationProperty rdf:about="http://purl.org/dc/terms/title"/>
    


    <!-- http://www.w3.org/2006/vcard/ns#fn -->

    <owl:AnnotationProperty rdf:about="http://www.w3.org/2006/vcard/ns#fn"/>
    


    <!-- http://www.w3.org/2006/vcard/ns#hasEmail -->

    <owl:AnnotationProperty rdf:about="http://www.w3.org/2006/vcard/ns#hasEmail"/>
    


    <!-- http://www.w3.org/ns/dcat#accessURL -->

    <owl:AnnotationProperty rdf:about="http://www.w3.org/ns/dcat#accessURL"/>
    


    <!-- http://www.w3.org/ns/dcat#downloadURL -->

    <owl:AnnotationProperty rdf:about="http://www.w3.org/ns/dcat#downloadURL"/>
    


    <!-- http://www.w3.org/ns/prov#wasDerivedFrom -->

    <owl:AnnotationProperty rdf:about="http://www.w3.org/ns/prov#wasDerivedFrom"/>
    


    <!-- http://www.w3.org/ns/prov#wasInfluencedBy -->

    <owl:AnnotationProperty rdf:about="http://www.w3.org/ns/prov#wasInfluencedBy"/>
    


    <!-- http://xmlns.com/foaf/0.1/name -->

    <owl:AnnotationProperty rdf:about="http://xmlns.com/foaf/0.1/name"/>
    


    <!-- https://w3id.org/italia/onto/ADMS/acronym -->

    <owl:AnnotationProperty rdf:about="https://w3id.org/italia/onto/ADMS/acronym"/>
    


    <!-- https://w3id.org/italia/onto/ADMS/hasContributor -->

    <owl:AnnotationProperty rdf:about="https://w3id.org/italia/onto/ADMS/hasContributor"/>
    


    <!-- https://w3id.org/italia/onto/ADMS/hasFormalityLevel -->

    <owl:AnnotationProperty rdf:about="https://w3id.org/italia/onto/ADMS/hasFormalityLevel"/>
    


    <!-- https://w3id.org/italia/onto/ADMS/hasKeyClass -->

    <owl:AnnotationProperty rdf:about="https://w3id.org/italia/onto/ADMS/hasKeyClass"/>
    


    <!-- https://w3id.org/italia/onto/ADMS/hasOntologyLanguage -->

    <owl:AnnotationProperty rdf:about="https://w3id.org/italia/onto/ADMS/hasOntologyLanguage"/>
    


    <!-- https://w3id.org/italia/onto/ADMS/hasSemanticAssetDistribution -->

    <owl:AnnotationProperty rdf:about="https://w3id.org/italia/onto/ADMS/hasSemanticAssetDistribution"/>
    


    <!-- https://w3id.org/italia/onto/ADMS/hasTask -->

    <owl:AnnotationProperty rdf:about="https://w3id.org/italia/onto/ADMS/hasTask"/>
    


    <!-- https://w3id.org/italia/onto/ADMS/officialURI -->

    <owl:AnnotationProperty rdf:about="https://w3id.org/italia/onto/ADMS/officialURI"/>
    


    <!-- https://w3id.org/italia/onto/ADMS/prefix -->

    <owl:AnnotationProperty rdf:about="https://w3id.org/italia/onto/ADMS/prefix"/>
    


    <!-- https://w3id.org/italia/onto/ADMS/semanticAssetInUse -->

    <owl:AnnotationProperty rdf:about="https://w3id.org/italia/onto/ADMS/semanticAssetInUse"/>
    


    <!-- https://w3id.org/italia/onto/ADMS/status -->

    <owl:AnnotationProperty rdf:about="https://w3id.org/italia/onto/ADMS/status"/>
    


    <!-- https://w3id.org/italia/onto/ADMS/target -->

    <owl:AnnotationProperty rdf:about="https://w3id.org/italia/onto/ADMS/target"/>
    


    <!-- https://w3id.org/italia/onto/ADMS/type -->

    <owl:AnnotationProperty rdf:about="https://w3id.org/italia/onto/ADMS/type"/>
    


    <!-- https://w3id.org/italia/onto/l0/controlledVocabulary -->

    <owl:AnnotationProperty rdf:about="https://w3id.org/italia/onto/l0/controlledVocabulary"/>
    


    <!-- https://w3id.org/italia/onto/l0/name -->

    <owl:AnnotationProperty rdf:about="https://w3id.org/italia/onto/l0/name"/>
    


    <!-- 
    ///////////////////////////////////////////////////////////////////////////////////////
    //
    // Object Properties
    //
    ///////////////////////////////////////////////////////////////////////////////////////
     -->

    


    <!-- https://w3id.org/leo/onto/weather/managedBy -->

    <owl:ObjectProperty rdf:about="https://w3id.org/leo/onto/weather/managedBy">
        <owl:inverseOf rdf:resource="https://w3id.org/leo/onto/weather/managesWeatherStation"/>
        <rdfs:domain rdf:resource="https://w3id.org/leo/onto/weather/WeatherStation"/>
        <rdfs:range rdf:resource="https://w3id.org/italia/onto/COV/Organization"/>
        <rdfs:comment xml:lang="en">Property that links the weather station to the organization it manages it</rdfs:comment>
        <rdfs:comment xml:lang="it">Proprietà che collega la stazione meteo all&apos;organizzazione che la gestisce.</rdfs:comment>
        <rdfs:isDefinedBy rdf:resource="https://w3id.org/leo/onto/weather"/>
        <rdfs:label xml:lang="it">gestita da</rdfs:label>
        <rdfs:label xml:lang="en">managed by</rdfs:label>
        <owl:versionInfo xml:lang="it">stabile</owl:versionInfo>
        <owl:versionInfo xml:lang="en">stable</owl:versionInfo>
    </owl:ObjectProperty>
    


    <!-- https://w3id.org/leo/onto/weather/managesWeatherStation -->

    <owl:ObjectProperty rdf:about="https://w3id.org/leo/onto/weather/managesWeatherStation">
        <rdfs:domain rdf:resource="https://w3id.org/italia/onto/COV/Organization"/>
        <rdfs:range rdf:resource="https://w3id.org/leo/onto/weather/WeatherStation"/>
        <rdfs:comment xml:lang="en">Inverse property of &quot;managed by&quot; that links an organization to the weather station it manages.</rdfs:comment>
        <rdfs:comment xml:lang="it">Proprietà inversa di &quot;gestita da&quot; che collega l&apos;organizzazione alla stazione meteo che essa gestisce.</rdfs:comment>
        <rdfs:isDefinedBy rdf:resource="https://w3id.org/leo/onto/weather"/>
        <rdfs:label xml:lang="it">gestisce stazione meteo</rdfs:label>
        <rdfs:label xml:lang="en">manages weather station</rdfs:label>
        <owl:versionInfo xml:lang="it">stabile</owl:versionInfo>
        <owl:versionInfo xml:lang="en">stable</owl:versionInfo>
    </owl:ObjectProperty>
    


    <!-- 
    ///////////////////////////////////////////////////////////////////////////////////////
    //
    // Classes
    //
    ///////////////////////////////////////////////////////////////////////////////////////
     -->

    


    <!-- https://w3id.org/leo/onto/weather/BioClimaticIndex -->

    <owl:Class rdf:about="https://w3id.org/leo/onto/weather/BioClimaticIndex">
        <rdfs:subClassOf rdf:resource="https://w3id.org/italia/onto/IoT/ObservationParameter"/>
        <owl:disjointWith rdf:resource="https://w3id.org/leo/onto/weather/WeatherObservableProperty"/>
        <rdfs:comment xml:lang="it">La classe degli indici bioclimatici. Le istanze di questa classe possono essere l&apos;indice temperatura umidità (THI), l&apos;indice temperatura umidità (THI) load, ecc.</rdfs:comment>
        <rdfs:comment xml:lang="en">The class of the bioclimatic indexes. Instances of this class can be the Temperature Humidity Index (THI), the Temperature Humidity Index (THI) load, etc.</rdfs:comment>
        <rdfs:isDefinedBy rdf:resource="https://w3id.org/leo/onto/weather"/>
        <rdfs:label xml:lang="en">Bioclimatic Index</rdfs:label>
        <rdfs:label xml:lang="it">Indice Bioclimatico</rdfs:label>
        <owl:versionInfo xml:lang="it">stabile</owl:versionInfo>
        <owl:versionInfo xml:lang="en">stable</owl:versionInfo>
    </owl:Class>
    


    <!-- https://w3id.org/leo/onto/weather/WeatherFeatureOfInterest -->

    <owl:Class rdf:about="https://w3id.org/leo/onto/weather/WeatherFeatureOfInterest">
        <rdfs:subClassOf rdf:resource="https://w3id.org/italia/onto/IoT/FeatureOfInterest"/>
        <rdfs:comment xml:lang="en">It represents the feature of interest in weather whose attribute is observed by a sensor to obtain a value. Examples of features of interest in weather are: air, rainfall, wind, etc.</rdfs:comment>
        <rdfs:comment xml:lang="it">Rappresenta la caratteristica di interesse meteo il cui attributo osservato è osservato da un sensore per ottenere un valore. Esempi di caratteristiche di interesse nell&apos;ambito meteo sono: l&apos;aria, la pioggia, il vento, ecc.</rdfs:comment>
        <rdfs:isDefinedBy rdf:resource="https://w3id.org/leo/onto/weather"/>
        <rdfs:label xml:lang="it">Caratteristica di interesse meteo</rdfs:label>
        <rdfs:label xml:lang="en">Weather Feature of Interest</rdfs:label>
        <owl:versionInfo xml:lang="it">stabile</owl:versionInfo>
        <owl:versionInfo xml:lang="en">stable</owl:versionInfo>
    </owl:Class>
    


    <!-- https://w3id.org/leo/onto/weather/WeatherObservableProperty -->

    <owl:Class rdf:about="https://w3id.org/leo/onto/weather/WeatherObservableProperty">
        <rdfs:subClassOf rdf:resource="https://w3id.org/italia/onto/IoT/ObservationParameter"/>
        <rdfs:comment xml:lang="it">La classe di tutte le proprietà di un&apos;osservazione che possono essere osservate nel contesto meteorologico.  Esempi includono: temperatura, umidità, pressione, precipitazione, ecc.</rdfs:comment>
        <rdfs:comment xml:lang="en">The class of all the properties of an observation that can be observed in the weather context. Examples include: temperature, humidity, pressure, precipitation, etc.</rdfs:comment>
        <rdfs:isDefinedBy rdf:resource="https://w3id.org/leo/onto/weather"/>
        <rdfs:label xml:lang="it">Proprietà Meteo Osservabile</rdfs:label>
        <rdfs:label xml:lang="en">Weather Observable Property</rdfs:label>
        <owl:versionInfo xml:lang="it">stabile</owl:versionInfo>
        <owl:versionInfo xml:lang="en">stable</owl:versionInfo>
    </owl:Class>
    


    <!-- https://w3id.org/leo/onto/weather/WeatherObservation -->

    <owl:Class rdf:about="https://w3id.org/leo/onto/weather/WeatherObservation">
        <rdfs:subClassOf rdf:resource="https://w3id.org/italia/onto/IoT/Observation"/>
        <rdfs:comment xml:lang="it">Questa classe rappresenta un&apos;osservazione di tipo meteo.</rdfs:comment>
        <rdfs:comment xml:lang="en">This class represents a specific observation of Meteo type</rdfs:comment>
        <rdfs:label rdf:resource="https://w3id.org/leo/onto/weather"/>
        <rdfs:label xml:lang="it">Osservazione Meteo</rdfs:label>
        <rdfs:label xml:lang="en">Weather Observation</rdfs:label>
        <owl:versionInfo xml:lang="it">stabile</owl:versionInfo>
        <owl:versionInfo xml:lang="en">stable</owl:versionInfo>
    </owl:Class>
    


    <!-- https://w3id.org/leo/onto/weather/WeatherStation -->

    <owl:Class rdf:about="https://w3id.org/leo/onto/weather/WeatherStation">
        <rdfs:subClassOf rdf:resource="https://w3id.org/italia/onto/IoT/Platform"/>
        <rdfs:subClassOf>
            <owl:Restriction>
                <owl:onProperty rdf:resource="https://w3id.org/italia/onto/CLV/hasSpatialCoverage"/>
                <owl:someValuesFrom rdf:resource="https://w3id.org/italia/onto/CLV/Feature"/>
            </owl:Restriction>
        </rdfs:subClassOf>
        <rdfs:subClassOf>
            <owl:Restriction>
                <owl:onProperty rdf:resource="https://w3id.org/italia/onto/CLV/hasGeometry"/>
                <owl:qualifiedCardinality rdf:datatype="http://www.w3.org/2001/XMLSchema#nonNegativeInteger">1</owl:qualifiedCardinality>
                <owl:onClass rdf:resource="https://w3id.org/italia/onto/CLV/Geometry"/>
            </owl:Restriction>
        </rdfs:subClassOf>
        <rdfs:subClassOf>
            <owl:Restriction>
                <owl:onProperty rdf:resource="https://w3id.org/leo/onto/weather/managedBy"/>
                <owl:maxQualifiedCardinality rdf:datatype="http://www.w3.org/2001/XMLSchema#nonNegativeInteger">1</owl:maxQualifiedCardinality>
                <owl:onClass rdf:resource="https://w3id.org/italia/onto/COV/Organization"/>
            </owl:Restriction>
        </rdfs:subClassOf>
        <rdfs:subClassOf>
            <owl:Restriction>
                <owl:onProperty rdf:resource="https://w3id.org/italia/onto/l0/name"/>
                <owl:someValuesFrom rdf:resource="http://www.w3.org/2000/01/rdf-schema#Literal"/>
            </owl:Restriction>
        </rdfs:subClassOf>
        <rdfs:subClassOf>
            <owl:Restriction>
                <owl:onProperty rdf:resource="https://w3id.org/italia/onto/l0/identifier"/>
                <owl:cardinality rdf:datatype="http://www.w3.org/2001/XMLSchema#nonNegativeInteger">1</owl:cardinality>
            </owl:Restriction>
        </rdfs:subClassOf>
        <rdfs:comment xml:lang="it">Questa classe rappresenta la stazione meteo. La stazione è identificata univocamente da un identificativo, è gestita da un&apos;organizzazione ed ha una geometria (tipicamente un punto) associata.</rdfs:comment>
        <rdfs:comment xml:lang="en">This class represents the weather station. The station is uniquely identified by an identifier, is managed by an organization and has a geometry (usually a point) associated with it.</rdfs:comment>
        <rdfs:isDefinedBy rdf:resource="https://w3id.org/leo/onto/weather"/>
        <rdfs:label xml:lang="it">Stazione Meteo</rdfs:label>
        <rdfs:label xml:lang="en">Weather Station</rdfs:label>
        <owl:versionInfo xml:lang="it">stabile</owl:versionInfo>
        <owl:versionInfo xml:lang="en">stable</owl:versionInfo>
    </owl:Class>
    


    <!-- 
    ///////////////////////////////////////////////////////////////////////////////////////
    //
    // Individuals
    //
    ///////////////////////////////////////////////////////////////////////////////////////
     -->

    


    <!-- https://w3id.org/leo/data/contact-point/onto-aia -->

    <owl:NamedIndividual rdf:about="https://w3id.org/leo/data/contact-point/onto-aia">
        <rdf:type rdf:resource="http://dati.gov.it/onto/dcatapit#Organization"/>
        <rdf:type rdf:resource="http://www.w3.org/2006/vcard/ns#Kind"/>
        <rdf:type rdf:resource="http://www.w3.org/2006/vcard/ns#Organization"/>
        <rdfs:label xml:lang="it">Sistemi informativi</rdfs:label>
        <vcard:fn xml:lang="it">Sistemi informativi</vcard:fn>
        <vcard:hasEmail rdf:resource="mailto:affarigenerali@pec.aia.it"/>
    </owl:NamedIndividual>
    


    <!-- https://w3id.org/leo/data/distribution/WT-JSON-LD -->

    <owl:NamedIndividual rdf:about="https://w3id.org/leo/data/distribution/WT-JSON-LD">
        <rdf:type rdf:resource="https://w3id.org/italia/onto/ADMS/SemanticAssetDistribution"/>
        <dct:description xml:lang="it">Questa è la distribuzione JSON-LD dell&apos;ontologia sul meteo</dct:description>
        <dct:description xml:lang="en">This is the distribution in JSON-LD of weather ontology</dct:description>
        <dct:format rdf:resource="http://publications.europa.eu/resource/authority/file-type/JSON_LD"/>
        <dct:label xml:lang="it">Distribuzione JSON-LD ontologia Weather</dct:label>
        <dct:label xml:lang="en">JSON-LD distribution of Weather Ontology</dct:label>
        <dct:license rdf:resource="https://w3id.org/italia/controlled-vocabulary/licences/A21_CCBY40"/>
        <dct:title xml:lang="it">Distribuzione JSON-LD ontologia Weather</dct:title>
        <dct:title xml:lang="en">JSON-LD distribution of Weather Ontology</dct:title>
        <rdfs:comment xml:lang="it">Questa è la distribuzione JSON-LD dell&apos;ontologia sul meteo</rdfs:comment>
        <rdfs:comment xml:lang="en">This is the distribution in JSON-LD of weather ontology</rdfs:comment>
        <dcat:accessURL rdf:resource="https://www.leo-project.it/Ontologie/weather/latest"/>
        <dcat:downloadURL rdf:resource="https://www.leo-project.it/Ontologie/weathr/latest/weather.jsonld"/>
    </owl:NamedIndividual>
    


    <!-- https://w3id.org/leo/data/distribution/WT-RDF-TURTLE -->

    <owl:NamedIndividual rdf:about="https://w3id.org/leo/data/distribution/WT-RDF-TURTLE">
        <rdf:type rdf:resource="https://w3id.org/italia/onto/ADMS/SemanticAssetDistribution"/>
        <dct:description xml:lang="it">Questa è la distribuzione RDF/Turtle dell&apos;ontologia sul meteo</dct:description>
        <dct:description xml:lang="en">This is the distribution in RDF/Turtle of Weather ontology</dct:description>
        <dct:format rdf:resource="http://publications.europa.eu/resource/authority/file-type/RDF_TURTLE"/>
        <dct:license rdf:resource="https://w3id.org/italia/controlled-vocabulary/licences/A21_CCBY40"/>
        <dct:title xml:lang="it">Distribuzione RDF/Turtle ontologia Weather</dct:title>
        <dct:title xml:lang="en">RDF/Turtle distribution of Weather Ontology</dct:title>
        <rdfs:comment xml:lang="it">Questa è la distribuzione RDF/Turtle dell&apos;ontologia sul meteo</rdfs:comment>
        <rdfs:comment xml:lang="en">This is the distribution in RDF/Turtle of Weather ontology</rdfs:comment>
        <rdfs:label xml:lang="it">Distribuzione RDF/Turtle ontologia Weather</rdfs:label>
        <rdfs:label xml:lang="en">RDF/Turtle distribution of Weather Ontology</rdfs:label>
        <dcat:accessURL rdf:resource="https://www.leo-project.it/Ontologie/weather/latest"/>
        <dcat:downloadURL rdf:resource="https://www.leo-project.it/Ontologie/weather/latest/weather.ttl"/>
    </owl:NamedIndividual>
    


    <!-- https://w3id.org/leo/data/distribution/WT-RDF-XML -->

    <owl:NamedIndividual rdf:about="https://w3id.org/leo/data/distribution/WT-RDF-XML">
        <rdf:type rdf:resource="https://w3id.org/italia/onto/ADMS/SemanticAssetDistribution"/>
        <dct:description xml:lang="it">Questa è la distribuzione RDF/XML dell&apos;ontologia sul meteo</dct:description>
        <dct:description xml:lang="en">This is the distribution in RDF/XML of Weather ontology</dct:description>
        <dct:format rdf:resource="http://publications.europa.eu/resource/authority/file-type/RDF_XML"/>
        <dct:license rdf:resource="https://w3id.org/italia/controlled-vocabulary/licences/A21_CCBY40"/>
        <dct:title xml:lang="it">Distribuzione RDF/XML ontologia Weather</dct:title>
        <dct:title xml:lang="en">RDF/XML distribution of Weather Ontology</dct:title>
        <rdfs:comment xml:lang="it">Questa è la distribuzione RDF/XML dell&apos;ontologia sul meteo</rdfs:comment>
        <rdfs:comment xml:lang="en">This is the distribution in RDF/XML of Weather ontology</rdfs:comment>
        <rdfs:label xml:lang="it">Distribuzione RDF/XML ontologia Weather</rdfs:label>
        <rdfs:label xml:lang="en">RDF/XML distribution of Weather Ontology</rdfs:label>
        <dcat:accessURL rdf:resource="https://www.leo-project.it/Ontologie/weather/latest"/>
        <dcat:downloadURL rdf:resource="https://www.leo-project.it/Ontologie/weather/latest/weather.rdf"/>
    </owl:NamedIndividual>
    


    <!-- https://w3id.org/leo/data/private-organization/00944701002 -->

    <owl:NamedIndividual rdf:about="https://w3id.org/leo/data/private-organization/00944701002">
        <rdf:type rdf:resource="http://dati.gov.it/onto/dcatapit#Agent"/>
        <rdf:type rdf:resource="http://xmlns.com/foaf/0.1/Agent"/>
        <dct:identifier>00944701002</dct:identifier>
        <foaf:name xml:lang="it">Associazione Italiana Allevatori</foaf:name>
        <foaf:name xml:lang="en">Italian Breeders&apos; Association</foaf:name>
    </owl:NamedIndividual>
    


    <!-- https://w3id.org/leo/data/private-organization/06695411006 -->

    <owl:NamedIndividual rdf:about="https://w3id.org/leo/data/private-organization/06695411006">
        <rdf:type rdf:resource="http://dati.gov.it/onto/dcatapit#Agent"/>
        <rdf:type rdf:resource="http://xmlns.com/foaf/0.1/Agent"/>
        <dct:identifier>06695411006</dct:identifier>
        <foaf:name xml:lang="en">Bluarancio</foaf:name>
        <foaf:name xml:lang="it">Bluarancio</foaf:name>
    </owl:NamedIndividual>
    


    <!-- https://w3id.org/leo/data/project/LEO -->

    <owl:NamedIndividual rdf:about="https://w3id.org/leo/data/project/LEO">
        <rdf:type rdf:resource="https://w3id.org/italia/onto/ADMS/Project"/>
        <rdfs:label xml:lang="it">LEO - Livestok Environment Open Data</rdfs:label>
        <l0:name xml:lang="it">LEO - Livestok Environment Open Data</l0:name>
    </owl:NamedIndividual>
    


    <!-- https://w3id.org/leo/onto/weather -->

    <owl:NamedIndividual rdf:about="https://w3id.org/leo/onto/weather">
        <rdf:type rdf:resource="https://w3id.org/italia/onto/ADMS/SemanticAsset"/>
    </owl:NamedIndividual>
    


    <!-- https://w3id.org/leo/onto/weather/Air -->

    <owl:NamedIndividual rdf:about="https://w3id.org/leo/onto/weather/Air">
        <rdf:type rdf:resource="https://w3id.org/leo/onto/weather/WeatherFeatureOfInterest"/>
        <rdfs:isDefinedBy rdf:resource="https://w3id.org/leo/onto/weather"/>
        <rdfs:label xml:lang="en">Air</rdfs:label>
        <rdfs:label xml:lang="it">Aria</rdfs:label>
        <owl:versionInfo xml:lang="it">stabile</owl:versionInfo>
        <owl:versionInfo xml:lang="en">stable</owl:versionInfo>
    </owl:NamedIndividual>
    


    <!-- https://w3id.org/leo/onto/weather/GroundLevelSoil -->

    <owl:NamedIndividual rdf:about="https://w3id.org/leo/onto/weather/GroundLevelSoil">
        <rdf:type rdf:resource="https://w3id.org/leo/onto/weather/WeatherFeatureOfInterest"/>
        <rdfs:isDefinedBy rdf:resource="https://w3id.org/leo/onto/weather"/>
        <rdfs:label xml:lang="en">Ground Level Soil</rdfs:label>
        <rdfs:label xml:lang="it">Livello del Suolo</rdfs:label>
        <owl:versionInfo xml:lang="it">stabile</owl:versionInfo>
        <owl:versionInfo xml:lang="en">stable</owl:versionInfo>
    </owl:NamedIndividual>
    


    <!-- https://w3id.org/leo/onto/weather/Rainfall -->

    <owl:NamedIndividual rdf:about="https://w3id.org/leo/onto/weather/Rainfall">
        <rdf:type rdf:resource="https://w3id.org/leo/onto/weather/WeatherFeatureOfInterest"/>
        <rdfs:isDefinedBy rdf:resource="https://w3id.org/leo/onto/weather"/>
        <rdfs:label xml:lang="it">Pioggia</rdfs:label>
        <rdfs:label xml:lang="en">Rainfall</rdfs:label>
        <owl:versionInfo xml:lang="it">stabile</owl:versionInfo>
        <owl:versionInfo xml:lang="en">stable</owl:versionInfo>
    </owl:NamedIndividual>
    


    <!-- https://w3id.org/leo/onto/weather/Wind -->

    <owl:NamedIndividual rdf:about="https://w3id.org/leo/onto/weather/Wind">
        <rdf:type rdf:resource="https://w3id.org/leo/onto/weather/WeatherFeatureOfInterest"/>
        <rdfs:isDefinedBy rdf:resource="https://w3id.org/leo/onto/weather"/>
        <rdfs:label xml:lang="it">Vento</rdfs:label>
        <rdfs:label xml:lang="en">Wind</rdfs:label>
        <owl:versionInfo xml:lang="it">stabile</owl:versionInfo>
        <owl:versionInfo xml:lang="en">stable</owl:versionInfo>
    </owl:NamedIndividual>
</rdf:RDF>



<!-- Generated by the OWL API (version 4.5.9.2019-02-01T07:24:44Z) https://github.com/owlcs/owlapi -->

