<?xml version="1.0"?>
<rdf:RDF xmlns="https://w3id.org/leo/onto/ale/"
     xml:base="https://w3id.org/leo/onto/ale/"
     xmlns:dc="http://purl.org/dc/elements/1.1/"
     xmlns:l0="https://w3id.org/italia/onto/l0/"
     xmlns:ns="http://www.w3.org/2006/vcard/ns#"
     xmlns:owl="http://www.w3.org/2002/07/owl#"
     xmlns:rdf="http://www.w3.org/1999/02/22-rdf-syntax-ns#"
     xmlns:xml="http://www.w3.org/XML/1998/namespace"
     xmlns:xsd="http://www.w3.org/2001/XMLSchema#"
     xmlns:ADMS="https://w3id.org/italia/onto/ADMS/"
     xmlns:dcat="http://www.w3.org/ns/dcat#"
     xmlns:foaf="http://xmlns.com/foaf/0.1/"
     xmlns:prov="http://www.w3.org/ns/prov#"
     xmlns:rdfs="http://www.w3.org/2000/01/rdf-schema#"
     xmlns:terms="http://purl.org/dc/terms/">
    <owl:Ontology rdf:about="https://w3id.org/leo/onto/ale">
        <owl:versionIRI rdf:resource="https://w3id.org/leo/onto/ale/1.0"/>
        <owl:imports rdf:resource="https://w3id.org/italia/onto/TI"/>
        <owl:imports rdf:resource="https://w3id.org/italia/onto/l0"/>
        <dc:description rdf:resource="https://raw.githubusercontent.com/Bluarancio/Leo-OpenData/master/RappresentazioneGraficaOntologie/PNG/AleModule.png"/>
        <terms:accrualPeriodicity rdf:resource="http://publications.europa.eu/resource/authority/frequency/IRREG"/>
        <terms:creator rdf:resource="https://w3id.org/leo/data/private-organization/00944701002"/>
        <terms:description xml:lang="it">Questa è l&apos;ontologia degli eventi della vita degli animali di allevamento, L&apos;ontologia rappresenta pertanto momenti importanti della vita degli animali come per esempio il parto, la nascita, l&apos;aborto, la fecondazione, i vari spostamenti in entrata e uscita dalle aziende di allevamento, il macello, ecc. Per ogni evento, l&apos;ontologia rappresenta elementi principali che caratterizzano ciascun evento.</terms:description>
        <terms:description xml:lang="en">The ontology thus represents important moments in the life of animals, such as birth, abortion, fertilisation, the various movements on and off farms, slaughter, etc. For each event, the ontology represents the main elements that characterise it.</terms:description>
        <terms:identifier>onto-BA-3</terms:identifier>
        <terms:issued rdf:datatype="http://www.w3.org/2001/XMLSchema#date">2018-06-18</terms:issued>
        <terms:language rdf:resource="http://publications.europa.eu/resource/authority/language/ENG"/>
        <terms:language rdf:resource="http://publications.europa.eu/resource/authority/language/ITA"/>
        <terms:modified>2023-06-20</terms:modified>
        <terms:publisher rdf:resource="https://w3id.org/leo/data/private-organization/00944701002"/>
        <terms:rightsHolder rdf:resource="https://w3id.org/leo/data/private-organization/00944701002"/>
        <terms:subject rdf:resource="http://eurovoc.europa.eu/100254"/>
        <terms:title xml:lang="en">Animal Life Event Ontology</terms:title>
        <terms:title xml:lang="it">Ontologia degli eventi della vita degli animali di allevamento</terms:title>
        <rdfs:comment xml:lang="it">Questa è l&apos;ontologia degli eventi della vita degli animali di allevamento, L&apos;ontologia rappresenta pertanto momenti importanti della vita degli animali come per esempio il parto, la nascita, l&apos;aborto, la fecondazione, i vari spostamenti in entrata e uscita dalle aziende di allevamento, il macello, ecc. Per ogni evento, l&apos;ontologia rappresenta elementi principali che caratterizzano ciascun evento.</rdfs:comment>
        <rdfs:comment xml:lang="en">The ontology thus represents important moments in the life of animals, such as birth, abortion, fertilisation, the various movements on and off farms, slaughter, etc. For each event, the ontology represents the main elements that characterise it.</rdfs:comment>
        <rdfs:isDefinedBy rdf:resource="https://w3id.org/leo/onto/ale"/>
        <rdfs:label xml:lang="en">Animal Life Event Ontology</rdfs:label>
        <rdfs:label xml:lang="it">Ontologia degli eventi della vita degli animali di allevamento</rdfs:label>
        <owl:versionInfo xml:lang="en">Version 1.0- June 2023 - Introduction of new animal life events, i.e., weaning, weighing, breast feeding termination, back fat thickness measurement, and related parameters.</owl:versionInfo>
        <owl:versionInfo xml:lang="it">Versione 1.0 - Giugno 2023 - Introduzione di nuovi eventi della vita, i.e., svezzamento, pesata, interruzione dell&apos;allattamento, misurazione dello spessore del grasso dorsale, e relativi parametri.</owl:versionInfo>
        <dcat:contactPoint rdf:resource="https://w3id.org/leo/data/contact-point/onto-aia"/>
        <dcat:keyword xml:lang="it">Animali d&apos;allevamento</dcat:keyword>
        <dcat:keyword xml:lang="en">Bovine</dcat:keyword>
        <dcat:keyword xml:lang="it">Bovini</dcat:keyword>
        <dcat:keyword xml:lang="it">Eventi della vita</dcat:keyword>
        <dcat:keyword xml:lang="en">Farm Animal</dcat:keyword>
        <dcat:keyword xml:lang="en">Life events</dcat:keyword>
        <dcat:theme rdf:resource="http://publications.europa.eu/resource/authority/data-theme/AGRI"/>
        <ADMS:acronym>ALE</ADMS:acronym>
        <ADMS:hasContributor rdf:resource="https://w3id.org/leo/data/private-organization/06695411006"/>
        <ADMS:hasFormalityLevel rdf:resource="https://w3id.org/italia/onto/ADMS/Formal"/>
        <ADMS:hasKeyClass rdf:resource="https://w3id.org/leo/onto/ale/AnimalLifeEvent"/>
        <ADMS:hasOntologyLanguage rdf:resource="https://w3id.org/italia/onto/ADMS/OWL"/>
        <ADMS:hasSemanticAssetDistribution rdf:resource="https://w3id.org/leo/data/distribution/ALE-JSON-LD"/>
        <ADMS:hasSemanticAssetDistribution rdf:resource="https://w3id.org/leo/data/distribution/ALE-RDF-TURTLE"/>
        <ADMS:hasSemanticAssetDistribution rdf:resource="https://w3id.org/leo/data/distribution/ALE-RDF-XML"/>
        <ADMS:hasTask rdf:resource="https://w3id.org/italia/onto/ADMS/AnnotationTask"/>
        <ADMS:hasTask rdf:resource="https://w3id.org/italia/onto/ADMS/QueryFormulationTask"/>
        <ADMS:hasTask rdf:resource="https://w3id.org/italia/onto/ADMS/SearchTask"/>
        <ADMS:officialURI rdf:datatype="http://www.w3.org/2001/XMLSchema#anyURI">https://w3id.org/leo/onto/ale</ADMS:officialURI>
        <ADMS:prefix>ale</ADMS:prefix>
        <ADMS:semanticAssetInUse rdf:resource="https://w3id.org/leo/data/project/LEO"/>
        <ADMS:status>catalogued</ADMS:status>
        <ADMS:target xml:lang="it">Comunità Open Data</ADMS:target>
        <ADMS:target>Imprese</ADMS:target>
        <ADMS:target xml:lang="it">Professionisti del settore zootecnico</ADMS:target>
        <ADMS:target>Pubbliche Amministrazioni</ADMS:target>
        <ADMS:type rdf:resource="https://w3id.org/italia/onto/ADMS/DomainOntology"/>
    </owl:Ontology>
    


    <!-- 
    ///////////////////////////////////////////////////////////////////////////////////////
    //
    // Annotation properties
    //
    ///////////////////////////////////////////////////////////////////////////////////////
     -->

    


    <!-- http://purl.org/dc/elements/1.1/description -->

    <owl:AnnotationProperty rdf:about="http://purl.org/dc/elements/1.1/description"/>
    


    <!-- http://purl.org/dc/terms/description -->

    <owl:AnnotationProperty rdf:about="http://purl.org/dc/terms/description"/>
    


    <!-- http://purl.org/dc/terms/format -->

    <owl:AnnotationProperty rdf:about="http://purl.org/dc/terms/format"/>
    


    <!-- http://purl.org/dc/terms/identifier -->

    <owl:AnnotationProperty rdf:about="http://purl.org/dc/terms/identifier"/>
    


    <!-- http://purl.org/dc/terms/license -->

    <owl:AnnotationProperty rdf:about="http://purl.org/dc/terms/license"/>
    


    <!-- http://purl.org/dc/terms/subject -->

    <owl:AnnotationProperty rdf:about="http://purl.org/dc/terms/subject"/>
    


    <!-- http://purl.org/dc/terms/title -->

    <owl:AnnotationProperty rdf:about="http://purl.org/dc/terms/title"/>
    


    <!-- http://www.w3.org/2006/vcard/ns#fn -->

    <owl:AnnotationProperty rdf:about="http://www.w3.org/2006/vcard/ns#fn"/>
    


    <!-- http://www.w3.org/2006/vcard/ns#hasEmail -->

    <owl:AnnotationProperty rdf:about="http://www.w3.org/2006/vcard/ns#hasEmail"/>
    


    <!-- http://www.w3.org/ns/dcat#accessURL -->

    <owl:AnnotationProperty rdf:about="http://www.w3.org/ns/dcat#accessURL"/>
    


    <!-- http://www.w3.org/ns/dcat#downloadURL -->

    <owl:AnnotationProperty rdf:about="http://www.w3.org/ns/dcat#downloadURL"/>
    


    <!-- http://www.w3.org/ns/prov#wasDerivedFrom -->

    <owl:AnnotationProperty rdf:about="http://www.w3.org/ns/prov#wasDerivedFrom"/>
    


    <!-- http://www.w3.org/ns/prov#wasInfluencedBy -->

    <owl:AnnotationProperty rdf:about="http://www.w3.org/ns/prov#wasInfluencedBy"/>
    


    <!-- http://xmlns.com/foaf/0.1/name -->

    <owl:AnnotationProperty rdf:about="http://xmlns.com/foaf/0.1/name"/>
    


    <!-- https://w3id.org/italia/onto/ADMS/acronym -->

    <owl:AnnotationProperty rdf:about="https://w3id.org/italia/onto/ADMS/acronym"/>
    


    <!-- https://w3id.org/italia/onto/ADMS/hasContributor -->

    <owl:AnnotationProperty rdf:about="https://w3id.org/italia/onto/ADMS/hasContributor"/>
    


    <!-- https://w3id.org/italia/onto/ADMS/hasFormalityLevel -->

    <owl:AnnotationProperty rdf:about="https://w3id.org/italia/onto/ADMS/hasFormalityLevel"/>
    


    <!-- https://w3id.org/italia/onto/ADMS/hasKeyClass -->

    <owl:AnnotationProperty rdf:about="https://w3id.org/italia/onto/ADMS/hasKeyClass"/>
    


    <!-- https://w3id.org/italia/onto/ADMS/hasOntologyLanguage -->

    <owl:AnnotationProperty rdf:about="https://w3id.org/italia/onto/ADMS/hasOntologyLanguage"/>
    


    <!-- https://w3id.org/italia/onto/ADMS/hasSemanticAssetDistribution -->

    <owl:AnnotationProperty rdf:about="https://w3id.org/italia/onto/ADMS/hasSemanticAssetDistribution"/>
    


    <!-- https://w3id.org/italia/onto/ADMS/hasTask -->

    <owl:AnnotationProperty rdf:about="https://w3id.org/italia/onto/ADMS/hasTask"/>
    


    <!-- https://w3id.org/italia/onto/ADMS/officialURI -->

    <owl:AnnotationProperty rdf:about="https://w3id.org/italia/onto/ADMS/officialURI"/>
    


    <!-- https://w3id.org/italia/onto/ADMS/prefix -->

    <owl:AnnotationProperty rdf:about="https://w3id.org/italia/onto/ADMS/prefix"/>
    


    <!-- https://w3id.org/italia/onto/ADMS/semanticAssetInUse -->

    <owl:AnnotationProperty rdf:about="https://w3id.org/italia/onto/ADMS/semanticAssetInUse"/>
    


    <!-- https://w3id.org/italia/onto/ADMS/status -->

    <owl:AnnotationProperty rdf:about="https://w3id.org/italia/onto/ADMS/status"/>
    


    <!-- https://w3id.org/italia/onto/ADMS/target -->

    <owl:AnnotationProperty rdf:about="https://w3id.org/italia/onto/ADMS/target"/>
    


    <!-- https://w3id.org/italia/onto/ADMS/type -->

    <owl:AnnotationProperty rdf:about="https://w3id.org/italia/onto/ADMS/type"/>
    


    <!-- https://w3id.org/italia/onto/l0/controlledVocabulary -->

    <owl:AnnotationProperty rdf:about="https://w3id.org/italia/onto/l0/controlledVocabulary"/>
    


    <!-- https://w3id.org/italia/onto/l0/name -->

    <owl:AnnotationProperty rdf:about="https://w3id.org/italia/onto/l0/name"/>
    


    <!-- 
    ///////////////////////////////////////////////////////////////////////////////////////
    //
    // Object Properties
    //
    ///////////////////////////////////////////////////////////////////////////////////////
     -->

    


    <!-- https://w3id.org/leo/onto/ale/appliesToSpecies -->

    <owl:ObjectProperty rdf:about="https://w3id.org/leo/onto/ale/appliesToSpecies">
        <rdfs:domain>
            <owl:Class>
                <owl:unionOf rdf:parseType="Collection">
                    <rdf:Description rdf:about="https://w3id.org/leo/onto/ale/CarcassCategory"/>
                    <rdf:Description rdf:about="https://w3id.org/leo/onto/ale/CarcassClassification"/>
                    <rdf:Description rdf:about="https://w3id.org/leo/onto/ale/CarcassConformation"/>
                    <rdf:Description rdf:about="https://w3id.org/leo/onto/ale/FatCover"/>
                </owl:unionOf>
            </owl:Class>
        </rdfs:domain>
        <rdfs:range rdf:resource="https://w3id.org/leo/onto/animal/LivestockSpecies"/>
        <rdfs:comment xml:lang="en">Property that links all the concepts for carcass classification (carcass category, carcass classification, carcass conformance and fat cover) to the related livestock species.</rdfs:comment>
        <rdfs:comment xml:lang="it">Proprietà che collega tutti i concetti relativi alla classificazione delle carcasse (categoria, classificazione, conformazione e stato di ingrassamento) alla specie zootecnica.</rdfs:comment>
        <rdfs:isDefinedBy rdf:resource="https://w3id.org/leo/onto/ale"/>
        <rdfs:label xml:lang="en">applies to species</rdfs:label>
        <rdfs:label xml:lang="it">si applica a specie zootecnica</rdfs:label>
        <owl:versionInfo xml:lang="it">stabile - introdotta in versione 0.4 dell&apos;ontologia</owl:versionInfo>
        <owl:versionInfo xml:lang="en">stable - introduced in version 0.4 of the ontology</owl:versionInfo>
    </owl:ObjectProperty>
    


    <!-- https://w3id.org/leo/onto/ale/carriedOutBy -->

    <owl:ObjectProperty rdf:about="https://w3id.org/leo/onto/ale/carriedOutBy">
        <rdfs:domain rdf:resource="https://w3id.org/leo/onto/ale/MilkConductivityMeasurement"/>
        <rdfs:range rdf:resource="https://w3id.org/leo/onto/co/LivestockFarm"/>
        <rdfs:comment xml:lang="en">Property that links the measurement of the milk conductivity to the company that provides the results.</rdfs:comment>
        <rdfs:comment xml:lang="it">Proprietà che collega la misurazione della conducibilità media del latte all&apos;azienda che fornisce i risultati.</rdfs:comment>
        <rdfs:isDefinedBy rdf:resource="https://w3id.org/leo/onto/ale"/>
        <rdfs:label xml:lang="en">carried out by</rdfs:label>
        <rdfs:label xml:lang="it">fatta da</rdfs:label>
        <owl:versionInfo xml:lang="it">stabile</owl:versionInfo>
        <owl:versionInfo xml:lang="en">stable</owl:versionInfo>
    </owl:ObjectProperty>
    


    <!-- https://w3id.org/leo/onto/ale/carriedOutBySlaughterhouse -->

    <owl:ObjectProperty rdf:about="https://w3id.org/leo/onto/ale/carriedOutBySlaughterhouse">
        <rdfs:subPropertyOf rdf:resource="https://w3id.org/leo/onto/ale/involvesCompany"/>
        <rdfs:domain rdf:resource="https://w3id.org/leo/onto/ale/Slaughter"/>
        <rdfs:range rdf:resource="https://w3id.org/leo/onto/co/Slaughterhouse"/>
        <rdfs:comment xml:lang="en">Association between the slaughter life event and the slaughterhouse that executes the slaughter</rdfs:comment>
        <rdfs:comment xml:lang="it">Relazione tra l&apos;evento di macellazione e il macello che esegue la macellazione.</rdfs:comment>
        <rdfs:isDefinedBy rdf:resource="https://w3id.org/leo/onto/ale"/>
        <rdfs:label xml:lang="en">carried out by slaughterhouse</rdfs:label>
        <rdfs:label xml:lang="it">eseguita da macello</rdfs:label>
        <owl:versionInfo xml:lang="it">stabile - introdotta nella versione 0.3 dell&apos;ontologia</owl:versionInfo>
        <owl:versionInfo xml:lang="en">stable - introduced in version 0.3 of the ontology</owl:versionInfo>
    </owl:ObjectProperty>
    


    <!-- https://w3id.org/leo/onto/ale/happensIn -->

    <owl:ObjectProperty rdf:about="https://w3id.org/leo/onto/ale/happensIn">
        <rdfs:domain rdf:resource="https://w3id.org/leo/onto/ale/AnimalLifeEvent"/>
        <rdfs:range rdf:resource="https://w3id.org/leo/onto/co/Site"/>
        <rdfs:comment xml:lang="en">Property that links the animal life event to the rural site where the event occured.</rdfs:comment>
        <rdfs:comment xml:lang="it">Proprietà che lega l&apos;evento della vita dell&apos;animale con l&apos;ambiente rurale dove l&apos;evento è avvenuto.</rdfs:comment>
        <rdfs:isDefinedBy rdf:resource="https://w3id.org/leo/onto/ale"/>
        <rdfs:label xml:lang="it">avviene in</rdfs:label>
        <rdfs:label xml:lang="en">happens in</rdfs:label>
        <owl:versionInfo xml:lang="it">stabile</owl:versionInfo>
        <owl:versionInfo xml:lang="en">stable</owl:versionInfo>
    </owl:ObjectProperty>
    


    <!-- https://w3id.org/leo/onto/ale/hasAbortionType -->

    <owl:ObjectProperty rdf:about="https://w3id.org/leo/onto/ale/hasAbortionType">
        <rdfs:domain rdf:resource="https://w3id.org/leo/onto/ale/Abortion"/>
        <rdfs:range rdf:resource="https://w3id.org/leo/onto/ale/AbortionType"/>
        <rdfs:comment xml:lang="en">Property that links the abortion animal life event with the type of abortion (belated, premature).</rdfs:comment>
        <rdfs:comment xml:lang="it">Proprietà che lega l&apos;evento della vita dell&apos;animale aborto ocn il tipo di aborto, tardivo o precoce.</rdfs:comment>
        <rdfs:isDefinedBy rdf:resource="https://w3id.org/leo/onto/ale"/>
        <rdfs:label xml:lang="it">ha tipo di aborto</rdfs:label>
        <rdfs:label xml:lang="en">has abortion type</rdfs:label>
        <owl:versionInfo xml:lang="it">stabile - introdotta nella versione 0.4 dell&apos;ontologia</owl:versionInfo>
        <owl:versionInfo xml:lang="en">stable - introduced in version 0.4 of the ontology</owl:versionInfo>
    </owl:ObjectProperty>
    


    <!-- https://w3id.org/leo/onto/ale/hasAnimalBirthCompany -->

    <owl:ObjectProperty rdf:about="https://w3id.org/leo/onto/ale/hasAnimalBirthCompany">
        <rdfs:subPropertyOf rdf:resource="https://w3id.org/leo/onto/ale/involvesCompany"/>
        <rdfs:domain rdf:resource="https://w3id.org/leo/onto/ale/Birth"/>
        <rdfs:range rdf:resource="https://w3id.org/leo/onto/co/LivestockFarm"/>
        <rdfs:comment xml:lang="en">Property used to link the birth life event to the birth company of the farm animal.</rdfs:comment>
        <rdfs:comment xml:lang="it">Proprietà che lega la nascita all&apos;azienda di nascita dell&apos;animale d&apos;allevamento.</rdfs:comment>
        <rdfs:isDefinedBy rdf:resource="https://w3id.org/leo/onto/ale"/>
        <rdfs:label xml:lang="it">ha azienda di nascita</rdfs:label>
        <rdfs:label xml:lang="en">has animal birth company</rdfs:label>
        <owl:versionInfo xml:lang="it">stabile - introdotta nella versione 0.4 dell&apos;ontologia</owl:versionInfo>
        <owl:versionInfo>stable - introduced in version 0.4 of the ontology</owl:versionInfo>
    </owl:ObjectProperty>
    


    <!-- https://w3id.org/leo/onto/ale/hasAnimalBirthWeight -->

    <owl:ObjectProperty rdf:about="https://w3id.org/leo/onto/ale/hasAnimalBirthWeight">
        <rdfs:subPropertyOf rdf:resource="https://w3id.org/leo/onto/ale/hasWeight"/>
        <rdfs:domain rdf:resource="https://w3id.org/leo/onto/ale/Birth"/>
        <rdfs:range rdf:resource="https://w3id.org/italia/onto/MU/Value"/>
        <rdfs:comment xml:lang="en">Association between the birth event and the weight of the farm animal when it was born</rdfs:comment>
        <rdfs:comment xml:lang="it">Associazione tra l&apos;evento nascita e il peso alla nascita dell&apos;animale.</rdfs:comment>
        <rdfs:isDefinedBy rdf:resource="https://w3id.org/leo/onto/ale"/>
        <rdfs:label xml:lang="it">ha peso dell&apos;animale alla nascita</rdfs:label>
        <rdfs:label xml:lang="en">has animal birth weight</rdfs:label>
        <owl:versionInfo xml:lang="it">stabile - introdotta in versione 0.3 dell&apos;ontologia</owl:versionInfo>
        <owl:versionInfo xml:lang="en">stable - introduced in version 0.3 of the ontology</owl:versionInfo>
    </owl:ObjectProperty>
    


    <!-- https://w3id.org/leo/onto/ale/hasAnimalDestinationCompany -->

    <owl:ObjectProperty rdf:about="https://w3id.org/leo/onto/ale/hasAnimalDestinationCompany">
        <rdfs:subPropertyOf rdf:resource="https://w3id.org/leo/onto/ale/involvesCompany"/>
        <rdfs:domain rdf:resource="https://w3id.org/leo/onto/ale/OutboundMovement"/>
        <rdfs:range rdf:resource="https://w3id.org/leo/onto/co/LivestockFarm"/>
        <rdfs:comment xml:lang="en">Property that allows one to specify the destination company for the farm animal.</rdfs:comment>
        <rdfs:comment xml:lang="it">Proprietà che consente di specificare l&apos;azienda di destinazione dell&apos;animale d&apos;allevamento.</rdfs:comment>
        <rdfs:isDefinedBy rdf:resource="https://w3id.org/leo/onto/ale"/>
        <rdfs:label xml:lang="it">ha azienda di destinazione</rdfs:label>
        <rdfs:label xml:lang="en">has animal destination company</rdfs:label>
        <owl:versionInfo xml:lang="it">stabile - introdotta nella versione 0.4 dell&apos;ontologia</owl:versionInfo>
        <owl:versionInfo xml:lang="en">stable - introduced in version 0.4 of the ontology</owl:versionInfo>
    </owl:ObjectProperty>
    


    <!-- https://w3id.org/leo/onto/ale/hasAnimalLifeEvent -->

    <owl:ObjectProperty rdf:about="https://w3id.org/leo/onto/ale/hasAnimalLifeEvent">
        <owl:inverseOf rdf:resource="https://w3id.org/leo/onto/ale/involvesFarmAnimal"/>
        <rdfs:domain rdf:resource="https://w3id.org/leo/onto/animal/FarmAnimal"/>
        <rdfs:range rdf:resource="https://w3id.org/leo/onto/ale/AnimalLifeEvent"/>
        <rdfs:comment xml:lang="en">Property that links the farm animal to the animal life events.</rdfs:comment>
        <rdfs:comment xml:lang="it">Proprietà che lega l&apos;animale  agli eventi della vita che gli possono accadere.</rdfs:comment>
        <rdfs:isDefinedBy rdf:resource="https://w3id.org/leo/onto/ale"/>
        <rdfs:label xml:lang="it">ha evento della vita dell&apos;animale</rdfs:label>
        <rdfs:label xml:lang="en">has animal life event</rdfs:label>
        <owl:versionInfo xml:lang="it">stabile</owl:versionInfo>
        <owl:versionInfo xml:lang="en">stable</owl:versionInfo>
    </owl:ObjectProperty>
    


    <!-- https://w3id.org/leo/onto/ale/hasAnimalLiveWeight -->

    <owl:ObjectProperty rdf:about="https://w3id.org/leo/onto/ale/hasAnimalLiveWeight">
        <rdfs:subPropertyOf rdf:resource="https://w3id.org/leo/onto/ale/hasWeight"/>
        <rdfs:domain rdf:resource="https://w3id.org/leo/onto/ale/Slaughter"/>
        <rdfs:range rdf:resource="https://w3id.org/italia/onto/MU/Value"/>
        <rdfs:comment xml:lang="en">Association between the slaughter event and the live weight of the animal subject to slaughter</rdfs:comment>
        <rdfs:comment xml:lang="it">Associazione tra l&apos;evento macellazione e il peso vivo dell&apos;animale soggetto alla macellazione.</rdfs:comment>
        <rdfs:isDefinedBy rdf:resource="https://w3id.org/leo/onto/ale"/>
        <rdfs:label xml:lang="it">ha peso vivo dell&apos;animale</rdfs:label>
        <rdfs:label xml:lang="en">has animal live weight</rdfs:label>
        <owl:versionInfo xml:lang="it">stabile - introdotta nella versione 0.3 dell&apos;ontologia</owl:versionInfo>
        <owl:versionInfo xml:lang="en">stable - introduced in version 0.3 of the ontology</owl:versionInfo>
    </owl:ObjectProperty>
    


    <!-- https://w3id.org/leo/onto/ale/hasAnimalOwnerCompany -->

    <owl:ObjectProperty rdf:about="https://w3id.org/leo/onto/ale/hasAnimalOwnerCompany">
        <rdfs:subPropertyOf rdf:resource="https://w3id.org/leo/onto/ale/involvesCompany"/>
        <rdfs:domain>
            <owl:Class>
                <owl:unionOf rdf:parseType="Collection">
                    <rdf:Description rdf:about="https://w3id.org/leo/onto/ale/InboundMovement"/>
                    <rdf:Description rdf:about="https://w3id.org/leo/onto/ale/OutboundMovement"/>
                </owl:unionOf>
            </owl:Class>
        </rdfs:domain>
        <rdfs:range rdf:resource="https://w3id.org/leo/onto/co/LivestockFarm"/>
        <rdfs:comment xml:lang="en">Property that allows one to specify the owner company for the farm animal in some of its life events.</rdfs:comment>
        <rdfs:comment xml:lang="it">Proprietà che consente di specificare l&apos;azienda proprietaria dell&apos;animale d&apos;allevamento per alcuni suoi eventi della vita.</rdfs:comment>
        <rdfs:isDefinedBy rdf:resource="https://w3id.org/leo/onto/ale"/>
        <rdfs:label xml:lang="it">ha azienda proprietaria</rdfs:label>
        <rdfs:label xml:lang="en">has animal owner company</rdfs:label>
        <owl:versionInfo xml:lang="it">stabile - introdotta nella versione 0.4 dell&apos;ontologia</owl:versionInfo>
        <owl:versionInfo xml:lang="en">stable - introduced in version 0.4 of the ontology</owl:versionInfo>
    </owl:ObjectProperty>
    


    <!-- https://w3id.org/leo/onto/ale/hasAnimalProvenanceCompany -->

    <owl:ObjectProperty rdf:about="https://w3id.org/leo/onto/ale/hasAnimalProvenanceCompany">
        <rdfs:subPropertyOf rdf:resource="https://w3id.org/leo/onto/ale/involvesCompany"/>
        <rdfs:domain>
            <owl:Class>
                <owl:unionOf rdf:parseType="Collection">
                    <rdf:Description rdf:about="https://w3id.org/leo/onto/ale/InboundMovement"/>
                    <rdf:Description rdf:about="https://w3id.org/leo/onto/ale/Slaughter"/>
                </owl:unionOf>
            </owl:Class>
        </rdfs:domain>
        <rdfs:range rdf:resource="https://w3id.org/leo/onto/co/LivestockFarm"/>
        <rdfs:comment xml:lang="en">Property that links the event of slaughter and inbound movement with the farm company of origin of the animal.</rdfs:comment>
        <rdfs:comment xml:lang="it">Proprietà che lega l&apos;evento della macellazione e spostamento in entrata con l&apos;azienda di provenienza dell&apos;animale.</rdfs:comment>
        <rdfs:isDefinedBy rdf:resource="https://w3id.org/leo/onto/ale"/>
        <rdfs:label xml:lang="it">ha azienda di provenienza dell&apos;animale</rdfs:label>
        <rdfs:label xml:lang="en">has animal provenance company</rdfs:label>
        <owl:versionInfo xml:lang="it">stabile  - introdotta nella versione 0.3 dell&apos;ontologia</owl:versionInfo>
        <owl:versionInfo xml:lang="en">stable - introduced in version 0.3 of the ontology</owl:versionInfo>
    </owl:ObjectProperty>
    


    <!-- https://w3id.org/leo/onto/ale/hasAnimalProvenanceCountry -->

    <owl:ObjectProperty rdf:about="https://w3id.org/leo/onto/ale/hasAnimalProvenanceCountry">
        <rdfs:domain rdf:resource="https://w3id.org/leo/onto/ale/Slaughter"/>
        <rdfs:range rdf:resource="http://www.w3.org/2004/02/skos/core#Concept"/>
        <rdfs:comment xml:lang="en">Relationship between the slaughter event and the country of origin of the animal subject to slaughter. In essence, this is the country where the last farm company from which the animal came is located.</rdfs:comment>
        <rdfs:comment xml:lang="it">Relazione tra l&apos;evento di macellazione e il paese di provenienza dell&apos;animale soggetto a macellazione. In sostanza è  il paese dove è sita l’ultima azienda da cui proviene l’animale.</rdfs:comment>
        <rdfs:isDefinedBy rdf:resource="https://w3id.org/leo/onto/ale"/>
        <rdfs:label xml:lang="it">ha paese di provenienza dell&apos;animale</rdfs:label>
        <rdfs:label xml:lang="en">has animal provenance country</rdfs:label>
        <owl:versionInfo xml:lang="it">stabile - introdotta nella versione 0.3 dell&apos;ontologia</owl:versionInfo>
        <owl:versionInfo xml:lang="en">stable - introduced in version 0.3 of the ontology</owl:versionInfo>
    </owl:ObjectProperty>
    


    <!-- https://w3id.org/leo/onto/ale/hasArtificialBreastFeedingDuration -->

    <owl:ObjectProperty rdf:about="https://w3id.org/leo/onto/ale/hasArtificialBreastFeedingDuration">
        <rdfs:subPropertyOf rdf:resource="https://w3id.org/italia/onto/TI/hasDuration"/>
        <rdfs:domain rdf:resource="https://w3id.org/leo/onto/ale/Weaning"/>
        <rdfs:range rdf:resource="https://w3id.org/italia/onto/TI/Duration"/>
        <rdfs:comment xml:lang="en">Property that allows one to specify the duration, typically in days, of artificial feeding in a weaning animal life event.</rdfs:comment>
        <rdfs:comment xml:lang="it">Proprietà che consente di specificare, per lo svezzamento, la durata, tipicamente in giorni, dell&apos;allattamento artificiale.</rdfs:comment>
        <rdfs:isDefinedBy rdf:resource="https://w3id.org/leo/onto/ale"/>
        <rdfs:label xml:lang="it">ha durata dell&apos;allattamento artificiale</rdfs:label>
        <rdfs:label xml:lang="it">has artificial breast feeding duration</rdfs:label>
        <owl:versionInfo xml:lang="it">stabile</owl:versionInfo>
        <owl:versionInfo xml:lang="en">stable</owl:versionInfo>
    </owl:ObjectProperty>
    


    <!-- https://w3id.org/leo/onto/ale/hasAvgMilkConductivity -->

    <owl:ObjectProperty rdf:about="https://w3id.org/leo/onto/ale/hasAvgMilkConductivity">
        <rdfs:domain rdf:resource="https://w3id.org/leo/onto/ale/MilkConductivityMeasurement"/>
        <rdfs:range rdf:resource="https://w3id.org/italia/onto/MU/Value"/>
        <rdfs:comment xml:lang="en">Property that links the measurement of the milk conductivity to its average value.</rdfs:comment>
        <rdfs:comment xml:lang="it">Proprietà che collega la misurazione della conduttività del latte al suo valore medio.</rdfs:comment>
        <rdfs:isDefinedBy rdf:resource="https://w3id.org/leo/onto/ale"/>
        <rdfs:label xml:lang="it">ha conducibilità latte media</rdfs:label>
        <rdfs:label xml:lang="en">has average milk conductivity</rdfs:label>
        <owl:versionInfo xml:lang="it">stabile</owl:versionInfo>
        <owl:versionInfo xml:lang="en">stable</owl:versionInfo>
    </owl:ObjectProperty>
    


    <!-- https://w3id.org/leo/onto/ale/hasBackFatThicknessValue -->

    <owl:ObjectProperty rdf:about="https://w3id.org/leo/onto/ale/hasBackFatThicknessValue">
        <rdfs:domain rdf:resource="https://w3id.org/leo/onto/ale/BackFatThicknessMeasurement"/>
        <rdfs:range rdf:resource="https://w3id.org/italia/onto/MU/Value"/>
    </owl:ObjectProperty>
    


    <!-- https://w3id.org/leo/onto/ale/hasBreastFeedingType -->

    <owl:ObjectProperty rdf:about="https://w3id.org/leo/onto/ale/hasBreastFeedingType">
        <rdfs:domain rdf:resource="https://w3id.org/leo/onto/ale/Weaning"/>
        <rdfs:range rdf:resource="https://w3id.org/leo/onto/ale/BreastFeedingType"/>
        <rdfs:comment xml:lang="en">Property linking weaning with the type of breastfeeding (artificial, natural, mixed).</rdfs:comment>
        <rdfs:comment xml:lang="it">Proprietà che collega lo svezzamento con la tipologia di allattamento (artificiale, naturale, misto).</rdfs:comment>
        <rdfs:isDefinedBy rdf:resource="https://w3id.org/leo/onto/ale"/>
        <rdfs:label xml:lang="it">ha tipo allattamento</rdfs:label>
        <rdfs:label xml:lang="en">has breast feeding type</rdfs:label>
        <owl:versionInfo xml:lang="it">stabile</owl:versionInfo>
        <owl:versionInfo xml:lang="en">stable</owl:versionInfo>
    </owl:ObjectProperty>
    


    <!-- https://w3id.org/leo/onto/ale/hasBreastFeedingWithNurseDuration -->

    <owl:ObjectProperty rdf:about="https://w3id.org/leo/onto/ale/hasBreastFeedingWithNurseDuration">
        <rdfs:subPropertyOf rdf:resource="https://w3id.org/italia/onto/TI/hasDuration"/>
        <rdfs:domain rdf:resource="https://w3id.org/leo/onto/ale/Weaning"/>
        <rdfs:range rdf:resource="https://w3id.org/italia/onto/TI/Duration"/>
        <rdfs:comment xml:lang="en">Property that allows one to specify the duration, typically in days, of breast feeding with nurse in a weaning animal life event.</rdfs:comment>
        <rdfs:comment xml:lang="it">Proprietà che consente di specificare, per lo svezzamento, la durata, tipicamente in giorni, dell&apos;allattamento con balia.</rdfs:comment>
        <rdfs:isDefinedBy rdf:resource="https://w3id.org/leo/onto/ale"/>
        <rdfs:label xml:lang="it">ha durata dell&apos;allattamento con balia</rdfs:label>
        <rdfs:label xml:lang="en">has breast feeding with nurse duration</rdfs:label>
        <owl:versionInfo xml:lang="it">stabile</owl:versionInfo>
        <owl:versionInfo xml:lang="en">stable</owl:versionInfo>
    </owl:ObjectProperty>
    


    <!-- https://w3id.org/leo/onto/ale/hasBreederBreed -->

    <owl:ObjectProperty rdf:about="https://w3id.org/leo/onto/ale/hasBreederBreed">
        <rdfs:domain>
            <owl:Class>
                <owl:unionOf rdf:parseType="Collection">
                    <rdf:Description rdf:about="https://w3id.org/leo/onto/ale/Fertilization"/>
                    <rdf:Description rdf:about="https://w3id.org/leo/onto/ale/Implantation"/>
                </owl:unionOf>
            </owl:Class>
        </rdfs:domain>
        <rdfs:range rdf:resource="https://w3id.org/leo/onto/animal/Breed"/>
        <rdfs:comment xml:lang="en">Property that links the fertilisation or implantation events to the breed of the breeder that is reported in the events. The breed of the breeder is the breed of the male used for the fertilization</rdfs:comment>
        <rdfs:comment xml:lang="it">Proprietà che lega gli eventi di fecondazione o impianto alla razza del riproduttore che viene riportata negli eventi. La razza del riproduttore è la razza del maschio utilizzato per la fecondazione</rdfs:comment>
        <rdfs:isDefinedBy rdf:resource="https://w3id.org/leo/onto/ale"/>
        <rdfs:label xml:lang="it">ha razza riproduttore</rdfs:label>
        <rdfs:label xml:lang="en">has breeder breed</rdfs:label>
        <owl:versionInfo xml:lang="it">stabile - cambiato nome nella versione 0.4 in ha razza riproduttore</owl:versionInfo>
        <owl:versionInfo xml:lang="en">stable - changed the name in hasBreederBreed in version 0.4</owl:versionInfo>
    </owl:ObjectProperty>
    


    <!-- https://w3id.org/leo/onto/ale/hasCarcassCategory -->

    <owl:ObjectProperty rdf:about="https://w3id.org/leo/onto/ale/hasCarcassCategory">
        <rdfs:domain rdf:resource="https://w3id.org/leo/onto/ale/FarmAnimalCarcass"/>
        <rdfs:range rdf:resource="https://w3id.org/leo/onto/ale/CarcassCategory"/>
        <rdfs:comment xml:lang="en">Association between the farm animal carcass and its category</rdfs:comment>
        <rdfs:comment xml:lang="it">Relazione che lega la carcassa dell&apos;animale d&apos;allevamento alla sua categoria</rdfs:comment>
        <rdfs:isDefinedBy rdf:resource="https://w3id.org/leo/onto/ale"/>
        <rdfs:label xml:lang="it">ha categoria carcassa</rdfs:label>
        <rdfs:label xml:lang="en">has carcass category</rdfs:label>
        <owl:versionInfo xml:lang="it">stabile - introdotta nella versione 0.3 dell&apos;ontologia</owl:versionInfo>
        <owl:versionInfo xml:lang="en">stable  - introduced in version 0.3 of the ontology</owl:versionInfo>
    </owl:ObjectProperty>
    


    <!-- https://w3id.org/leo/onto/ale/hasCarcassClassification -->

    <owl:ObjectProperty rdf:about="https://w3id.org/leo/onto/ale/hasCarcassClassification">
        <rdfs:domain rdf:resource="https://w3id.org/leo/onto/ale/FarmAnimalCarcass"/>
        <rdfs:range rdf:resource="https://w3id.org/leo/onto/ale/CarcassClassification"/>
        <rdfs:comment xml:lang="en">Association between the farm animal carcass and its classification</rdfs:comment>
        <rdfs:comment xml:lang="it">Relazione tra la carcassa dell&apos;animale e la sua classificazione</rdfs:comment>
        <rdfs:isDefinedBy rdf:resource="https://w3id.org/leo/onto/ale"/>
        <rdfs:label xml:lang="it">ha classificazione carcassa</rdfs:label>
        <rdfs:label xml:lang="en">has carcass classification</rdfs:label>
        <owl:versionInfo xml:lang="it">stabile - introdotta nella versione 0.3 dell&apos;ontologia</owl:versionInfo>
        <owl:versionInfo xml:lang="en">stable  - introduced in version 0.3 of the ontology</owl:versionInfo>
    </owl:ObjectProperty>
    


    <!-- https://w3id.org/leo/onto/ale/hasCarcassWeight -->

    <owl:ObjectProperty rdf:about="https://w3id.org/leo/onto/ale/hasCarcassWeight">
        <rdfs:subPropertyOf rdf:resource="https://w3id.org/leo/onto/ale/hasWeight"/>
        <rdfs:domain rdf:resource="https://w3id.org/leo/onto/ale/FarmAnimalCarcass"/>
        <rdfs:range rdf:resource="https://w3id.org/italia/onto/MU/Value"/>
        <rdfs:comment xml:lang="en">Association between the farm animal carcass and its weight</rdfs:comment>
        <rdfs:comment xml:lang="it">Relazione tra la carcassa e il suo peso</rdfs:comment>
        <rdfs:isDefinedBy rdf:resource="https://w3id.org/leo/onto/ale"/>
        <rdfs:label xml:lang="it">ha peso carcassa</rdfs:label>
        <rdfs:label xml:lang="en">has carcass weight</rdfs:label>
        <owl:versionInfo xml:lang="it">stabile  - introdotta nella version 0.3 dell&apos;ontologia</owl:versionInfo>
        <owl:versionInfo xml:lang="en">stable - introduced in version 0.3 of the ontology</owl:versionInfo>
    </owl:ObjectProperty>
    


    <!-- https://w3id.org/leo/onto/ale/hasConstituent -->

    <owl:ObjectProperty rdf:about="https://w3id.org/leo/onto/ale/hasConstituent">
        <rdfs:domain rdf:resource="https://w3id.org/leo/onto/ale/CarcassClassification"/>
        <rdfs:range>
            <owl:Class>
                <owl:unionOf rdf:parseType="Collection">
                    <rdf:Description rdf:about="https://w3id.org/leo/onto/ale/CarcassConformation"/>
                    <rdf:Description rdf:about="https://w3id.org/leo/onto/ale/FatCover"/>
                </owl:unionOf>
            </owl:Class>
        </rdfs:range>
        <rdfs:comment xml:lang="en">Associate between the carcass classification with the elements that contribute to create it; that is, fat cover and carcass conformation</rdfs:comment>
        <rdfs:comment xml:lang="it">Relazione tra la classificazione delle carcasse e i suoi elementi costitutivi ossia lo stado d&apos;ingrassamento e la conformazione delle carcasse.</rdfs:comment>
        <rdfs:isDefinedBy rdf:resource="https://w3id.org/leo/onto/ale"/>
        <rdfs:label xml:lang="it">ha costituente</rdfs:label>
        <rdfs:label xml:lang="en">has constituent</rdfs:label>
        <owl:versionInfo xml:lang="it">stabile - introdotta nella versione 0.3 dell&apos;ontologia</owl:versionInfo>
        <owl:versionInfo xml:lang="en">stable - introduced in version 0.3 of the ontology</owl:versionInfo>
    </owl:ObjectProperty>
    


    <!-- https://w3id.org/leo/onto/ale/hasDisposalReason -->

    <owl:ObjectProperty rdf:about="https://w3id.org/leo/onto/ale/hasDisposalReason">
        <rdf:type rdf:resource="http://www.w3.org/2002/07/owl#FunctionalProperty"/>
        <rdfs:domain rdf:resource="https://w3id.org/leo/onto/ale/Disposal"/>
        <rdfs:range rdf:resource="https://w3id.org/leo/onto/ale/DisposalReason"/>
        <rdfs:comment xml:lang="en">Property that links the event of disposal of the animal to the reason for the disposal.</rdfs:comment>
        <rdfs:comment xml:lang="it">Proprietà che collega l&apos;evento dell&apos;eliminazione dell&apos;animale alla ragione per l&apos;eliminazione.</rdfs:comment>
        <rdfs:isDefinedBy rdf:resource="https://w3id.org/leo/onto/ale"/>
        <rdfs:label xml:lang="it">ha motivazione eliminazione</rdfs:label>
        <rdfs:label xml:lang="en">has disposal reason</rdfs:label>
        <owl:versionInfo xml:lang="it">stabile - aggiunto nella seconda versione dell&apos;ontologia</owl:versionInfo>
        <owl:versionInfo xml:lang="en">stable - added in the second version of the ontology</owl:versionInfo>
    </owl:ObjectProperty>
    


    <!-- https://w3id.org/leo/onto/ale/hasEaseOfParturition -->

    <owl:ObjectProperty rdf:about="https://w3id.org/leo/onto/ale/hasEaseOfParturition">
        <rdf:type rdf:resource="http://www.w3.org/2002/07/owl#FunctionalProperty"/>
        <rdfs:domain rdf:resource="https://w3id.org/leo/onto/ale/Parturition"/>
        <rdfs:range rdf:resource="https://w3id.org/leo/onto/ale/EaseOfParturition"/>
        <rdfs:comment xml:lang="en">Property that links the birth event to the reported ease of parturition, i.e. links the birth to the subjective assessment of the breeder or technician by which it is indicated whether the female gave birth without problems or needed assistance.</rdfs:comment>
        <rdfs:comment xml:lang="it">Proprietà che collega l&apos;evento del parto alla facilità di parto riportata, ovvero collega il parto  alla valutazione soggettiva dell’allevatore o del tecnico attraverso la quale viene indicato se la femmina ha partorito senza problemi o ha avuto bisogno di assistenza.</rdfs:comment>
        <rdfs:isDefinedBy rdf:resource="https://w3id.org/leo/onto/ale"/>
        <rdfs:label xml:lang="it">ha facilità parto</rdfs:label>
        <rdfs:label xml:lang="en">has ease of parturition</rdfs:label>
        <owl:versionInfo xml:lang="it">stabile</owl:versionInfo>
        <owl:versionInfo xml:lang="en">stable</owl:versionInfo>
    </owl:ObjectProperty>
    


    <!-- https://w3id.org/leo/onto/ale/hasEntryInFarmReason -->

    <owl:ObjectProperty rdf:about="https://w3id.org/leo/onto/ale/hasEntryInFarmReason">
        <rdfs:domain rdf:resource="https://w3id.org/leo/onto/ale/InboundMovement"/>
        <rdfs:range rdf:resource="https://w3id.org/leo/onto/ale/EntryInFarmReason"/>
        <rdfs:comment xml:lang="en">Association between the &apos;Inbound movement&apos; animal life event to the reason for the entry in farm.</rdfs:comment>
        <rdfs:comment xml:lang="it">Associazione tra l&apos;evento della vita dell&apos;animale d&apos;allevamento &apos;spostamento in entrata&apos; con le motivazioni per lo spostamento dell&apos;animale nell&apos;allevamento.</rdfs:comment>
        <rdfs:isDefinedBy rdf:resource="https://w3id.org/leo/onto/ale"/>
        <rdfs:label xml:lang="it">ha motivo ingresso allevamento</rdfs:label>
        <rdfs:label xml:lang="en">has entry in farm reason</rdfs:label>
        <owl:versionInfo xml:lang="it">stabile - introdotta nella versione 0.4 dell&apos;ontologia</owl:versionInfo>
        <owl:versionInfo xml:lang="en">stable - introduced in version 0.4 of the ontology</owl:versionInfo>
    </owl:ObjectProperty>
    


    <!-- https://w3id.org/leo/onto/ale/hasExitFromFarmReason -->

    <owl:ObjectProperty rdf:about="https://w3id.org/leo/onto/ale/hasExitFromFarmReason">
        <rdfs:domain rdf:resource="https://w3id.org/leo/onto/ale/OutboundMovement"/>
        <rdfs:range rdf:resource="https://w3id.org/leo/onto/ale/ExitFromFarmReason"/>
        <rdfs:comment xml:lang="en">Association between the animal life event &apos;outbound movement&apos; to the reasons for the exit from farm.</rdfs:comment>
        <rdfs:comment xml:lang="it">Associazione tra l&apos;evento della vita dell&apos;animale d&apos;allevamento &apos;spostamento in uscita&apos; con le motivazioni per il suo spostamento in uscita dall&apos;allevamento</rdfs:comment>
        <rdfs:isDefinedBy rdf:resource="https://w3id.org/leo/onto/ale"/>
        <rdfs:label xml:lang="it">ha motivo d&apos;uscita allevamento</rdfs:label>
        <rdfs:label xml:lang="en">has exit from farm reason</rdfs:label>
        <owl:versionInfo xml:lang="it">stabile - introdotta nella versione 0.4 dell&apos;ontologia</owl:versionInfo>
        <owl:versionInfo xml:lang="en">stable - introduced in version 0.4 of the ontology</owl:versionInfo>
    </owl:ObjectProperty>
    


    <!-- https://w3id.org/leo/onto/ale/hasFertilizationType -->

    <owl:ObjectProperty rdf:about="https://w3id.org/leo/onto/ale/hasFertilizationType">
        <rdf:type rdf:resource="http://www.w3.org/2002/07/owl#FunctionalProperty"/>
        <rdfs:domain rdf:resource="https://w3id.org/leo/onto/ale/Fertilization"/>
        <rdfs:range rdf:resource="https://w3id.org/leo/onto/ale/FertilizationType"/>
        <rdfs:comment xml:lang="en">Property that links the event Fertilization to the tyoe of fertilization that is carried out in the event</rdfs:comment>
        <rdfs:comment xml:lang="it">Proprietà che lega l&apos;evento della fecondazione/inseminazione al tipo di inseminazione/fecondazione svolta nell&apos;evento.</rdfs:comment>
        <rdfs:isDefinedBy rdf:resource="https://w3id.org/leo/onto/ale"/>
        <rdfs:label xml:lang="en">ha fertilization type</rdfs:label>
        <rdfs:label xml:lang="it">ha tipo inseminazione/fecondazione</rdfs:label>
        <owl:versionInfo xml:lang="it">stabile</owl:versionInfo>
        <owl:versionInfo xml:lang="en">stable</owl:versionInfo>
    </owl:ObjectProperty>
    


    <!-- https://w3id.org/leo/onto/ale/hasMilkYield -->

    <owl:ObjectProperty rdf:about="https://w3id.org/leo/onto/ale/hasMilkYield">
        <rdfs:domain rdf:resource="https://w3id.org/leo/onto/ale/MilkingSession"/>
        <rdfs:range rdf:resource="https://w3id.org/italia/onto/MU/Value"/>
        <rdfs:comment xml:lang="en">Property linking the milking session to the amount of milk produced (in hectograms (hg)).</rdfs:comment>
        <rdfs:comment xml:lang="it">Proprietà che lega la sessione di mungitura alla quantità di latte prodotto (in ettogrammi (hg)).</rdfs:comment>
        <rdfs:isDefinedBy rdf:resource="https://w3id.org/leo/onto/ale"/>
        <rdfs:label xml:lang="it">ha produzione latte (mungitura)</rdfs:label>
        <rdfs:label xml:lang="en">has milk yield</rdfs:label>
        <owl:versionInfo xml:lang="it">stabile</owl:versionInfo>
        <owl:versionInfo xml:lang="en">stable</owl:versionInfo>
    </owl:ObjectProperty>
    


    <!-- https://w3id.org/leo/onto/ale/hasPregnancyResult -->

    <owl:ObjectProperty rdf:about="https://w3id.org/leo/onto/ale/hasPregnancyResult">
        <rdfs:domain rdf:resource="https://w3id.org/leo/onto/ale/PregnancyDiagnosis"/>
        <rdfs:range rdf:resource="https://w3id.org/leo/onto/ale/PregnancyResult"/>
        <rdfs:comment xml:lang="en">Property that links the specific pregnancy diagnosis event to the obtained results.</rdfs:comment>
        <rdfs:comment xml:lang="it">Proprietà che collega lo specifico evento di diagnosi gravidanza ai risultati ottenuti.</rdfs:comment>
        <rdfs:isDefinedBy rdf:resource="https://w3id.org/leo/onto/ale"/>
        <rdfs:label xml:lang="it">ha esito della diagnosi di gravidanza</rdfs:label>
        <rdfs:label xml:lang="en">has pregnancy result</rdfs:label>
        <owl:versionInfo xml:lang="it">stabile</owl:versionInfo>
        <owl:versionInfo xml:lang="en">stable</owl:versionInfo>
    </owl:ObjectProperty>
    


    <!-- https://w3id.org/leo/onto/ale/hasWeight -->

    <owl:ObjectProperty rdf:about="https://w3id.org/leo/onto/ale/hasWeight">
        <rdfs:domain rdf:resource="https://w3id.org/italia/onto/l0/Entity"/>
        <rdfs:range rdf:resource="https://w3id.org/italia/onto/MU/Value"/>
        <rdfs:comment xml:lang="en">A general property that allows one to specify the weight in situations (e.g., the detected weight of the animal during the weighing, the weight of the animal during the birth, etc. ) or the weight of specific entities (e.g., the weight of the carcass of a farm animal).</rdfs:comment>
        <rdfs:comment xml:lang="it">Una proprietà generale che consente di specificare il peso in eventi della vita dell&apos;animale (ad esempio, il peso rilevato dell&apos;animale durante la pesatura, il peso dell&apos;animale alla nascita, ecc.) o il peso di entità specifiche (ad esempio, il peso della carcassa di un animale da allevamento).</rdfs:comment>
        <rdfs:isDefinedBy rdf:resource="https://w3id.org/leo/onto/ale"/>
        <rdfs:label xml:lang="it">ha peso</rdfs:label>
        <rdfs:label xml:lang="en">has weight</rdfs:label>
        <owl:versionInfo xml:lang="it">stabile</owl:versionInfo>
        <owl:versionInfo xml:lang="en">stable</owl:versionInfo>
    </owl:ObjectProperty>
    


    <!-- https://w3id.org/leo/onto/ale/involvesCompany -->

    <owl:ObjectProperty rdf:about="https://w3id.org/leo/onto/ale/involvesCompany">
        <owl:inverseOf rdf:resource="https://w3id.org/leo/onto/ale/isInvolvedInEvent"/>
        <rdfs:domain rdf:resource="https://w3id.org/leo/onto/ale/AnimalLifeEvent"/>
        <rdfs:range rdf:resource="https://w3id.org/leo/onto/co/LivestockCompany"/>
        <rdfs:comment xml:lang="en">Property that links the animal life event to the company in which it occurs.</rdfs:comment>
        <rdfs:comment xml:lang="it">Proprietà che collega l&apos;evento della vita dell&apos;animale all&apos;azienda in cui avviene.</rdfs:comment>
        <rdfs:isDefinedBy rdf:resource="https://w3id.org/leo/onto/ale"/>
        <rdfs:label xml:lang="it">coinvolge azienda</rdfs:label>
        <rdfs:label xml:lang="en">involves company</rdfs:label>
        <owl:versionInfo xml:lang="it">stabile</owl:versionInfo>
        <owl:versionInfo xml:lang="en">stable</owl:versionInfo>
    </owl:ObjectProperty>
    


    <!-- https://w3id.org/leo/onto/ale/involvesFarmAnimal -->

    <owl:ObjectProperty rdf:about="https://w3id.org/leo/onto/ale/involvesFarmAnimal">
        <rdfs:domain rdf:resource="https://w3id.org/leo/onto/ale/AnimalLifeEvent"/>
        <rdfs:range rdf:resource="https://w3id.org/leo/onto/animal/FarmAnimal"/>
        <rdfs:comment xml:lang="en">Inverse property of &quot;has animal life event&quot; that links the animal life event to the animal itself.</rdfs:comment>
        <rdfs:comment xml:lang="it">Proprietà inversa di &quot;ha evento della vita dell&apos;animale&quot; che collega l&apos;evento della vita dell&apos;animale all&apos;animale stesso.</rdfs:comment>
        <rdfs:isDefinedBy rdf:resource="https://w3id.org/leo/onto/ale"/>
        <rdfs:label xml:lang="it">coinvolge animale di allevamento</rdfs:label>
        <rdfs:label xml:lang="en">involves farm animal</rdfs:label>
        <owl:versionInfo xml:lang="it">stabile</owl:versionInfo>
        <owl:versionInfo xml:lang="en">stable</owl:versionInfo>
    </owl:ObjectProperty>
    


    <!-- https://w3id.org/leo/onto/ale/isCarcassOf -->

    <owl:ObjectProperty rdf:about="https://w3id.org/leo/onto/ale/isCarcassOf">
        <rdfs:domain rdf:resource="https://w3id.org/leo/onto/ale/FarmAnimalCarcass"/>
        <rdfs:range rdf:resource="https://w3id.org/leo/onto/animal/FarmAnimal"/>
        <rdfs:comment xml:lang="en">Association between the farm animal carcass to the animal itself</rdfs:comment>
        <rdfs:comment xml:lang="it">Relazione che lega la carcassa all&apos;animale d&apos;allevamento.</rdfs:comment>
        <rdfs:isDefinedBy rdf:resource="https://w3id.org/leo/onto/ale"/>
        <rdfs:label xml:lang="en">is carcass of</rdfs:label>
        <rdfs:label xml:lang="it">è carcassa di</rdfs:label>
        <owl:versionInfo xml:lang="it">stabile - introdotta nella versione 0.3 dell&apos;ontologia</owl:versionInfo>
        <owl:versionInfo xml:lang="en">stable - introduced in version 0.3 of the ontology</owl:versionInfo>
    </owl:ObjectProperty>
    


    <!-- https://w3id.org/leo/onto/ale/isInvolvedInEvent -->

    <owl:ObjectProperty rdf:about="https://w3id.org/leo/onto/ale/isInvolvedInEvent">
        <rdfs:domain rdf:resource="https://w3id.org/leo/onto/co/LivestockCompany"/>
        <rdfs:range rdf:resource="https://w3id.org/leo/onto/ale/AnimalLifeEvent"/>
        <rdfs:comment xml:lang="en">Inverse property of &quot;involces company&quot; that links the company with the animal life event.</rdfs:comment>
        <rdfs:comment xml:lang="it">Proprietà inversa di &quot;coinvolge azienda&quot; che lega l&apos;azienda all&apos;evento della vita dell&apos;animale.</rdfs:comment>
        <rdfs:isDefinedBy rdf:resource="https://w3id.org/leo/onto/ale"/>
        <rdfs:label xml:lang="en">is involved in event</rdfs:label>
        <rdfs:label xml:lang="it">è coinvolta in evento</rdfs:label>
        <owl:versionInfo xml:lang="it">stabile</owl:versionInfo>
        <owl:versionInfo xml:lang="en">stable</owl:versionInfo>
    </owl:ObjectProperty>
    


    <!-- https://w3id.org/leo/onto/ale/measuredForFarmAnimal -->

    <owl:ObjectProperty rdf:about="https://w3id.org/leo/onto/ale/measuredForFarmAnimal">
        <rdfs:domain rdf:resource="https://w3id.org/leo/onto/ale/MilkConductivityMeasurement"/>
        <rdfs:range rdf:resource="https://w3id.org/leo/onto/animal/FarmAnimal"/>
        <rdfs:comment xml:lang="en">Property linking the measurement of average milk conductivity to the farm animal</rdfs:comment>
        <rdfs:comment xml:lang="it">Proprietà che lega la misurazione della conducibilità media del latte all&apos;animale d&apos;allevamento</rdfs:comment>
        <rdfs:isDefinedBy rdf:resource="https://w3id.org/leo/onto/ale"/>
        <rdfs:label xml:lang="en">measured for farm animal</rdfs:label>
        <rdfs:label xml:lang="it">misurata per animale d&apos;allevamento</rdfs:label>
        <owl:versionInfo xml:lang="it">stabile</owl:versionInfo>
        <owl:versionInfo xml:lang="en">stable</owl:versionInfo>
    </owl:ObjectProperty>
    


    <!-- https://w3id.org/leo/onto/ale/producesCarcass -->

    <owl:ObjectProperty rdf:about="https://w3id.org/leo/onto/ale/producesCarcass">
        <rdfs:domain rdf:resource="https://w3id.org/leo/onto/ale/Slaughter"/>
        <rdfs:range rdf:resource="https://w3id.org/leo/onto/ale/FarmAnimalCarcass"/>
        <rdfs:comment xml:lang="en">Association between the slaughter life event and the carcass of the farm animal produced by the slaughter process.</rdfs:comment>
        <rdfs:comment xml:lang="it">Relazione tra l&apos;evento macellazione e la carcassa dell&apos;animale che è prodotta dal processo di macellazione.</rdfs:comment>
        <rdfs:isDefinedBy rdf:resource="https://w3id.org/leo/onto/ale"/>
        <rdfs:label xml:lang="it">produce carcassa</rdfs:label>
        <rdfs:label xml:lang="en">produces carcass</rdfs:label>
        <owl:versionInfo xml:lang="it">stabile - introdotta nelal versione 0.3 dell&apos;ontologia.</owl:versionInfo>
        <owl:versionInfo xml:lang="en">stable - introduced in version 0.3 of the ontology</owl:versionInfo>
    </owl:ObjectProperty>
    


    <!-- https://w3id.org/leo/onto/ale/withinMilkingSession -->

    <owl:ObjectProperty rdf:about="https://w3id.org/leo/onto/ale/withinMilkingSession">
        <rdf:type rdf:resource="http://www.w3.org/2002/07/owl#FunctionalProperty"/>
        <rdfs:domain rdf:resource="https://w3id.org/leo/onto/ale/MilkConductivityMeasurement"/>
        <rdfs:range rdf:resource="https://w3id.org/leo/onto/ale/MilkingSession"/>
        <rdfs:comment xml:lang="en">Property linking the measurment of the milk conductivity to its milking session during which is measured.</rdfs:comment>
        <rdfs:comment xml:lang="it">Proprietà che collega la misurazione della conduttività del latte alla sessione di mungitura durante la quale viene misurata.</rdfs:comment>
        <rdfs:isDefinedBy rdf:resource="https://w3id.org/leo/onto/ale"/>
        <rdfs:label xml:lang="it">durante sessione di mungitura</rdfs:label>
        <rdfs:label xml:lang="en">within milking session</rdfs:label>
        <owl:versionInfo xml:lang="it">stabile</owl:versionInfo>
        <owl:versionInfo xml:lang="en">stable</owl:versionInfo>
    </owl:ObjectProperty>
    


    <!-- https://w3id.org/leo/onto/animal/hasAnimalDestination -->

    <owl:ObjectProperty rdf:about="https://w3id.org/leo/onto/animal/hasAnimalDestination"/>
    


    <!-- https://w3id.org/leo/onto/animal/hasBreed -->

    <owl:ObjectProperty rdf:about="https://w3id.org/leo/onto/animal/hasBreed"/>
    


    <!-- https://w3id.org/leo/onto/animal/hasProductionTarget -->

    <owl:ObjectProperty rdf:about="https://w3id.org/leo/onto/animal/hasProductionTarget"/>
    


    <!-- 
    ///////////////////////////////////////////////////////////////////////////////////////
    //
    // Data properties
    //
    ///////////////////////////////////////////////////////////////////////////////////////
     -->

    


    <!-- https://w3id.org/italia/onto/l0/identifier -->

    <owl:DatatypeProperty rdf:about="https://w3id.org/italia/onto/l0/identifier"/>
    


    <!-- https://w3id.org/leo/onto/ale/abortionDate -->

    <owl:DatatypeProperty rdf:about="https://w3id.org/leo/onto/ale/abortionDate">
        <rdfs:subPropertyOf rdf:resource="https://w3id.org/italia/onto/TI/date"/>
        <rdfs:domain rdf:resource="https://w3id.org/leo/onto/ale/Abortion"/>
        <rdfs:range>
            <rdfs:Datatype>
                <owl:unionOf rdf:parseType="Collection">
                    <rdf:Description rdf:about="http://www.w3.org/2001/XMLSchema#date"/>
                    <rdf:Description rdf:about="http://www.w3.org/2001/XMLSchema#dateTime"/>
                </owl:unionOf>
            </rdfs:Datatype>
        </rdfs:range>
        <rdfs:comment xml:lang="it">Data di espulsione del feto.</rdfs:comment>
        <rdfs:comment xml:lang="en">Date of expulsion of the foetus.</rdfs:comment>
        <rdfs:isDefinedBy rdf:resource="https://w3id.org/leo/onto/ale"/>
        <rdfs:label xml:lang="en">abortion date</rdfs:label>
        <rdfs:label xml:lang="it">data aborto</rdfs:label>
        <owl:versionInfo xml:lang="it">stabile</owl:versionInfo>
        <owl:versionInfo xml:lang="en">stable</owl:versionInfo>
    </owl:DatatypeProperty>
    


    <!-- https://w3id.org/leo/onto/ale/animalArrivedDeadAtSlaughterhouse -->

    <owl:DatatypeProperty rdf:about="https://w3id.org/leo/onto/ale/animalArrivedDeadAtSlaughterhouse">
        <rdf:type rdf:resource="http://www.w3.org/2002/07/owl#FunctionalProperty"/>
        <rdfs:domain rdf:resource="https://w3id.org/leo/onto/ale/Slaughter"/>
        <rdfs:range rdf:resource="http://www.w3.org/2001/XMLSchema#boolean"/>
        <rdfs:comment xml:lang="it">Indica se l&apos;animale è arrivato morto o meno al macello</rdfs:comment>
        <rdfs:comment xml:lang="en">It indicates whether the animal is arrived dead or not at slaughterhouse</rdfs:comment>
        <rdfs:isDefinedBy rdf:resource="https://w3id.org/leo/onto/ale"/>
        <rdfs:label xml:lang="en">animal arrived dead at slaughterhouse</rdfs:label>
        <rdfs:label xml:lang="it">animale arrivato morto al macello</rdfs:label>
        <owl:versionInfo xml:lang="it">stabile - introdotta nella versione 0.3 dell&apos;ontologia</owl:versionInfo>
        <owl:versionInfo xml:lang="en">stable - introduced in version 0.3 of the ontology</owl:versionInfo>
    </owl:DatatypeProperty>
    


    <!-- https://w3id.org/leo/onto/ale/bftMeasurementDate -->

    <owl:DatatypeProperty rdf:about="https://w3id.org/leo/onto/ale/bftMeasurementDate">
        <rdfs:subPropertyOf rdf:resource="https://w3id.org/italia/onto/TI/date"/>
        <rdfs:domain rdf:resource="https://w3id.org/leo/onto/ale/BackFatThicknessMeasurement"/>
        <rdfs:range>
            <rdfs:Datatype>
                <owl:unionOf rdf:parseType="Collection">
                    <rdf:Description rdf:about="http://www.w3.org/2001/XMLSchema#date"/>
                    <rdf:Description rdf:about="http://www.w3.org/2001/XMLSchema#dateTime"/>
                </owl:unionOf>
            </rdfs:Datatype>
        </rdfs:range>
        <rdfs:comment xml:lang="it">La proprietà è usata per indicare  la data in cui viene effettuata la misurazione dello spessore del grasso dorsale</rdfs:comment>
        <rdfs:comment xml:lang="en">The property is used to indicate the date on which the measurement of back fat thickness is taken</rdfs:comment>
        <rdfs:isDefinedBy rdf:resource="https://w3id.org/leo/onto/ale"/>
        <rdfs:label xml:lang="en">back fact thickness measurement date</rdfs:label>
        <rdfs:label xml:lang="it">data misurazione spessore grasso dorsale</rdfs:label>
        <owl:versionInfo xml:lang="it">stabile</owl:versionInfo>
        <owl:versionInfo xml:lang="en">stable</owl:versionInfo>
    </owl:DatatypeProperty>
    


    <!-- https://w3id.org/leo/onto/ale/breastFeedingTerminationDate -->

    <owl:DatatypeProperty rdf:about="https://w3id.org/leo/onto/ale/breastFeedingTerminationDate">
        <rdfs:subPropertyOf rdf:resource="https://w3id.org/italia/onto/TI/date"/>
        <rdfs:domain rdf:resource="https://w3id.org/leo/onto/ale/BreastFeedingTermination"/>
        <rdfs:range>
            <rdfs:Datatype>
                <owl:unionOf rdf:parseType="Collection">
                    <rdf:Description rdf:about="http://www.w3.org/2001/XMLSchema#date"/>
                    <rdf:Description rdf:about="http://www.w3.org/2001/XMLSchema#dateTime"/>
                </owl:unionOf>
            </rdfs:Datatype>
        </rdfs:range>
        <rdfs:comment xml:lang="en">La proprietà è usata per indicare  la data in cui la madre termina l&apos;allattamento.</rdfs:comment>
        <rdfs:comment xml:lang="it">The property is used to indicate the date on which the mother ends breast-feeding</rdfs:comment>
        <rdfs:isDefinedBy rdf:resource="https://w3id.org/leo/onto/ale"/>
        <rdfs:label xml:lang="en">breast feeding termination date</rdfs:label>
        <rdfs:label xml:lang="it">data interruzione allattamento</rdfs:label>
        <owl:versionInfo xml:lang="it">stabile</owl:versionInfo>
        <owl:versionInfo xml:lang="en">stable</owl:versionInfo>
    </owl:DatatypeProperty>
    


    <!-- https://w3id.org/leo/onto/ale/deadReason -->

    <owl:DatatypeProperty rdf:about="https://w3id.org/leo/onto/ale/deadReason">
        <rdfs:domain rdf:resource="https://w3id.org/leo/onto/ale/Slaughter"/>
        <rdfs:range rdf:resource="http://www.w3.org/2000/01/rdf-schema#Literal"/>
        <rdfs:comment xml:lang="it">Indica le cause della morte dell&apos;animale. Al tempo di stesura della versione 0.3 dell&apos;ontologia, non esiste alcun vocabolario controllato per questa proprietà e si è scelto quindi di usare direttamente un valore stringa. Se in futuro un vocabolario fosse adottato, questa proprietà potrebbe essere trasformata per collegare l&apos;evento di macellazione con un concetto e un codice associato (object property).</rdfs:comment>
        <rdfs:comment xml:lang="en">It indicates the causes of the animal death. At the time of writing version 0.3 of the ontology, there is no controlled vocabulary for this property and it was therefore chosen to use a string value directly. If a vocabulary were to be adopted in the future, this property could be transformed to link the slaughter event with a concept and associated code (object property).</rdfs:comment>
        <rdfs:isDefinedBy rdf:resource="https://w3id.org/leo/onto/ale"/>
        <rdfs:label xml:lang="it">causale di morte</rdfs:label>
        <rdfs:label xml:lang="en">dead reason</rdfs:label>
        <owl:versionInfo xml:lang="it">stabile - introdotta nella versione 0.3 dell&apos;ontologia. Da sostituire in caso di disponibilità di un vocabolario controllato</owl:versionInfo>
        <owl:versionInfo xml:lang="en">stable - introduced in version 0.3 of the ontology. To be replaced in case of the availability of a controlled vocabulary</owl:versionInfo>
    </owl:DatatypeProperty>
    


    <!-- https://w3id.org/leo/onto/ale/destinationType -->

    <owl:DatatypeProperty rdf:about="https://w3id.org/leo/onto/ale/destinationType">
        <rdfs:domain rdf:resource="https://w3id.org/leo/onto/ale/OutboundMovement"/>
        <rdfs:range rdf:resource="http://www.w3.org/2000/01/rdf-schema#Literal"/>
        <rdfs:comment xml:lang="it">La proprietà è utilizzata per categorizzare (o descrivere) la destinazione dell&apos;animale d&apos;allevamento. Per esempio: &apos;macello&apos;. Al tempo di stesura della versione 0.4 dell&apos;ontologia, non esiste alcun vocabolario controllato per questa proprietà e si è scelto quindi di usare direttamente un valore stringa. Se in futuro un vocabolario fosse adottato, questa proprietà potrebbe essere trasformata per collegare l&apos;evento di spostamento in uscita con un concetto e un codice associato (object property).</rdfs:comment>
        <rdfs:comment xml:lang="en">The property is used to categorise (or describe) the destination of the farm animal. For example: &apos;slaughterhouse&apos;. At the time of writing version 0.4 of the ontology, there is no controlled vocabulary for this property and it was therefore chosen to use a string value directly. If a vocabulary were to be adopted in the future, this property could be transformed to link the outbound movement event with a concept and associated code (object property).</rdfs:comment>
        <rdfs:label rdf:resource="https://w3id.org/leo/onto/ale"/>
        <rdfs:label xml:lang="en">destination type</rdfs:label>
        <rdfs:label xml:lang="it">tipo di destinazione</rdfs:label>
        <owl:versionInfo xml:lang="it">stabile - introdotta nella versione 0.4 dell&apos;ontologia. Da sostituire in caso di disponibilità di un vocabolario controllato</owl:versionInfo>
        <owl:versionInfo xml:lang="en">stable - introduced in version 0.4 of the ontology. To be replaced in case of the availability of a controlled vocabulary</owl:versionInfo>
    </owl:DatatypeProperty>
    


    <!-- https://w3id.org/leo/onto/ale/detectionDate -->

    <owl:DatatypeProperty rdf:about="https://w3id.org/leo/onto/ale/detectionDate">
        <rdfs:subPropertyOf rdf:resource="https://w3id.org/italia/onto/TI/date"/>
        <rdfs:domain rdf:resource="http://www.w3.org/2002/07/owl#Thing"/>
        <rdfs:range>
            <rdfs:Datatype>
                <owl:unionOf rdf:parseType="Collection">
                    <rdf:Description rdf:about="http://www.w3.org/2001/XMLSchema#date"/>
                    <rdf:Description rdf:about="http://www.w3.org/2001/XMLSchema#dateTime"/>
                </owl:unionOf>
            </rdfs:Datatype>
        </rdfs:range>
        <rdfs:comment xml:lang="it">La data  usata per riportare informazioni di vario genere nel dominio di riferimento.</rdfs:comment>
        <rdfs:comment xml:lang="en">The date in which information is reported.</rdfs:comment>
        <rdfs:isDefinedBy rdf:resource="https://w3id.org/leo/onto/ale"/>
        <rdfs:label xml:lang="it">data di rilevazione</rdfs:label>
        <rdfs:label xml:lang="en">detection date</rdfs:label>
        <owl:versionInfo xml:lang="it">stabile</owl:versionInfo>
        <owl:versionInfo xml:lang="en">stable</owl:versionInfo>
    </owl:DatatypeProperty>
    


    <!-- https://w3id.org/leo/onto/ale/diagnosisDate -->

    <owl:DatatypeProperty rdf:about="https://w3id.org/leo/onto/ale/diagnosisDate">
        <rdfs:subPropertyOf rdf:resource="https://w3id.org/italia/onto/TI/date"/>
        <rdfs:domain rdf:resource="https://w3id.org/leo/onto/ale/Diagnosis"/>
        <rdfs:range>
            <rdfs:Datatype>
                <owl:unionOf rdf:parseType="Collection">
                    <rdf:Description rdf:about="http://www.w3.org/2001/XMLSchema#date"/>
                    <rdf:Description rdf:about="http://www.w3.org/2001/XMLSchema#dateTime"/>
                </owl:unionOf>
            </rdfs:Datatype>
        </rdfs:range>
        <rdfs:comment xml:lang="it">Data nella quale vengono fatte delle diagnosi sull&apos;animale. Nel caso di diagnosi di gravidanza, rappresenta la data nella quale attraverso visite ginecologiche o analisi di laboratorio viene determinato se la femmina è gravida.</rdfs:comment>
        <rdfs:comment xml:lang="en">Date on which diagnoses are made on the animal. In the case of a diagnosis of pregnancy, it is the date on which gynaecological examinations or laboratory tests determine whether the female is pregnant.</rdfs:comment>
        <rdfs:isDefinedBy rdf:resource="https://w3id.org/leo/onto/ale"/>
        <rdfs:label xml:lang="it">data diagnosi</rdfs:label>
        <rdfs:label xml:lang="en">diagnosis date</rdfs:label>
        <owl:versionInfo xml:lang="it">stabile - aggiunto nella seconda versione dell&apos;ontologia</owl:versionInfo>
        <owl:versionInfo xml:lang="en">stable - added in the second version of the ontology</owl:versionInfo>
    </owl:DatatypeProperty>
    


    <!-- https://w3id.org/leo/onto/ale/disposalDate -->

    <owl:DatatypeProperty rdf:about="https://w3id.org/leo/onto/ale/disposalDate">
        <rdfs:subPropertyOf rdf:resource="https://w3id.org/italia/onto/TI/date"/>
        <rdfs:domain>
            <owl:Class>
                <owl:unionOf rdf:parseType="Collection">
                    <rdf:Description rdf:about="https://w3id.org/leo/onto/ale/Disposal"/>
                    <rdf:Description rdf:about="https://w3id.org/leo/onto/animal/FarmAnimal"/>
                </owl:unionOf>
            </owl:Class>
        </rdfs:domain>
        <rdfs:range>
            <rdfs:Datatype>
                <owl:unionOf rdf:parseType="Collection">
                    <rdf:Description rdf:about="http://www.w3.org/2001/XMLSchema#date"/>
                    <rdf:Description rdf:about="http://www.w3.org/2001/XMLSchema#dateTime"/>
                </owl:unionOf>
            </rdfs:Datatype>
        </rdfs:range>
        <rdfs:comment xml:lang="it">Data nella quale l’animale esce dall’allevamento e la sua destinazione NON è un altro allevamento nel quale verrà allevato</rdfs:comment>
        <rdfs:comment xml:lang="en">Date on which the animal leaves the farm and its destination is NOT another farm on which it will be bred</rdfs:comment>
        <rdfs:isDefinedBy rdf:resource="https://w3id.org/leo/onto/ale"/>
        <rdfs:label xml:lang="it">data di eliminazione</rdfs:label>
        <rdfs:label xml:lang="en">disposal date</rdfs:label>
        <owl:versionInfo xml:lang="it">stabile - aggiunto nella seconda versione dell&apos;ontologia</owl:versionInfo>
        <owl:versionInfo xml:lang="en">stable - added in the second version of the ontology</owl:versionInfo>
    </owl:DatatypeProperty>
    


    <!-- https://w3id.org/leo/onto/ale/dryDate -->

    <owl:DatatypeProperty rdf:about="https://w3id.org/leo/onto/ale/dryDate">
        <rdfs:subPropertyOf rdf:resource="https://w3id.org/italia/onto/TI/date"/>
        <rdfs:domain rdf:resource="https://w3id.org/leo/onto/ale/Dry"/>
        <rdfs:range>
            <rdfs:Datatype>
                <owl:unionOf rdf:parseType="Collection">
                    <rdf:Description rdf:about="http://www.w3.org/2001/XMLSchema#date"/>
                    <rdf:Description rdf:about="http://www.w3.org/2001/XMLSchema#dateTime"/>
                </owl:unionOf>
            </rdfs:Datatype>
        </rdfs:range>
        <rdfs:comment xml:lang="en">It represents the date on which the animal is put out to dry.</rdfs:comment>
        <rdfs:comment xml:lang="it">Rappresenta la data in cui l’animale viene messo in asciutta.</rdfs:comment>
        <rdfs:isDefinedBy rdf:resource="https://w3id.org/leo/onto/ale"/>
        <rdfs:label xml:lang="it">data asciutta</rdfs:label>
        <rdfs:label xml:lang="en">dry date</rdfs:label>
        <owl:versionInfo xml:lang="it">stabile</owl:versionInfo>
        <owl:versionInfo xml:lang="en">stable</owl:versionInfo>
    </owl:DatatypeProperty>
    


    <!-- https://w3id.org/leo/onto/ale/embryoResorptionDate -->

    <owl:DatatypeProperty rdf:about="https://w3id.org/leo/onto/ale/embryoResorptionDate">
        <rdfs:subPropertyOf rdf:resource="https://w3id.org/italia/onto/TI/date"/>
        <rdfs:domain rdf:resource="https://w3id.org/leo/onto/ale/EmbryoResorption"/>
        <rdfs:range>
            <rdfs:Datatype>
                <owl:unionOf rdf:parseType="Collection">
                    <rdf:Description rdf:about="http://www.w3.org/2001/XMLSchema#date"/>
                    <rdf:Description rdf:about="http://www.w3.org/2001/XMLSchema#dateTime"/>
                </owl:unionOf>
            </rdfs:Datatype>
        </rdfs:range>
        <rdfs:comment xml:lang="it">Data in cui viene segnalato il riassorbimento embrionale.</rdfs:comment>
        <rdfs:comment xml:lang="en">Date on which embryo resorption is reported.</rdfs:comment>
        <rdfs:isDefinedBy rdf:resource="https://w3id.org/leo/onto/ale"/>
        <rdfs:label xml:lang="it">data riassorbimento embrionale</rdfs:label>
        <rdfs:label xml:lang="en">embryo resorption date</rdfs:label>
        <owl:versionInfo xml:lang="it">stabile</owl:versionInfo>
        <owl:versionInfo xml:lang="en">stable</owl:versionInfo>
    </owl:DatatypeProperty>
    


    <!-- https://w3id.org/leo/onto/ale/entryInFarmDate -->

    <owl:DatatypeProperty rdf:about="https://w3id.org/leo/onto/ale/entryInFarmDate">
        <rdfs:subPropertyOf rdf:resource="https://w3id.org/italia/onto/TI/date"/>
        <rdfs:domain rdf:resource="https://w3id.org/leo/onto/ale/InboundMovement"/>
        <rdfs:range>
            <rdfs:Datatype>
                <owl:unionOf rdf:parseType="Collection">
                    <rdf:Description rdf:about="http://www.w3.org/2001/XMLSchema#date"/>
                    <rdf:Description rdf:about="http://www.w3.org/2001/XMLSchema#dateTime"/>
                </owl:unionOf>
            </rdfs:Datatype>
        </rdfs:range>
        <rdfs:comment xml:lang="it">Data nella quale l’animale è entrato in allevamento, potrebbe coincidere con la data di nascita se rappresenta un ingresso di un nato in stalla.</rdfs:comment>
        <rdfs:comment xml:lang="en">Date on which the animal entered the herd, it could coincide with the date of birth if it represents an entry of a stable born.</rdfs:comment>
        <rdfs:isDefinedBy rdf:resource="https://w3id.org/leo/onto/ale"/>
        <rdfs:label xml:lang="it">data entrata in allevamento</rdfs:label>
        <rdfs:label xml:lang="en">entry in farm date</rdfs:label>
        <owl:versionInfo xml:lang="it">stabile - aggiunto nella seconda versione dell&apos;ontologia</owl:versionInfo>
        <owl:versionInfo xml:lang="en">stable - added in the second version of the ontology</owl:versionInfo>
    </owl:DatatypeProperty>
    


    <!-- https://w3id.org/leo/onto/ale/exitFromFarmDate -->

    <owl:DatatypeProperty rdf:about="https://w3id.org/leo/onto/ale/exitFromFarmDate">
        <rdfs:subPropertyOf rdf:resource="https://w3id.org/italia/onto/TI/date"/>
        <rdfs:domain rdf:resource="https://w3id.org/leo/onto/ale/OutboundMovement"/>
        <rdfs:range>
            <rdfs:Datatype>
                <owl:unionOf rdf:parseType="Collection">
                    <rdf:Description rdf:about="http://www.w3.org/2001/XMLSchema#date"/>
                    <rdf:Description rdf:about="http://www.w3.org/2001/XMLSchema#dateTime"/>
                </owl:unionOf>
            </rdfs:Datatype>
        </rdfs:range>
        <rdfs:comment xml:lang="it">Data nella quale l’animale esce dall’allevamento se la sua destinazione è un altro allevamento nel quale verrà allevato.</rdfs:comment>
        <rdfs:comment xml:lang="en">Date on which the animal leaves the farm if its destination is another farm on which it will be reared.</rdfs:comment>
        <rdfs:isDefinedBy rdf:resource="https://w3id.org/leo/onto/ale"/>
        <rdfs:label xml:lang="it">data uscita dall&apos;allevamento</rdfs:label>
        <rdfs:label xml:lang="en">exit from farm date</rdfs:label>
        <owl:versionInfo xml:lang="it">stabile - aggiunto nella seconda versione dell&apos;ontologia</owl:versionInfo>
        <owl:versionInfo xml:lang="en">stable - added in the second version of the ontology</owl:versionInfo>
    </owl:DatatypeProperty>
    


    <!-- https://w3id.org/leo/onto/ale/fertilizationDate -->

    <owl:DatatypeProperty rdf:about="https://w3id.org/leo/onto/ale/fertilizationDate">
        <rdfs:subPropertyOf rdf:resource="https://w3id.org/italia/onto/TI/date"/>
        <rdfs:domain rdf:resource="https://w3id.org/leo/onto/ale/Fertilization"/>
        <rdfs:range>
            <rdfs:Datatype>
                <owl:unionOf rdf:parseType="Collection">
                    <rdf:Description rdf:about="http://www.w3.org/2001/XMLSchema#date"/>
                    <rdf:Description rdf:about="http://www.w3.org/2001/XMLSchema#dateTime"/>
                </owl:unionOf>
            </rdfs:Datatype>
        </rdfs:range>
        <rdfs:comment xml:lang="it">Data in cui viene effettuato l&apos;impianto embrionale.</rdfs:comment>
        <rdfs:comment xml:lang="en">The date on which the embryo implantation event occurs.</rdfs:comment>
        <rdfs:isDefinedBy rdf:resource="https://w3id.org/leo/onto/ale"/>
        <rdfs:label xml:lang="it">data di fecondazione/inseminazione</rdfs:label>
        <rdfs:label xml:lang="en">fertilization date</rdfs:label>
        <owl:versionInfo xml:lang="it">stabile - aggiunto nella seconda versione dell&apos;ontologia</owl:versionInfo>
        <owl:versionInfo xml:lang="en">stable - added in the second version of the ontology</owl:versionInfo>
    </owl:DatatypeProperty>
    


    <!-- https://w3id.org/leo/onto/ale/identificationDate -->

    <owl:DatatypeProperty rdf:about="https://w3id.org/leo/onto/ale/identificationDate">
        <rdfs:subPropertyOf rdf:resource="https://w3id.org/italia/onto/TI/date"/>
        <rdfs:domain>
            <owl:Class>
                <owl:unionOf rdf:parseType="Collection">
                    <rdf:Description rdf:about="https://w3id.org/leo/onto/ale/Identification"/>
                    <rdf:Description rdf:about="https://w3id.org/leo/onto/animal/FarmAnimal"/>
                </owl:unionOf>
            </owl:Class>
        </rdfs:domain>
        <rdfs:range>
            <rdfs:Datatype>
                <owl:unionOf rdf:parseType="Collection">
                    <rdf:Description rdf:about="http://www.w3.org/2001/XMLSchema#date"/>
                    <rdf:Description rdf:about="http://www.w3.org/2001/XMLSchema#dateTime"/>
                </owl:unionOf>
            </rdfs:Datatype>
        </rdfs:range>
        <rdfs:comment xml:lang="it">Data in cui l&apos;animale da allevamento è identificato in modo univoco secondo diversi meccanismi. Questa data può coincidere con la data di applicazione della marca (quando viene applicato il marchio auricolare) dell&apos;animale.</rdfs:comment>
        <rdfs:comment xml:lang="en">Date on which the farm animal is uniquely identified according to different mechanisms. This date may coincide with the tagging date (when the eartag is applied) of the animal.</rdfs:comment>
        <rdfs:isDefinedBy rdf:resource="https://w3id.org/leo/onto/ale"/>
        <rdfs:label xml:lang="it">data di identificazione univoca</rdfs:label>
        <rdfs:label xml:lang="en">identification date</rdfs:label>
        <owl:versionInfo xml:lang="it">stabile - revisionata nella versione 0.5 dell&apos;ontologia</owl:versionInfo>
        <owl:versionInfo xml:lang="en">stable - revised in version 0.5 of the ontology</owl:versionInfo>
    </owl:DatatypeProperty>
    


    <!-- https://w3id.org/leo/onto/ale/implantationDate -->

    <owl:DatatypeProperty rdf:about="https://w3id.org/leo/onto/ale/implantationDate">
        <rdfs:subPropertyOf rdf:resource="https://w3id.org/italia/onto/TI/date"/>
        <rdfs:domain rdf:resource="https://w3id.org/leo/onto/ale/Implantation"/>
        <rdfs:range>
            <rdfs:Datatype>
                <owl:unionOf rdf:parseType="Collection">
                    <rdf:Description rdf:about="http://www.w3.org/2001/XMLSchema#date"/>
                    <rdf:Description rdf:about="http://www.w3.org/2001/XMLSchema#dateTime"/>
                </owl:unionOf>
            </rdfs:Datatype>
        </rdfs:range>
        <rdfs:comment xml:lang="it">La data nella quale viene introdotto un embrione nella vacca ricevente.</rdfs:comment>
        <rdfs:comment xml:lang="it">The date on which an embryo is introduced into the receiving cow.</rdfs:comment>
        <rdfs:isDefinedBy rdf:resource="https://w3id.org/leo/onto/ale"/>
        <rdfs:label xml:lang="it">data impianto</rdfs:label>
        <rdfs:label xml:lang="en">implantation date</rdfs:label>
        <owl:versionInfo xml:lang="it">stabile - aggiunto nella seconda versione dell&apos;ontologia</owl:versionInfo>
        <owl:versionInfo xml:lang="en">stable - added in the second version of the ontology</owl:versionInfo>
    </owl:DatatypeProperty>
    


    <!-- https://w3id.org/leo/onto/ale/isCarcassForConsumption -->

    <owl:DatatypeProperty rdf:about="https://w3id.org/leo/onto/ale/isCarcassForConsumption">
        <rdf:type rdf:resource="http://www.w3.org/2002/07/owl#FunctionalProperty"/>
        <rdfs:domain rdf:resource="https://w3id.org/leo/onto/ale/FarmAnimalCarcass"/>
        <rdfs:range rdf:resource="http://www.w3.org/2001/XMLSchema#boolean"/>
        <rdfs:comment xml:lang="en">Property used to indicate whether the carcass is for consumption or not</rdfs:comment>
        <rdfs:comment xml:lang="it">Proprietà che indica se una carcassa è destinata al consumo umano o meno</rdfs:comment>
        <rdfs:isDefinedBy rdf:resource="https://w3id.org/leo/onto/ale"/>
        <rdfs:label xml:lang="en">is carcass for consumption</rdfs:label>
        <rdfs:label xml:lang="it">è carcassa per consumo</rdfs:label>
        <owl:versionInfo xml:lang="it">stabile - introdotta nella versione 0.3 dell&apos;ontologia</owl:versionInfo>
        <owl:versionInfo xml:lang="en">stable - introduced in version 0.3 of the ontology</owl:versionInfo>
    </owl:DatatypeProperty>
    


    <!-- https://w3id.org/leo/onto/ale/milkConductivityDetectionDate -->

    <owl:DatatypeProperty rdf:about="https://w3id.org/leo/onto/ale/milkConductivityDetectionDate">
        <rdfs:subPropertyOf rdf:resource="https://w3id.org/italia/onto/TI/date"/>
        <rdfs:domain rdf:resource="https://w3id.org/leo/onto/ale/MilkConductivityMeasurement"/>
        <rdfs:range>
            <rdfs:Datatype>
                <owl:unionOf rdf:parseType="Collection">
                    <rdf:Description rdf:about="http://www.w3.org/2001/XMLSchema#date"/>
                    <rdf:Description rdf:about="http://www.w3.org/2001/XMLSchema#dateTime"/>
                </owl:unionOf>
            </rdfs:Datatype>
        </rdfs:range>
        <rdfs:comment xml:lang="it">Momento nel quale si inizia a rilevare la conducibilità media del latte</rdfs:comment>
        <rdfs:comment xml:lang="en">Time at which the average conductivity of milk starts to be measured</rdfs:comment>
        <rdfs:isDefinedBy rdf:resource="https://w3id.org/leo/onto/ale"/>
        <rdfs:label xml:lang="it">data rilevamento conducibilità latte</rdfs:label>
        <rdfs:label xml:lang="en">milk conductivity detection date</rdfs:label>
        <owl:versionInfo xml:lang="it">stabile</owl:versionInfo>
        <owl:versionInfo xml:lang="en">stable</owl:versionInfo>
    </owl:DatatypeProperty>
    


    <!-- https://w3id.org/leo/onto/ale/milkingSessionDate -->

    <owl:DatatypeProperty rdf:about="https://w3id.org/leo/onto/ale/milkingSessionDate">
        <rdfs:subPropertyOf rdf:resource="https://w3id.org/italia/onto/TI/date"/>
        <rdfs:domain rdf:resource="https://w3id.org/leo/onto/ale/MilkingSession"/>
        <rdfs:range>
            <rdfs:Datatype>
                <owl:unionOf rdf:parseType="Collection">
                    <rdf:Description rdf:about="http://www.w3.org/2001/XMLSchema#date"/>
                    <rdf:Description rdf:about="http://www.w3.org/2001/XMLSchema#dateTime"/>
                </owl:unionOf>
            </rdfs:Datatype>
        </rdfs:range>
        <rdfs:comment xml:lang="it">Momento nel quale si inizia a mungere l’animale (data e ora)</rdfs:comment>
        <rdfs:comment xml:lang="en">Time when milking starts (date and time)</rdfs:comment>
        <rdfs:isDefinedBy rdf:resource="https://w3id.org/leo/onto/ale"/>
        <rdfs:label xml:lang="it">data sessione mungitura</rdfs:label>
        <rdfs:label xml:lang="en">milking session date</rdfs:label>
        <owl:versionInfo xml:lang="it">stabile</owl:versionInfo>
        <owl:versionInfo xml:lang="en">stable</owl:versionInfo>
    </owl:DatatypeProperty>
    


    <!-- https://w3id.org/leo/onto/ale/numberOfBorn -->

    <owl:DatatypeProperty rdf:about="https://w3id.org/leo/onto/ale/numberOfBorn">
        <rdfs:domain rdf:resource="https://w3id.org/leo/onto/ale/Parturition"/>
        <rdfs:range rdf:resource="http://www.w3.org/2001/XMLSchema#integer"/>
        <rdfs:comment xml:lang="it">La proprietà è utilizzata per indicare il numero complessivo dei nati quando non è disponibile una suddivisione per maschi/femmine, vivi/morti.</rdfs:comment>
        <rdfs:comment xml:lang="en">The property is used to indicate the total number of births when a breakdown by male/female, live/dead is not available.</rdfs:comment>
        <rdfs:isDefinedBy rdf:resource="https://w3id.org/leo/onto/ale"/>
        <rdfs:label xml:lang="en">number of born</rdfs:label>
        <rdfs:label xml:lang="it">numero di nati</rdfs:label>
        <owl:versionInfo xml:lang="it">stabile</owl:versionInfo>
        <owl:versionInfo xml:lang="en">stable</owl:versionInfo>
    </owl:DatatypeProperty>
    


    <!-- https://w3id.org/leo/onto/ale/numberOfBornAliveFemales -->

    <owl:DatatypeProperty rdf:about="https://w3id.org/leo/onto/ale/numberOfBornAliveFemales">
        <rdfs:domain rdf:resource="https://w3id.org/leo/onto/ale/Parturition"/>
        <rdfs:range rdf:resource="http://www.w3.org/2001/XMLSchema#integer"/>
        <rdfs:comment xml:lang="it">Il numero di femmine nate vive dal parto.</rdfs:comment>
        <rdfs:comment xml:lang="en">The number of females born alive in the parturition event.</rdfs:comment>
        <rdfs:isDefinedBy rdf:resource="https://w3id.org/leo/onto/ale"/>
        <rdfs:label xml:lang="en">number of born alive females</rdfs:label>
        <rdfs:label xml:lang="it">numero di femmine nate vive</rdfs:label>
        <owl:versionInfo xml:lang="it">stabile - aggiunto nella seconda versione dell&apos;ontologia</owl:versionInfo>
        <owl:versionInfo xml:lang="en">stable - added in the second version of the ontology</owl:versionInfo>
    </owl:DatatypeProperty>
    


    <!-- https://w3id.org/leo/onto/ale/numberOfBornAliveMales -->

    <owl:DatatypeProperty rdf:about="https://w3id.org/leo/onto/ale/numberOfBornAliveMales">
        <rdfs:domain rdf:resource="https://w3id.org/leo/onto/ale/Parturition"/>
        <rdfs:range rdf:resource="http://www.w3.org/2001/XMLSchema#integer"/>
        <rdfs:comment xml:lang="it">Il numero di maschi nati vivi dal parto.</rdfs:comment>
        <rdfs:comment xml:lang="en">The number of males born alive in the parturition event.</rdfs:comment>
        <rdfs:isDefinedBy rdf:resource="https://w3id.org/leo/onto/ale"/>
        <rdfs:label xml:lang="en">number of born alive males</rdfs:label>
        <rdfs:label xml:lang="it">numero di maschi nati vivi</rdfs:label>
        <owl:versionInfo xml:lang="it">stabile - aggiunto nella seconda versione dell&apos;ontologia</owl:versionInfo>
        <owl:versionInfo xml:lang="en">stable - added in the second version of the ontology</owl:versionInfo>
    </owl:DatatypeProperty>
    


    <!-- https://w3id.org/leo/onto/ale/numberOfBornDeadFemales -->

    <owl:DatatypeProperty rdf:about="https://w3id.org/leo/onto/ale/numberOfBornDeadFemales">
        <rdfs:domain>
            <owl:Class>
                <owl:unionOf rdf:parseType="Collection">
                    <rdf:Description rdf:about="https://w3id.org/leo/onto/ale/Abortion"/>
                    <rdf:Description rdf:about="https://w3id.org/leo/onto/ale/Parturition"/>
                </owl:unionOf>
            </owl:Class>
        </rdfs:domain>
        <rdfs:range rdf:resource="http://www.w3.org/2001/XMLSchema#integer"/>
        <rdfs:comment xml:lang="en">Number of female foetuses expelled in case of abortion or stillbirth.</rdfs:comment>
        <rdfs:comment xml:lang="it">Numero di feti femmina espulsi in caso di aborto o nate morte.</rdfs:comment>
        <rdfs:isDefinedBy rdf:resource="https://w3id.org/leo/onto/ale"/>
        <rdfs:label xml:lang="en">number of born dead females</rdfs:label>
        <rdfs:label xml:lang="it">numero di femmine nate morte</rdfs:label>
        <owl:versionInfo xml:lang="it">stabile - aggiunto nella seconda versione dell&apos;ontologia</owl:versionInfo>
        <owl:versionInfo xml:lang="en">stable - added in the second version of the ontology</owl:versionInfo>
    </owl:DatatypeProperty>
    


    <!-- https://w3id.org/leo/onto/ale/numberOfBornDeadMales -->

    <owl:DatatypeProperty rdf:about="https://w3id.org/leo/onto/ale/numberOfBornDeadMales">
        <rdfs:domain>
            <owl:Class>
                <owl:unionOf rdf:parseType="Collection">
                    <rdf:Description rdf:about="https://w3id.org/leo/onto/ale/Abortion"/>
                    <rdf:Description rdf:about="https://w3id.org/leo/onto/ale/Parturition"/>
                </owl:unionOf>
            </owl:Class>
        </rdfs:domain>
        <rdfs:range rdf:resource="http://www.w3.org/2001/XMLSchema#integer"/>
        <rdfs:comment xml:lang="en">Number of males foetuses expelled in case of abortion or stillbirth.</rdfs:comment>
        <rdfs:comment xml:lang="it">Numero di feti maschi espulsi in caso di aborto o nati morti.</rdfs:comment>
        <rdfs:isDefinedBy rdf:resource="https://w3id.org/leo/onto/ale"/>
        <rdfs:label xml:lang="en">number of born dead males</rdfs:label>
        <rdfs:label xml:lang="it">numero di maschi nati morti</rdfs:label>
        <owl:versionInfo xml:lang="it">stabile - aggiunto nella seconda versione dell&apos;ontologia</owl:versionInfo>
        <owl:versionInfo xml:lang="en">stable - added in the second version of the ontology</owl:versionInfo>
    </owl:DatatypeProperty>
    


    <!-- https://w3id.org/leo/onto/ale/numberOfTeats -->

    <owl:DatatypeProperty rdf:about="https://w3id.org/leo/onto/ale/numberOfTeats">
        <rdfs:domain rdf:resource="https://w3id.org/leo/onto/ale/Birth"/>
        <rdfs:range rdf:resource="http://www.w3.org/2001/XMLSchema#integer"/>
        <rdfs:comment xml:lang="it">La proprietà è utilizzata per indicare il numero totale di capezzoli ed è utilizzata solo per la specie Suina.</rdfs:comment>
        <rdfs:comment xml:lang="en">The property is used to indicate the total number of teats and is only used for the species swine.</rdfs:comment>
        <rdfs:isDefinedBy rdf:resource="https://w3id.org/leo/onto/ale"/>
        <rdfs:label xml:lang="en">number of teats</rdfs:label>
        <rdfs:label xml:lang="it">numero di capezzoli</rdfs:label>
        <owl:versionInfo xml:lang="it">stabile</owl:versionInfo>
        <owl:versionInfo xml:lang="en">stable</owl:versionInfo>
    </owl:DatatypeProperty>
    


    <!-- https://w3id.org/leo/onto/ale/parturitionDate -->

    <owl:DatatypeProperty rdf:about="https://w3id.org/leo/onto/ale/parturitionDate">
        <rdfs:subPropertyOf rdf:resource="https://w3id.org/italia/onto/TI/date"/>
        <rdfs:domain rdf:resource="https://w3id.org/leo/onto/ale/Parturition"/>
        <rdfs:range>
            <rdfs:Datatype>
                <owl:unionOf rdf:parseType="Collection">
                    <rdf:Description rdf:about="http://www.w3.org/2001/XMLSchema#date"/>
                    <rdf:Description rdf:about="http://www.w3.org/2001/XMLSchema#dateTime"/>
                </owl:unionOf>
            </rdfs:Datatype>
        </rdfs:range>
        <rdfs:comment xml:lang="it">Data in cui avviene il parto dell&apos;animale.</rdfs:comment>
        <rdfs:comment xml:lang="en">Date on which the parturition of the animal occurs.</rdfs:comment>
        <rdfs:isDefinedBy rdf:resource="https://w3id.org/leo/onto/ale"/>
        <rdfs:label xml:lang="it">data parto</rdfs:label>
        <rdfs:label xml:lang="en">parturition date</rdfs:label>
        <owl:versionInfo xml:lang="it">stabile</owl:versionInfo>
        <owl:versionInfo xml:lang="en">stable</owl:versionInfo>
    </owl:DatatypeProperty>
    


    <!-- https://w3id.org/leo/onto/ale/provenanceType -->

    <owl:DatatypeProperty rdf:about="https://w3id.org/leo/onto/ale/provenanceType">
        <rdfs:domain rdf:resource="https://w3id.org/leo/onto/ale/InboundMovement"/>
        <rdfs:range rdf:resource="http://www.w3.org/2000/01/rdf-schema#Literal"/>
        <rdfs:comment xml:lang="it">La proprietà è utilizzata per categorizzare (o descrivere) la provenienza dell&apos;animale d&apos;allevamento. Per esempio: &apos;allevamento&apos;. Al tempo di stesura della versione 0.4 dell&apos;ontologia, non esiste alcun vocabolario controllato per questa proprietà e si è scelto quindi di usare direttamente un valore stringa. Se in futuro un vocabolario fosse adottato, questa proprietà potrebbe essere trasformata per collegare l&apos;evento di spostamento in entrata con un concetto e un codice associato (object property).</rdfs:comment>
        <rdfs:comment xml:lang="en">The property is used to categorise (or describe) the provenance of the farm animal. For example: &apos;farming&apos;. At the time of writing version 0.4 of the ontology, there is no controlled vocabulary for this property and it was therefore chosen to use a string value directly. If a vocabulary were to be adopted in the future, this property could be transformed to link the inbound movement event with a concept and associated code (object property).</rdfs:comment>
        <rdfs:isDefinedBy rdf:resource="https://w3id.org/leo/onto/ale"/>
        <rdfs:label xml:lang="en">provenance type</rdfs:label>
        <rdfs:label xml:lang="it">tipo di provenienza</rdfs:label>
        <owl:versionInfo xml:lang="it">stabile - introdotta nella versione 0.4 dell&apos;ontologia. Da sostituire in caso di disponibilità di un vocabolario controllato</owl:versionInfo>
        <owl:versionInfo xml:lang="en">stable - introduced in version 0.4 of the ontology. To be replaced in case of the availability of a controlled vocabulary</owl:versionInfo>
    </owl:DatatypeProperty>
    


    <!-- https://w3id.org/leo/onto/ale/slaughterDate -->

    <owl:DatatypeProperty rdf:about="https://w3id.org/leo/onto/ale/slaughterDate">
        <rdfs:subPropertyOf rdf:resource="https://w3id.org/italia/onto/TI/date"/>
        <rdfs:domain rdf:resource="https://w3id.org/leo/onto/ale/Slaughter"/>
        <rdfs:range>
            <rdfs:Datatype>
                <owl:unionOf rdf:parseType="Collection">
                    <rdf:Description rdf:about="http://www.w3.org/2001/XMLSchema#date"/>
                    <rdf:Description rdf:about="http://www.w3.org/2001/XMLSchema#dateTime"/>
                </owl:unionOf>
            </rdfs:Datatype>
        </rdfs:range>
        <rdfs:comment xml:lang="it">Indica la data in cui è avvenuta la macellazione</rdfs:comment>
        <rdfs:comment xml:lang="en">It indicates the date on which the slaughter occured.</rdfs:comment>
        <rdfs:isDefinedBy rdf:resource="https://w3id.org/leo/onto/ale"/>
        <rdfs:label xml:lang="it">data di macellazione</rdfs:label>
        <rdfs:label xml:lang="en">slaughter date</rdfs:label>
        <owl:versionInfo xml:lang="it">stabile - introdotta nella versione 0.3 dell&apos;ontologia</owl:versionInfo>
        <owl:versionInfo xml:lang="en">stable - introduced in version 0.3 of the ontology</owl:versionInfo>
    </owl:DatatypeProperty>
    


    <!-- https://w3id.org/leo/onto/ale/weaningDate -->

    <owl:DatatypeProperty rdf:about="https://w3id.org/leo/onto/ale/weaningDate">
        <rdfs:subPropertyOf rdf:resource="https://w3id.org/italia/onto/TI/date"/>
        <rdfs:domain rdf:resource="https://w3id.org/leo/onto/ale/Weaning"/>
        <rdfs:range>
            <rdfs:Datatype>
                <owl:unionOf rdf:parseType="Collection">
                    <rdf:Description rdf:about="http://www.w3.org/2001/XMLSchema#date"/>
                    <rdf:Description rdf:about="http://www.w3.org/2001/XMLSchema#dateTime"/>
                </owl:unionOf>
            </rdfs:Datatype>
        </rdfs:range>
        <rdfs:comment xml:lang="it">La proprietà è utilizzata per indicare la data di svezzamento.</rdfs:comment>
        <rdfs:comment xml:lang="en">The property is used to indicate the date of weaning.</rdfs:comment>
        <rdfs:isDefinedBy rdf:resource="https://w3id.org/leo/onto/ale"/>
        <rdfs:label xml:lang="it">data svezzamento</rdfs:label>
        <rdfs:label xml:lang="en">weaning date</rdfs:label>
        <owl:versionInfo xml:lang="it">stabile</owl:versionInfo>
        <owl:versionInfo xml:lang="en">stable</owl:versionInfo>
    </owl:DatatypeProperty>
    


    <!-- https://w3id.org/leo/onto/ale/weighingDate -->

    <owl:DatatypeProperty rdf:about="https://w3id.org/leo/onto/ale/weighingDate">
        <rdfs:subPropertyOf rdf:resource="https://w3id.org/italia/onto/TI/date"/>
        <rdfs:domain rdf:resource="https://w3id.org/leo/onto/ale/Weighing"/>
        <rdfs:range>
            <rdfs:Datatype>
                <owl:unionOf rdf:parseType="Collection">
                    <rdf:Description rdf:about="http://www.w3.org/2001/XMLSchema#date"/>
                    <rdf:Description rdf:about="http://www.w3.org/2001/XMLSchema#dateTime"/>
                </owl:unionOf>
            </rdfs:Datatype>
        </rdfs:range>
        <rdfs:comment xml:lang="it">La proprietà è usata per indicare la data in cui viene effettuata la misurazione del peso dell&apos;animale.</rdfs:comment>
        <rdfs:comment xml:lang="en">The property is used to indicate the date on which the animal&apos;s weight is measured.</rdfs:comment>
        <rdfs:isDefinedBy rdf:resource="https://w3id.org/leo/onto/ale"/>
        <rdfs:label xml:lang="it">data della pesata</rdfs:label>
        <rdfs:label xml:lang="en">weighing date</rdfs:label>
        <owl:versionInfo xml:lang="it">stabile</owl:versionInfo>
        <owl:versionInfo xml:lang="en">stable</owl:versionInfo>
    </owl:DatatypeProperty>
    


    <!-- https://w3id.org/leo/onto/animal/uniqueAnimalNumber -->

    <owl:DatatypeProperty rdf:about="https://w3id.org/leo/onto/animal/uniqueAnimalNumber"/>
    


    <!-- 
    ///////////////////////////////////////////////////////////////////////////////////////
    //
    // Classes
    //
    ///////////////////////////////////////////////////////////////////////////////////////
     -->

    


    <!-- http://www.w3.org/2004/02/skos/core#Concept -->

    <owl:Class rdf:about="http://www.w3.org/2004/02/skos/core#Concept"/>
    


    <!-- https://w3id.org/italia/onto/l0/Concept -->

    <owl:Class rdf:about="https://w3id.org/italia/onto/l0/Concept"/>
    


    <!-- https://w3id.org/italia/onto/l0/Object -->

    <owl:Class rdf:about="https://w3id.org/italia/onto/l0/Object"/>
    


    <!-- https://w3id.org/italia/onto/l0/Topic -->

    <owl:Class rdf:about="https://w3id.org/italia/onto/l0/Topic"/>
    


    <!-- https://w3id.org/leo/onto/ale/Abortion -->

    <owl:Class rdf:about="https://w3id.org/leo/onto/ale/Abortion">
        <rdfs:subClassOf rdf:resource="https://w3id.org/leo/onto/ale/AnimalLifeEvent"/>
        <rdfs:subClassOf>
            <owl:Restriction>
                <owl:onProperty rdf:resource="https://w3id.org/leo/onto/ale/hasAbortionType"/>
                <owl:maxQualifiedCardinality rdf:datatype="http://www.w3.org/2001/XMLSchema#nonNegativeInteger">1</owl:maxQualifiedCardinality>
                <owl:onClass rdf:resource="https://w3id.org/leo/onto/ale/AbortionType"/>
            </owl:Restriction>
        </rdfs:subClassOf>
        <rdfs:subClassOf>
            <owl:Restriction>
                <owl:onProperty rdf:resource="https://w3id.org/leo/onto/ale/abortionDate"/>
                <owl:qualifiedCardinality rdf:datatype="http://www.w3.org/2001/XMLSchema#nonNegativeInteger">1</owl:qualifiedCardinality>
                <owl:onDataRange>
                    <rdfs:Datatype>
                        <owl:unionOf rdf:parseType="Collection">
                            <rdf:Description rdf:about="http://www.w3.org/2001/XMLSchema#date"/>
                            <rdf:Description rdf:about="http://www.w3.org/2001/XMLSchema#dateTime"/>
                        </owl:unionOf>
                    </rdfs:Datatype>
                </owl:onDataRange>
            </owl:Restriction>
        </rdfs:subClassOf>
        <rdfs:subClassOf>
            <owl:Restriction>
                <owl:onProperty rdf:resource="https://w3id.org/leo/onto/ale/numberOfBornDeadFemales"/>
                <owl:maxQualifiedCardinality rdf:datatype="http://www.w3.org/2001/XMLSchema#nonNegativeInteger">1</owl:maxQualifiedCardinality>
                <owl:onDataRange rdf:resource="http://www.w3.org/2001/XMLSchema#integer"/>
            </owl:Restriction>
        </rdfs:subClassOf>
        <rdfs:subClassOf>
            <owl:Restriction>
                <owl:onProperty rdf:resource="https://w3id.org/leo/onto/ale/numberOfBornDeadMales"/>
                <owl:maxQualifiedCardinality rdf:datatype="http://www.w3.org/2001/XMLSchema#nonNegativeInteger">1</owl:maxQualifiedCardinality>
                <owl:onDataRange rdf:resource="http://www.w3.org/2001/XMLSchema#integer"/>
            </owl:Restriction>
        </rdfs:subClassOf>
        <dc:description rdf:resource="https://raw.githubusercontent.com/Bluarancio/Leo-OpenData/master/RappresentazioneGraficaOntologie/PNG/Ale_Abort.png"/>
        <rdfs:comment xml:lang="it">L&apos;evento di aborto dell&apos;animale. In particolare, rappresenta l&apos;interruzione della gravidanza con espulsione del feto. In particolare, nei bovini da latte si definisce aborto l&apos;interruzione della gravidanza con l&apos;espulsione del feto dal 42° al 260° post – fecondazione. Da non confondere con il parto prematuro (nascita di un vitello capace di vita autonoma dopo il 260° giorno di gravidanza) o parto a termine di un vitello morto o disvitale (&apos;stillbirth”). Sempre nei bovini da latte, si ha aborto precoce dal 42° al 90° giorno di gravidanza, e aborto tardivo, dopo il 90° giorno.

Possibili Applicazioni: Riproduzione e Benessere. Calcolo dello stato riproduttivo dell&apos;animale. Calcolo del tasso di abortività aziendale, dei fattori di rischio per il benessere e per la fertilità. Assistenza tecnica, Gestione sanitaria</rdfs:comment>
        <rdfs:comment xml:lang="en">The event of abortion of the animal. In particular, it represents the termination of pregnancy with expulsion of the foetus. Specifically, in dairy cattle, abortion is defined as the termination of pregnancy with expulsion of the foetus from the 42nd to the 260th post - fertilisation. Not to be confused with premature birth (birth of a calf capable of independent life after the 260th day of pregnancy) or term birth of a stillborn calf. In dairy cattle, early abortion occurs from day 42 to day 90 of pregnancy, and late abortion after day 90.

Possible applications: Reproduction and Welfare. Calculation of the reproductive status of the animal. Calculation of abortion rate, welfare and fertility risk factors. Technical assistance, Health management</rdfs:comment>
        <rdfs:isDefinedBy rdf:resource="https://w3id.org/leo/onto/ale"/>
        <rdfs:label xml:lang="en">Abortion</rdfs:label>
        <rdfs:label xml:lang="it">Aborto</rdfs:label>
        <owl:versionInfo xml:lang="it">stabile</owl:versionInfo>
        <owl:versionInfo xml:lang="en">stable</owl:versionInfo>
    </owl:Class>
    


    <!-- https://w3id.org/leo/onto/ale/AbortionType -->

    <owl:Class rdf:about="https://w3id.org/leo/onto/ale/AbortionType">
        <owl:equivalentClass>
            <owl:Class>
                <owl:oneOf rdf:parseType="Collection">
                    <rdf:Description rdf:about="https://w3id.org/leo/onto/ale/P"/>
                    <rdf:Description rdf:about="https://w3id.org/leo/onto/ale/T"/>
                </owl:oneOf>
            </owl:Class>
        </owl:equivalentClass>
        <rdfs:subClassOf rdf:resource="https://w3id.org/italia/onto/l0/Characteristic"/>
        <rdfs:comment xml:lang="it">Questa classe modella il tipo di aborto. Ci sono due tipi di aborto: Tardivo (T) e Precoce (P). L&apos;aborto Tardivo inizia una nuova lattazione.</rdfs:comment>
        <rdfs:comment xml:lang="en">This class allows one to represent the type of abortion. There are two types of abortion: belated (T) and premature (P). Late abortion starts a new lactation.</rdfs:comment>
        <rdfs:isDefinedBy rdf:resource="https://w3id.org/leo/onto/ale"/>
        <rdfs:label xml:lang="en">Abortion Type</rdfs:label>
        <rdfs:label xml:lang="it">Tipo di Aborto</rdfs:label>
        <owl:versionInfo xml:lang="it">stabile - introdotta in versione 0.3</owl:versionInfo>
        <owl:versionInfo xml:lang="en">stable - introduced in version 0.3</owl:versionInfo>
    </owl:Class>
    


    <!-- https://w3id.org/leo/onto/ale/AnimalLifeEvent -->

    <owl:Class rdf:about="https://w3id.org/leo/onto/ale/AnimalLifeEvent">
        <rdfs:subClassOf rdf:resource="https://w3id.org/italia/onto/TI/TimeIndexedEvent"/>
        <rdfs:subClassOf>
            <owl:Restriction>
                <owl:onProperty rdf:resource="https://w3id.org/leo/onto/ale/happensIn"/>
                <owl:allValuesFrom rdf:resource="https://w3id.org/leo/onto/co/Site"/>
            </owl:Restriction>
        </rdfs:subClassOf>
        <rdfs:subClassOf>
            <owl:Restriction>
                <owl:onProperty rdf:resource="https://w3id.org/leo/onto/ale/involvesCompany"/>
                <owl:allValuesFrom rdf:resource="https://w3id.org/leo/onto/co/LivestockFarm"/>
            </owl:Restriction>
        </rdfs:subClassOf>
        <rdfs:subClassOf>
            <owl:Restriction>
                <owl:onProperty rdf:resource="https://w3id.org/leo/onto/ale/involvesFarmAnimal"/>
                <owl:allValuesFrom rdf:resource="https://w3id.org/leo/onto/animal/FarmAnimal"/>
            </owl:Restriction>
        </rdfs:subClassOf>
        <rdfs:subClassOf>
            <owl:Restriction>
                <owl:onProperty rdf:resource="https://w3id.org/leo/onto/ale/detectionDate"/>
                <owl:qualifiedCardinality rdf:datatype="http://www.w3.org/2001/XMLSchema#nonNegativeInteger">1</owl:qualifiedCardinality>
                <owl:onDataRange>
                    <rdfs:Datatype>
                        <owl:unionOf rdf:parseType="Collection">
                            <rdf:Description rdf:about="http://www.w3.org/2001/XMLSchema#date"/>
                            <rdf:Description rdf:about="http://www.w3.org/2001/XMLSchema#dateTime"/>
                        </owl:unionOf>
                    </rdfs:Datatype>
                </owl:onDataRange>
            </owl:Restriction>
        </rdfs:subClassOf>
        <rdfs:comment xml:lang="it">L&apos;evento della vita per un animale. Esso può un aborto, la nascita, la fecondazione, la riproduzione, la mungitura per alcuni tipi di specie, ecc.</rdfs:comment>
        <rdfs:comment xml:lang="en">The life event of an animal. It may be abortion, birth, fertilization, reproduction, milking for certain types of species, etc.</rdfs:comment>
        <rdfs:isDefinedBy rdf:resource="https://w3id.org/leo/onto/ale"/>
        <rdfs:label xml:lang="en">Animal Life Event</rdfs:label>
        <rdfs:label xml:lang="it">Evento della Vita Animale di Allevamento</rdfs:label>
        <owl:versionInfo xml:lang="it">stabile</owl:versionInfo>
        <owl:versionInfo xml:lang="en">stable</owl:versionInfo>
    </owl:Class>
    


    <!-- https://w3id.org/leo/onto/ale/BackFatThicknessMeasurement -->

    <owl:Class rdf:about="https://w3id.org/leo/onto/ale/BackFatThicknessMeasurement">
        <rdfs:subClassOf rdf:resource="https://w3id.org/leo/onto/ale/AnimalLifeEvent"/>
        <rdfs:subClassOf>
            <owl:Restriction>
                <owl:onProperty rdf:resource="https://w3id.org/leo/onto/ale/hasBackFatThicknessValue"/>
                <owl:someValuesFrom rdf:resource="https://w3id.org/italia/onto/MU/Value"/>
            </owl:Restriction>
        </rdfs:subClassOf>
        <rdfs:subClassOf>
            <owl:Restriction>
                <owl:onProperty rdf:resource="https://w3id.org/leo/onto/ale/hasBackFatThicknessValue"/>
                <owl:allValuesFrom rdf:resource="https://w3id.org/italia/onto/MU/Value"/>
            </owl:Restriction>
        </rdfs:subClassOf>
        <rdfs:subClassOf>
            <owl:Restriction>
                <owl:onProperty rdf:resource="https://w3id.org/leo/onto/ale/bftMeasurementDate"/>
                <owl:qualifiedCardinality rdf:datatype="http://www.w3.org/2001/XMLSchema#nonNegativeInteger">1</owl:qualifiedCardinality>
                <owl:onDataRange>
                    <rdfs:Datatype>
                        <owl:unionOf rdf:parseType="Collection">
                            <rdf:Description rdf:about="http://www.w3.org/2001/XMLSchema#date"/>
                            <rdf:Description rdf:about="http://www.w3.org/2001/XMLSchema#dateTime"/>
                        </owl:unionOf>
                    </rdfs:Datatype>
                </owl:onDataRange>
            </owl:Restriction>
        </rdfs:subClassOf>
        <dc:description rdf:resource="https://raw.githubusercontent.com/Bluarancio/Leo-OpenData/master/RappresentazioneGraficaOntologie/PNG/BackFatThicknessMeasurement.png"/>
        <rdfs:comment xml:lang="it">La classe rappresenta l&apos;evento con il quale si indica la misurazione dello spessore del grasso dorsale. Lo spessore del grasso dorsale (SGD) è un parametro di registrazione comune nei suini ed il monitoraggio della sua evoluzione durante il ciclo produttivo viene interpretato come un indice di mobilizzazione e reintegrazione delle riserve corporee. 
Comunemente, lo SGD viene generalmente misurato almeno allo svezzamento, dopo la diagnosi di gravidanza e all&apos;ingresso delle sale parto.</rdfs:comment>
        <rdfs:comment xml:lang="en">The class represents the event by which backfat thickness is measured. Back fat thickness (SGD) is a common recording parameter in pigs and monitoring its development during the production cycle is interpreted as an index of mobilisation and replenishment of body reserves. 
Commonly, SGD is measured at least at weaning, after pregnancy diagnosis and at farrowing.</rdfs:comment>
        <rdfs:isDefinedBy rdf:resource="https://w3id.org/leo/onto/ale"/>
        <rdfs:label xml:lang="en">Back Fat Thickness Measurement</rdfs:label>
        <rdfs:label xml:lang="it">Misurazione Spessore Grasso Dorsale</rdfs:label>
        <owl:versionInfo xml:lang="it">stabile</owl:versionInfo>
        <owl:versionInfo xml:lang="en">stable</owl:versionInfo>
    </owl:Class>
    


    <!-- https://w3id.org/leo/onto/ale/Birth -->

    <owl:Class rdf:about="https://w3id.org/leo/onto/ale/Birth">
        <rdfs:subClassOf rdf:resource="https://w3id.org/leo/onto/ale/AnimalLifeEvent"/>
        <rdfs:subClassOf>
            <owl:Restriction>
                <owl:onProperty rdf:resource="https://w3id.org/leo/onto/ale/hasAnimalBirthCompany"/>
                <owl:qualifiedCardinality rdf:datatype="http://www.w3.org/2001/XMLSchema#nonNegativeInteger">1</owl:qualifiedCardinality>
                <owl:onClass rdf:resource="https://w3id.org/leo/onto/co/LivestockFarm"/>
            </owl:Restriction>
        </rdfs:subClassOf>
        <rdfs:subClassOf>
            <owl:Restriction>
                <owl:onProperty rdf:resource="https://w3id.org/leo/onto/ale/hasAnimalBirthWeight"/>
                <owl:maxQualifiedCardinality rdf:datatype="http://www.w3.org/2001/XMLSchema#nonNegativeInteger">1</owl:maxQualifiedCardinality>
                <owl:onClass rdf:resource="https://w3id.org/italia/onto/MU/Value"/>
            </owl:Restriction>
        </rdfs:subClassOf>
        <rdfs:subClassOf>
            <owl:Restriction>
                <owl:onProperty rdf:resource="https://w3id.org/leo/onto/animal/hasAnimalDestination"/>
                <owl:maxQualifiedCardinality rdf:datatype="http://www.w3.org/2001/XMLSchema#nonNegativeInteger">1</owl:maxQualifiedCardinality>
                <owl:onClass rdf:resource="https://w3id.org/leo/onto/animal/FarmAnimalDestination"/>
            </owl:Restriction>
        </rdfs:subClassOf>
        <rdfs:subClassOf>
            <owl:Restriction>
                <owl:onProperty rdf:resource="https://w3id.org/leo/onto/ale/numberOfTeats"/>
                <owl:maxQualifiedCardinality rdf:datatype="http://www.w3.org/2001/XMLSchema#nonNegativeInteger">1</owl:maxQualifiedCardinality>
                <owl:onDataRange rdf:resource="http://www.w3.org/2001/XMLSchema#integer"/>
            </owl:Restriction>
        </rdfs:subClassOf>
        <dc:description rdf:resource="https://raw.githubusercontent.com/Bluarancio/Leo-OpenData/master/RappresentazioneGraficaOntologie/PNG/Ale_Birth.png"/>
        <rdfs:comment xml:lang="it">L&apos;evento di nascita dell&apos;animale</rdfs:comment>
        <rdfs:comment xml:lang="en">The birth event of the animal</rdfs:comment>
        <rdfs:isDefinedBy rdf:resource="https://w3id.org/leo/onto/ale"/>
        <rdfs:label xml:lang="en">Birth</rdfs:label>
        <rdfs:label xml:lang="it">Nascita</rdfs:label>
        <owl:versionInfo xml:lang="it">stabile</owl:versionInfo>
        <owl:versionInfo xml:lang="en">stable</owl:versionInfo>
    </owl:Class>
    


    <!-- https://w3id.org/leo/onto/ale/BreastFeedingTermination -->

    <owl:Class rdf:about="https://w3id.org/leo/onto/ale/BreastFeedingTermination">
        <rdfs:subClassOf rdf:resource="https://w3id.org/leo/onto/ale/AnimalLifeEvent"/>
        <rdfs:subClassOf>
            <owl:Restriction>
                <owl:onProperty rdf:resource="https://w3id.org/leo/onto/ale/breastFeedingTerminationDate"/>
                <owl:qualifiedCardinality rdf:datatype="http://www.w3.org/2001/XMLSchema#nonNegativeInteger">1</owl:qualifiedCardinality>
                <owl:onDataRange>
                    <rdfs:Datatype>
                        <owl:unionOf rdf:parseType="Collection">
                            <rdf:Description rdf:about="http://www.w3.org/2001/XMLSchema#date"/>
                            <rdf:Description rdf:about="http://www.w3.org/2001/XMLSchema#dateTime"/>
                        </owl:unionOf>
                    </rdfs:Datatype>
                </owl:onDataRange>
            </owl:Restriction>
        </rdfs:subClassOf>
        <dc:description rdf:resource="https://raw.githubusercontent.com/Bluarancio/Leo-OpenData/master/RappresentazioneGraficaOntologie/PNG/BreastFeedingTermination.png"/>
        <rdfs:comment xml:lang="it">La classe rappresenta l&apos;evento con il quale si indica quando la madre termina l’allattamento dei figli.</rdfs:comment>
        <rdfs:comment xml:lang="en">The class represents the event indicating when the mother finishes breastfeeding her children.</rdfs:comment>
        <rdfs:isDefinedBy rdf:resource="https://w3id.org/leo/onto/ale"/>
        <rdfs:label xml:lang="en">Breast Feeding Termination</rdfs:label>
        <rdfs:label xml:lang="it">Fine dell&apos;Allattamento</rdfs:label>
        <owl:versionInfo xml:lang="it">stabile</owl:versionInfo>
        <owl:versionInfo xml:lang="en">stable</owl:versionInfo>
    </owl:Class>
    


    <!-- https://w3id.org/leo/onto/ale/BreastFeedingType -->

    <owl:Class rdf:about="https://w3id.org/leo/onto/ale/BreastFeedingType">
        <rdfs:subClassOf rdf:resource="https://w3id.org/italia/onto/l0/Characteristic"/>
        <rdfs:comment xml:lang="it">La classe rappresenta il tipo di allattamento che può essere artificiale, naturale o misto.</rdfs:comment>
        <rdfs:comment xml:lang="en">The class represents the type of breastfeeding, which can be artificial, natural or mixed.</rdfs:comment>
        <rdfs:isDefinedBy rdf:resource="https://w3id.org/leo/onto/ale"/>
        <rdfs:label xml:lang="en">Breast Feeding Type</rdfs:label>
        <rdfs:label xml:lang="it">Tipo Allattamento</rdfs:label>
        <owl:versionInfo xml:lang="it">stabile</owl:versionInfo>
        <owl:versionInfo xml:lang="en">stable</owl:versionInfo>
    </owl:Class>
    


    <!-- https://w3id.org/leo/onto/ale/CarcassCategory -->

    <owl:Class rdf:about="https://w3id.org/leo/onto/ale/CarcassCategory">
        <rdfs:subClassOf rdf:resource="https://w3id.org/italia/onto/l0/Concept"/>
        <rdfs:comment xml:lang="it">Categoria utilizzata per la categorizzazione delle carcasse degli animali. Le carcasse sono ripartite in categorie secondo le direttive del regolamento (UE) n. 1308/2013 del Parlamento europeo e del Consiglio del 17 dicembre 2013.

Le categorie in cui sono ripartite le carcasse sono definite in un apposito vocabolario controllato.</rdfs:comment>
        <rdfs:comment xml:lang="en">Category used for the categorisation of animal carcasses. Carcasses are categorised according to the guidelines of Regulation (EU) No 1308/2013 of the European Parliament and of the Council of 17 December 2013.

The categories into which carcasses are divided are defined in a controlled vocabulary.</rdfs:comment>
        <rdfs:isDefinedBy rdf:resource="https://w3id.org/leo/onto/ale"/>
        <rdfs:label xml:lang="en">Carcass Category</rdfs:label>
        <rdfs:label xml:lang="it">Categoria della Carcassa</rdfs:label>
        <owl:versionInfo xml:lang="it">stabile - introdotta nella versione 0.3 dell&apos;ontologia</owl:versionInfo>
        <owl:versionInfo xml:lang="en">stable - introduced in version 0.3 of the ontology</owl:versionInfo>
        <prov:wasDerivedFrom rdf:resource="http://www.w3.org/2004/02/skos/core#"/>
    </owl:Class>
    


    <!-- https://w3id.org/leo/onto/ale/CarcassClassification -->

    <owl:Class rdf:about="https://w3id.org/leo/onto/ale/CarcassClassification">
        <rdfs:subClassOf rdf:resource="https://w3id.org/italia/onto/l0/Topic"/>
        <rdfs:comment xml:lang="en">Classification of the carcass, based on the assessment of its muscle conformation and fat cover.
Muscle conformation defines the development of the carcass profiles and in particular of its essential parts (thigh, back and shoulder).
Fat cover defines the mass of fat on the outside of the carcase and on the inner wall of the thoracic cavity.
Carcass classification is defined in Regulation (EU) No 1308/2013 of the European Parliament and of the Council of 17 December 2013.

Classes for carcass classification are defined in a controlled vocabulary.</rdfs:comment>
        <rdfs:comment xml:lang="it">Classificazione della carcassa, basata sulla valutazione della sua conformazione muscolare e dello stato di ingrassamento.
La Conformazione muscolare definisce lo sviluppo dei profili della carcassa e segnatamente delle sue parti essenziali (coscia, schiena e spalla).
Lo Stato di ingrassamento definisce la massa di grasso all’esterno della carcassa e sulla parete interna della cassa toracica.
La classificazione delle carcasse è definita nel regolamento (UE) n. 1308/2013 del Parlamento europeo e del Consiglio del 17 dicembre 2013.

Le classi per la classificazione delle carcasse sono definite in un apposito vocabolario controllato.</rdfs:comment>
        <rdfs:isDefinedBy rdf:resource="https://w3id.org/leo/onto/ale"/>
        <rdfs:label xml:lang="en">Carcass Classification</rdfs:label>
        <rdfs:label xml:lang="it">Classificazione Carcassa</rdfs:label>
        <owl:versionInfo xml:lang="it">stabile - introdotta nella versione 0.3 dell&apos;ontologia</owl:versionInfo>
        <owl:versionInfo xml:lang="en">stable - introduced in version 0.3 of the ontology</owl:versionInfo>
        <prov:wasDerivedFrom rdf:resource="http://www.w3.org/2004/02/skos/core#"/>
    </owl:Class>
    


    <!-- https://w3id.org/leo/onto/ale/CarcassConformation -->

    <owl:Class rdf:about="https://w3id.org/leo/onto/ale/CarcassConformation">
        <rdfs:subClassOf rdf:resource="https://w3id.org/italia/onto/l0/Concept"/>
        <rdfs:comment xml:lang="en">Carcass conformation, defined as the development of the carcass profiles and in particular of its essential parts (leg, back, shoulder). Carcasses are classified according to conformation in accordance with the guidelines of Regulation (EU) No 1308/2013 of the European Parliament and of the Council of 17 December 2013.

Conformation classes for carcasses are defined in a controlled vocabulary.</rdfs:comment>
        <rdfs:comment xml:lang="it">Conformazione della carcassa, definita come sviluppo dei profili della carcassa e segnatamente delle sue parti essenziali (coscia, schiena, spalla). Le carcasse sono classificate in base alla conformazione secondo le direttive del regolamento (UE) n. 1308/2013 del Parlamento europeo e del Consiglio del 17 dicembre 2013.

Le classi di conformazione per le carcasse sono definite in un apposito vocabolario controllato.</rdfs:comment>
        <rdfs:isDefinedBy rdf:resource="https://w3id.org/leo/onto/ale"/>
        <rdfs:label xml:lang="en">Carcass Conformation</rdfs:label>
        <rdfs:label xml:lang="it">Conformazione Carcassa</rdfs:label>
        <owl:versionInfo xml:lang="it">stabile - introdotta nella versione 0.3 dell&apos;ontologia</owl:versionInfo>
        <owl:versionInfo xml:lang="en">stable - introduced in version 0.3 of the ontology</owl:versionInfo>
        <prov:wasDerivedFrom rdf:resource="http://www.w3.org/2004/02/skos/core#"/>
    </owl:Class>
    


    <!-- https://w3id.org/leo/onto/ale/Diagnosis -->

    <owl:Class rdf:about="https://w3id.org/leo/onto/ale/Diagnosis">
        <rdfs:subClassOf rdf:resource="https://w3id.org/leo/onto/ale/AnimalLifeEvent"/>
        <rdfs:subClassOf>
            <owl:Restriction>
                <owl:onProperty rdf:resource="https://w3id.org/leo/onto/ale/diagnosisDate"/>
                <owl:qualifiedCardinality rdf:datatype="http://www.w3.org/2001/XMLSchema#nonNegativeInteger">1</owl:qualifiedCardinality>
                <owl:onDataRange>
                    <rdfs:Datatype>
                        <owl:unionOf rdf:parseType="Collection">
                            <rdf:Description rdf:about="http://www.w3.org/2001/XMLSchema#date"/>
                            <rdf:Description rdf:about="http://www.w3.org/2001/XMLSchema#dateTime"/>
                        </owl:unionOf>
                    </rdfs:Datatype>
                </owl:onDataRange>
            </owl:Restriction>
        </rdfs:subClassOf>
        <dc:description rdf:resource="https://raw.githubusercontent.com/Bluarancio/Leo-OpenData/master/RappresentazioneGraficaOntologie/PNG/Ale_Diagnosis.png"/>
        <rdfs:comment xml:lang="it">L&apos;evento della diagnosi di qualsiasi tipo. Include la diagnosi della gravidanza.</rdfs:comment>
        <rdfs:comment xml:lang="en">The event of diagnosis including the pregnancy diagnosis</rdfs:comment>
        <rdfs:isDefinedBy rdf:resource="https://w3id.org/leo/onto/ale"/>
        <rdfs:label xml:lang="it">Diagnosi</rdfs:label>
        <rdfs:label xml:lang="en">Diagnosis</rdfs:label>
        <owl:versionInfo xml:lang="it">stabile</owl:versionInfo>
        <owl:versionInfo xml:lang="en">stable</owl:versionInfo>
    </owl:Class>
    


    <!-- https://w3id.org/leo/onto/ale/Disposal -->

    <owl:Class rdf:about="https://w3id.org/leo/onto/ale/Disposal">
        <rdfs:subClassOf rdf:resource="https://w3id.org/leo/onto/ale/AnimalLifeEvent"/>
        <rdfs:subClassOf>
            <owl:Restriction>
                <owl:onProperty rdf:resource="https://w3id.org/leo/onto/ale/hasDisposalReason"/>
                <owl:maxQualifiedCardinality rdf:datatype="http://www.w3.org/2001/XMLSchema#nonNegativeInteger">1</owl:maxQualifiedCardinality>
                <owl:onClass rdf:resource="https://w3id.org/leo/onto/ale/DisposalReason"/>
            </owl:Restriction>
        </rdfs:subClassOf>
        <rdfs:subClassOf>
            <owl:Restriction>
                <owl:onProperty rdf:resource="https://w3id.org/leo/onto/ale/disposalDate"/>
                <owl:qualifiedCardinality rdf:datatype="http://www.w3.org/2001/XMLSchema#nonNegativeInteger">1</owl:qualifiedCardinality>
                <owl:onDataRange>
                    <rdfs:Datatype>
                        <owl:unionOf rdf:parseType="Collection">
                            <rdf:Description rdf:about="http://www.w3.org/2001/XMLSchema#date"/>
                            <rdf:Description rdf:about="http://www.w3.org/2001/XMLSchema#dateTime"/>
                        </owl:unionOf>
                    </rdfs:Datatype>
                </owl:onDataRange>
            </owl:Restriction>
        </rdfs:subClassOf>
        <dc:description rdf:resource="https://raw.githubusercontent.com/Bluarancio/Leo-OpenData/master/RappresentazioneGraficaOntologie/PNG/Ale_Disposal.png"/>
        <rdfs:comment xml:lang="en">This is the event whereby the farmed animal is removed from the farm permanently for a number of reasons related to management or to pathological or metabolic states. Disposal represents the exit of the animal from the farm for any reason (e.g. sale to another farm, slaughter, death on the farm, etc.).

Possible applications: Managerial. Calculation of the length of the productive career of the animal, of the average farm longevity. Correct identification of the movements (sale/purchase) of the animal. Technical assistance data for estimation of company replacement rates</rdfs:comment>
        <rdfs:comment xml:lang="it">È l’evento per il quale l’animale allevato viene allontanato dall’azienda in maniera definitiva per una serie di cause legate alla managerialità o a stati patologici o metabolici. L’eliminazione rappresenta l’uscita del capo dall’azienda per qualsiasi motivo (ad esempio, vendita ad altro allevamento, macellazione, morte in azienda, ecc).

Possibili Applicazioni: Manageriale. Calcolo della lunghezza della carriera produttiva dell&apos;animale, della longevità media aziendale. Corretta identificazione degli spostamenti (vendita/acquisto) del soggetto. Dato di assistenza tecnica per la stima dei tassi di rimonta aziendali.</rdfs:comment>
        <rdfs:isDefinedBy rdf:resource="https://w3id.org/leo/onto/ale"/>
        <rdfs:label xml:lang="en">Disposal</rdfs:label>
        <rdfs:label xml:lang="it">Eliminazione</rdfs:label>
        <owl:versionInfo xml:lang="it">stabile</owl:versionInfo>
        <owl:versionInfo xml:lang="en">stable</owl:versionInfo>
    </owl:Class>
    


    <!-- https://w3id.org/leo/onto/ale/DisposalReason -->

    <owl:Class rdf:about="https://w3id.org/leo/onto/ale/DisposalReason">
        <owl:equivalentClass>
            <owl:Class>
                <owl:oneOf rdf:parseType="Collection">
                    <rdf:Description rdf:about="https://w3id.org/leo/onto/ale/DeathPasture"/>
                    <rdf:Description rdf:about="https://w3id.org/leo/onto/ale/DeathStable"/>
                    <rdf:Description rdf:about="https://w3id.org/leo/onto/ale/SelfConsumptionSlaughtering"/>
                    <rdf:Description rdf:about="https://w3id.org/leo/onto/ale/SlaughterHealth"/>
                    <rdf:Description rdf:about="https://w3id.org/leo/onto/ale/SlaughterWellness"/>
                    <rdf:Description rdf:about="https://w3id.org/leo/onto/ale/Slaughterhouse"/>
                    <rdf:Description rdf:about="https://w3id.org/leo/onto/ale/Theft"/>
                    <rdf:Description rdf:about="https://w3id.org/leo/onto/ale/UrgentSlaughterStable"/>
                </owl:oneOf>
            </owl:Class>
        </owl:equivalentClass>
        <rdfs:subClassOf rdf:resource="https://w3id.org/italia/onto/l0/Characteristic"/>
        <rdfs:comment xml:lang="en">It is the reason why the animal was eliminated.</rdfs:comment>
        <rdfs:comment xml:lang="it">È il motivo per il quale l&apos;animale è stato eliminato.</rdfs:comment>
        <rdfs:isDefinedBy rdf:resource="https://w3id.org/leo/onto/ale"/>
        <rdfs:label xml:lang="en">Disposal Reason</rdfs:label>
        <rdfs:label xml:lang="it">Motivazione Eliminazione</rdfs:label>
        <owl:versionInfo xml:lang="it">stabile</owl:versionInfo>
        <owl:versionInfo xml:lang="en">stable</owl:versionInfo>
    </owl:Class>
    


    <!-- https://w3id.org/leo/onto/ale/Dry -->

    <owl:Class rdf:about="https://w3id.org/leo/onto/ale/Dry">
        <rdfs:subClassOf rdf:resource="https://w3id.org/leo/onto/ale/AnimalLifeEvent"/>
        <rdfs:subClassOf>
            <owl:Restriction>
                <owl:onProperty rdf:resource="https://w3id.org/leo/onto/ale/dryDate"/>
                <owl:qualifiedCardinality rdf:datatype="http://www.w3.org/2001/XMLSchema#nonNegativeInteger">1</owl:qualifiedCardinality>
                <owl:onDataRange>
                    <rdfs:Datatype>
                        <owl:unionOf rdf:parseType="Collection">
                            <rdf:Description rdf:about="http://www.w3.org/2001/XMLSchema#date"/>
                            <rdf:Description rdf:about="http://www.w3.org/2001/XMLSchema#dateTime"/>
                        </owl:unionOf>
                    </rdfs:Datatype>
                </owl:onDataRange>
            </owl:Restriction>
        </rdfs:subClassOf>
        <dc:description rdf:resource="https://raw.githubusercontent.com/Bluarancio/Leo-OpenData/master/RappresentazioneGraficaOntologie/PNG/Ale_Dry.png"/>
        <rdfs:comment xml:lang="it">L&apos;evento dell&apos;asciutta. Nei soggetti allevati per la produzione di latte, il termine indica la cessazione, naturale o più spesso indotta con opportune pratiche dall&apos;allevatore, della produzione di latte nell&apos;ultima fase di lattazione in modo che l&apos;animale possa utilizzare le energie esclusivamente per recupero del peso e formazione di riserve corporee per il parto e la lattazione successiva.

Possibili applicazioni: Riproduzione. Calcolo dello stato riproduttivo dell&apos;animale. Calcolo lunghezza della lattazione e della durata della preparazione al parto successivo. Individuazione lattazioni corte. Assistenza tecnica.</rdfs:comment>
        <rdfs:comment xml:lang="en">The dry event. In animals bred for milk production, the term indicates the cessation, natural or more often induced with appropriate practices by the farmer, of milk production in the last phase of lactation so that the animal can use its energy exclusively for weight recovery and the formation of body reserves for parturition and subsequent lactation.

Possible applications: Reproduction. Calculation of the animal&apos;s reproductive status. Calculation of lactation length and duration of preparation for the next calving. Identification of short lactations. Technical assistance.</rdfs:comment>
        <rdfs:isDefinedBy rdf:resource="https://w3id.org/leo/onto/ale"/>
        <rdfs:label xml:lang="it">Asciutta</rdfs:label>
        <rdfs:label xml:lang="en">Dry</rdfs:label>
        <owl:versionInfo xml:lang="it">stabile</owl:versionInfo>
        <owl:versionInfo xml:lang="en">stable</owl:versionInfo>
    </owl:Class>
    


    <!-- https://w3id.org/leo/onto/ale/EaseOfParturition -->

    <owl:Class rdf:about="https://w3id.org/leo/onto/ale/EaseOfParturition">
        <owl:equivalentClass>
            <owl:Class>
                <owl:oneOf rdf:parseType="Collection">
                    <rdf:Description rdf:about="https://w3id.org/leo/onto/ale/Assistant"/>
                    <rdf:Description rdf:about="https://w3id.org/leo/onto/ale/CaesareanSection"/>
                    <rdf:Description rdf:about="https://w3id.org/leo/onto/ale/Difficult"/>
                    <rdf:Description rdf:about="https://w3id.org/leo/onto/ale/Easy"/>
                    <rdf:Description rdf:about="https://w3id.org/leo/onto/ale/Embryotomy"/>
                </owl:oneOf>
            </owl:Class>
        </owl:equivalentClass>
        <rdfs:subClassOf rdf:resource="https://w3id.org/italia/onto/l0/Characteristic"/>
        <rdfs:comment xml:lang="en">Subjective assessment of the breeder or technician to indicate whether the female has given birth without problems or needs assistance. The instances of the class can assume one of these values: &quot;Easy&quot;, &quot;Assistant, no tools&quot;, &quot;Cesarean Section&quot;, &quot;Difficult, with multiple assistants&quot;, &quot;Embryotomy&quot;.</rdfs:comment>
        <rdfs:comment xml:lang="it">Valutazione soggettiva dell’allevatore o del tecnico attraverso la quale viene indicato se la femmina ha partorito senza problemi o ha avuto bisogno di assistenza. Le istanze della classe possono assumere uno tra questi valori: &quot;Facile&quot;, &quot;Assistente, no strumenti&quot;, &quot;Taglio Cesareo&quot;, &quot;Difficile, con più assitenti&quot;, &quot;Embriotomia&quot;.</rdfs:comment>
        <rdfs:isDefinedBy rdf:resource="https://w3id.org/leo/onto/ale"/>
        <rdfs:label xml:lang="en">Ease of Parturition</rdfs:label>
        <rdfs:label xml:lang="it">Facilità di Parto</rdfs:label>
        <owl:versionInfo xml:lang="it">stabile - aggiunto nella seconda versione dell&apos;ontologia</owl:versionInfo>
        <owl:versionInfo xml:lang="en">stable - added in the second version of the ontology</owl:versionInfo>
    </owl:Class>
    


    <!-- https://w3id.org/leo/onto/ale/EmbryoResorption -->

    <owl:Class rdf:about="https://w3id.org/leo/onto/ale/EmbryoResorption">
        <rdfs:subClassOf rdf:resource="https://w3id.org/leo/onto/ale/AnimalLifeEvent"/>
        <rdfs:subClassOf>
            <owl:Restriction>
                <owl:onProperty rdf:resource="https://w3id.org/leo/onto/ale/embryoResorptionDate"/>
                <owl:qualifiedCardinality rdf:datatype="http://www.w3.org/2001/XMLSchema#nonNegativeInteger">1</owl:qualifiedCardinality>
                <owl:onDataRange>
                    <rdfs:Datatype>
                        <owl:unionOf rdf:parseType="Collection">
                            <rdf:Description rdf:about="http://www.w3.org/2001/XMLSchema#date"/>
                            <rdf:Description rdf:about="http://www.w3.org/2001/XMLSchema#dateTime"/>
                        </owl:unionOf>
                    </rdfs:Datatype>
                </owl:onDataRange>
            </owl:Restriction>
        </rdfs:subClassOf>
        <dc:description rdf:resource="https://raw.githubusercontent.com/Bluarancio/Leo-OpenData/master/RappresentazioneGraficaOntologie/PNG/Ale_EmbryonicResorption.png"/>
        <rdfs:comment xml:lang="it">L&apos;evento della vita dell&apos;animale di riassorbimento embrionale avvenuto in azienda. Definito in termini clinici come &apos;morte embrionale”, è un fenomeno che consiste nella morte dell&apos;embrione/feto durante le prime fasi di gravidanza. Nei bovini da latte la morte embrionale si distingue in tre sottogruppi: morte embrionale precoce (primi 16 giorni dall&apos;inseminazione), morte embrionale tardiva (da 17 a 42 giorni dall&apos;inseminazione) e morte fetale dopo i 42 giorni di gravidanza.

Possibili Applicazioni: Riproduzione e Benessere. Calcolo dello stato riproduttivo dell&apos;animale. Calcolo del tasso di abortività aziendale, dei fattori di rischio per il benessere e per la fertilità. Assistenza tecnica. Gestione sanitaria</rdfs:comment>
        <rdfs:comment xml:lang="en">The event in the animal&apos;s life of embryo resorption occurring on the farm company. Defined in clinical terms as &apos;embryonic death&apos;, it is a phenomenon consisting of the death of the embryo/fetus during the early stages of pregnancy. In dairy cattle, embryo death can be divided into three subgroups: early embryo death (first 16 days after insemination), late embryo death (17 to 42 days after insemination) and foetal death after 42 days of pregnancy.

Possible applications: Reproduction and Welfare. Calculation of the reproductive status of the animal. Calculation of abortion rate, welfare and fertility risk factors. Technical assistance. Health management.</rdfs:comment>
        <rdfs:isDefinedBy rdf:resource="https://w3id.org/leo/onto/ale"/>
        <rdfs:label xml:lang="en">Embryo Resorption</rdfs:label>
        <rdfs:label xml:lang="it">Riassorbimento Embrionale</rdfs:label>
        <owl:versionInfo xml:lang="it">stabile</owl:versionInfo>
        <owl:versionInfo xml:lang="en">stable</owl:versionInfo>
    </owl:Class>
    


    <!-- https://w3id.org/leo/onto/ale/EntryInFarmReason -->

    <owl:Class rdf:about="https://w3id.org/leo/onto/ale/EntryInFarmReason">
        <rdfs:subClassOf rdf:resource="https://w3id.org/italia/onto/l0/Characteristic"/>
        <rdfs:comment xml:lang="it">La classe rappresenta tutte le motivazioni per l&apos;ingresso in allevamento di un&apos;animale d&apos;allevamento. Gli individui di questa classe sono tutti i concetti come definiti nel seguente vocabolario controllato: https://w3id.org/leo/controlled-vocabulary/entry-in-farm-reason. Esempi includono: nato in stalla, acquistato da un paese EU, ecc.</rdfs:comment>
        <rdfs:comment xml:lang="en">The class represents all the possible reasons for a farm animal to enter in a livestock company. The individuals of this class are all the concepts of the following controlled vocabulary https://w3id.org/leo/controlled-vocabulary/entry-in-farm-reason. Examples include: born in stable, bought from an EU country, etc.</rdfs:comment>
        <rdfs:isDefinedBy rdf:resource="https://w3id.org/leo/onto/ale"/>
        <rdfs:label xml:lang="en">Entry in Farm Reason</rdfs:label>
        <rdfs:label xml:lang="it">Motivo di Ingresso in Allevamento</rdfs:label>
        <owl:versionInfo xml:lang="it">stabile - introdotta nella versione 0.4 dell&apos;ontologia</owl:versionInfo>
        <owl:versionInfo xml:lang="en">stable - introduced in versione 0.4 of the ontology</owl:versionInfo>
        <prov:wasDerivedFrom rdf:resource="http://www.w3.org/2004/02/skos/core#"/>
    </owl:Class>
    


    <!-- https://w3id.org/leo/onto/ale/ExitFromFarmReason -->

    <owl:Class rdf:about="https://w3id.org/leo/onto/ale/ExitFromFarmReason">
        <rdfs:subClassOf rdf:resource="https://w3id.org/italia/onto/l0/Characteristic"/>
        <rdfs:comment xml:lang="it">La classe di tutti i possibili motivi di uscita dall&apos;allevamento dell&apos;animale d&apos;allevamento. Gli individui della classe sono tutti i concetti rappresentati nel seguente vocabolario controllato https://w3id.org/leo/controlled-vocabulary/exit-from-farm-reason. Esempi includono:  uscita verso macello, uscita verso circo, venduto a paese estero, ecc.</rdfs:comment>
        <rdfs:comment xml:lang="en">The class of all the possible reasons for a farm animal to exit from a livestock company. The individuals of this class are all the concepts of the following controlled vocabulary: https://w3id.org/leo/controlled-vocabulary/exit-from-farm-reason. Examples include: exit toward slaughterhouse, sold to a foreign country, etc.</rdfs:comment>
        <rdfs:isDefinedBy rdf:resource="https://w3id.org/leo/onto/ale"/>
        <rdfs:label xml:lang="en">Exit from Farm Reason</rdfs:label>
        <rdfs:label xml:lang="it">Motivo di Uscita dall&apos;Allevamento</rdfs:label>
        <owl:versionInfo xml:lang="it">stabile - introdotta nella versione 0.4 dell&apos;ontologia</owl:versionInfo>
        <owl:versionInfo xml:lang="en">stable - introduced in version 0.4 of the ontology</owl:versionInfo>
        <prov:wasDerivedFrom rdf:resource="http://www.w3.org/2004/02/skos/core#"/>
    </owl:Class>
    


    <!-- https://w3id.org/leo/onto/ale/FarmAnimalCarcass -->

    <owl:Class rdf:about="https://w3id.org/leo/onto/ale/FarmAnimalCarcass">
        <rdfs:subClassOf rdf:resource="https://w3id.org/italia/onto/l0/Object"/>
        <rdfs:comment xml:lang="it">La classe delle carcasse degli animali d&apos;allevamento. Per &apos;carcassa&apos; si intende il corpo dell&apos;animale macellato. Nel caso di bovini, si intende il corpo intero dell&apos;animale macellato, dopo le operazioni di dissanguamento, svisceramento e scuoiamento.</rdfs:comment>
        <rdfs:comment xml:lang="en">The class of the carcass of the farm animals. &apos;Carcass&apos; means the body of the slaughtered animal. In the case of bovine animals, it means the whole body of the slaughtered animal, after bleeding, evisceration and skinning.</rdfs:comment>
        <rdfs:isDefinedBy rdf:resource="https://w3id.org/leo/onto/ale"/>
        <rdfs:label xml:lang="it">Carcassa dell&apos;Animale</rdfs:label>
        <rdfs:label xml:lang="en">Farm Animal Carcass</rdfs:label>
        <owl:versionInfo xml:lang="it">stabile - introdotta della versione 0.3 dell&apos;ontologia</owl:versionInfo>
        <owl:versionInfo xml:lang="en">stable - introduced in version 0.3 of the ontology</owl:versionInfo>
    </owl:Class>
    


    <!-- https://w3id.org/leo/onto/ale/FatCover -->

    <owl:Class rdf:about="https://w3id.org/leo/onto/ale/FatCover">
        <rdfs:subClassOf rdf:resource="https://w3id.org/italia/onto/l0/Concept"/>
        <rdfs:comment xml:lang="en">Fat cover status of the carcass, defined as the mass of fat on the outside of the carcass and on the inner wall of the thoracic cavity. Carcasses are classified according to their fat cover status in accordance with the guidelines of Regulation (EU) No 1308/2013 of the European Parliament and of the Council of 17 December 2013.

Classes of fat cover status for carcasses are defined in a controlled vocabulary.</rdfs:comment>
        <rdfs:comment xml:lang="it">Stato d&apos;ingrassamento della carcassa, definito come massa di grasso all&apos;esterno della carcassa e sulla parete interna della cassa toracica. Le carcasse sono classificate in base allo stato d&apos;ingrassamento secondo le direttive del regolamento (UE) n. 1308/2013 del Parlamento europeo e del Consiglio del 17 dicembre 2013.

Le classi di stato di ingrassamento per le carcasse sono definite in un apposito vocabolario controllato.</rdfs:comment>
        <rdfs:isDefinedBy rdf:resource="https://w3id.org/leo/onto/ale"/>
        <rdfs:label xml:lang="en">Fat Cover</rdfs:label>
        <rdfs:label xml:lang="it">Stato d&apos;Ingrassamento</rdfs:label>
        <owl:versionInfo xml:lang="it">stabile - introdotta nella versione 0.3 dell&apos;ontologia</owl:versionInfo>
        <owl:versionInfo xml:lang="en">stable - introduced in the version 0.3 of the ontology</owl:versionInfo>
        <prov:wasDerivedFrom rdf:resource="http://www.w3.org/2004/02/skos/core#"/>
    </owl:Class>
    


    <!-- https://w3id.org/leo/onto/ale/Fertilization -->

    <owl:Class rdf:about="https://w3id.org/leo/onto/ale/Fertilization">
        <rdfs:subClassOf rdf:resource="https://w3id.org/leo/onto/ale/AnimalLifeEvent"/>
        <rdfs:subClassOf>
            <owl:Restriction>
                <owl:onProperty rdf:resource="https://w3id.org/leo/onto/ale/hasBreederBreed"/>
                <owl:maxQualifiedCardinality rdf:datatype="http://www.w3.org/2001/XMLSchema#nonNegativeInteger">1</owl:maxQualifiedCardinality>
                <owl:onClass rdf:resource="https://w3id.org/leo/onto/animal/Breed"/>
            </owl:Restriction>
        </rdfs:subClassOf>
        <rdfs:subClassOf>
            <owl:Restriction>
                <owl:onProperty rdf:resource="https://w3id.org/leo/onto/ale/hasFertilizationType"/>
                <owl:maxQualifiedCardinality rdf:datatype="http://www.w3.org/2001/XMLSchema#nonNegativeInteger">1</owl:maxQualifiedCardinality>
                <owl:onClass rdf:resource="https://w3id.org/leo/onto/ale/FertilizationType"/>
            </owl:Restriction>
        </rdfs:subClassOf>
        <rdfs:subClassOf>
            <owl:Restriction>
                <owl:onProperty rdf:resource="https://w3id.org/leo/onto/ale/fertilizationDate"/>
                <owl:qualifiedCardinality rdf:datatype="http://www.w3.org/2001/XMLSchema#nonNegativeInteger">1</owl:qualifiedCardinality>
                <owl:onDataRange>
                    <rdfs:Datatype>
                        <owl:unionOf rdf:parseType="Collection">
                            <rdf:Description rdf:about="http://www.w3.org/2001/XMLSchema#date"/>
                            <rdf:Description rdf:about="http://www.w3.org/2001/XMLSchema#dateTime"/>
                        </owl:unionOf>
                    </rdfs:Datatype>
                </owl:onDataRange>
            </owl:Restriction>
        </rdfs:subClassOf>
        <dc:description rdf:resource="https://raw.githubusercontent.com/Bluarancio/Leo-OpenData/master/RappresentazioneGraficaOntologie/PNG/Ale_Fertilization.png"/>
        <rdfs:comment xml:lang="it">L&apos;evento di fecondazione dell&apos;animale. È l’atto fecondativo dell’animale. La più diffusa, in particolare nei bovini, è l’inseminazione artificiale che è la pratica di introdurre seme nell’utero di una riproduttrice tramite un’apposita strumentazione senza ricorrere all’accoppiamento. Fondamentale nell’attività di miglioramento genetico, permette di migliorare, nella progenie, la produzione di latte o altre caratteristiche diffondendo i geni favorevoli del maschio nella popolazione.

Possibili Applicazioni: Riproduzione e Benessere. Calcolo dello stato riproduttivo dell&apos;animale. Calcolo dei parametri di fertilità. Assistenza tecnica. Miglioramento genetico (fertilità).</rdfs:comment>
        <rdfs:comment xml:lang="en">The fertilization of the animal event. This is the fertilising act of the animal. The most widely used, particularly in cattle, is artificial insemination, which is the practice of introducing semen into the uterus of a breeding animal by means of a special device without recourse to mating. It is essential in genetic improvement, as it improves milk production or other characteristics in the offspring by spreading favourable male genes throughout the population.

Possible applications: Reproduction and Welfare. Calculation of the reproductive status of the animal. Calculation of fertility parameters. Technical assistance. Genetic improvement (fertility).</rdfs:comment>
        <rdfs:isDefinedBy rdf:resource="https://w3id.org/leo/onto/ale"/>
        <rdfs:label xml:lang="it">Fecondazione</rdfs:label>
        <rdfs:label xml:lang="en">Fertilization</rdfs:label>
        <rdfs:label xml:lang="en">Insemination</rdfs:label>
        <rdfs:label xml:lang="it">Inseminazione</rdfs:label>
        <owl:versionInfo xml:lang="it">stabile</owl:versionInfo>
        <owl:versionInfo xml:lang="en">stable</owl:versionInfo>
    </owl:Class>
    


    <!-- https://w3id.org/leo/onto/ale/FertilizationType -->

    <owl:Class rdf:about="https://w3id.org/leo/onto/ale/FertilizationType">
        <owl:equivalentClass>
            <owl:Class>
                <owl:oneOf rdf:parseType="Collection">
                    <rdf:Description rdf:about="https://w3id.org/leo/onto/ale/FEA"/>
                    <rdf:Description rdf:about="https://w3id.org/leo/onto/ale/FEG"/>
                    <rdf:Description rdf:about="https://w3id.org/leo/onto/ale/FEN"/>
                </owl:oneOf>
            </owl:Class>
        </owl:equivalentClass>
        <rdfs:subClassOf rdf:resource="https://w3id.org/italia/onto/l0/Characteristic"/>
        <rdfs:comment xml:lang="it">Indica se la fecondazione subita dalla femmina è stata effettuata attraverso una fecondazione artificiale o naturale o gestita in un gruppo di monta.</rdfs:comment>
        <rdfs:comment xml:lang="en">Indicates whether the fertilisation undergone by the female was carried out through artificial or natural fertilisation or managed in a mating group.</rdfs:comment>
        <rdfs:isDefinedBy rdf:resource="https://w3id.org/leo/onto/ale"/>
        <rdfs:label xml:lang="en">Fertilization Type</rdfs:label>
        <rdfs:label xml:lang="it">Tipo Fecondazione</rdfs:label>
        <owl:versionInfo xml:lang="it">stabile</owl:versionInfo>
        <owl:versionInfo xml:lang="en">stable</owl:versionInfo>
    </owl:Class>
    


    <!-- https://w3id.org/leo/onto/ale/Identification -->

    <owl:Class rdf:about="https://w3id.org/leo/onto/ale/Identification">
        <rdfs:subClassOf rdf:resource="https://w3id.org/leo/onto/ale/AnimalLifeEvent"/>
        <rdfs:subClassOf>
            <owl:Restriction>
                <owl:onProperty rdf:resource="https://w3id.org/leo/onto/animal/uniqueAnimalNumber"/>
                <owl:cardinality rdf:datatype="http://www.w3.org/2001/XMLSchema#nonNegativeInteger">1</owl:cardinality>
            </owl:Restriction>
        </rdfs:subClassOf>
        <rdfs:subClassOf>
            <owl:Restriction>
                <owl:onProperty rdf:resource="https://w3id.org/leo/onto/ale/identificationDate"/>
                <owl:maxQualifiedCardinality rdf:datatype="http://www.w3.org/2001/XMLSchema#nonNegativeInteger">1</owl:maxQualifiedCardinality>
                <owl:onDataRange>
                    <rdfs:Datatype>
                        <owl:unionOf rdf:parseType="Collection">
                            <rdf:Description rdf:about="http://www.w3.org/2001/XMLSchema#date"/>
                            <rdf:Description rdf:about="http://www.w3.org/2001/XMLSchema#dateTime"/>
                        </owl:unionOf>
                    </rdfs:Datatype>
                </owl:onDataRange>
            </owl:Restriction>
        </rdfs:subClassOf>
        <dc:description rdf:resource="https://raw.githubusercontent.com/Bluarancio/Leo-OpenData/master/RappresentazioneGraficaOntologie/PNG/Ale_Identification.png"/>
        <rdfs:comment xml:lang="it">L&apos;evento della vita dell&apos;animale che consente la sua identificazione in azienda. In particolare, è l’evento con il quale avviene l’immatricolazione del soggetto. Il codice attribuito è unico sul territorio nazionale. Permette una identificazione univoca dell’animale in tutte le fasi dell’allevamento e di tracciarne gli spostamenti fino al macello. Fondamentale sia per la gestione dell’azienda sia per tutte le attività legate alla profilassi zootecnica e tracciamento dell’animale e dei suoi prodotti.

Possibili Applicazioni: Identificativo. Univoca identificazione del soggetto, dato chiave nel database relazionale.</rdfs:comment>
        <rdfs:comment xml:lang="en">The event in the life of the animal that enables it to be identified on the farm. In particular, it is the event with which the registration of the animal takes place. The code assigned is unique on the national territory. It allows a unique identification of the animal in all the phases of the breeding and to trace its movements up to the slaughterhouse. Fundamental both for management of the farm and for all activities linked to zootechnical prophylaxis and tracking of the animal and its products.

Possible applications: Identification. Unique identification of the subject, key data in the relational database.</rdfs:comment>
        <rdfs:isDefinedBy rdf:resource="https://w3id.org/leo/onto/ale"/>
        <rdfs:label xml:lang="en">Identification</rdfs:label>
        <rdfs:label xml:lang="it">Identificazione</rdfs:label>
        <owl:versionInfo xml:lang="it">provvisorio</owl:versionInfo>
        <owl:versionInfo xml:lang="en">unstable</owl:versionInfo>
    </owl:Class>
    


    <!-- https://w3id.org/leo/onto/ale/Implantation -->

    <owl:Class rdf:about="https://w3id.org/leo/onto/ale/Implantation">
        <rdfs:subClassOf rdf:resource="https://w3id.org/leo/onto/ale/AnimalLifeEvent"/>
        <rdfs:subClassOf>
            <owl:Restriction>
                <owl:onProperty rdf:resource="https://w3id.org/leo/onto/ale/hasBreederBreed"/>
                <owl:maxQualifiedCardinality rdf:datatype="http://www.w3.org/2001/XMLSchema#nonNegativeInteger">1</owl:maxQualifiedCardinality>
                <owl:onClass rdf:resource="https://w3id.org/leo/onto/animal/Breed"/>
            </owl:Restriction>
        </rdfs:subClassOf>
        <rdfs:subClassOf>
            <owl:Restriction>
                <owl:onProperty rdf:resource="https://w3id.org/leo/onto/ale/implantationDate"/>
                <owl:qualifiedCardinality rdf:datatype="http://www.w3.org/2001/XMLSchema#nonNegativeInteger">1</owl:qualifiedCardinality>
                <owl:onDataRange>
                    <rdfs:Datatype>
                        <owl:unionOf rdf:parseType="Collection">
                            <rdf:Description rdf:about="http://www.w3.org/2001/XMLSchema#date"/>
                            <rdf:Description rdf:about="http://www.w3.org/2001/XMLSchema#dateTime"/>
                        </owl:unionOf>
                    </rdfs:Datatype>
                </owl:onDataRange>
            </owl:Restriction>
        </rdfs:subClassOf>
        <dc:description rdf:resource="https://raw.githubusercontent.com/Bluarancio/Leo-OpenData/master/RappresentazioneGraficaOntologie/PNG/Ale_Implantation.png"/>
        <rdfs:comment xml:lang="it">L&apos;evento della vita dell&apos;animale dell&apos;impianto.</rdfs:comment>
        <rdfs:comment xml:lang="en">The animal&apos;s life event of the implantation.</rdfs:comment>
        <rdfs:isDefinedBy rdf:resource="https://w3id.org/leo/onto/ale"/>
        <rdfs:label xml:lang="it">Impianto</rdfs:label>
        <rdfs:label xml:lang="en">Implantation</rdfs:label>
        <owl:versionInfo xml:lang="it">stabile - aggiunto nella seconda versione dell&apos;ontologia</owl:versionInfo>
        <owl:versionInfo xml:lang="en">stable - added in the second version of the ontology</owl:versionInfo>
    </owl:Class>
    


    <!-- https://w3id.org/leo/onto/ale/InboundMovement -->

    <owl:Class rdf:about="https://w3id.org/leo/onto/ale/InboundMovement">
        <rdfs:subClassOf rdf:resource="https://w3id.org/leo/onto/ale/AnimalLifeEvent"/>
        <rdfs:subClassOf>
            <owl:Restriction>
                <owl:onProperty rdf:resource="https://w3id.org/leo/onto/ale/hasEntryInFarmReason"/>
                <owl:allValuesFrom rdf:resource="https://w3id.org/leo/onto/ale/EntryInFarmReason"/>
            </owl:Restriction>
        </rdfs:subClassOf>
        <rdfs:subClassOf>
            <owl:Restriction>
                <owl:onProperty rdf:resource="https://w3id.org/leo/onto/ale/hasAnimalOwnerCompany"/>
                <owl:maxQualifiedCardinality rdf:datatype="http://www.w3.org/2001/XMLSchema#nonNegativeInteger">1</owl:maxQualifiedCardinality>
                <owl:onClass rdf:resource="https://w3id.org/leo/onto/co/LivestockFarm"/>
            </owl:Restriction>
        </rdfs:subClassOf>
        <rdfs:subClassOf>
            <owl:Restriction>
                <owl:onProperty rdf:resource="https://w3id.org/leo/onto/animal/hasProductionTarget"/>
                <owl:maxQualifiedCardinality rdf:datatype="http://www.w3.org/2001/XMLSchema#nonNegativeInteger">1</owl:maxQualifiedCardinality>
                <owl:onClass rdf:resource="https://w3id.org/leo/onto/animal/ProductionType"/>
            </owl:Restriction>
        </rdfs:subClassOf>
        <rdfs:subClassOf>
            <owl:Restriction>
                <owl:onProperty rdf:resource="https://w3id.org/leo/onto/ale/provenanceType"/>
                <owl:allValuesFrom rdf:resource="http://www.w3.org/2000/01/rdf-schema#Literal"/>
            </owl:Restriction>
        </rdfs:subClassOf>
        <rdfs:subClassOf>
            <owl:Restriction>
                <owl:onProperty rdf:resource="https://w3id.org/leo/onto/ale/entryInFarmDate"/>
                <owl:qualifiedCardinality rdf:datatype="http://www.w3.org/2001/XMLSchema#nonNegativeInteger">1</owl:qualifiedCardinality>
                <owl:onDataRange>
                    <rdfs:Datatype>
                        <owl:unionOf rdf:parseType="Collection">
                            <rdf:Description rdf:about="http://www.w3.org/2001/XMLSchema#date"/>
                            <rdf:Description rdf:about="http://www.w3.org/2001/XMLSchema#dateTime"/>
                        </owl:unionOf>
                    </rdfs:Datatype>
                </owl:onDataRange>
            </owl:Restriction>
        </rdfs:subClassOf>
        <dc:description rdf:resource="https://raw.githubusercontent.com/Bluarancio/Leo-OpenData/master/RappresentazioneGraficaOntologie/PNG/Ale_InboundMovement.png"/>
        <rdfs:comment xml:lang="it">L&apos;evento della vita dell&apos;animale che rappresenta l&apos;entrata/ingresso dell&apos;animale in azienda (ad esempio, acquisto di un soggetto non nato in azienda).

Possibili Applicazioni: Manageriale. Corretta identificazione degli spostamenti (vendita/acquisto) del soggetto), stima dell&apos;effetto ambientale.</rdfs:comment>
        <rdfs:comment xml:lang="en">The event in the life of the animal that represents the entry of the animal into the farm company (e.g. purchase of an animal not born in the company).

Possible applications: Managerial. Correct identification of movements (sale/purchase) of the subject), estimation of environmental effect</rdfs:comment>
        <rdfs:isDefinedBy rdf:resource="https://w3id.org/leo/onto/ale"/>
        <rdfs:label xml:lang="en">Inbound Movement</rdfs:label>
        <rdfs:label xml:lang="it">Spostamento in Entrata</rdfs:label>
        <owl:versionInfo xml:lang="it">stabile -cambiato URI nella versione 0.4 dell&apos;ontologia</owl:versionInfo>
        <owl:versionInfo xml:lang="en">stable - renamed the URI with InboundMovement in version 0.4 of the ontology</owl:versionInfo>
    </owl:Class>
    


    <!-- https://w3id.org/leo/onto/ale/MilkConductivityMeasurement -->

    <owl:Class rdf:about="https://w3id.org/leo/onto/ale/MilkConductivityMeasurement">
        <rdfs:subClassOf rdf:resource="https://w3id.org/italia/onto/TI/TimeIndexedEvent"/>
        <rdfs:subClassOf>
            <owl:Restriction>
                <owl:onProperty rdf:resource="https://w3id.org/leo/onto/ale/withinMilkingSession"/>
                <owl:allValuesFrom rdf:resource="https://w3id.org/leo/onto/ale/MilkingSession"/>
            </owl:Restriction>
        </rdfs:subClassOf>
        <rdfs:subClassOf>
            <owl:Restriction>
                <owl:onProperty rdf:resource="https://w3id.org/leo/onto/ale/carriedOutBy"/>
                <owl:qualifiedCardinality rdf:datatype="http://www.w3.org/2001/XMLSchema#nonNegativeInteger">1</owl:qualifiedCardinality>
                <owl:onClass rdf:resource="https://w3id.org/leo/onto/co/LivestockFarm"/>
            </owl:Restriction>
        </rdfs:subClassOf>
        <rdfs:subClassOf>
            <owl:Restriction>
                <owl:onProperty rdf:resource="https://w3id.org/leo/onto/ale/measuredForFarmAnimal"/>
                <owl:qualifiedCardinality rdf:datatype="http://www.w3.org/2001/XMLSchema#nonNegativeInteger">1</owl:qualifiedCardinality>
                <owl:onClass rdf:resource="https://w3id.org/leo/onto/animal/FarmAnimal"/>
            </owl:Restriction>
        </rdfs:subClassOf>
        <rdfs:subClassOf>
            <owl:Restriction>
                <owl:onProperty rdf:resource="https://w3id.org/leo/onto/ale/hasAvgMilkConductivity"/>
                <owl:maxQualifiedCardinality rdf:datatype="http://www.w3.org/2001/XMLSchema#nonNegativeInteger">1</owl:maxQualifiedCardinality>
                <owl:onClass rdf:resource="https://w3id.org/italia/onto/MU/Value"/>
            </owl:Restriction>
        </rdfs:subClassOf>
        <rdfs:comment xml:lang="it">La classe rappresenta la misurazione della conduttività media del latte. Questa viene rilevata in una data all&apos;interno di una sessione di mungitura. È registrata per un animale da allevamento e i dati sono prodotti da un&apos;azienda agricola.</rdfs:comment>
        <rdfs:comment xml:lang="en">The class represents the measurement of the average milk conductivity. This is detected in a date within a milking session. It is registered for a farm animal and the data are produced by a farm company.</rdfs:comment>
        <rdfs:isDefinedBy rdf:resource="https://w3id.org/leo/onto/ale"/>
        <rdfs:label xml:lang="en">Milk Conductivity Measurement</rdfs:label>
        <rdfs:label xml:lang="it">Misurazione Conducibilità (Media) del Latte</rdfs:label>
        <owl:versionInfo xml:lang="it">stabile</owl:versionInfo>
        <owl:versionInfo xml:lang="en">stable</owl:versionInfo>
    </owl:Class>
    


    <!-- https://w3id.org/leo/onto/ale/MilkingSession -->

    <owl:Class rdf:about="https://w3id.org/leo/onto/ale/MilkingSession">
        <rdfs:subClassOf rdf:resource="https://w3id.org/leo/onto/ale/AnimalLifeEvent"/>
        <rdfs:subClassOf>
            <owl:Restriction>
                <owl:onProperty rdf:resource="https://w3id.org/italia/onto/TI/hasDuration"/>
                <owl:maxQualifiedCardinality rdf:datatype="http://www.w3.org/2001/XMLSchema#nonNegativeInteger">1</owl:maxQualifiedCardinality>
                <owl:onClass rdf:resource="https://w3id.org/italia/onto/TI/Duration"/>
            </owl:Restriction>
        </rdfs:subClassOf>
        <rdfs:subClassOf>
            <owl:Restriction>
                <owl:onProperty rdf:resource="https://w3id.org/leo/onto/ale/hasMilkYield"/>
                <owl:maxQualifiedCardinality rdf:datatype="http://www.w3.org/2001/XMLSchema#nonNegativeInteger">1</owl:maxQualifiedCardinality>
                <owl:onClass rdf:resource="https://w3id.org/italia/onto/MU/Value"/>
            </owl:Restriction>
        </rdfs:subClassOf>
        <rdfs:subClassOf>
            <owl:Restriction>
                <owl:onProperty rdf:resource="https://w3id.org/leo/onto/ale/milkingSessionDate"/>
                <owl:qualifiedCardinality rdf:datatype="http://www.w3.org/2001/XMLSchema#nonNegativeInteger">1</owl:qualifiedCardinality>
                <owl:onDataRange>
                    <rdfs:Datatype>
                        <owl:unionOf rdf:parseType="Collection">
                            <rdf:Description rdf:about="http://www.w3.org/2001/XMLSchema#date"/>
                            <rdf:Description rdf:about="http://www.w3.org/2001/XMLSchema#dateTime"/>
                        </owl:unionOf>
                    </rdfs:Datatype>
                </owl:onDataRange>
            </owl:Restriction>
        </rdfs:subClassOf>
        <dc:description rdf:resource="https://raw.githubusercontent.com/Bluarancio/Leo-OpenData/master/RappresentazioneGraficaOntologie/PNG/Milking.png"/>
        <rdfs:comment xml:lang="it">L&apos;evento per il quale un animale è sottoposto a una sessione di mungitura.</rdfs:comment>
        <rdfs:comment xml:lang="en">The event for which an animal is subject to a milking session.</rdfs:comment>
        <rdfs:isDefinedBy rdf:resource="https://w3id.org/leo/onto/ale"/>
        <rdfs:label xml:lang="en">Milking Session</rdfs:label>
        <rdfs:label xml:lang="it">Sessione di Mungitura</rdfs:label>
        <owl:versionInfo xml:lang="it">stabile</owl:versionInfo>
        <owl:versionInfo xml:lang="en">stable</owl:versionInfo>
    </owl:Class>
    


    <!-- https://w3id.org/leo/onto/ale/OutboundMovement -->

    <owl:Class rdf:about="https://w3id.org/leo/onto/ale/OutboundMovement">
        <rdfs:subClassOf rdf:resource="https://w3id.org/leo/onto/ale/AnimalLifeEvent"/>
        <rdfs:subClassOf>
            <owl:Restriction>
                <owl:onProperty rdf:resource="https://w3id.org/leo/onto/ale/hasExitFromFarmReason"/>
                <owl:allValuesFrom rdf:resource="https://w3id.org/leo/onto/ale/ExitFromFarmReason"/>
            </owl:Restriction>
        </rdfs:subClassOf>
        <rdfs:subClassOf>
            <owl:Restriction>
                <owl:onProperty rdf:resource="https://w3id.org/leo/onto/ale/hasAnimalOwnerCompany"/>
                <owl:maxQualifiedCardinality rdf:datatype="http://www.w3.org/2001/XMLSchema#nonNegativeInteger">1</owl:maxQualifiedCardinality>
                <owl:onClass rdf:resource="https://w3id.org/leo/onto/co/LivestockFarm"/>
            </owl:Restriction>
        </rdfs:subClassOf>
        <rdfs:subClassOf>
            <owl:Restriction>
                <owl:onProperty rdf:resource="https://w3id.org/leo/onto/ale/destinationType"/>
                <owl:allValuesFrom rdf:resource="http://www.w3.org/2000/01/rdf-schema#Literal"/>
            </owl:Restriction>
        </rdfs:subClassOf>
        <rdfs:subClassOf>
            <owl:Restriction>
                <owl:onProperty rdf:resource="https://w3id.org/leo/onto/ale/exitFromFarmDate"/>
                <owl:qualifiedCardinality rdf:datatype="http://www.w3.org/2001/XMLSchema#nonNegativeInteger">1</owl:qualifiedCardinality>
                <owl:onDataRange rdf:resource="http://www.w3.org/2001/XMLSchema#date"/>
            </owl:Restriction>
        </rdfs:subClassOf>
        <dc:description rdf:resource="https://raw.githubusercontent.com/Bluarancio/Leo-OpenData/master/RappresentazioneGraficaOntologie/PNG/Ale_OutboundMovement.png"/>
        <rdfs:comment xml:lang="it">L&apos;evento di uscita dall&apos;animale dall&apos;allevamento (ad esempio, vendita del soggetto ad altro allevamento, ecc.).

Possibili Applicazioni: Manageriale. Corretta identificazione degli spostamenti (vendita/acquisto) del soggetto), stima dell&apos;effetto ambientale.</rdfs:comment>
        <rdfs:comment xml:lang="en">The event of the animal leaving the farm company (e.g. sale of the animal to another farm, etc.).

Possible Applications: Managerial. Correct identification of movements (sale/purchase) of the subject), estimation of the environmental effect.</rdfs:comment>
        <rdfs:isDefinedBy rdf:resource="https://w3id.org/leo/onto/ale"/>
        <rdfs:label xml:lang="en">Outbound Movement</rdfs:label>
        <rdfs:label xml:lang="it">Spostamento in Uscita</rdfs:label>
        <owl:versionInfo xml:lang="it">stabile - cambiato l&apos;URI nella versione 0.4 dell&apos;ontologia</owl:versionInfo>
        <owl:versionInfo xml:lang="en">stable - renamed the URI with &apos;OutboundMovement&apos; in version 0.4 of the ontology</owl:versionInfo>
    </owl:Class>
    


    <!-- https://w3id.org/leo/onto/ale/Parturition -->

    <owl:Class rdf:about="https://w3id.org/leo/onto/ale/Parturition">
        <rdfs:subClassOf rdf:resource="https://w3id.org/leo/onto/ale/AnimalLifeEvent"/>
        <rdfs:subClassOf>
            <owl:Restriction>
                <owl:onProperty rdf:resource="https://w3id.org/leo/onto/ale/hasEaseOfParturition"/>
                <owl:maxQualifiedCardinality rdf:datatype="http://www.w3.org/2001/XMLSchema#nonNegativeInteger">1</owl:maxQualifiedCardinality>
                <owl:onClass rdf:resource="https://w3id.org/leo/onto/ale/EaseOfParturition"/>
            </owl:Restriction>
        </rdfs:subClassOf>
        <rdfs:subClassOf>
            <owl:Restriction>
                <owl:onProperty rdf:resource="https://w3id.org/leo/onto/ale/parturitionDate"/>
                <owl:qualifiedCardinality rdf:datatype="http://www.w3.org/2001/XMLSchema#nonNegativeInteger">1</owl:qualifiedCardinality>
                <owl:onDataRange>
                    <rdfs:Datatype>
                        <owl:unionOf rdf:parseType="Collection">
                            <rdf:Description rdf:about="http://www.w3.org/2001/XMLSchema#date"/>
                            <rdf:Description rdf:about="http://www.w3.org/2001/XMLSchema#dateTime"/>
                        </owl:unionOf>
                    </rdfs:Datatype>
                </owl:onDataRange>
            </owl:Restriction>
        </rdfs:subClassOf>
        <rdfs:subClassOf>
            <owl:Restriction>
                <owl:onProperty rdf:resource="https://w3id.org/leo/onto/ale/numberOfBorn"/>
                <owl:maxQualifiedCardinality rdf:datatype="http://www.w3.org/2001/XMLSchema#nonNegativeInteger">1</owl:maxQualifiedCardinality>
                <owl:onDataRange rdf:resource="http://www.w3.org/2001/XMLSchema#integer"/>
            </owl:Restriction>
        </rdfs:subClassOf>
        <rdfs:subClassOf>
            <owl:Restriction>
                <owl:onProperty rdf:resource="https://w3id.org/leo/onto/ale/numberOfBornAliveFemales"/>
                <owl:maxQualifiedCardinality rdf:datatype="http://www.w3.org/2001/XMLSchema#nonNegativeInteger">1</owl:maxQualifiedCardinality>
                <owl:onDataRange rdf:resource="http://www.w3.org/2001/XMLSchema#integer"/>
            </owl:Restriction>
        </rdfs:subClassOf>
        <rdfs:subClassOf>
            <owl:Restriction>
                <owl:onProperty rdf:resource="https://w3id.org/leo/onto/ale/numberOfBornAliveMales"/>
                <owl:maxQualifiedCardinality rdf:datatype="http://www.w3.org/2001/XMLSchema#nonNegativeInteger">1</owl:maxQualifiedCardinality>
                <owl:onDataRange rdf:resource="http://www.w3.org/2001/XMLSchema#integer"/>
            </owl:Restriction>
        </rdfs:subClassOf>
        <rdfs:subClassOf>
            <owl:Restriction>
                <owl:onProperty rdf:resource="https://w3id.org/leo/onto/ale/numberOfBornDeadFemales"/>
                <owl:maxQualifiedCardinality rdf:datatype="http://www.w3.org/2001/XMLSchema#nonNegativeInteger">1</owl:maxQualifiedCardinality>
                <owl:onDataRange rdf:resource="http://www.w3.org/2001/XMLSchema#integer"/>
            </owl:Restriction>
        </rdfs:subClassOf>
        <rdfs:subClassOf>
            <owl:Restriction>
                <owl:onProperty rdf:resource="https://w3id.org/leo/onto/ale/numberOfBornDeadMales"/>
                <owl:maxQualifiedCardinality rdf:datatype="http://www.w3.org/2001/XMLSchema#nonNegativeInteger">1</owl:maxQualifiedCardinality>
                <owl:onDataRange rdf:resource="http://www.w3.org/2001/XMLSchema#integer"/>
            </owl:Restriction>
        </rdfs:subClassOf>
        <dc:description rdf:resource="https://raw.githubusercontent.com/Bluarancio/Leo-OpenData/master/RappresentazioneGraficaOntologie/PNG/Ale_Parturition.png"/>
        <rdfs:comment xml:lang="en">This is the event that ends gestation and consists of the expulsion of the foetus/fetuses from the animal&apos;s uterus. It can be natural or aided by people. In dairy cattle, if it occurs after the 260th day of gestation and the baby is capable of independent life, it is called early birth; if the birth occurs at the normal distance from fertilisation but the baby is dead or unviable, it is called stillbirth.

Possible applications: Reproduction. calculation of the animal&apos;s reproductive status and days to lactation. Technical assistance, calculation of welfare indicators, fertility indicators, genetic improvement.</rdfs:comment>
        <rdfs:comment xml:lang="it">È l&apos;evento che termina la gestazione e consiste nell&apos;espulsione del feto/feti dall&apos;utero dell&apos;animale. Può essere naturale o aiutato dall&apos;uomo. Nei bovini da latte, se avviene dopo il 260° giorno di gestazione ed il nato è capace di vita autonoma si parla di parto precoce; se il parto avviene alla normale distanza dalla fecondazione ma il nato è morto o disvitale, prende il termine di &apos;stillbirth”.

Possibili Applicazioni: Riproduzione. calcolo dello stato riproduttivo dell&apos;animale e dei giorni di lattazione. Assistenza tecnica, calcolo indicatore di benessere, indicatori di fertilità, miglioramento genetico.</rdfs:comment>
        <rdfs:isDefinedBy rdf:resource="https://w3id.org/leo/onto/ale"/>
        <rdfs:label xml:lang="it">Parto</rdfs:label>
        <rdfs:label xml:lang="en">Parturition</rdfs:label>
        <owl:versionInfo xml:lang="it">stabile</owl:versionInfo>
        <owl:versionInfo xml:lang="en">stable</owl:versionInfo>
    </owl:Class>
    


    <!-- https://w3id.org/leo/onto/ale/PregnancyDiagnosis -->

    <owl:Class rdf:about="https://w3id.org/leo/onto/ale/PregnancyDiagnosis">
        <rdfs:subClassOf rdf:resource="https://w3id.org/leo/onto/ale/Diagnosis"/>
        <rdfs:subClassOf>
            <owl:Restriction>
                <owl:onProperty rdf:resource="https://w3id.org/leo/onto/ale/hasPregnancyResult"/>
                <owl:maxQualifiedCardinality rdf:datatype="http://www.w3.org/2001/XMLSchema#nonNegativeInteger">1</owl:maxQualifiedCardinality>
                <owl:onClass rdf:resource="https://w3id.org/leo/onto/ale/PregnancyResult"/>
            </owl:Restriction>
        </rdfs:subClassOf>
        <rdfs:comment xml:lang="en">This is the event whereby the presence of a foetus is verified after insemination. Diagnoses are made by veterinary surgeons and rarely by other specialised personnel. They are carried out using ultrasound equipment, palpation or rapid test kits for hormone dosage.

Possible applications: Reproduction and Welfare. Calculation of the reproductive status of the animal. Technical assistance, genetic improvement.</rdfs:comment>
        <rdfs:comment xml:lang="it">È l’evento con il quale si verifica la presenza di feto dopo una inseminazione. Le diagnosi vengono effettuate dai medici veterinari e raramente da altro personale specializzato. Vengono effettuate con strumentazione ecografica, con palpazione o con kit di analisi rapidi per il dosaggio ormonale.

Possibili applicazioni: Riproduzione e Benessere. Calcolo dello stato riproduttivo dell&apos;animale. Assistenza tecnica, miglioramento genetico.</rdfs:comment>
        <rdfs:isDefinedBy rdf:resource="https://w3id.org/leo/onto/ale"/>
        <rdfs:label xml:lang="it">Diagnosi Gravidanza</rdfs:label>
        <rdfs:label xml:lang="en">Pragnacy Diagnosis</rdfs:label>
        <owl:versionInfo xml:lang="it">stabile</owl:versionInfo>
        <owl:versionInfo xml:lang="en">stable</owl:versionInfo>
    </owl:Class>
    


    <!-- https://w3id.org/leo/onto/ale/PregnancyResult -->

    <owl:Class rdf:about="https://w3id.org/leo/onto/ale/PregnancyResult">
        <owl:equivalentClass>
            <owl:Class>
                <owl:oneOf rdf:parseType="Collection">
                    <rdf:Description rdf:about="https://w3id.org/leo/onto/ale/Negative"/>
                    <rdf:Description rdf:about="https://w3id.org/leo/onto/ale/Positive"/>
                    <rdf:Description rdf:about="https://w3id.org/leo/onto/ale/Revisable"/>
                </owl:oneOf>
            </owl:Class>
        </owl:equivalentClass>
        <rdfs:subClassOf rdf:resource="https://w3id.org/italia/onto/l0/Characteristic"/>
        <rdfs:comment xml:lang="it">Esito della diagnosi di gravidanza. Indica se la diagnosi è Positiva, Negativa o Rivedibile.</rdfs:comment>
        <rdfs:comment xml:lang="en">Result of pregnancy diagnosis. Indicates whether the diagnosis is Positive, Negative or Revisable.</rdfs:comment>
        <rdfs:label xml:lang="it">Esito Diagnosi Gravidanza</rdfs:label>
        <rdfs:label xml:lang="en">Pregnancy Result</rdfs:label>
        <owl:priorVersion rdf:resource="https://w3id.org/leo/onto/ale"/>
        <owl:versionInfo xml:lang="it">stabile</owl:versionInfo>
        <owl:versionInfo xml:lang="en">stable</owl:versionInfo>
    </owl:Class>
    


    <!-- https://w3id.org/leo/onto/ale/Slaughter -->

    <owl:Class rdf:about="https://w3id.org/leo/onto/ale/Slaughter">
        <rdfs:subClassOf rdf:resource="https://w3id.org/leo/onto/ale/AnimalLifeEvent"/>
        <rdfs:subClassOf>
            <owl:Restriction>
                <owl:onProperty rdf:resource="https://w3id.org/leo/onto/ale/hasAnimalLiveWeight"/>
                <owl:maxQualifiedCardinality rdf:datatype="http://www.w3.org/2001/XMLSchema#nonNegativeInteger">1</owl:maxQualifiedCardinality>
                <owl:onClass rdf:resource="https://w3id.org/italia/onto/MU/Value"/>
            </owl:Restriction>
        </rdfs:subClassOf>
        <rdfs:subClassOf>
            <owl:Restriction>
                <owl:onProperty rdf:resource="https://w3id.org/leo/onto/ale/hasAnimalProvenanceCompany"/>
                <owl:maxQualifiedCardinality rdf:datatype="http://www.w3.org/2001/XMLSchema#nonNegativeInteger">1</owl:maxQualifiedCardinality>
                <owl:onClass rdf:resource="https://w3id.org/leo/onto/co/LivestockFarm"/>
            </owl:Restriction>
        </rdfs:subClassOf>
        <rdfs:subClassOf>
            <owl:Restriction>
                <owl:onProperty rdf:resource="https://w3id.org/leo/onto/ale/hasAnimalProvenanceCountry"/>
                <owl:maxQualifiedCardinality rdf:datatype="http://www.w3.org/2001/XMLSchema#nonNegativeInteger">1</owl:maxQualifiedCardinality>
                <owl:onClass rdf:resource="http://www.w3.org/2004/02/skos/core#Concept"/>
            </owl:Restriction>
        </rdfs:subClassOf>
        <rdfs:subClassOf>
            <owl:Restriction>
                <owl:onProperty rdf:resource="https://w3id.org/leo/onto/ale/hasCarcassCategory"/>
                <owl:maxQualifiedCardinality rdf:datatype="http://www.w3.org/2001/XMLSchema#nonNegativeInteger">1</owl:maxQualifiedCardinality>
                <owl:onClass rdf:resource="https://w3id.org/leo/onto/ale/CarcassCategory"/>
            </owl:Restriction>
        </rdfs:subClassOf>
        <rdfs:subClassOf>
            <owl:Restriction>
                <owl:onProperty rdf:resource="https://w3id.org/leo/onto/ale/hasCarcassClassification"/>
                <owl:maxQualifiedCardinality rdf:datatype="http://www.w3.org/2001/XMLSchema#nonNegativeInteger">1</owl:maxQualifiedCardinality>
                <owl:onClass rdf:resource="https://w3id.org/leo/onto/ale/CarcassClassification"/>
            </owl:Restriction>
        </rdfs:subClassOf>
        <rdfs:subClassOf>
            <owl:Restriction>
                <owl:onProperty rdf:resource="https://w3id.org/leo/onto/ale/hasCarcassWeight"/>
                <owl:maxQualifiedCardinality rdf:datatype="http://www.w3.org/2001/XMLSchema#nonNegativeInteger">1</owl:maxQualifiedCardinality>
                <owl:onClass rdf:resource="https://w3id.org/italia/onto/MU/Value"/>
            </owl:Restriction>
        </rdfs:subClassOf>
        <rdfs:subClassOf>
            <owl:Restriction>
                <owl:onProperty rdf:resource="https://w3id.org/leo/onto/ale/slaughterDate"/>
                <owl:qualifiedCardinality rdf:datatype="http://www.w3.org/2001/XMLSchema#nonNegativeInteger">1</owl:qualifiedCardinality>
                <owl:onDataRange>
                    <rdfs:Datatype>
                        <owl:unionOf rdf:parseType="Collection">
                            <rdf:Description rdf:about="http://www.w3.org/2001/XMLSchema#date"/>
                            <rdf:Description rdf:about="http://www.w3.org/2001/XMLSchema#dateTime"/>
                        </owl:unionOf>
                    </rdfs:Datatype>
                </owl:onDataRange>
            </owl:Restriction>
        </rdfs:subClassOf>
        <rdfs:subClassOf>
            <owl:Restriction>
                <owl:onProperty rdf:resource="https://w3id.org/leo/onto/ale/animalArrivedDeadAtSlaughterhouse"/>
                <owl:maxQualifiedCardinality rdf:datatype="http://www.w3.org/2001/XMLSchema#nonNegativeInteger">1</owl:maxQualifiedCardinality>
                <owl:onDataRange rdf:resource="http://www.w3.org/2001/XMLSchema#boolean"/>
            </owl:Restriction>
        </rdfs:subClassOf>
        <rdfs:subClassOf>
            <owl:Restriction>
                <owl:onProperty rdf:resource="https://w3id.org/leo/onto/ale/deadReason"/>
                <owl:maxCardinality rdf:datatype="http://www.w3.org/2001/XMLSchema#nonNegativeInteger">1</owl:maxCardinality>
            </owl:Restriction>
        </rdfs:subClassOf>
        <rdfs:subClassOf>
            <owl:Restriction>
                <owl:onProperty rdf:resource="https://w3id.org/leo/onto/ale/isCarcassForConsumption"/>
                <owl:maxQualifiedCardinality rdf:datatype="http://www.w3.org/2001/XMLSchema#nonNegativeInteger">1</owl:maxQualifiedCardinality>
                <owl:onDataRange rdf:resource="http://www.w3.org/2001/XMLSchema#boolean"/>
            </owl:Restriction>
        </rdfs:subClassOf>
        <dc:description rdf:resource="https://raw.githubusercontent.com/Bluarancio/Leo-OpenData/master/RappresentazioneGraficaOntologie/PNG/Slaughter.png"/>
        <rdfs:comment xml:lang="en">It is the event in the life of the animal that relates to its killing, using appropriate methods, for commercial purposes on a slaughterhouse-type farm. This event follows the exit of the animal from the farm company and produces a carcass that can be used for human consumption.

Possible Applications: Managerial. Information recorded at slaughter (e.g.: meat classification, destination for consumption, country of origin, date of slaughter, etc.) useful information for genetic improvement (meat production), management (correct feeding).</rdfs:comment>
        <rdfs:comment xml:lang="it">È l&apos;evento della vita dell&apos;animale che riguarda la sua uccisione, con opportuni metodi, per scopi commerciali presso un&apos;azienda di tipo macello. Tale evento segue l&apos;uscita dell&apos;animale dall&apos;allevamento e produce una carcassa che può essere destinata al consumo umano.

Possibili Applicazioni: Manageriale. Informazioni registrate in macellazione (es.: classificazione carni, destinazione al consumo, paese di provenienza, data di macellazione, ecc.) informazioni utili per il miglioramento genetico (produzione carne), gestionale (corretta alimentazione).</rdfs:comment>
        <rdfs:isDefinedBy rdf:resource="https://w3id.org/leo/onto/ale"/>
        <rdfs:label xml:lang="it">Macellazione</rdfs:label>
        <rdfs:label xml:lang="en">Slaughter</rdfs:label>
        <owl:versionInfo xml:lang="it">stabile - Introdotto nella versione 0.3 dell&apos;ontologia</owl:versionInfo>
        <owl:versionInfo xml:lang="en">stable - introduced in version 0.3 of the ontology</owl:versionInfo>
    </owl:Class>
    


    <!-- https://w3id.org/leo/onto/ale/Weaning -->

    <owl:Class rdf:about="https://w3id.org/leo/onto/ale/Weaning">
        <rdfs:subClassOf rdf:resource="https://w3id.org/leo/onto/ale/AnimalLifeEvent"/>
        <rdfs:subClassOf>
            <owl:Restriction>
                <owl:onProperty rdf:resource="https://w3id.org/leo/onto/ale/hasWeight"/>
                <owl:allValuesFrom rdf:resource="https://w3id.org/italia/onto/MU/Value"/>
            </owl:Restriction>
        </rdfs:subClassOf>
        <rdfs:subClassOf>
            <owl:Restriction>
                <owl:onProperty rdf:resource="https://w3id.org/leo/onto/ale/hasArtificialBreastFeedingDuration"/>
                <owl:maxQualifiedCardinality rdf:datatype="http://www.w3.org/2001/XMLSchema#nonNegativeInteger">1</owl:maxQualifiedCardinality>
                <owl:onClass rdf:resource="https://w3id.org/italia/onto/TI/Duration"/>
            </owl:Restriction>
        </rdfs:subClassOf>
        <rdfs:subClassOf>
            <owl:Restriction>
                <owl:onProperty rdf:resource="https://w3id.org/leo/onto/ale/hasBreastFeedingType"/>
                <owl:maxQualifiedCardinality rdf:datatype="http://www.w3.org/2001/XMLSchema#nonNegativeInteger">1</owl:maxQualifiedCardinality>
                <owl:onClass rdf:resource="https://w3id.org/leo/onto/ale/BreastFeedingType"/>
            </owl:Restriction>
        </rdfs:subClassOf>
        <rdfs:subClassOf>
            <owl:Restriction>
                <owl:onProperty rdf:resource="https://w3id.org/leo/onto/ale/hasBreastFeedingWithNurseDuration"/>
                <owl:maxQualifiedCardinality rdf:datatype="http://www.w3.org/2001/XMLSchema#nonNegativeInteger">1</owl:maxQualifiedCardinality>
                <owl:onClass rdf:resource="https://w3id.org/italia/onto/TI/Duration"/>
            </owl:Restriction>
        </rdfs:subClassOf>
        <rdfs:subClassOf>
            <owl:Restriction>
                <owl:onProperty rdf:resource="https://w3id.org/leo/onto/ale/weaningDate"/>
                <owl:qualifiedCardinality rdf:datatype="http://www.w3.org/2001/XMLSchema#nonNegativeInteger">1</owl:qualifiedCardinality>
                <owl:onDataRange>
                    <rdfs:Datatype>
                        <owl:unionOf rdf:parseType="Collection">
                            <rdf:Description rdf:about="http://www.w3.org/2001/XMLSchema#date"/>
                            <rdf:Description rdf:about="http://www.w3.org/2001/XMLSchema#dateTime"/>
                        </owl:unionOf>
                    </rdfs:Datatype>
                </owl:onDataRange>
            </owl:Restriction>
        </rdfs:subClassOf>
        <dc:description rdf:resource="https://raw.githubusercontent.com/Bluarancio/Leo-OpenData/master/RappresentazioneGraficaOntologie/PNG/Weaning.png"/>
        <rdfs:comment xml:lang="it">La classe rappresenta l&apos;evento per cui un animale giovane termina l’allattamento della madre o della balia o artificiale e inizia ad assumere una diversa alimentazione.
L’età allo svezzamento e il programma di alimentazione influenzano le performance durante l&apos;accrescimento.</rdfs:comment>
        <rdfs:comment xml:lang="en">The class represents the event whereby a young animal terminates suckling from its mother or wet nurse and begins to take on a different diet.
Age at weaning and feeding schedule influence performance during growth.</rdfs:comment>
        <rdfs:isDefinedBy rdf:resource="https://w3id.org/leo/onto/ale"/>
        <rdfs:label xml:lang="it">Svezzamento</rdfs:label>
        <rdfs:label xml:lang="en">Weaning</rdfs:label>
        <owl:versionInfo xml:lang="it">stabile</owl:versionInfo>
        <owl:versionInfo xml:lang="en">stable</owl:versionInfo>
    </owl:Class>
    


    <!-- https://w3id.org/leo/onto/ale/Weighing -->

    <owl:Class rdf:about="https://w3id.org/leo/onto/ale/Weighing">
        <rdfs:subClassOf rdf:resource="https://w3id.org/leo/onto/ale/AnimalLifeEvent"/>
        <rdfs:subClassOf>
            <owl:Restriction>
                <owl:onProperty rdf:resource="https://w3id.org/leo/onto/ale/hasWeight"/>
                <owl:someValuesFrom rdf:resource="https://w3id.org/italia/onto/MU/Value"/>
            </owl:Restriction>
        </rdfs:subClassOf>
        <rdfs:subClassOf>
            <owl:Restriction>
                <owl:onProperty rdf:resource="https://w3id.org/leo/onto/ale/hasWeight"/>
                <owl:allValuesFrom rdf:resource="https://w3id.org/italia/onto/MU/Value"/>
            </owl:Restriction>
        </rdfs:subClassOf>
        <rdfs:subClassOf>
            <owl:Restriction>
                <owl:onProperty rdf:resource="https://w3id.org/leo/onto/ale/weighingDate"/>
                <owl:qualifiedCardinality rdf:datatype="http://www.w3.org/2001/XMLSchema#nonNegativeInteger">1</owl:qualifiedCardinality>
                <owl:onDataRange>
                    <rdfs:Datatype>
                        <owl:unionOf rdf:parseType="Collection">
                            <rdf:Description rdf:about="http://www.w3.org/2001/XMLSchema#date"/>
                            <rdf:Description rdf:about="http://www.w3.org/2001/XMLSchema#dateTime"/>
                        </owl:unionOf>
                    </rdfs:Datatype>
                </owl:onDataRange>
            </owl:Restriction>
        </rdfs:subClassOf>
        <dc:description rdf:resource="https://raw.githubusercontent.com/Bluarancio/Leo-OpenData/master/RappresentazioneGraficaOntologie/PNG/Weighing.png"/>
        <rdfs:comment xml:lang="it">L&apos;evento della vita dell&apos;animale relativo alla misurazione del suo peso.</rdfs:comment>
        <rdfs:comment xml:lang="en">The event in the animal&apos;s life relating to the measurement of its weight.</rdfs:comment>
        <rdfs:isDefinedBy rdf:resource="https://w3id.org/leo/onto/ale"/>
        <rdfs:label xml:lang="it">Pesata</rdfs:label>
        <rdfs:label xml:lang="en">Weighing</rdfs:label>
        <owl:versionInfo xml:lang="it">stabile</owl:versionInfo>
        <owl:versionInfo xml:lang="en">stable</owl:versionInfo>
    </owl:Class>
    


    <!-- https://w3id.org/leo/onto/animal/Breed -->

    <owl:Class rdf:about="https://w3id.org/leo/onto/animal/Breed"/>
    


    <!-- https://w3id.org/leo/onto/animal/FarmAnimal -->

    <owl:Class rdf:about="https://w3id.org/leo/onto/animal/FarmAnimal"/>
    


    <!-- https://w3id.org/leo/onto/animal/FarmAnimalDestination -->

    <owl:Class rdf:about="https://w3id.org/leo/onto/animal/FarmAnimalDestination"/>
    


    <!-- https://w3id.org/leo/onto/animal/LivestockSpecies -->

    <owl:Class rdf:about="https://w3id.org/leo/onto/animal/LivestockSpecies"/>
    


    <!-- https://w3id.org/leo/onto/animal/ProductionType -->

    <owl:Class rdf:about="https://w3id.org/leo/onto/animal/ProductionType"/>
    


    <!-- https://w3id.org/leo/onto/co/LivestockCompany -->

    <owl:Class rdf:about="https://w3id.org/leo/onto/co/LivestockCompany"/>
    


    <!-- https://w3id.org/leo/onto/co/LivestockFarm -->

    <owl:Class rdf:about="https://w3id.org/leo/onto/co/LivestockFarm"/>
    


    <!-- https://w3id.org/leo/onto/co/Site -->

    <owl:Class rdf:about="https://w3id.org/leo/onto/co/Site"/>
    


    <!-- https://w3id.org/leo/onto/co/Slaughterhouse -->

    <owl:Class rdf:about="https://w3id.org/leo/onto/co/Slaughterhouse"/>
    


    <!-- 
    ///////////////////////////////////////////////////////////////////////////////////////
    //
    // Individuals
    //
    ///////////////////////////////////////////////////////////////////////////////////////
     -->

    


    <!-- https://w3id.org/leo/data/contact-point/onto-aia -->

    <owl:NamedIndividual rdf:about="https://w3id.org/leo/data/contact-point/onto-aia">
        <rdf:type rdf:resource="http://dati.gov.it/onto/dcatapit#Organization"/>
        <rdf:type rdf:resource="http://www.w3.org/2006/vcard/ns#Kind"/>
        <rdf:type rdf:resource="http://www.w3.org/2006/vcard/ns#Organization"/>
        <rdfs:label xml:lang="en">Infomation systems</rdfs:label>
        <rdfs:label xml:lang="it">Sistemi informativi</rdfs:label>
        <ns:fn>Sistemi informativi</ns:fn>
        <ns:hasEmail rdf:resource="mailto:affarigenerali@pec.aia.it"/>
    </owl:NamedIndividual>
    


    <!-- https://w3id.org/leo/data/distribution/ALE-JSON-LD -->

    <owl:NamedIndividual rdf:about="https://w3id.org/leo/data/distribution/ALE-JSON-LD">
        <rdf:type rdf:resource="https://w3id.org/italia/onto/ADMS/SemanticAssetDistribution"/>
        <terms:description xml:lang="it">Questa è la distribuzione JSON-LD dell&apos;ontologia sugli eventi della vita degli animali da allevamento</terms:description>
        <terms:description xml:lang="en">This is the distribution in JSON-LD of Animal Life Events ontology</terms:description>
        <terms:format rdf:resource="http://publications.europa.eu/resource/authority/file-type/JSON_LD"/>
        <terms:license rdf:resource="https://w3id.org/italia/controlled-vocabulary/licences/A21_CCBY40"/>
        <terms:title xml:lang="it">Distribuzione JSON-LD ontologia ALE</terms:title>
        <terms:title xml:lang="en">JSON-LD distribution of ALE Ontology</terms:title>
        <rdfs:comment xml:lang="it">Questa è la distribuzione JSON-LD dell&apos;ontologia sugli eventi della vita degli animali da allevamento</rdfs:comment>
        <rdfs:comment xml:lang="en">This is the distribution in JSON-LD of Animal Life Events ontology</rdfs:comment>
        <rdfs:label xml:lang="it">Distribuzione JSON-LD ontologia ALE</rdfs:label>
        <rdfs:label xml:lang="en">JSON-LD distribution of ALE Ontology</rdfs:label>
        <dcat:accessURL rdf:resource="https://www.leo-project.it/Ontologie/ale/latest"/>
        <dcat:downloadURL rdf:resource="https://www.leo-project.it/Ontologie/ale/latest/ale.jsonld"/>
    </owl:NamedIndividual>
    


    <!-- https://w3id.org/leo/data/distribution/ALE-RDF-TURTLE -->

    <owl:NamedIndividual rdf:about="https://w3id.org/leo/data/distribution/ALE-RDF-TURTLE">
        <rdf:type rdf:resource="https://w3id.org/italia/onto/ADMS/SemanticAssetDistribution"/>
        <terms:description xml:lang="it">Questa è la distribuzione RDF/Turtle dell&apos;ontologia sugli eventi della vita degli animali da allevamento</terms:description>
        <terms:description xml:lang="en">This is the distribution in RDF/Turtle of Animal Life Events ontology</terms:description>
        <terms:format rdf:resource="http://publications.europa.eu/resource/authority/file-type/RDF_TURTLE"/>
        <terms:license rdf:resource="https://w3id.org/italia/controlled-vocabulary/licences/A21_CCBY40"/>
        <terms:title xml:lang="it">Distribuzione RDF/Turtle ontologia ALE</terms:title>
        <terms:title xml:lang="en">RDF/Turtle distribution of ALE Ontology</terms:title>
        <rdfs:comment xml:lang="it">Questa è la distribuzione RDF/Turtle dell&apos;ontologia sugli eventi della vita degli animali da allevamento</rdfs:comment>
        <rdfs:comment xml:lang="en">This is the distribution in RDF/Turtle of Animal Life Events ontology</rdfs:comment>
        <rdfs:label xml:lang="it">Distribuzione RDF/Turtle ontologia ALE</rdfs:label>
        <rdfs:label xml:lang="en">RDF/Turtle distribution of ALE Ontology</rdfs:label>
        <dcat:accessURL rdf:resource="https://www.leo-project.it/Ontologie/ale/latest"/>
        <dcat:downloadURL rdf:resource="https://www.leo-project.it/Ontologie/ale/latest/ale.ttl"/>
    </owl:NamedIndividual>
    


    <!-- https://w3id.org/leo/data/distribution/ALE-RDF-XML -->

    <owl:NamedIndividual rdf:about="https://w3id.org/leo/data/distribution/ALE-RDF-XML">
        <rdf:type rdf:resource="https://w3id.org/italia/onto/ADMS/SemanticAssetDistribution"/>
        <terms:description xml:lang="it">Questa è la distribuzione RDF/XML dell&apos;ontologia sugli eventi della vita degli animali da allevamento</terms:description>
        <terms:description xml:lang="en">This is the distribution in RDF/XML of Animal Life Events ontology</terms:description>
        <terms:format rdf:resource="http://publications.europa.eu/resource/authority/file-type/RDF_XML"/>
        <terms:license rdf:resource="https://w3id.org/italia/controlled-vocabulary/licences/A21_CCBY40"/>
        <terms:title xml:lang="it">Distribuzione RDF/XML ontologia ALE</terms:title>
        <terms:title xml:lang="en">RDF/XML distribution of ALE Ontology</terms:title>
        <rdfs:comment xml:lang="it">Questa è la distribuzione RDF/XML dell&apos;ontologia sugli eventi della vita degli animali da allevamento</rdfs:comment>
        <rdfs:comment xml:lang="en">This is the distribution in RDF/XML of Animal Life Events ontology</rdfs:comment>
        <rdfs:label xml:lang="it">Distribuzione RDF/XML ontologia ALE</rdfs:label>
        <rdfs:label xml:lang="en">RDF/XML distribution of ALE Ontology</rdfs:label>
        <dcat:accessURL rdf:resource="https://www.leo-project.it/Ontologie/ale/latest"/>
        <dcat:downloadURL rdf:resource="https://www.leo-project.it/Ontologie/ale/latest/ale.rdf"/>
    </owl:NamedIndividual>
    


    <!-- https://w3id.org/leo/data/private-organization/00944701002 -->

    <owl:NamedIndividual rdf:about="https://w3id.org/leo/data/private-organization/00944701002">
        <rdf:type rdf:resource="http://dati.gov.it/onto/dcatapit#Agent"/>
        <rdf:type rdf:resource="http://xmlns.com/foaf/0.1/Agent"/>
        <terms:identifier>00944701002</terms:identifier>
        <foaf:name xml:lang="it">Associazione Italiana Allevatori</foaf:name>
        <foaf:name xml:lang="en">Italian Breeders&apos; Association</foaf:name>
    </owl:NamedIndividual>
    


    <!-- https://w3id.org/leo/data/private-organization/06695411006 -->

    <owl:NamedIndividual rdf:about="https://w3id.org/leo/data/private-organization/06695411006">
        <rdf:type rdf:resource="http://dati.gov.it/onto/dcatapit#Agent"/>
        <rdf:type rdf:resource="http://xmlns.com/foaf/0.1/Agent"/>
        <terms:identifier>06695411006</terms:identifier>
        <foaf:name xml:lang="en">Bluarancio</foaf:name>
        <foaf:name xml:lang="it">Bluarancio</foaf:name>
    </owl:NamedIndividual>
    


    <!-- https://w3id.org/leo/data/project/LEO -->

    <owl:NamedIndividual rdf:about="https://w3id.org/leo/data/project/LEO">
        <rdf:type rdf:resource="https://w3id.org/italia/onto/ADMS/Project"/>
        <rdfs:comment xml:lang="it">Il progetto LEO dove viene usata l&apos;ontologia</rdfs:comment>
        <rdfs:comment xml:lang="en">LEO project where the ontology is used</rdfs:comment>
        <rdfs:label xml:lang="en">LEO - Livestok Environment Open Data</rdfs:label>
        <rdfs:label xml:lang="it">LEO - Livestok Environment Open Data</rdfs:label>
        <l0:name xml:lang="it">LEO - Livestok Environment Open Data</l0:name>
    </owl:NamedIndividual>
    


    <!-- https://w3id.org/leo/onto/ale -->

    <owl:NamedIndividual rdf:about="https://w3id.org/leo/onto/ale">
        <rdf:type rdf:resource="https://w3id.org/italia/onto/ADMS/SemanticAsset"/>
    </owl:NamedIndividual>
    


    <!-- https://w3id.org/leo/onto/ale/Artificial -->

    <owl:NamedIndividual rdf:about="https://w3id.org/leo/onto/ale/Artificial">
        <rdf:type rdf:resource="https://w3id.org/leo/onto/ale/BreastFeedingType"/>
    </owl:NamedIndividual>
    


    <!-- https://w3id.org/leo/onto/ale/Assistant -->

    <owl:NamedIndividual rdf:about="https://w3id.org/leo/onto/ale/Assistant">
        <rdf:type rdf:resource="https://w3id.org/leo/onto/ale/EaseOfParturition"/>
        <rdfs:isDefinedBy rdf:resource="https://w3id.org/leo/onto/ale"/>
        <rdfs:label xml:lang="en">An assistant, no tools</rdfs:label>
        <rdfs:label xml:lang="it">Un assistente, senza strumenti</rdfs:label>
        <owl:versionInfo xml:lang="it">provvisorio - aggiunto nella seconda versione dell&apos;ontologia</owl:versionInfo>
        <owl:versionInfo xml:lang="en">unstable - added in the second version of the ontology</owl:versionInfo>
    </owl:NamedIndividual>
    


    <!-- https://w3id.org/leo/onto/ale/CaesareanSection -->

    <owl:NamedIndividual rdf:about="https://w3id.org/leo/onto/ale/CaesareanSection">
        <rdf:type rdf:resource="https://w3id.org/leo/onto/ale/EaseOfParturition"/>
        <rdfs:isDefinedBy rdf:resource="https://w3id.org/leo/onto/ale"/>
        <rdfs:label xml:lang="en">Caesarean Section</rdfs:label>
        <rdfs:label xml:lang="it">Taglio Cesareo</rdfs:label>
        <owl:versionInfo xml:lang="it">provvisorio - aggiunto nella seconda versione dell&apos;ontologia</owl:versionInfo>
        <owl:versionInfo xml:lang="en">unstable - added in the second version of the ontology</owl:versionInfo>
    </owl:NamedIndividual>
    


    <!-- https://w3id.org/leo/onto/ale/DeathPasture -->

    <owl:NamedIndividual rdf:about="https://w3id.org/leo/onto/ale/DeathPasture">
        <rdf:type rdf:resource="https://w3id.org/leo/onto/ale/DisposalReason"/>
        <rdfs:isDefinedBy rdf:resource="https://w3id.org/leo/onto/ale"/>
        <rdfs:label xml:lang="en">Death in the pasture</rdfs:label>
        <rdfs:label xml:lang="it">Morte al Pascolo</rdfs:label>
        <owl:versionInfo xml:lang="it">provvisorio - aggiunto nella seconda versione dell&apos;ontologia</owl:versionInfo>
        <owl:versionInfo xml:lang="en">unstable - added in the second version of the ontology</owl:versionInfo>
    </owl:NamedIndividual>
    


    <!-- https://w3id.org/leo/onto/ale/DeathStable -->

    <owl:NamedIndividual rdf:about="https://w3id.org/leo/onto/ale/DeathStable">
        <rdf:type rdf:resource="https://w3id.org/leo/onto/ale/DisposalReason"/>
        <rdfs:isDefinedBy rdf:resource="https://w3id.org/leo/onto/ale"/>
        <rdfs:label xml:lang="en">Death in stable</rdfs:label>
        <rdfs:label xml:lang="it">Morte in stalla</rdfs:label>
        <owl:versionInfo xml:lang="it">provvisorio - aggiunto nella seconda versione dell&apos;ontologia</owl:versionInfo>
        <owl:versionInfo xml:lang="en">unstable - added in the second version of the ontology</owl:versionInfo>
    </owl:NamedIndividual>
    


    <!-- https://w3id.org/leo/onto/ale/Difficult -->

    <owl:NamedIndividual rdf:about="https://w3id.org/leo/onto/ale/Difficult">
        <rdf:type rdf:resource="https://w3id.org/leo/onto/ale/EaseOfParturition"/>
        <rdfs:isDefinedBy rdf:resource="https://w3id.org/leo/onto/ale"/>
        <rdfs:label xml:lang="it">Difficile, con più assistenti</rdfs:label>
        <rdfs:label xml:lang="en">Difficult, with multiple assistants</rdfs:label>
        <owl:versionInfo xml:lang="it">provvisorio - aggiunto nella seconda versione dell&apos;ontologia</owl:versionInfo>
        <owl:versionInfo xml:lang="en">unstable - added in the second version of the ontology</owl:versionInfo>
    </owl:NamedIndividual>
    


    <!-- https://w3id.org/leo/onto/ale/Easy -->

    <owl:NamedIndividual rdf:about="https://w3id.org/leo/onto/ale/Easy">
        <rdf:type rdf:resource="https://w3id.org/leo/onto/ale/EaseOfParturition"/>
        <rdfs:isDefinedBy rdf:resource="https://w3id.org/leo/onto/ale"/>
        <rdfs:label xml:lang="en">Easy</rdfs:label>
        <rdfs:label xml:lang="it">Facile</rdfs:label>
        <owl:versionInfo xml:lang="it">provvisorio - aggiunto nella seconda versione dell&apos;ontologia</owl:versionInfo>
        <owl:versionInfo xml:lang="en">unstable - added in the second version of the ontology</owl:versionInfo>
    </owl:NamedIndividual>
    


    <!-- https://w3id.org/leo/onto/ale/Embryotomy -->

    <owl:NamedIndividual rdf:about="https://w3id.org/leo/onto/ale/Embryotomy">
        <rdf:type rdf:resource="https://w3id.org/leo/onto/ale/EaseOfParturition"/>
        <rdfs:isDefinedBy rdf:resource="https://w3id.org/leo/onto/ale"/>
        <rdfs:label xml:lang="it">Embriotomia</rdfs:label>
        <rdfs:label xml:lang="en">Embryotomy</rdfs:label>
        <owl:versionInfo xml:lang="it">provvisorio - aggiunto nelal seconda versione dell&apos;ontologia</owl:versionInfo>
        <owl:versionInfo xml:lang="en">unstable - added in the second version of the ontology</owl:versionInfo>
    </owl:NamedIndividual>
    


    <!-- https://w3id.org/leo/onto/ale/FEA -->

    <owl:NamedIndividual rdf:about="https://w3id.org/leo/onto/ale/FEA">
        <rdf:type rdf:resource="https://w3id.org/leo/onto/ale/FertilizationType"/>
        <rdfs:isDefinedBy rdf:resource="https://w3id.org/leo/onto/ale"/>
        <rdfs:label xml:lang="en">Artificial Fertilization</rdfs:label>
        <rdfs:label xml:lang="it">Inseminazione Artificiale</rdfs:label>
        <owl:versionInfo xml:lang="it">stabile - cambiato codice nella versione 0.4 dell&apos;ontologia</owl:versionInfo>
        <owl:versionInfo xml:lang="en">stable - changed the code in the version 0.4 of the ontology</owl:versionInfo>
    </owl:NamedIndividual>
    


    <!-- https://w3id.org/leo/onto/ale/FEG -->

    <owl:NamedIndividual rdf:about="https://w3id.org/leo/onto/ale/FEG">
        <rdf:type rdf:resource="https://w3id.org/leo/onto/ale/FertilizationType"/>
        <rdfs:isDefinedBy rdf:resource="https://w3id.org/leo/onto/ale"/>
        <rdfs:label xml:lang="en">Group Fertilization</rdfs:label>
        <rdfs:label xml:lang="it">inseminazione in Gruppo</rdfs:label>
        <owl:versionInfo xml:lang="it">stabile - cambiato codice nella versione 0.4 dell&apos;ontologia</owl:versionInfo>
        <owl:versionInfo xml:lang="en">stable - chenaged the code in version 0.4 of the ontology</owl:versionInfo>
    </owl:NamedIndividual>
    


    <!-- https://w3id.org/leo/onto/ale/FEN -->

    <owl:NamedIndividual rdf:about="https://w3id.org/leo/onto/ale/FEN">
        <rdf:type rdf:resource="https://w3id.org/leo/onto/ale/FertilizationType"/>
        <rdfs:isDefinedBy rdf:resource="https://w3id.org/leo/onto/ale"/>
        <rdfs:label xml:lang="it">Inseminazione Naturale</rdfs:label>
        <rdfs:label xml:lang="en">Natural Fertilization</rdfs:label>
        <owl:versionInfo xml:lang="it">stabile - cambiato codice nella versione 0.4 dell&apos;ontologia</owl:versionInfo>
        <owl:versionInfo xml:lang="en">stable - changed code in version 0.4 of the ontology</owl:versionInfo>
    </owl:NamedIndividual>
    


    <!-- https://w3id.org/leo/onto/ale/Lost -->

    <owl:NamedIndividual rdf:about="https://w3id.org/leo/onto/ale/Lost">
        <rdf:type rdf:resource="https://w3id.org/leo/onto/ale/DisposalReason"/>
        <rdfs:isDefinedBy rdf:resource="https://w3id.org/leo/onto/ale"/>
        <rdfs:label xml:lang="en">Lost</rdfs:label>
        <rdfs:label xml:lang="it">Smarrito</rdfs:label>
        <owl:versionInfo xml:lang="it">Inserito nella versione 0.4 dell&apos;ontologia</owl:versionInfo>
        <owl:versionInfo xml:lang="en">Introduced in version 0.4 of the ontology</owl:versionInfo>
    </owl:NamedIndividual>
    


    <!-- https://w3id.org/leo/onto/ale/Mixed -->

    <owl:NamedIndividual rdf:about="https://w3id.org/leo/onto/ale/Mixed">
        <rdf:type rdf:resource="https://w3id.org/leo/onto/ale/BreastFeedingType"/>
    </owl:NamedIndividual>
    


    <!-- https://w3id.org/leo/onto/ale/Natural -->

    <owl:NamedIndividual rdf:about="https://w3id.org/leo/onto/ale/Natural">
        <rdf:type rdf:resource="https://w3id.org/leo/onto/ale/BreastFeedingType"/>
    </owl:NamedIndividual>
    


    <!-- https://w3id.org/leo/onto/ale/Negative -->

    <owl:NamedIndividual rdf:about="https://w3id.org/leo/onto/ale/Negative">
        <rdf:type rdf:resource="https://w3id.org/leo/onto/ale/PregnancyResult"/>
        <rdfs:isDefinedBy rdf:resource="https://w3id.org/leo/onto/ale"/>
        <rdfs:label xml:lang="it">Negativa</rdfs:label>
        <rdfs:label xml:lang="en">Negative</rdfs:label>
        <owl:versionInfo xml:lang="it">stabile</owl:versionInfo>
        <owl:versionInfo xml:lang="en">stable</owl:versionInfo>
    </owl:NamedIndividual>
    


    <!-- https://w3id.org/leo/onto/ale/P -->

    <owl:NamedIndividual rdf:about="https://w3id.org/leo/onto/ale/P">
        <rdf:type rdf:resource="https://w3id.org/leo/onto/ale/AbortionType"/>
        <rdfs:isDefinedBy rdf:resource="https://w3id.org/leo/onto/ale"/>
        <rdfs:label xml:lang="it">Precoce</rdfs:label>
        <rdfs:label xml:lang="en">Premature</rdfs:label>
        <owl:versionInfo xml:lang="it">stabile</owl:versionInfo>
        <owl:versionInfo xml:lang="en">stable</owl:versionInfo>
    </owl:NamedIndividual>
    


    <!-- https://w3id.org/leo/onto/ale/Positive -->

    <owl:NamedIndividual rdf:about="https://w3id.org/leo/onto/ale/Positive">
        <rdf:type rdf:resource="https://w3id.org/leo/onto/ale/PregnancyResult"/>
        <rdfs:isDefinedBy rdf:resource="https://w3id.org/leo/onto/ale"/>
        <rdfs:label xml:lang="it">Positiva</rdfs:label>
        <rdfs:label xml:lang="en">Positive</rdfs:label>
        <owl:versionInfo xml:lang="it">stabile</owl:versionInfo>
        <owl:versionInfo xml:lang="en">stable</owl:versionInfo>
    </owl:NamedIndividual>
    


    <!-- https://w3id.org/leo/onto/ale/Revisable -->

    <owl:NamedIndividual rdf:about="https://w3id.org/leo/onto/ale/Revisable">
        <rdf:type rdf:resource="https://w3id.org/leo/onto/ale/PregnancyResult"/>
        <rdfs:isDefinedBy rdf:resource="https://w3id.org/leo/onto/ale"/>
        <rdfs:label xml:lang="en">Revisable</rdfs:label>
        <rdfs:label xml:lang="it">Rivedibile</rdfs:label>
        <owl:versionInfo xml:lang="it">stabile</owl:versionInfo>
        <owl:versionInfo xml:lang="en">stable</owl:versionInfo>
    </owl:NamedIndividual>
    


    <!-- https://w3id.org/leo/onto/ale/SelfConsumptionSlaughtering -->

    <owl:NamedIndividual rdf:about="https://w3id.org/leo/onto/ale/SelfConsumptionSlaughtering">
        <rdf:type rdf:resource="https://w3id.org/leo/onto/ale/DisposalReason"/>
        <rdfs:isDefinedBy rdf:resource="https://w3id.org/leo/onto/ale"/>
        <rdfs:label xml:lang="it">Macellazione per autoconsumo</rdfs:label>
        <rdfs:label xml:lang="en">Self Consumption Slaughtering</rdfs:label>
        <owl:versionInfo xml:lang="it">provvisorio - aggiunto nella seconda versione dell&apos;ontologia</owl:versionInfo>
        <owl:versionInfo xml:lang="en">unstable - added in the second version of the ontology</owl:versionInfo>
    </owl:NamedIndividual>
    


    <!-- https://w3id.org/leo/onto/ale/SlaughterHealth -->

    <owl:NamedIndividual rdf:about="https://w3id.org/leo/onto/ale/SlaughterHealth">
        <rdf:type rdf:resource="https://w3id.org/leo/onto/ale/DisposalReason"/>
        <rdfs:isDefinedBy rdf:resource="https://w3id.org/leo/onto/ale"/>
        <rdfs:label xml:lang="it">Abbattimento Prov.Sanitario</rdfs:label>
        <rdfs:label xml:lang="en">Slaughter for Health reasons</rdfs:label>
        <owl:versionInfo xml:lang="it">provvisorio - aggiunto nella seconda versione dell&apos;ontologia</owl:versionInfo>
        <owl:versionInfo xml:lang="en">unstable - added in the second version of the ontology</owl:versionInfo>
    </owl:NamedIndividual>
    


    <!-- https://w3id.org/leo/onto/ale/SlaughterWellness -->

    <owl:NamedIndividual rdf:about="https://w3id.org/leo/onto/ale/SlaughterWellness">
        <rdf:type rdf:resource="https://w3id.org/leo/onto/ale/DisposalReason"/>
        <rdfs:isDefinedBy rdf:resource="https://w3id.org/leo/onto/ale"/>
        <rdfs:label xml:lang="it">Abbattimento motivi di benessere</rdfs:label>
        <rdfs:label xml:lang="en">Slaughter for wellness reasons</rdfs:label>
        <owl:versionInfo xml:lang="it">provvisorio - aggiunto nella seconda versione dell&apos;ontologia</owl:versionInfo>
        <owl:versionInfo xml:lang="en">unstable - added in the second version of the ontology</owl:versionInfo>
    </owl:NamedIndividual>
    


    <!-- https://w3id.org/leo/onto/ale/Slaughterhouse -->

    <owl:NamedIndividual rdf:about="https://w3id.org/leo/onto/ale/Slaughterhouse">
        <rdf:type rdf:resource="https://w3id.org/leo/onto/ale/DisposalReason"/>
        <rdfs:isDefinedBy rdf:resource="https://w3id.org/leo/onto/ale"/>
        <rdfs:label xml:lang="it">Macello</rdfs:label>
        <rdfs:label xml:lang="en">Slaughterhouse</rdfs:label>
        <owl:versionInfo xml:lang="it">provvisorio - aggiunto nella seconda versione dell&apos;ontologia</owl:versionInfo>
        <owl:versionInfo xml:lang="en">unstable - added in the second version of the ontology</owl:versionInfo>
    </owl:NamedIndividual>
    


    <!-- https://w3id.org/leo/onto/ale/T -->

    <owl:NamedIndividual rdf:about="https://w3id.org/leo/onto/ale/T">
        <rdf:type rdf:resource="https://w3id.org/leo/onto/ale/AbortionType"/>
        <rdfs:isDefinedBy rdf:resource="https://w3id.org/leo/onto/ale"/>
        <rdfs:label xml:lang="en">Belated</rdfs:label>
        <rdfs:label xml:lang="it">Tardivo</rdfs:label>
        <owl:versionInfo xml:lang="it">stabile</owl:versionInfo>
        <owl:versionInfo xml:lang="en">stable</owl:versionInfo>
    </owl:NamedIndividual>
    


    <!-- https://w3id.org/leo/onto/ale/Theft -->

    <owl:NamedIndividual rdf:about="https://w3id.org/leo/onto/ale/Theft">
        <rdf:type rdf:resource="https://w3id.org/leo/onto/ale/DisposalReason"/>
        <rdfs:isDefinedBy rdf:resource="https://w3id.org/leo/onto/ale"/>
        <rdfs:label xml:lang="it">Furto</rdfs:label>
        <rdfs:label xml:lang="en">Theft</rdfs:label>
        <owl:versionInfo xml:lang="en">stabile - introdotto nella versione 0.5 dell&apos;ontologia</owl:versionInfo>
        <owl:versionInfo xml:lang="en">stable - introduced in version 0.5 of the ontology</owl:versionInfo>
    </owl:NamedIndividual>
    


    <!-- https://w3id.org/leo/onto/ale/UrgentSlaughterStable -->

    <owl:NamedIndividual rdf:about="https://w3id.org/leo/onto/ale/UrgentSlaughterStable">
        <rdf:type rdf:resource="https://w3id.org/leo/onto/ale/DisposalReason"/>
        <rdfs:isDefinedBy rdf:resource="https://w3id.org/leo/onto/ale"/>
        <rdfs:label xml:lang="it">Macellazione urgente in stalla</rdfs:label>
        <rdfs:label xml:lang="en">Urgent slaughter in stable</rdfs:label>
        <owl:versionInfo xml:lang="it">provvisorio - aggiunto nella seconda versione dell&apos;ontologia</owl:versionInfo>
        <owl:versionInfo xml:lang="en">unstable - added in the second version of the ontology</owl:versionInfo>
    </owl:NamedIndividual>
</rdf:RDF>



<!-- Generated by the OWL API (version 4.5.9.2019-02-01T07:24:44Z) https://github.com/owlcs/owlapi -->

